<?xml version="1.0"?>
<rdf:RDF xmlns="https://w3id.org/mep#"
     xml:base="https://w3id.org/mep"
     xmlns:dc="http://purl.org/dc/elements/1.1/"
     xmlns:ns="http://creativecommons.org/ns#"
     xmlns:owl="http://www.w3.org/2002/07/owl#"
     xmlns:rdf="http://www.w3.org/1999/02/22-rdf-syntax-ns#"
     xmlns:xml="http://www.w3.org/XML/1998/namespace"
     xmlns:xsd="http://www.w3.org/2001/XMLSchema#"
     xmlns:rdfs="http://www.w3.org/2000/01/rdf-schema#"
     xmlns:vann="http://purl.org/vocab/vann/">
    <owl:Ontology rdf:about="https://w3id.org/mep#">
        <owl:versionIRI rdf:resource="https://w3id.org/mep#"/>
        <ns:license>http://creativecommons.org/licenses/by/3.0/</ns:license>
        <dc:abstract>This Ontology is automatically using the IFCExpress2MEP custom converter developed  by Carlos Ramonell (carlos.ramonell@upc.edu)</dc:abstract>
        <dc:creator>Carlos Ramonell Cazador (carlos.ramonell@upc.edu)</dc:creator>
        <dc:date>2024/04/11</dc:date>
        <dc:description>OWL ontology to describe built elements in the built environment. It is based on the Product ontology descibed in IFC (Insutry Foundation Classes) schema.</dc:description>
        <dc:identifier>Distribution Element Ontology</dc:identifier>
        <dc:language>en</dc:language>
        <dc:title>Distribution Element Ontology</dc:title>
        <vann:preferredNamespacePrefix>mep</vann:preferredNamespacePrefix>
        <vann:preferredNamespaceUri>https://w3id.org/mep#</vann:preferredNamespaceUri>
        <owl:versionInfo>1.0</owl:versionInfo>
    </owl:Ontology>
    


    <!-- 
    ///////////////////////////////////////////////////////////////////////////////////////
    //
    // Annotation properties
    //
    ///////////////////////////////////////////////////////////////////////////////////////
     -->


    


    <!-- http://creativecommons.org/ns#license -->


    <owl:AnnotationProperty rdf:about="http://creativecommons.org/ns#license"/>
    


    <!-- http://purl.org/dc/elements/1.1/abstract -->


    <owl:AnnotationProperty rdf:about="http://purl.org/dc/elements/1.1/abstract"/>
    


    <!-- http://purl.org/dc/elements/1.1/contributor -->


    <owl:AnnotationProperty rdf:about="http://purl.org/dc/elements/1.1/contributor"/>
    


    <!-- http://purl.org/dc/elements/1.1/creator -->


    <owl:AnnotationProperty rdf:about="http://purl.org/dc/elements/1.1/creator"/>
    


    <!-- http://purl.org/dc/elements/1.1/date -->


    <owl:AnnotationProperty rdf:about="http://purl.org/dc/elements/1.1/date"/>
    


    <!-- http://purl.org/dc/elements/1.1/description -->


    <owl:AnnotationProperty rdf:about="http://purl.org/dc/elements/1.1/description"/>
    


    <!-- http://purl.org/dc/elements/1.1/identifier -->


    <owl:AnnotationProperty rdf:about="http://purl.org/dc/elements/1.1/identifier"/>
    


    <!-- http://purl.org/dc/elements/1.1/language -->


    <owl:AnnotationProperty rdf:about="http://purl.org/dc/elements/1.1/language"/>
    


    <!-- http://purl.org/dc/elements/1.1/title -->


    <owl:AnnotationProperty rdf:about="http://purl.org/dc/elements/1.1/title"/>
    


    <!-- http://purl.org/vocab/vann/preferredNamespacePrefix -->


    <owl:AnnotationProperty rdf:about="http://purl.org/vocab/vann/preferredNamespacePrefix"/>
    


    <!-- http://purl.org/vocab/vann/preferredNamespaceUri -->


    <owl:AnnotationProperty rdf:about="http://purl.org/vocab/vann/preferredNamespaceUri"/>
    


    <!-- 
    ///////////////////////////////////////////////////////////////////////////////////////
    //
    // Classes
    //
    ///////////////////////////////////////////////////////////////////////////////////////
     -->


    


    <!-- https://schema.org/Product -->


    <owl:Class rdf:about="https://schema.org/Product"/>
    


    <!-- https://w3id.org/mep#Accesspoint -->


    <owl:Class rdf:about="https://w3id.org/mep#Accesspoint">
        <rdfs:subClassOf rdf:resource="https://w3id.org/mep#MobileTelecommunicationsAppliance"/>
        <rdfs:comment xml:lang="en">An access point is a device that allows wireless devices to connect to a wired network.</rdfs:comment>
        <rdfs:comment xml:lang="es">Un punto de acceso es un dispositivo que permite a los dispositivos inalámbricos conectarse a una red cableada.</rdfs:comment>
        <rdfs:label xml:lang="en">Access point</rdfs:label>
        <rdfs:label xml:lang="es">Punto de Acceso</rdfs:label>
    </owl:Class>
    


    <!-- https://w3id.org/mep#ActiveCooledBeam -->


    <owl:Class rdf:about="https://w3id.org/mep#ActiveCooledBeam">
        <rdfs:subClassOf rdf:resource="https://w3id.org/mep#CooledBeam"/>
        <rdfs:comment xml:lang="en">An active or ventilated cooled beam provides cooling (and heating) but can also function as an air terminal in a ventilation system.</rdfs:comment>
        <rdfs:comment xml:lang="es">Una viga de refrigeración activa o ventilada proporciona refrigeración (y calefacción), pero también puede funcionar como terminal de aire en un sistema de ventilación.</rdfs:comment>
        <rdfs:label xml:lang="en">Active Cooled Beam</rdfs:label>
        <rdfs:label xml:lang="es">Viga Refrigerante Activa</rdfs:label>
    </owl:Class>
    


    <!-- https://w3id.org/mep#Actuator -->


    <owl:Class rdf:about="https://w3id.org/mep#Actuator">
        <rdfs:subClassOf rdf:resource="https://w3id.org/mep#DistributionControlElement"/>
        <rdfs:comment xml:lang="en">An actuator is a mechanical device for moving or controlling a mechanism or system. An actuator takes energy, usually created by air, electricity, or liquid, and converts that into some kind of motion.</rdfs:comment>
        <rdfs:comment xml:lang="es">Un actuador es un dispositivo mecánico para mover o controlar un mecanismo o sistema. Un actuador toma energía, generalmente creada por aire, electricidad o líquido, y la convierte en algún tipo de movimiento.</rdfs:comment>
        <rdfs:label xml:lang="es">Actuador</rdfs:label>
        <rdfs:label xml:lang="en">Actuator</rdfs:label>
    </owl:Class>
    


    <!-- https://w3id.org/mep#AdiabaticAirWasher -->


    <owl:Class rdf:about="https://w3id.org/mep#AdiabaticAirWasher">
        <rdfs:subClassOf rdf:resource="https://w3id.org/mep#Humidifier"/>
        <rdfs:comment xml:lang="es">El vapor de agua se agrega a la corriente de aire mediante evaporación adiabática utilizando un elemento de lavado de aire.</rdfs:comment>
        <rdfs:comment xml:lang="en">Water vapor is added into the airstream through adiabatic evaporation using an air washing element.</rdfs:comment>
        <rdfs:label xml:lang="en">Adiabatic Air Washer</rdfs:label>
        <rdfs:label xml:lang="es">Air Wash Adiabatico</rdfs:label>
    </owl:Class>
    


    <!-- https://w3id.org/mep#AdiabaticAtomizingHumidifier -->


    <owl:Class rdf:about="https://w3id.org/mep#AdiabaticAtomizingHumidifier">
        <rdfs:subClassOf rdf:resource="https://w3id.org/mep#Humidifier"/>
        <rdfs:comment xml:lang="es">El vapor de agua se agrega a la corriente de aire mediante evaporación adiabática utilizando un elemento atomizador.</rdfs:comment>
        <rdfs:comment xml:lang="en">Water vapor is added into the airstream through adiabatic evaporation using an atomizing element.</rdfs:comment>
        <rdfs:label xml:lang="en">Adiabatic Atomizing Humidifier</rdfs:label>
        <rdfs:label xml:lang="es">Humidificador Atomizador Adiabatico</rdfs:label>
    </owl:Class>
    


    <!-- https://w3id.org/mep#AdiabaticCompressedAirNozzleHumidifier -->


    <owl:Class rdf:about="https://w3id.org/mep#AdiabaticCompressedAirNozzleHumidifier">
        <rdfs:subClassOf rdf:resource="https://w3id.org/mep#Humidifier"/>
        <rdfs:comment xml:lang="es">El vapor de agua se agrega a la corriente de aire mediante evaporación adiabática utilizando una boquilla de aire comprimido.</rdfs:comment>
        <rdfs:comment xml:lang="en">Water vapor is added into the airstream through adiabatic evaporation using a compressed air nozzle.</rdfs:comment>
        <rdfs:label xml:lang="en">Adiabatic Compressed Air Nozzle Humidifier</rdfs:label>
        <rdfs:label xml:lang="es">Humidificador Adiabatico de Boquilla de Aire Comprimido</rdfs:label>
    </owl:Class>
    


    <!-- https://w3id.org/mep#AdiabaticPan -->


    <owl:Class rdf:about="https://w3id.org/mep#AdiabaticPan">
        <rdfs:subClassOf rdf:resource="https://w3id.org/mep#Humidifier"/>
        <rdfs:comment xml:lang="es">El vapor de agua se añade al flujo de aire mediante evaporación adiabática utilizando una bandeja</rdfs:comment>
        <rdfs:comment xml:lang="en">Water vapor is added into the airstream through adiabatic evaporation using a pan.</rdfs:comment>
        <rdfs:label xml:lang="en">Adiabatic Pan</rdfs:label>
        <rdfs:label xml:lang="es">Pan Adiabatico</rdfs:label>
    </owl:Class>
    


    <!-- https://w3id.org/mep#AdiabaticRigidMediaHumidifier -->


    <owl:Class rdf:about="https://w3id.org/mep#AdiabaticRigidMediaHumidifier">
        <rdfs:subClassOf rdf:resource="https://w3id.org/mep#Humidifier"/>
        <rdfs:comment xml:lang="es">El vapor de agua se agrega a la corriente de aire mediante evaporación adiabática utilizando un medio rígido.</rdfs:comment>
        <rdfs:comment xml:lang="en">Water vapor is added into the airstream through adiabatic evaporation using a rigid media.</rdfs:comment>
        <rdfs:label xml:lang="en">Adiabatic Rigid Media Humidifier</rdfs:label>
        <rdfs:label xml:lang="es">Humidificador Adiabatico con Medios Rígidos</rdfs:label>
    </owl:Class>
    


    <!-- https://w3id.org/mep#AdiabaticUltrasonicHumidifier -->


    <owl:Class rdf:about="https://w3id.org/mep#AdiabaticUltrasonicHumidifier">
        <rdfs:subClassOf rdf:resource="https://w3id.org/mep#Humidifier"/>
        <rdfs:comment xml:lang="es">El vapor de agua se agrega a la corriente de aire mediante evaporación adiabática utilizando un elemento ultrasónico.</rdfs:comment>
        <rdfs:comment xml:lang="en">Water vapor is added into the airstream through adiabatic evaporation using an ultrasonic element.</rdfs:comment>
        <rdfs:label xml:lang="en">Adiabatic Ultrasonic Humidifier</rdfs:label>
        <rdfs:label xml:lang="es">Humidificador Ultrasonico Adiabatico</rdfs:label>
    </owl:Class>
    


    <!-- https://w3id.org/mep#AdiabaticWettedElement -->


    <owl:Class rdf:about="https://w3id.org/mep#AdiabaticWettedElement">
        <rdfs:subClassOf rdf:resource="https://w3id.org/mep#Humidifier"/>
        <rdfs:comment xml:lang="es">El vapor de agua se agrega a la corriente de aire mediante evaporación adiabática utilizando un elemento humedecido.</rdfs:comment>
        <rdfs:comment xml:lang="en">Water vapor is added into the airstream through adiabatic evaporation using a wetted element.</rdfs:comment>
        <rdfs:label xml:lang="en">Adiabatic Wetted Element</rdfs:label>
        <rdfs:label xml:lang="es">Elemento Adiabatico con Superficie Humeda</rdfs:label>
    </owl:Class>
    


    <!-- https://w3id.org/mep#Air-cooledCondenser -->


    <owl:Class rdf:about="https://w3id.org/mep#Air-cooledCondenser">
        <rdfs:subClassOf rdf:resource="https://w3id.org/mep#Condenser"/>
        <rdfs:comment xml:lang="en"> A condenser in which heat is transferred to an air-stream.</rdfs:comment>
        <rdfs:comment xml:lang="es">Condensador en el que el calor se transfiere a una corriente de aire.</rdfs:comment>
        <rdfs:label xml:lang="en">Air-cooled Condenser</rdfs:label>
        <rdfs:label xml:lang="es">Condensador Refrigerado por Aire</rdfs:label>
    </owl:Class>
    


    <!-- https://w3id.org/mep#AirConditioningUnit -->


    <owl:Class rdf:about="https://w3id.org/mep#AirConditioningUnit">
        <rdfs:subClassOf rdf:resource="https://w3id.org/mep#UnitaryEquipment"/>
        <rdfs:comment xml:lang="en">A unitary packaged air-conditioning unit typically used in residential or light commercial applications.</rdfs:comment>
        <rdfs:comment xml:lang="es">Unidad de aire acondicionado que se utiliza normalmente en aplicaciones residenciales o comerciales ligeras.</rdfs:comment>
        <rdfs:label xml:lang="en">Air Conditioning Unit</rdfs:label>
        <rdfs:label xml:lang="es">Unidad de Aire Acondicionado</rdfs:label>
    </owl:Class>
    


    <!-- https://w3id.org/mep#AirHandler -->


    <owl:Class rdf:about="https://w3id.org/mep#AirHandler">
        <rdfs:subClassOf rdf:resource="https://w3id.org/mep#UnitaryEquipment"/>
        <rdfs:comment xml:lang="en">A unitary air handling unit typically containing a fan, economizer, and coils.</rdfs:comment>
        <rdfs:comment xml:lang="es">Unidad de tratamiento de aire que normalmente contiene un ventilador, un economizador y serpentines.</rdfs:comment>
        <rdfs:label xml:lang="en">Air Handler</rdfs:label>
        <rdfs:label xml:lang="es">Unidad de Tratamiento de Aire</rdfs:label>
    </owl:Class>
    


    <!-- https://w3id.org/mep#AirParticlefilter -->


    <owl:Class rdf:about="https://w3id.org/mep#AirParticlefilter">
        <rdfs:subClassOf rdf:resource="https://w3id.org/mep#Filter"/>
        <rdfs:comment xml:lang="en">A filter used to remove particulates from air.</rdfs:comment>
        <rdfs:comment xml:lang="es">Un filtro utilizado para eliminar partículas del aire.</rdfs:comment>
        <rdfs:label xml:lang="en">Air Particle filter</rdfs:label>
        <rdfs:label xml:lang="es">Filtro de Particulas de Aire</rdfs:label>
    </owl:Class>
    


    <!-- https://w3id.org/mep#AirReleaseValve -->


    <owl:Class rdf:about="https://w3id.org/mep#AirReleaseValve">
        <rdfs:subClassOf rdf:resource="https://w3id.org/mep#Valve"/>
        <rdfs:comment xml:lang="en">Valve used to release air from a pipe or fitting.</rdfs:comment>
        <rdfs:comment xml:lang="es">Válvula utilizada para liberar aire de una tubería o accesorio.</rdfs:comment>
        <rdfs:label xml:lang="en">Air Release Valve</rdfs:label>
        <rdfs:label xml:lang="es">Valvula de Liberación de Aire</rdfs:label>
    </owl:Class>
    


    <!-- https://w3id.org/mep#AirStation -->


    <owl:Class rdf:about="https://w3id.org/mep#AirStation">
        <rdfs:subClassOf rdf:resource="https://w3id.org/mep#MedicalDevice"/>
        <rdfs:comment xml:lang="en">Device that provides purified medical air, composed of an air compressor and air treatment line.</rdfs:comment>
        <rdfs:comment xml:lang="es">Dispositivo que proporciona aire medicinal purificado, compuesto por un compresor de aire y una línea de tratamiento de aire.</rdfs:comment>
        <rdfs:label xml:lang="en">Air Station</rdfs:label>
        <rdfs:label xml:lang="es">Estacion de Aire</rdfs:label>
    </owl:Class>
    


    <!-- https://w3id.org/mep#AirTerminal -->


    <owl:Class rdf:about="https://w3id.org/mep#AirTerminal">
        <rdfs:subClassOf rdf:resource="https://w3id.org/mep#FlowTerminal"/>
        <rdfs:comment xml:lang="en">An air terminal is a terminating or origination point for the transfer of air between distribution system(s) and one or more spaces. It can also be used for the transfer of air between adjacent spaces.</rdfs:comment>
        <rdfs:comment xml:lang="es">Una terminal aérea es un punto de terminación o de origen para la transferencia de aire entre sistemas de distribución y uno o más espacios. También se puede utilizar para la transferencia de aire entre espacios adyacentes.</rdfs:comment>
        <rdfs:label xml:lang="en">Air Terminal</rdfs:label>
        <rdfs:label xml:lang="es">Terminal de Aire</rdfs:label>
    </owl:Class>
    


    <!-- https://w3id.org/mep#AirTerminalBox -->


    <owl:Class rdf:about="https://w3id.org/mep#AirTerminalBox">
        <rdfs:subClassOf rdf:resource="https://w3id.org/mep#FlowController"/>
        <rdfs:comment xml:lang="en">An air terminal box typically participates in an HVAC duct distribution system and is used to control or modulate the amount of air delivered to its downstream ductwork. An air terminal box type is often referred to as an &apos;air flow regulator&apos;.</rdfs:comment>
        <rdfs:comment xml:lang="es">Una caja terminal de aire normalmente participa en un sistema de distribución de conductos HVAC y se utiliza para controlar o modular la cantidad de aire entregado a sus conductos aguas abajo. Un tipo de caja terminal de aire a menudo se denomina &apos;regulador de flujo de aire&apos;.</rdfs:comment>
        <rdfs:label xml:lang="en">Air Terminal Box</rdfs:label>
        <rdfs:label xml:lang="es">Caja Terminal de Aire</rdfs:label>
    </owl:Class>
    


    <!-- https://w3id.org/mep#AirToAirHeatRecovery -->


    <owl:Class rdf:about="https://w3id.org/mep#AirToAirHeatRecovery">
        <rdfs:subClassOf rdf:resource="https://w3id.org/mep#EnergyConversionDevice"/>
        <rdfs:comment xml:lang="en">An air-to-air heat recovery device employs a counter-flow heat exchanger between inbound and outbound air flow. It is typically used to transfer heat from warmer air in one chamber to cooler air in the second chamber (i.e., typically used to recover heat from the conditioned air being exhausted and the outside air being supplied to a building), resulting in energy savings from reduced heating (or cooling) requirements.</rdfs:comment>
        <rdfs:comment xml:lang="es">Un dispositivo de recuperación de calor aire-aire emplea un intercambiador de calor de contraflujo entre el flujo de aire entrante y saliente. Por lo general, se usa para transferir calor del aire más cálido en una cámara al aire más frío en la segunda cámara (es decir, generalmente se usa para recuperar calor del aire acondicionado que se extrae y del aire exterior que se suministra a un edificio), lo que resulta en ahorros de energía de requisitos reducidos de calefacción (o refrigeración).</rdfs:comment>
        <rdfs:label xml:lang="en">Air-to-Air Heat Recovery</rdfs:label>
        <rdfs:label xml:lang="es">Dispositivo de Recuperación de Calor Aire-Aire</rdfs:label>
    </owl:Class>
    


    <!-- https://w3id.org/mep#AircooledChiller -->


    <owl:Class rdf:about="https://w3id.org/mep#AircooledChiller">
        <rdfs:subClassOf rdf:resource="https://w3id.org/mep#Chiller"/>
        <rdfs:comment xml:lang="en">Air cooled chiller.</rdfs:comment>
        <rdfs:comment xml:lang="es">Enfriador Refrigerado po Aire</rdfs:comment>
        <rdfs:label xml:lang="en">Air cooled Chiller</rdfs:label>
        <rdfs:label xml:lang="es">Enfriador Refrigerado po Aire</rdfs:label>
    </owl:Class>
    


    <!-- https://w3id.org/mep#Alarm -->


    <owl:Class rdf:about="https://w3id.org/mep#Alarm">
        <rdfs:subClassOf rdf:resource="https://w3id.org/mep#DistributionControlElement"/>
        <rdfs:comment xml:lang="en">An alarm is a device that signals the existence of a condition or situation that is outside the boundaries of normal expectation or that activates such a device. Alarms include the provision of break glass buttons and manual pull boxes that are used to activate alarms.</rdfs:comment>
        <rdfs:comment xml:lang="es">Una alarma es un dispositivo que señala la existencia de una condición o situación que está fuera de los límites de la expectativa normal o que activa dicho dispositivo. Las alarmas incluyen la provisión de botones para romper cristales y cajas de extracción manuales que se utilizan para activar alarmas.</rdfs:comment>
        <rdfs:label xml:lang="en">Alarm</rdfs:label>
        <rdfs:label xml:lang="es">Alarma</rdfs:label>
    </owl:Class>
    


    <!-- https://w3id.org/mep#AlarmPanel -->


    <owl:Class rdf:about="https://w3id.org/mep#AlarmPanel">
        <rdfs:subClassOf rdf:resource="https://w3id.org/mep#UnitaryControlElement"/>
        <rdfs:comment xml:lang="en">A control element at which alarms are annunciated.</rdfs:comment>
        <rdfs:comment xml:lang="es">Un elemento de control en el que se anuncian las alarmas.</rdfs:comment>
        <rdfs:label xml:lang="en">Alarm Panel</rdfs:label>
        <rdfs:label xml:lang="es">Panel de Alarmas</rdfs:label>
    </owl:Class>
    


    <!-- https://w3id.org/mep#Ammeter -->


    <owl:Class rdf:about="https://w3id.org/mep#Ammeter">
        <rdfs:subClassOf rdf:resource="https://w3id.org/mep#FlowInstrument"/>
        <rdfs:comment xml:lang="en">A device that reads and displays the current flow in a circuit.</rdfs:comment>
        <rdfs:comment xml:lang="es">Dispositivo que lee y muestra el flujo de corriente en un circuito.</rdfs:comment>
        <rdfs:label xml:lang="en">Ammeter</rdfs:label>
        <rdfs:label xml:lang="es">Amperimetro</rdfs:label>
    </owl:Class>
    


    <!-- https://w3id.org/mep#Amplifier -->


    <owl:Class rdf:about="https://w3id.org/mep#Amplifier">
        <rdfs:subClassOf rdf:resource="https://w3id.org/mep#AudioVisualAppliance"/>
        <rdfs:comment xml:lang="en">A device that receives an audio signal and amplifies it to play through speakers.</rdfs:comment>
        <rdfs:comment xml:lang="es">Dispositivo que recibe una señal de audio y la amplifica para reproducirla a través de altavoces.</rdfs:comment>
        <rdfs:label xml:lang="es">Amplificador</rdfs:label>
        <rdfs:label xml:lang="en">Amplifier</rdfs:label>
    </owl:Class>
    


    <!-- https://w3id.org/mep#Antenna -->


    <owl:Class rdf:about="https://w3id.org/mep#Antenna">
        <rdfs:subClassOf rdf:resource="https://w3id.org/mep#CommunicationsAppliance"/>
        <rdfs:comment xml:lang="en">A transducer designed to transmit or receive electromagnetic waves.</rdfs:comment>
        <rdfs:comment xml:lang="es">Transductor diseñado para transmitir o recibir ondas electromagnéticas.</rdfs:comment>
        <rdfs:label xml:lang="es">Antena</rdfs:label>
        <rdfs:label xml:lang="en">Antenna</rdfs:label>
    </owl:Class>
    


    <!-- https://w3id.org/mep#Anti-ArcingDevice -->


    <owl:Class rdf:about="https://w3id.org/mep#Anti-ArcingDevice">
        <rdfs:subClassOf rdf:resource="https://w3id.org/mep#ProtectiveDevice"/>
        <rdfs:comment xml:lang="en">An anti-arcing device is an equipment that prevents electric arc.</rdfs:comment>
        <rdfs:comment xml:lang="es">Un dispositivo antiarco es un equipo que impide el arco eléctrico.</rdfs:comment>
        <rdfs:label xml:lang="en">Anti-Arcing Device</rdfs:label>
        <rdfs:label xml:lang="es">Dispositivo Anti-Arco</rdfs:label>
    </owl:Class>
    


    <!-- https://w3id.org/mep#AntivacuumValve -->


    <owl:Class rdf:about="https://w3id.org/mep#AntivacuumValve">
        <rdfs:subClassOf rdf:resource="https://w3id.org/mep#Valve"/>
        <rdfs:comment xml:lang="en">Valve that opens to admit air if the pressure falls below atmospheric pressure.</rdfs:comment>
        <rdfs:comment xml:lang="es">Válvula que se abre para admitir aire si la presión cae por debajo de la presión atmosférica.</rdfs:comment>
        <rdfs:label xml:lang="en">Antivacuum Valve</rdfs:label>
        <rdfs:label xml:lang="es">Valvula Antivacio</rdfs:label>
    </owl:Class>
    


    <!-- https://w3id.org/mep#AssistedElectricHumidifier -->


    <owl:Class rdf:about="https://w3id.org/mep#AssistedElectricHumidifier">
        <rdfs:subClassOf rdf:resource="https://w3id.org/mep#Humidifier"/>
        <rdfs:comment xml:lang="en"></rdfs:comment>
        <rdfs:comment xml:lang="es"></rdfs:comment>
        <rdfs:label xml:lang="en">Assisted Electric Humidifier</rdfs:label>
        <rdfs:label xml:lang="es">Humidificador Asistido Electrico</rdfs:label>
    </owl:Class>
    


    <!-- https://w3id.org/mep#AssistedNaturalGasHumidifier -->


    <owl:Class rdf:about="https://w3id.org/mep#AssistedNaturalGasHumidifier">
        <rdfs:subClassOf rdf:resource="https://w3id.org/mep#Humidifier"/>
        <rdfs:comment xml:lang="en"></rdfs:comment>
        <rdfs:comment xml:lang="es"></rdfs:comment>
        <rdfs:label xml:lang="en">Assisted Natural Gas Humidifier</rdfs:label>
        <rdfs:label xml:lang="es">Humidificador Asistido de Gas Natural</rdfs:label>
    </owl:Class>
    


    <!-- https://w3id.org/mep#AssistedPropaneHumidifier -->


    <owl:Class rdf:about="https://w3id.org/mep#AssistedPropaneHumidifier">
        <rdfs:subClassOf rdf:resource="https://w3id.org/mep#Humidifier"/>
        <rdfs:comment xml:lang="es">El vapor de agua se agrega a la corriente de aire a través de la evaporación calentada por agua usando un calentador de propano.</rdfs:comment>
        <rdfs:comment xml:lang="en">Water vapor is added into the airstream through water heated evaporation using a propane heater.</rdfs:comment>
        <rdfs:label xml:lang="en">Assisted Propane Humidifier</rdfs:label>
        <rdfs:label xml:lang="es">Humidificador Asistido de Propano</rdfs:label>
    </owl:Class>
    


    <!-- https://w3id.org/mep#AssistedSteamHumidifier -->


    <owl:Class rdf:about="https://w3id.org/mep#AssistedSteamHumidifier">
        <rdfs:subClassOf rdf:resource="https://w3id.org/mep#Humidifier"/>
        <rdfs:comment xml:lang="es">El vapor de agua se agrega a la corriente de aire a través de la evaporación calentada por agua usando un calentador de vapor.</rdfs:comment>
        <rdfs:comment xml:lang="en">Water vapor is added into the airstream through water heated evaporation using a steam heater.</rdfs:comment>
        <rdfs:label xml:lang="en">Assisted Steam Humidifier</rdfs:label>
        <rdfs:label xml:lang="es">Humidificador Asisitido de Vapor</rdfs:label>
    </owl:Class>
    


    <!-- https://w3id.org/mep#AssitedButaneHumidifier -->


    <owl:Class rdf:about="https://w3id.org/mep#AssitedButaneHumidifier">
        <rdfs:subClassOf rdf:resource="https://w3id.org/mep#Humidifier"/>
        <rdfs:comment xml:lang="es">El vapor de agua se agrega a la corriente de aire a través de la evaporación calentada por agua usando un calentador de butano.</rdfs:comment>
        <rdfs:comment xml:lang="en">Water vapor is added into the airstream through water heated evaporation using a butane heater.</rdfs:comment>
        <rdfs:label xml:lang="en">Assited Butane Humidifier</rdfs:label>
        <rdfs:label xml:lang="es">Humidificador Asistido de Butano</rdfs:label>
    </owl:Class>
    


    <!-- https://w3id.org/mep#AudioSignalingDevice -->


    <owl:Class rdf:about="https://w3id.org/mep#AudioSignalingDevice">
        <rdfs:subClassOf rdf:resource="https://w3id.org/mep#Signal"/>
        <rdfs:comment xml:lang="en">A signal type formed of an active device conveying information by emitting an audio signal such as a beep, ring, horn or explosive sound.</rdfs:comment>
        <rdfs:comment xml:lang="es">Tipo de señal formada por un dispositivo activo que transmite información emitiendo una señal acústica, como un pitido, un timbre, una bocina o un sonido explosivo.</rdfs:comment>
        <rdfs:label xml:lang="en">Audio Signaling Device</rdfs:label>
        <rdfs:label xml:lang="es">Dispositivo de señalización de audio</rdfs:label>
    </owl:Class>
    


    <!-- https://w3id.org/mep#AudioVisualAppliance -->


    <owl:Class rdf:about="https://w3id.org/mep#AudioVisualAppliance">
        <rdfs:subClassOf rdf:resource="https://w3id.org/mep#FlowTerminal"/>
        <rdfs:comment xml:lang="en">An audio-visual appliance is a device that displays, captures, transmits, or receives audio or video. Audio-visual appliances may be fixed in place or may be able to be moved from one space to another. They may require an electrical supply that may be supplied either by an electrical circuit or provided from a local battery source. Audio-visual appliances may be connected to data circuits including specialist circuits for audio visual purposes only.</rdfs:comment>
        <rdfs:comment xml:lang="es">Dispositivo que muestra, captura, transmite o recibe audio o video. Los aparatos audiovisuales pueden estar fijos en su lugar o trasladarse de un espacio a otro. Es posible que requieran un suministro eléctrico que puede provenir de un circuito eléctrico o de una fuente de batería local. Los aparatos audiovisuales podrán conectarse a circuitos de datos, incluidos circuitos especializados, únicamente con fines audiovisuales.</rdfs:comment>
        <rdfs:label xml:lang="en">Audio-visual Appliance</rdfs:label>
        <rdfs:label xml:lang="es">Dispositivo Audiovisual</rdfs:label>
    </owl:Class>
    


    <!-- https://w3id.org/mep#AudiovisualOutlet -->


    <owl:Class rdf:about="https://w3id.org/mep#AudiovisualOutlet">
        <rdfs:subClassOf rdf:resource="https://w3id.org/mep#Outlet"/>
        <rdfs:comment xml:lang="en">An outlet used for an audio or visual device.</rdfs:comment>
        <rdfs:comment xml:lang="es">Salida utilizada para un dispositivo de audio o visual.</rdfs:comment>
        <rdfs:label xml:lang="en">Audiovisual Outlet</rdfs:label>
        <rdfs:label xml:lang="es">Salida Audiovisual</rdfs:label>
    </owl:Class>
    


    <!-- https://w3id.org/mep#Automaton -->


    <owl:Class rdf:about="https://w3id.org/mep#Automaton">
        <rdfs:subClassOf rdf:resource="https://w3id.org/mep#CommunicationsAppliance"/>
        <rdfs:comment xml:lang="en">A self-acting artificial device, the behaviour of which is governed either in a stepwise manner by given decision rules or continuously in time by defined relationships, while the output variables of which are created from its input and state variables. Note: definition from IEC 60050-351-42-32.</rdfs:comment>
        <rdfs:comment xml:lang="es">Dispositivo artificial que actúa por sí mismo, cuyo comportamiento se rige de forma escalonada por reglas de decisión dadas o de forma continua en el tiempo por relaciones definidas, mientras que sus variables de salida se crean a partir de sus variables de entrada y de estado. Nota: definición de la norma IEC 60050-351-42-32.</rdfs:comment>
        <rdfs:label xml:lang="en">Automaton</rdfs:label>
        <rdfs:label xml:lang="es">Automaton</rdfs:label>
    </owl:Class>
    


    <!-- https://w3id.org/mep#BackdraftDamper -->


    <owl:Class rdf:about="https://w3id.org/mep#BackdraftDamper">
        <rdfs:subClassOf rdf:resource="https://w3id.org/mep#Damper"/>
        <rdfs:comment xml:lang="es">Compuerta utilizada para equilibrar manualmente las diferencias de presión. Suele accionarse mediante ajuste mecánico.</rdfs:comment>
        <rdfs:comment xml:lang="en">Damper used for purposes of manually balancing pressure differences. Commonly operated by mechanical adjustment.</rdfs:comment>
        <rdfs:label xml:lang="en">Backdraft Damper</rdfs:label>
        <rdfs:label xml:lang="es">Compuerta de Contratiraje</rdfs:label>
    </owl:Class>
    


    <!-- https://w3id.org/mep#BalancingDamper -->


    <owl:Class rdf:about="https://w3id.org/mep#BalancingDamper">
        <rdfs:subClassOf rdf:resource="https://w3id.org/mep#Damper"/>
        <rdfs:comment xml:lang="en">Backdraft damper used to restrict the movement of air in one direction. Commonly operated by mechanical spring.</rdfs:comment>
        <rdfs:comment xml:lang="es">Compuerta de contratiraje utilizada para restringir el movimiento del aire en una dirección. Suele accionarse mediante un muelle mecánico.</rdfs:comment>
        <rdfs:label xml:lang="en">Balancing Damper</rdfs:label>
        <rdfs:label xml:lang="es">Compuerta de Equilibrado</rdfs:label>
    </owl:Class>
    


    <!-- https://w3id.org/mep#BaseStationController -->


    <owl:Class rdf:about="https://w3id.org/mep#BaseStationController">
        <rdfs:subClassOf rdf:resource="https://w3id.org/mep#UnitaryControlElement"/>
        <rdfs:comment xml:lang="en">A base station controller (BSC) is a network component with the functions for controlling one or more base transceiver stations. BSC is responsible for the management of various interfaces, wireless resources and parameters, the signalling processing of call establishment and the channel allocation in the cell.</rdfs:comment>
        <rdfs:comment xml:lang="es">Un controlador de estación base (BSC) es un componente de red con funciones para controlar una o más estaciones transceptoras base. BSC es responsable de la gestión de varias interfaces, recursos y parámetros inalámbricos, el procesamiento de señalización del establecimiento de llamadas y la asignación de canales en la celda.</rdfs:comment>
        <rdfs:label xml:lang="en">Base Station Controller</rdfs:label>
        <rdfs:label xml:lang="es">Controlador de Estacion Base</rdfs:label>
    </owl:Class>
    


    <!-- https://w3id.org/mep#BaseTranscieverStation -->


    <owl:Class rdf:about="https://w3id.org/mep#BaseTranscieverStation">
        <rdfs:subClassOf rdf:resource="https://w3id.org/mep#MobileTelecommunicationsAppliance"/>
        <rdfs:comment xml:lang="en">A base transceiver station (BTS) is a network component which serves one cell. It completes the conversion between base station controller and wireless channel, and realizes the wireless transmission and related control functions between base station controller and mobile switching through the air interface.</rdfs:comment>
        <rdfs:comment xml:lang="es">Una estación transceptora base (BTS) es un componente de red que da servicio a una célula. Completa la conversión entre el controlador de la estación base y el canal inalámbrico, y realiza la transmisión inalámbrica y las funciones de control relacionadas entre el controlador de la estación base y la conmutación móvil a través de la interfaz aérea.</rdfs:comment>
        <rdfs:label xml:lang="en">Base Transciever Station</rdfs:label>
        <rdfs:label xml:lang="es">Estacion Transceptora Base</rdfs:label>
    </owl:Class>
    


    <!-- https://w3id.org/mep#BasebandUnit -->


    <owl:Class rdf:about="https://w3id.org/mep#BasebandUnit">
        <rdfs:subClassOf rdf:resource="https://w3id.org/mep#MobileTelecommunicationsAppliance"/>
        <rdfs:comment xml:lang="en">A baseband unit is a component of a distributed base transceiver station for implementing baseband processing functions.</rdfs:comment>
        <rdfs:comment xml:lang="es">Una unidad de banda base es un componente de una estación transceptora de base distribuida para implementar funciones de procesamiento de banda base.</rdfs:comment>
        <rdfs:label xml:lang="en">Baseband Unit</rdfs:label>
        <rdfs:label xml:lang="es">Unidad de Banda Base</rdfs:label>
    </owl:Class>
    


    <!-- https://w3id.org/mep#Basin -->


    <owl:Class rdf:about="https://w3id.org/mep#Basin">
        <rdfs:subClassOf rdf:resource="https://w3id.org/mep#Tank"/>
        <rdfs:comment xml:lang="en">An arbitrary open tank type.</rdfs:comment>
        <rdfs:comment xml:lang="es">Un tipo de tanque abierto arbitrario.</rdfs:comment>
        <rdfs:label xml:lang="es">Balsa</rdfs:label>
        <rdfs:label xml:lang="en">Basin</rdfs:label>
    </owl:Class>
    


    <!-- https://w3id.org/mep#Bath -->


    <owl:Class rdf:about="https://w3id.org/mep#Bath">
        <rdfs:subClassOf rdf:resource="https://w3id.org/mep#SanitaryTerminal"/>
        <rdfs:comment xml:lang="es">Aparato sanitario para la inmersión del cuerpo humano o partes del mismo.</rdfs:comment>
        <rdfs:comment xml:lang="en">Sanitary appliance for immersion of the human body or parts of it.</rdfs:comment>
        <rdfs:label xml:lang="en">Bath</rdfs:label>
        <rdfs:label xml:lang="es">Bañera</rdfs:label>
    </owl:Class>
    


    <!-- https://w3id.org/mep#Battery -->


    <owl:Class rdf:about="https://w3id.org/mep#Battery">
        <rdfs:subClassOf rdf:resource="https://w3id.org/mep#ElectricFlowStorageDevice"/>
        <rdfs:comment xml:lang="en">A device for storing energy in chemical form so that it can be released as electrical energy.</rdfs:comment>
        <rdfs:comment xml:lang="es">Dispositivo que almacena energía en forma química para liberarla en forma de energía eléctrica.</rdfs:comment>
        <rdfs:label xml:lang="es">Bateria</rdfs:label>
        <rdfs:label xml:lang="en">Battery</rdfs:label>
    </owl:Class>
    


    <!-- https://w3id.org/mep#Bell -->


    <owl:Class rdf:about="https://w3id.org/mep#Bell">
        <rdfs:subClassOf rdf:resource="https://w3id.org/mep#Alarm"/>
        <rdfs:comment xml:lang="en">An audible alarm.</rdfs:comment>
        <rdfs:comment xml:lang="es">Una alarma sonora.</rdfs:comment>
        <rdfs:label xml:lang="en">Bell</rdfs:label>
        <rdfs:label xml:lang="es">Campana</rdfs:label>
    </owl:Class>
    


    <!-- https://w3id.org/mep#BeltConveyor -->


    <owl:Class rdf:about="https://w3id.org/mep#BeltConveyor">
        <rdfs:subClassOf rdf:resource="https://w3id.org/mep#ConveyorSegment"/>
        <rdfs:comment xml:lang="en">An endless belt for carrying material without stretching.</rdfs:comment>
        <rdfs:comment xml:lang="es">Una cinta sin fin para transportar material sin estirarlo.</rdfs:comment>
        <rdfs:label xml:lang="en">Belt Conveyor</rdfs:label>
        <rdfs:label xml:lang="es">Cinta Transportadora</rdfs:label>
    </owl:Class>
    


    <!-- https://w3id.org/mep#BeltDrive -->


    <owl:Class rdf:about="https://w3id.org/mep#BeltDrive">
        <rdfs:subClassOf rdf:resource="https://w3id.org/mep#MotorConnection"/>
        <rdfs:comment xml:lang="en">An indirect connection made through the medium of a shaped, flexible continuous loop.</rdfs:comment>
        <rdfs:comment xml:lang="es">Conexión indirecta realizada a través de un bucle continuo flexible con forma.</rdfs:comment>
        <rdfs:label xml:lang="en">Belt Drive</rdfs:label>
        <rdfs:label xml:lang="es">Transmision por Correa</rdfs:label>
    </owl:Class>
    


    <!-- https://w3id.org/mep#Bidet -->


    <owl:Class rdf:about="https://w3id.org/mep#Bidet">
        <rdfs:subClassOf rdf:resource="https://w3id.org/mep#SanitaryTerminal"/>
        <rdfs:comment xml:lang="es">Aparato de aguas residuales para lavar los órganos excretores sentado a horcajadas.</rdfs:comment>
        <rdfs:comment xml:lang="en">Waste water appliance for washing the excretory organs while sitting astride the bowl.</rdfs:comment>
        <rdfs:label xml:lang="es">Bide</rdfs:label>
        <rdfs:label xml:lang="en">Bidet</rdfs:label>
    </owl:Class>
    


    <!-- https://w3id.org/mep#BirdCage -->


    <owl:Class rdf:about="https://w3id.org/mep#BirdCage">
        <rdfs:subClassOf rdf:resource="https://w3id.org/mep#StackTerminal"/>
        <rdfs:comment xml:lang="en">Guard cage, typically wire mesh, at the top of the stack preventing access by birds.</rdfs:comment>
        <rdfs:comment xml:lang="es">Jaula de protección, normalmente de malla metálica, en la parte superior de la pila que impide el acceso de las aves.</rdfs:comment>
        <rdfs:label xml:lang="en">Bird Cage</rdfs:label>
        <rdfs:label xml:lang="es">Jaula para Pajaros</rdfs:label>
    </owl:Class>
    


    <!-- https://w3id.org/mep#BlastDamper -->


    <owl:Class rdf:about="https://w3id.org/mep#BlastDamper">
        <rdfs:subClassOf rdf:resource="https://w3id.org/mep#Damper"/>
        <rdfs:comment xml:lang="en">Blast damper used to prevent protect occupants and equipment against overpressures resultant of an explosion. Commonly operated by mechanical spring.</rdfs:comment>
        <rdfs:comment xml:lang="es">Compuerta antiexplosión utilizada para proteger a los ocupantes y los equipos contra las sobrepresiones resultantes de una explosión. Suele accionarse mediante un muelle mecánico.</rdfs:comment>
        <rdfs:label xml:lang="en">Blast Damper</rdfs:label>
        <rdfs:label xml:lang="es">Compuerta Antiexplosion</rdfs:label>
    </owl:Class>
    


    <!-- https://w3id.org/mep#Boiler -->


    <owl:Class rdf:about="https://w3id.org/mep#Boiler">
        <rdfs:subClassOf rdf:resource="https://w3id.org/mep#EnergyConversionDevice"/>
        <rdfs:comment xml:lang="en">A boiler is a closed, pressure-rated vessel in which water or other fluid is heated using an energy source such as natural gas, heating oil, or electricity. The fluid in the vessel is then circulated out of the boiler for use in various processes or heating applications.</rdfs:comment>
        <rdfs:comment xml:lang="es">Una caldera es un recipiente cerrado con presión nominal en el que se calienta agua u otro fluido utilizando una fuente de energía como gas natural, combustible para calefacción o electricidad. Luego, el fluido del recipiente circula fuera de la caldera para su uso en diversos procesos o aplicaciones de calefacción.</rdfs:comment>
        <rdfs:label xml:lang="en">Boiler</rdfs:label>
        <rdfs:label xml:lang="es">Caldera</rdfs:label>
    </owl:Class>
    


    <!-- https://w3id.org/mep#Booster -->


    <owl:Class rdf:about="https://w3id.org/mep#Booster">
        <rdfs:subClassOf rdf:resource="https://w3id.org/mep#Compressor"/>
        <rdfs:comment xml:lang="es">Compresor alternativo de desplazamiento positivo en el que la presión se incrementa mediante un booster.</rdfs:comment>
        <rdfs:comment xml:lang="en">Positive-displacement reciprocating compressor where pressure is increased by a booster.</rdfs:comment>
        <rdfs:label xml:lang="en">Booster</rdfs:label>
        <rdfs:label xml:lang="es">Booster</rdfs:label>
    </owl:Class>
    


    <!-- https://w3id.org/mep#BreakPressureTank -->


    <owl:Class rdf:about="https://w3id.org/mep#BreakPressureTank">
        <rdfs:subClassOf rdf:resource="https://w3id.org/mep#Tank"/>
        <rdfs:comment xml:lang="en">An open container that breaks the hydraulic pressure in a distribution system, typically located between the fluid reservoir and the fluid supply points. A typical break pressure tank allows the flow to discharge into the atmosphere, thereby reducing its hydrostatic pressure to zero.</rdfs:comment>
        <rdfs:comment xml:lang="es">Recipiente abierto que rompe la presión hidráulica en un sistema de distribución, situado normalmente entre el depósito de fluido y los puntos de suministro de fluido. Un depósito de ruptura de presión típico permite que el flujo se descargue en la atmósfera, reduciendo así su presión hidrostática a cero.</rdfs:comment>
        <rdfs:label xml:lang="en">Break Pressure Tank</rdfs:label>
        <rdfs:label xml:lang="es">Tanque de Presion de Ruptura</rdfs:label>
    </owl:Class>
    


    <!-- https://w3id.org/mep#BreakglassButton -->


    <owl:Class rdf:about="https://w3id.org/mep#BreakglassButton">
        <rdfs:subClassOf rdf:resource="https://w3id.org/mep#Alarm"/>
        <rdfs:comment xml:lang="en">An alarm activation mechanism in which a protective glass has to be broken to enable a button to be pressed.</rdfs:comment>
        <rdfs:comment xml:lang="es">Un mecanismo de activación de alarma en el que es necesario romper un cristal protector para poder pulsar un botón.</rdfs:comment>
        <rdfs:label xml:lang="es">Boton de Romper Cristal</rdfs:label>
        <rdfs:label xml:lang="en">Breakglass Button</rdfs:label>
    </owl:Class>
    


    <!-- https://w3id.org/mep#BreechingInlet -->


    <owl:Class rdf:about="https://w3id.org/mep#BreechingInlet">
        <rdfs:subClassOf rdf:resource="https://w3id.org/mep#FireSuppressionTerminal"/>
        <rdfs:comment xml:lang="es">Accesorio de tubería simétrico que une dos o más entradas en una sola tubería. Puede utilizarse en un ascensor húmedo o seco. El personal de los servicios de bomberos lo utiliza para una conexión rápida de mangueras de aparatos contra incendios. También puede usarse para espuma .</rdfs:comment>
        <rdfs:comment xml:lang="en">Symmetrical pipe fitting that unites two or more inlets into a single pipe. A breeching inlet may be used on either a wet or dry riser. Used by fire services personnel for fast connection of fire appliance hose reels. May also be used for foam.</rdfs:comment>
        <rdfs:label xml:lang="en">Breeching Inlet</rdfs:label>
        <rdfs:label xml:lang="es">Entrada de Toma de Agua</rdfs:label>
    </owl:Class>
    


    <!-- https://w3id.org/mep#BucketConveyor -->


    <owl:Class rdf:about="https://w3id.org/mep#BucketConveyor">
        <rdfs:subClassOf rdf:resource="https://w3id.org/mep#ConveyorSegment"/>
        <rdfs:comment xml:lang="en">A conveyor in the form of connected buckets or segments that move in a continuous loop</rdfs:comment>
        <rdfs:comment xml:lang="es">Transportador en forma de cangilones o segmentos conectados que se mueven en un bucle continuo.</rdfs:comment>
        <rdfs:label xml:lang="en">Bucket Conveyor</rdfs:label>
        <rdfs:label xml:lang="es">Transportador de Cagilones</rdfs:label>
    </owl:Class>
    


    <!-- https://w3id.org/mep#Burner -->


    <owl:Class rdf:about="https://w3id.org/mep#Burner">
        <rdfs:subClassOf rdf:resource="https://w3id.org/mep#EnergyConversionDevice"/>
        <rdfs:comment xml:lang="en">A burner is a device that converts fuel into heat through combustion. It includes gas, oil, and wood burners.</rdfs:comment>
        <rdfs:comment xml:lang="es">Una estufa es un dispositivo que convierte el combustible en calor mediante la combustión. Incluye estufas de gas, gasóleo y leña.</rdfs:comment>
        <rdfs:label xml:lang="en">Burner</rdfs:label>
        <rdfs:label xml:lang="es">Estufa</rdfs:label>
    </owl:Class>
    


    <!-- https://w3id.org/mep#BusBarSegment -->


    <owl:Class rdf:about="https://w3id.org/mep#BusBarSegment">
        <rdfs:subClassOf rdf:resource="https://w3id.org/mep#CableSegment"/>
        <rdfs:comment xml:lang="es">Conductor eléctrico que realiza una conexión común entre varios circuitos eléctricos. Las propiedades de una barra colectora son las mismas que las de un segmento de cable y están capturadas por el conjunto de propiedades del segmento de cable.</rdfs:comment>
        <rdfs:comment xml:lang="en">Electrical conductor that makes a common connection between several electrical circuits. Properties of a busbar are the same as those of a cable segment and are captured by the cable segment property set.</rdfs:comment>
        <rdfs:label xml:lang="en">Bus Bar Segment</rdfs:label>
        <rdfs:label xml:lang="es">Segmento de Barra Colectora</rdfs:label>
    </owl:Class>
    


    <!-- https://w3id.org/mep#CHP -->


    <owl:Class rdf:about="https://w3id.org/mep#CHP">
        <rdfs:subClassOf rdf:resource="https://w3id.org/mep#ElectricGenerator"/>
        <rdfs:comment xml:lang="en">Combined heat and power supply, used not only as a source of electric energy but also as a heating source for the building. It may therefore be not only part of an electrical system but also of a heating system.</rdfs:comment>
        <rdfs:comment xml:lang="es">Suministro combinado de calor y electricidad, utilizado no sólo como fuente de energía eléctrica sino también como fuente de calefacción para el edificio. Por tanto, puede formar parte no sólo de un sistema eléctrico sino también de un sistema de calefacción.</rdfs:comment>
        <rdfs:label xml:lang="en">CHP</rdfs:label>
        <rdfs:label xml:lang="es">CHP</rdfs:label>
    </owl:Class>
    


    <!-- https://w3id.org/mep#CO2Sensor -->


    <owl:Class rdf:about="https://w3id.org/mep#CO2Sensor">
        <rdfs:subClassOf rdf:resource="https://w3id.org/mep#Sensor"/>
        <rdfs:comment xml:lang="en">A device that senses or detects carbon dioxide.</rdfs:comment>
        <rdfs:comment xml:lang="es">Dispositivo que detecta el dióxido de carbono.</rdfs:comment>
        <rdfs:label xml:lang="en">CO2 Sensor</rdfs:label>
        <rdfs:label xml:lang="es">Sensor de CO2</rdfs:label>
    </owl:Class>
    


    <!-- https://w3id.org/mep#COSensor -->


    <owl:Class rdf:about="https://w3id.org/mep#COSensor">
        <rdfs:subClassOf rdf:resource="https://w3id.org/mep#Sensor"/>
        <rdfs:comment xml:lang="en">A device that senses or detects carbon monoxide.</rdfs:comment>
        <rdfs:comment xml:lang="es">Dispositivo que detecta el monóxido de carbono.</rdfs:comment>
        <rdfs:label xml:lang="en">CO Sensor</rdfs:label>
        <rdfs:label xml:lang="es">Sensor de CO</rdfs:label>
    </owl:Class>
    


    <!-- https://w3id.org/mep#CableBracket -->


    <owl:Class rdf:about="https://w3id.org/mep#CableBracket">
        <rdfs:subClassOf rdf:resource="https://w3id.org/mep#CableCarrierSegment"/>
        <rdfs:comment xml:lang="en">A cable bracket is a horizontal cable support fixed at one end only, spaced at intervals, on which cables rest.</rdfs:comment>
        <rdfs:comment xml:lang="es">Una abrazadera es un soporte para cables horizontal fijado en un solo extremo, espaciado a intervalos, sobre el que descansan los cables.</rdfs:comment>
        <rdfs:label xml:lang="es">Abrazadera</rdfs:label>
        <rdfs:label xml:lang="en">Cable Bracket</rdfs:label>
    </owl:Class>
    


    <!-- https://w3id.org/mep#CableCarrierBend -->


    <owl:Class rdf:about="https://w3id.org/mep#CableCarrierBend">
        <rdfs:subClassOf rdf:resource="https://w3id.org/mep#CableCarrierFitting"/>
        <rdfs:comment xml:lang="en">A fitting that changes the route of the cable carrier.</rdfs:comment>
        <rdfs:comment xml:lang="es">Un accessorio que cambia el recorrido del portacables.</rdfs:comment>
        <rdfs:label xml:lang="en">Cable Carrier Bend</rdfs:label>
        <rdfs:label xml:lang="es">Codo de Accesorio Portacables</rdfs:label>
    </owl:Class>
    


    <!-- https://w3id.org/mep#CableCarrierConnector -->


    <owl:Class rdf:about="https://w3id.org/mep#CableCarrierConnector">
        <rdfs:subClassOf rdf:resource="https://w3id.org/mep#CableCarrierFitting"/>
        <rdfs:comment xml:lang="es">Accesorio conector, normalmente utilizado para unir dos puertos dentro de un sistema de distribución de flujo (por ejemplo, un acoplamiento utilizado para unir dos segmentos de conducto).</rdfs:comment>
        <rdfs:comment xml:lang="en">Connector fitting, typically used to join two ports together within a flow distribution system (e.g., a coupling used to join two duct segments).</rdfs:comment>
        <rdfs:label xml:lang="en">Cable Carrier Connector</rdfs:label>
        <rdfs:label xml:lang="es">Conector de Accesorio Portacables</rdfs:label>
    </owl:Class>
    


    <!-- https://w3id.org/mep#CableCarrierFitting -->


    <owl:Class rdf:about="https://w3id.org/mep#CableCarrierFitting">
        <rdfs:subClassOf rdf:resource="https://w3id.org/mep#FlowFitting"/>
        <rdfs:comment xml:lang="en">A cable carrier fitting is a fitting that is placed at junction or transition in a cable carrier system.</rdfs:comment>
        <rdfs:comment xml:lang="es">Un accesorio portacables es un accesorio que se coloca en una unión o transición en un sistema portacables.</rdfs:comment>
        <rdfs:label xml:lang="es">Accesorio Portacables</rdfs:label>
        <rdfs:label xml:lang="en">Cable Carrier Fitting</rdfs:label>
    </owl:Class>
    


    <!-- https://w3id.org/mep#CableCarrierJunction -->


    <owl:Class rdf:about="https://w3id.org/mep#CableCarrierJunction">
        <rdfs:subClassOf rdf:resource="https://w3id.org/mep#CableCarrierFitting"/>
        <rdfs:comment xml:lang="en">A fitting with typically more than two ports used to redistribute flow among the ports and/or to change the direction of flow between connected elements (e.g, tee, cross, wye, etc.).</rdfs:comment>
        <rdfs:comment xml:lang="es">Un accesorio que normalmente tiene más de dos puertos se utiliza para redistribuir el flujo entre los puertos y/o para cambiar la dirección del flujo entre elementos conectados (por ejemplo, T, cruz, estrella, etc.).</rdfs:comment>
        <rdfs:label xml:lang="en">Cable Carrier Junction</rdfs:label>
        <rdfs:label xml:lang="es">Union de Accesorio Portacables</rdfs:label>
    </owl:Class>
    


    <!-- https://w3id.org/mep#CableCarrierSegment -->


    <owl:Class rdf:about="https://w3id.org/mep#CableCarrierSegment">
        <rdfs:subClassOf rdf:resource="https://w3id.org/mep#FlowSegment"/>
        <rdfs:comment xml:lang="en">A cable carrier segment is a flow segment that is specifically used to carry and support cabling.</rdfs:comment>
        <rdfs:comment xml:lang="es">Un segmento portacables es un segmento de flujo que se utiliza específicamente para transportar y soportar cableado.</rdfs:comment>
        <rdfs:label xml:lang="en">Cable Carrier Segment</rdfs:label>
        <rdfs:label xml:lang="es">Segmento de Portador de Cables</rdfs:label>
    </owl:Class>
    


    <!-- https://w3id.org/mep#CableCarrierTransition -->


    <owl:Class rdf:about="https://w3id.org/mep#CableCarrierTransition">
        <rdfs:subClassOf rdf:resource="https://w3id.org/mep#CableCarrierFitting"/>
        <rdfs:comment xml:lang="en">A fitting with typically two ports having different shapes or sizes. Can also be used to change the direction of flow between connected elements.</rdfs:comment>
        <rdfs:comment xml:lang="es">Un accesorio con normalmente dos puertos que tienen diferentes formas o tamaños. También se puede utilizar para cambiar la dirección del flujo entre elementos conectados.</rdfs:comment>
        <rdfs:label xml:lang="en">Cable Carrier Transition</rdfs:label>
        <rdfs:label xml:lang="es">Trasicion de Accesorio Portacables</rdfs:label>
    </owl:Class>
    


    <!-- https://w3id.org/mep#CableConnector -->


    <owl:Class rdf:about="https://w3id.org/mep#CableConnector">
        <rdfs:subClassOf rdf:resource="https://w3id.org/mep#CableFitting"/>
        <rdfs:comment xml:lang="en">A fitting that joins two cable segments of the same connector type (though potentially different gender).</rdfs:comment>
        <rdfs:comment xml:lang="es">Un accesorio que une dos segmentos de cable del mismo tipo de conector (aunque potencialmente de diferente sexo).</rdfs:comment>
        <rdfs:label xml:lang="en">Cable Connector</rdfs:label>
        <rdfs:label xml:lang="es">Conector de Cables</rdfs:label>
    </owl:Class>
    


    <!-- https://w3id.org/mep#CableEntry -->


    <owl:Class rdf:about="https://w3id.org/mep#CableEntry">
        <rdfs:subClassOf rdf:resource="https://w3id.org/mep#CableFitting"/>
        <rdfs:comment xml:lang="en">A fitting that begins a cable segment at a non-electrical element such as a grounding clamp attached to a pipe.</rdfs:comment>
        <rdfs:comment xml:lang="es">Accesorio que comienza un segmento de cable en un elemento no eléctrico, como una abrazadera de conexión a tierra unida a una tubería.</rdfs:comment>
        <rdfs:label xml:lang="en">Cable Entry</rdfs:label>
        <rdfs:label xml:lang="es">Entrada de Cables</rdfs:label>
    </owl:Class>
    


    <!-- https://w3id.org/mep#CableExit -->


    <owl:Class rdf:about="https://w3id.org/mep#CableExit">
        <rdfs:subClassOf rdf:resource="https://w3id.org/mep#CableFitting"/>
        <rdfs:comment xml:lang="en">A fitting that ends a cable segment at a non-electrical element such as a grounding clamp attached to a pipe or to the ground.</rdfs:comment>
        <rdfs:comment xml:lang="es">Accesorio que termina un segmento de cable en un elemento no eléctrico, como una abrazadera de conexión a tierra unida a una tubería o al suelo.</rdfs:comment>
        <rdfs:label xml:lang="en">Cable Exit</rdfs:label>
        <rdfs:label xml:lang="es">Salida de Cables</rdfs:label>
    </owl:Class>
    


    <!-- https://w3id.org/mep#CableFanout -->


    <owl:Class rdf:about="https://w3id.org/mep#CableFanout">
        <rdfs:subClassOf rdf:resource="https://w3id.org/mep#CableFitting"/>
        <rdfs:comment xml:lang="en">A fan out is a special cable fitting that provides a safe transition from multi-fiber cable units to individual fibers.</rdfs:comment>
        <rdfs:comment xml:lang="es">Un fanout es un accesorio de cable especial que proporciona una transición segura de unidades de cable multifibra a fibras individuales.</rdfs:comment>
        <rdfs:label xml:lang="en">Cable Fanout</rdfs:label>
        <rdfs:label xml:lang="es">Fanout de Cables</rdfs:label>
    </owl:Class>
    


    <!-- https://w3id.org/mep#CableFitting -->


    <owl:Class rdf:about="https://w3id.org/mep#CableFitting">
        <rdfs:subClassOf rdf:resource="https://w3id.org/mep#FlowFitting"/>
        <rdfs:comment xml:lang="en">A cable fitting is a fitting that is placed at a junction, transition or termination in a cable system.</rdfs:comment>
        <rdfs:comment xml:lang="es">Un accesorio para cables es un accesorio que se coloca en una unión, transición o terminación en un sistema de cables.</rdfs:comment>
        <rdfs:label xml:lang="es">Accesorio de Cable </rdfs:label>
        <rdfs:label xml:lang="en">Cable Fitting</rdfs:label>
    </owl:Class>
    


    <!-- https://w3id.org/mep#CableJunction -->


    <owl:Class rdf:about="https://w3id.org/mep#CableJunction">
        <rdfs:subClassOf rdf:resource="https://w3id.org/mep#CableFitting"/>
        <rdfs:comment xml:lang="en">A fitting that joins three or more segments of arbitrary connector types for signal splitting or multiplexing.</rdfs:comment>
        <rdfs:comment xml:lang="es">Un accesorio que une tres o más segmentos de tipos de conectores arbitrarios para dividir o multiplexar señales.</rdfs:comment>
        <rdfs:label xml:lang="en">Cable Junction</rdfs:label>
        <rdfs:label xml:lang="es">Union de Cables</rdfs:label>
    </owl:Class>
    


    <!-- https://w3id.org/mep#CableLadderSegment -->


    <owl:Class rdf:about="https://w3id.org/mep#CableLadderSegment">
        <rdfs:subClassOf rdf:resource="https://w3id.org/mep#CableCarrierSegment"/>
        <rdfs:comment xml:lang="en">An open carrier segment on which cables are carried on a ladder structure.</rdfs:comment>
        <rdfs:comment xml:lang="es">Un segmento portador abierto sobre el cual se transportan los cables en una estructura de escalera.</rdfs:comment>
        <rdfs:label xml:lang="en">Cable Ladder Segment</rdfs:label>
        <rdfs:label xml:lang="es">Segmento de Escalera de Cables</rdfs:label>
    </owl:Class>
    


    <!-- https://w3id.org/mep#CableSegment -->


    <owl:Class rdf:about="https://w3id.org/mep#CableSegment">
        <rdfs:subClassOf rdf:resource="https://w3id.org/mep#FlowSegment"/>
        <rdfs:comment xml:lang="en">A cable segment is a flow segment used to carry electrical power, data, or telecommunications signals. A cable segment is used to typically join two sections of an electrical network or a network of components carrying the electrical service.</rdfs:comment>
        <rdfs:comment xml:lang="es">Un segmento de cable es un segmento de flujo que se utiliza para transportar energía eléctrica, datos o señales de telecomunicaciones. Un segmento de cable se utiliza normalmente para unir dos secciones de una red eléctrica o una red de componentes que transportan el servicio eléctrico.</rdfs:comment>
        <rdfs:label xml:lang="en">Cable Segment</rdfs:label>
        <rdfs:label xml:lang="es">Segmento de Cable</rdfs:label>
    </owl:Class>
    


    <!-- https://w3id.org/mep#CableTransition -->


    <owl:Class rdf:about="https://w3id.org/mep#CableTransition">
        <rdfs:subClassOf rdf:resource="https://w3id.org/mep#CableFitting"/>
        <rdfs:comment xml:lang="en">A fitting that joins two cable segments of different connector types.</rdfs:comment>
        <rdfs:comment xml:lang="es">Accesorio que une dos segmentos de cable de diferentes tipos de conectores.</rdfs:comment>
        <rdfs:label xml:lang="en">Cable Transition</rdfs:label>
        <rdfs:label xml:lang="es">Transicion de Cable</rdfs:label>
    </owl:Class>
    


    <!-- https://w3id.org/mep#CableTraySegment -->


    <owl:Class rdf:about="https://w3id.org/mep#CableTraySegment">
        <rdfs:subClassOf rdf:resource="https://w3id.org/mep#CableCarrierSegment"/>
        <rdfs:comment xml:lang="en">A (typically) open carrier segment onto which cables are laid.</rdfs:comment>
        <rdfs:comment xml:lang="es">Un segmento portador (normalmente) abierto sobre el que se tienden los cables.</rdfs:comment>
        <rdfs:label xml:lang="en">Cable Tray Segment</rdfs:label>
        <rdfs:label xml:lang="es">Segmentode Bandeja de Cables</rdfs:label>
    </owl:Class>
    


    <!-- https://w3id.org/mep#CableTrunkingSegment -->


    <owl:Class rdf:about="https://w3id.org/mep#CableTrunkingSegment">
        <rdfs:subClassOf rdf:resource="https://w3id.org/mep#CableCarrierSegment"/>
        <rdfs:comment xml:lang="en">An enclosed carrier segment with one or more compartments into which cables are placed.</rdfs:comment>
        <rdfs:comment xml:lang="es">Un segmento de soporte cerrado con uno o más compartimentos en los que se colocan los cables.</rdfs:comment>
        <rdfs:label xml:lang="en">Cable Trunking Segment</rdfs:label>
        <rdfs:label xml:lang="es">Segmento de Canalizacion de Cables</rdfs:label>
    </owl:Class>
    


    <!-- https://w3id.org/mep#Camera -->


    <owl:Class rdf:about="https://w3id.org/mep#Camera">
        <rdfs:subClassOf rdf:resource="https://w3id.org/mep#AudioVisualAppliance"/>
        <rdfs:comment xml:lang="en">A device that records images, either as a still photograph or as moving images known as videos or movies. Note that a camera may operate with light from the visible spectrum or from other parts of the electromagnetic spectrum such as infrared or ultraviolet.</rdfs:comment>
        <rdfs:comment xml:lang="es">Dispositivo que graba imágenes, ya sea como fotografía fija o como imágenes en movimiento conocidas como videos o películas. Tenga en cuenta que una cámara puede funcionar con luz del espectro visible o de otras partes del espectro electromagnético, como la infrarroja o la ultravioleta.</rdfs:comment>
        <rdfs:label xml:lang="es">Camara</rdfs:label>
        <rdfs:label xml:lang="en">Camera</rdfs:label>
    </owl:Class>
    


    <!-- https://w3id.org/mep#Capacitor -->


    <owl:Class rdf:about="https://w3id.org/mep#Capacitor">
        <rdfs:subClassOf rdf:resource="https://w3id.org/mep#ElectricFlowStorageDevice"/>
        <rdfs:comment xml:lang="en">A device that stores electric charge when an external power supply is present using the electrical property of capacitance. Two-terminal device characterized essentially by its capacitance. Note: definition from IEC 60050 151-13-28.</rdfs:comment>
        <rdfs:comment xml:lang="es">Dispositivo que almacena carga eléctrica cuando hay una fuente de alimentación externa utilizando la propiedad eléctrica de la capacitancia. Dispositivo de dos terminales caracterizado esencialmente por su capacitancia. Nota: definición de la norma IEC 60050 151-13-28.</rdfs:comment>
        <rdfs:label xml:lang="en">Capacitor</rdfs:label>
        <rdfs:label xml:lang="es">Condensador</rdfs:label>
    </owl:Class>
    


    <!-- https://w3id.org/mep#CapacitorBank -->


    <owl:Class rdf:about="https://w3id.org/mep#CapacitorBank">
        <rdfs:subClassOf rdf:resource="https://w3id.org/mep#ElectricFlowStorageDevice"/>
        <rdfs:comment xml:lang="en">A device that stores electrical energy when an external power supply is present using the electrical property of capacitance.</rdfs:comment>
        <rdfs:comment xml:lang="es">Dispositivo que almacena energía eléctrica cuando hay una fuente de alimentación externa utilizando la propiedad eléctrica de la capacitancia.</rdfs:comment>
        <rdfs:label xml:lang="es">Bateria de Condensadores</rdfs:label>
        <rdfs:label xml:lang="en">Capacitor Bank</rdfs:label>
    </owl:Class>
    


    <!-- https://w3id.org/mep#CatenaryWire -->


    <owl:Class rdf:about="https://w3id.org/mep#CatenaryWire">
        <rdfs:subClassOf rdf:resource="https://w3id.org/mep#CableCarrierSegment"/>
        <rdfs:comment xml:lang="en">A catenary wire is a longitudinal wire supporting the grooved contact wires either directly or indirectly. Note: definition from UIC 719-1.</rdfs:comment>
        <rdfs:comment xml:lang="es">Un cable de catenaria es un cable longitudinal que soporta los cables de contacto ranurados directa o indirectamente. Nota: definición de UIC 719-1.</rdfs:comment>
        <rdfs:label xml:lang="es">Catenaria</rdfs:label>
        <rdfs:label xml:lang="en">Catenary Wire</rdfs:label>
    </owl:Class>
    


    <!-- https://w3id.org/mep#CentrfugalForward-CurvedFan -->


    <owl:Class rdf:about="https://w3id.org/mep#CentrfugalForward-CurvedFan">
        <rdfs:subClassOf rdf:resource="https://w3id.org/mep#Fan"/>
        <rdfs:comment xml:lang="en">Air flows through the impeller radially using blades that are forward curved.</rdfs:comment>
        <rdfs:comment xml:lang="es">El aire fluye a través del impulsor radialmente mediante palas curvadas hacia adelante.</rdfs:comment>
        <rdfs:label xml:lang="en">Centrfugal Forward-Curved Fan</rdfs:label>
        <rdfs:label xml:lang="es">Ventilador Centrifugo de Alabes Curvados hacia Alante</rdfs:label>
    </owl:Class>
    


    <!-- https://w3id.org/mep#CentrifugalAirfoilFan -->


    <owl:Class rdf:about="https://w3id.org/mep#CentrifugalAirfoilFan">
        <rdfs:subClassOf rdf:resource="https://w3id.org/mep#Fan"/>
        <rdfs:comment xml:lang="en">Air flows through the impeller radially using blades that are airfoil shaped.</rdfs:comment>
        <rdfs:comment xml:lang="es">El aire fluye a través del impulsor radialmente utilizando palas que tienen forma de perfil aerodinámico.</rdfs:comment>
        <rdfs:label xml:lang="en">Centrifugal Airfoil Fan</rdfs:label>
        <rdfs:label xml:lang="es">Ventilador Centrifugo de Alabes</rdfs:label>
    </owl:Class>
    


    <!-- https://w3id.org/mep#CentrifugalBackward-InclinedCurvedFan -->


    <owl:Class rdf:about="https://w3id.org/mep#CentrifugalBackward-InclinedCurvedFan">
        <rdfs:subClassOf rdf:resource="https://w3id.org/mep#Fan"/>
        <rdfs:comment xml:lang="en">Air flows through the impeller radially using blades that are backward curved.</rdfs:comment>
        <rdfs:comment xml:lang="es">El aire fluye a través del impulsor radialmente mediante palas curvadas hacia atrás.</rdfs:comment>
        <rdfs:label xml:lang="en">Centrifugal Backward-Inclined Curved Fan</rdfs:label>
        <rdfs:label xml:lang="es">Ventilador Centrifugo de Alabes Curvados hacia Atras</rdfs:label>
    </owl:Class>
    


    <!-- https://w3id.org/mep#CentrifugalRadialFan -->


    <owl:Class rdf:about="https://w3id.org/mep#CentrifugalRadialFan">
        <rdfs:subClassOf rdf:resource="https://w3id.org/mep#Fan"/>
        <rdfs:comment xml:lang="en">Air flows through the impeller radially using blades that are uncurved or slightly forward curved.</rdfs:comment>
        <rdfs:comment xml:lang="es">El aire fluye a través del impulsor radialmente usando palas que no están curvadas o ligeramente curvadas hacia adelante.</rdfs:comment>
        <rdfs:label xml:lang="en">Centrifugal Radial Fan</rdfs:label>
        <rdfs:label xml:lang="es">Ventilador Centrifugo de Alabes Radiales</rdfs:label>
    </owl:Class>
    


    <!-- https://w3id.org/mep#ChangeoverValve -->


    <owl:Class rdf:about="https://w3id.org/mep#ChangeoverValve">
        <rdfs:subClassOf rdf:resource="https://w3id.org/mep#Valve"/>
        <rdfs:comment xml:lang="en">Valve that enables flow to be switched between pipelines (3 or 4 port).</rdfs:comment>
        <rdfs:comment xml:lang="es">Válvula que permite cambiar el flujo entre tuberías (3 o 4 vías).</rdfs:comment>
        <rdfs:label xml:lang="en">Changeover Valve</rdfs:label>
        <rdfs:label xml:lang="es">Valvula de Cambio</rdfs:label>
    </owl:Class>
    


    <!-- https://w3id.org/mep#CheckValve -->


    <owl:Class rdf:about="https://w3id.org/mep#CheckValve">
        <rdfs:subClassOf rdf:resource="https://w3id.org/mep#Valve"/>
        <rdfs:comment xml:lang="en">Valve that permits water to flow in one direction only and is enclosed when there is no flow (2 port).</rdfs:comment>
        <rdfs:comment xml:lang="es">Válvula que permite que el agua fluya en una sola dirección y se cierra cuando no hay flujo (2 puertos).</rdfs:comment>
        <rdfs:label xml:lang="en">Check Valve</rdfs:label>
        <rdfs:label xml:lang="es">Valvula de Retencion</rdfs:label>
    </owl:Class>
    


    <!-- https://w3id.org/mep#Chiller -->


    <owl:Class rdf:about="https://w3id.org/mep#Chiller">
        <rdfs:subClassOf rdf:resource="https://w3id.org/mep#EnergyConversionDevice"/>
        <rdfs:comment xml:lang="en">A chiller is a device used to remove heat from a liquid via a vapor-compression or absorption refrigeration cycle to cool a fluid, typically water or a mixture of water and glycol. The chilled fluid is then used to cool and dehumidify air in a building.</rdfs:comment>
        <rdfs:comment xml:lang="es">Un refrigerador es un dispositivo que se utiliza para eliminar el calor de un líquido mediante un ciclo de refrigeración por absorción o compresión de vapor para enfriar un fluido, generalmente agua o una mezcla de agua y glicol. Luego, el fluido enfriado se utiliza para enfriar y deshumidificar el aire en un edificio.</rdfs:comment>
        <rdfs:label xml:lang="en">Chiller</rdfs:label>
        <rdfs:label xml:lang="es">Refrigerador</rdfs:label>
    </owl:Class>
    


    <!-- https://w3id.org/mep#Chopper -->


    <owl:Class rdf:about="https://w3id.org/mep#Chopper">
        <rdfs:subClassOf rdf:resource="https://w3id.org/mep#Transformer"/>
        <rdfs:comment xml:lang="es"> es un convertidor de CC de potencia electrónico sin un enlace de CA intermedio que proporciona un voltaje de salida variable al variar los períodos de conducción y no conducción en una proporción ajustable.</rdfs:comment>
        <rdfs:comment xml:lang="en">A chopper is an electronic power DC convertor without an intermediate AC link giving a variable output voltage by varying the periods of conduction and non-conduction in an adjustable ratio.</rdfs:comment>
        <rdfs:label xml:lang="en">Chopper</rdfs:label>
        <rdfs:label xml:lang="es">Chopper</rdfs:label>
    </owl:Class>
    


    <!-- https://w3id.org/mep#ChuteConveyor -->


    <owl:Class rdf:about="https://w3id.org/mep#ChuteConveyor">
        <rdfs:subClassOf rdf:resource="https://w3id.org/mep#ConveyorSegment"/>
        <rdfs:comment xml:lang="en">Gravity-operated conveyor where media descends through a trough or chute.</rdfs:comment>
        <rdfs:comment xml:lang="es">Transportador accionado por gravedad en el que el material desciende por una canaleta o vertedero.</rdfs:comment>
        <rdfs:label xml:lang="en">Chute Conveyor</rdfs:label>
        <rdfs:label xml:lang="es">Transportador de Canaleta</rdfs:label>
    </owl:Class>
    


    <!-- https://w3id.org/mep#CircuitBreaker -->


    <owl:Class rdf:about="https://w3id.org/mep#CircuitBreaker">
        <rdfs:subClassOf rdf:resource="https://w3id.org/mep#ProtectiveDevice"/>
        <rdfs:comment xml:lang="en">A mechanical switching device capable of making, carrying, and breaking currents under normal circuit conditions and also making, carrying for a specified time and breaking, current under specified abnormal circuit conditions such as those of short circuit.</rdfs:comment>
        <rdfs:comment xml:lang="es">Dispositivo mecánico de conmutación capaz de generar, transportar y cortar corriente en condiciones de circuito normales y también de generar, transportar durante un tiempo determinado y cortar corriente en condiciones de circuito anormales especificadas, como las de cortocircuito.</rdfs:comment>
        <rdfs:label xml:lang="en">Circuit Breaker</rdfs:label>
        <rdfs:label xml:lang="es">Disyuntor</rdfs:label>
    </owl:Class>
    


    <!-- https://w3id.org/mep#CirculatorPump -->


    <owl:Class rdf:about="https://w3id.org/mep#CirculatorPump">
        <rdfs:subClassOf rdf:resource="https://w3id.org/mep#Pump"/>
        <rdfs:comment xml:lang="en">A Circulator pump is a generic low-pressure, low-capacity pump. It may have a wet rotor and may be driven by a flexible-coupled motor.</rdfs:comment>
        <rdfs:comment xml:lang="es">Una bomba circuladora es una bomba genérica de baja presión y capacidad. Puede tener un rotor húmedo y estar accionada por un motor de acoplamiento flexible.</rdfs:comment>
        <rdfs:label xml:lang="es">Bomba Circuladora</rdfs:label>
        <rdfs:label xml:lang="en">Circulator Pump</rdfs:label>
    </owl:Class>
    


    <!-- https://w3id.org/mep#Cistern -->


    <owl:Class rdf:about="https://w3id.org/mep#Cistern">
        <rdfs:subClassOf rdf:resource="https://w3id.org/mep#SanitaryTerminal"/>
        <rdfs:comment xml:lang="en">A water storage unit attached to a sanitary terminal that is fitted with a device, operated automatically or by the user, that discharges water to cleanse a water closet (toilet) pan, urinal or slop hopper.</rdfs:comment>
        <rdfs:comment xml:lang="es">Unidad de almacenamiento de agua acoplada a un terminal sanitario que está equipada con un dispositivo, accionado automáticamente o por el usuario, que descarga agua para limpiar un inodoro, un urinario o una tolva.</rdfs:comment>
        <rdfs:label xml:lang="en">Cistern</rdfs:label>
        <rdfs:label xml:lang="es">Cisterna</rdfs:label>
    </owl:Class>
    


    <!-- https://w3id.org/mep#Coil -->


    <owl:Class rdf:about="https://w3id.org/mep#Coil">
        <rdfs:subClassOf rdf:resource="https://w3id.org/mep#EnergyConversionDevice"/>
        <rdfs:comment xml:lang="en">A coil is a device used to provide heat transfer between non-mixing media. A common example is a cooling coil, which utilizes a finned coil in which circulates chilled water, antifreeze, or refrigerant that is used to remove heat from air moving across the surface of the coil. A coil may be used either for heating or cooling purposes by placing a series of tubes (the coil) carrying a heating or cooling fluid into an airstream. The coil may be constructed from tubes bundled in a serpentine form or from finned tubes that give a extended heat transfer surface.Coils may also be used for non-airflow cases such as embedded in a floor slab.</rdfs:comment>
        <rdfs:comment xml:lang="es">Un serpentin es un dispositivo que se utiliza para proporcionar transferencia de calor entre medios que no se mezclan. Un ejemplo común es un serpentín de enfriamiento, que utiliza un serpentín con aletas por el que circula agua fría, anticongelante o refrigerante que se utiliza para eliminar el calor del aire que se mueve a través de la superficie del serpentín. Se puede utilizar un serpentín para calentar o enfriar colocando una serie de tubos (el serpentín) que transportan un fluido de calentamiento o enfriamiento a una corriente de aire. El serpentín se puede construir a partir de tubos agrupados en forma de serpentina o de tubos con aletas que proporcionan una superficie de transferencia de calor extendida. Los serpentines también se pueden usar para casos sin flujo de aire, como los empotrados en una losa de piso.</rdfs:comment>
        <rdfs:label xml:lang="en">Coil</rdfs:label>
        <rdfs:label xml:lang="es">Serpentin</rdfs:label>
    </owl:Class>
    


    <!-- https://w3id.org/mep#CombinedControlElement -->


    <owl:Class rdf:about="https://w3id.org/mep#CombinedControlElement">
        <rdfs:subClassOf rdf:resource="https://w3id.org/mep#UnitaryControlElement"/>
        <rdfs:comment xml:lang="es">Combinación de al menos dos tipos predefinidos de elemento de control unitario.</rdfs:comment>
        <rdfs:comment xml:lang="en">Combination of at least two predefined types of unitary control element.</rdfs:comment>
        <rdfs:label xml:lang="en">Combined Control Element</rdfs:label>
        <rdfs:label xml:lang="es">Elemento de Control Combinado</rdfs:label>
    </owl:Class>
    


    <!-- https://w3id.org/mep#CombinedFlowInstrument -->


    <owl:Class rdf:about="https://w3id.org/mep#CombinedFlowInstrument">
        <rdfs:subClassOf rdf:resource="https://w3id.org/mep#FlowInstrument"/>
        <rdfs:comment xml:lang="en">A device that reads and displays the value of multiple properties of a system at a point, or displays the difference in the value of a property between two points.</rdfs:comment>
        <rdfs:comment xml:lang="es">Dispositivo que lee y muestra el valor de múltiples propiedades de un sistema en un punto, o muestra la diferencia en el valor de una propiedad entre dos puntos.</rdfs:comment>
        <rdfs:label xml:lang="en">Combined Flow Instrument</rdfs:label>
        <rdfs:label xml:lang="es">Instrumento de Flujo Combinado</rdfs:label>
    </owl:Class>
    


    <!-- https://w3id.org/mep#CombinedTransformer -->


    <owl:Class rdf:about="https://w3id.org/mep#CombinedTransformer">
        <rdfs:subClassOf rdf:resource="https://w3id.org/mep#Transformer"/>
        <rdfs:comment xml:lang="en">A transformer that changes different quantities between circuits.</rdfs:comment>
        <rdfs:comment xml:lang="es">Un conversor que cambia diferentes cantidades entre circuitos.</rdfs:comment>
        <rdfs:label xml:lang="en">Combined Transformer</rdfs:label>
        <rdfs:label xml:lang="es">Conversor Combinado</rdfs:label>
    </owl:Class>
    


    <!-- https://w3id.org/mep#CommissioningValve -->


    <owl:Class rdf:about="https://w3id.org/mep#CommissioningValve">
        <rdfs:subClassOf rdf:resource="https://w3id.org/mep#Valve"/>
        <rdfs:comment xml:lang="en">Valve used to facilitate commissioning of a system (2 port).</rdfs:comment>
        <rdfs:comment xml:lang="es">Válvula utilizada para facilitar la puesta en marcha de un sistema (2 puertos).</rdfs:comment>
        <rdfs:label xml:lang="en">Commissioning Valve</rdfs:label>
        <rdfs:label xml:lang="es">Válvula de Puesta en Servicio</rdfs:label>
    </owl:Class>
    


    <!-- https://w3id.org/mep#CommunicationOutlet -->


    <owl:Class rdf:about="https://w3id.org/mep#CommunicationOutlet">
        <rdfs:subClassOf rdf:resource="https://w3id.org/mep#Outlet"/>
        <rdfs:comment xml:lang="en">An outlet used for connecting communications equipment.</rdfs:comment>
        <rdfs:comment xml:lang="es">Salida utilizada para conectar equipos de comunicaciones.</rdfs:comment>
        <rdfs:label xml:lang="en">Communication Outlet</rdfs:label>
        <rdfs:label xml:lang="es">Salida de Comunicaciones</rdfs:label>
    </owl:Class>
    


    <!-- https://w3id.org/mep#CommunicationTerminal -->


    <owl:Class rdf:about="https://w3id.org/mep#CommunicationTerminal">
        <rdfs:subClassOf rdf:resource="https://w3id.org/mep#AudioVisualAppliance"/>
        <rdfs:comment xml:lang="en">A communication terminal is an audio communication device that is usually installed along transportation infrastructure (railways, roads, tunnels etc.) in order to be used by the general public or operation agents for communication. It may specifically be used to make calls to emergency services in tunnels.</rdfs:comment>
        <rdfs:comment xml:lang="es">Un terminal de comunicación es un dispositivo de comunicación de audio que generalmente se instala a lo largo de la infraestructura de transporte (ferrocarriles, carreteras, túneles, etc.) para ser utilizado por el público en general o los agentes operativos para la comunicación. Puede utilizarse específicamente para realizar llamadas a los servicios de emergencia en túneles.</rdfs:comment>
        <rdfs:label xml:lang="en">Communication Terminal</rdfs:label>
        <rdfs:label xml:lang="es">Terminal de Comunicacion</rdfs:label>
    </owl:Class>
    


    <!-- https://w3id.org/mep#CommunicationsAppliance -->


    <owl:Class rdf:about="https://w3id.org/mep#CommunicationsAppliance">
        <rdfs:subClassOf rdf:resource="https://w3id.org/mep#FlowTerminal"/>
        <rdfs:comment xml:lang="en">A communications appliance transmits and receives electronic or digital information as data or sound. Communication appliances may be fixed in place or may be able to be moved from one space to another. Communication appliances require an electrical supply that may be supplied either by an electrical circuit or provided from a local battery source.</rdfs:comment>
        <rdfs:comment xml:lang="es">Un dispositivo de comunicación transmite y recibe información electrónica o digital en forma de datos o sonido. Los aparatos de comunicación pueden ser fijos o móviles. Los aparatos de comunicación requieren un suministro eléctrico que puede proceder de un circuito eléctrico o de una batería local.</rdfs:comment>
        <rdfs:label xml:lang="en">CommunicationsAppliance</rdfs:label>
        <rdfs:label xml:lang="es">Dispositivo de Comunicacion</rdfs:label>
    </owl:Class>
    


    <!-- https://w3id.org/mep#CompactFluorescentLamp -->


    <owl:Class rdf:about="https://w3id.org/mep#CompactFluorescentLamp">
        <rdfs:subClassOf rdf:resource="https://w3id.org/mep#Lamp"/>
        <rdfs:comment xml:lang="en">A fluorescent lamp having a compact form factor produced by shaping the tube.</rdfs:comment>
        <rdfs:comment xml:lang="es">Una lámpara fluorescente que tiene un factor de forma compacto producido al darle forma al tubo.</rdfs:comment>
        <rdfs:label xml:lang="en">Compact Fluorescent Lamp</rdfs:label>
        <rdfs:label xml:lang="es">Lampara Fluorescente Compacta</rdfs:label>
    </owl:Class>
    


    <!-- https://w3id.org/mep#Compensator -->


    <owl:Class rdf:about="https://w3id.org/mep#Compensator">
        <rdfs:subClassOf rdf:resource="https://w3id.org/mep#ElectricFlowStorageDevice"/>
        <rdfs:comment xml:lang="en">A device that is used to fix or adjust the parameter of electric energy, such as voltage loss, power factor and so on.</rdfs:comment>
        <rdfs:comment xml:lang="es">Dispositivo que se utiliza para fijar o ajustar los parámetros de la energía eléctrica, como la pérdida de tensión, el factor de potencia, etc.</rdfs:comment>
        <rdfs:label xml:lang="es">Compensador</rdfs:label>
        <rdfs:label xml:lang="en">Compensator</rdfs:label>
    </owl:Class>
    


    <!-- https://w3id.org/mep#CompressedAirFilter -->


    <owl:Class rdf:about="https://w3id.org/mep#CompressedAirFilter">
        <rdfs:subClassOf rdf:resource="https://w3id.org/mep#Filter"/>
        <rdfs:comment xml:lang="en">A filter used to remove particulates from compressed air.</rdfs:comment>
        <rdfs:comment xml:lang="es">Un filtro utilizado para eliminar partículas del aire comprimido.</rdfs:comment>
        <rdfs:label xml:lang="en">Compressed Air Filter</rdfs:label>
        <rdfs:label xml:lang="es">Filtro de Aire Comprimido</rdfs:label>
    </owl:Class>
    


    <!-- https://w3id.org/mep#Compressor -->


    <owl:Class rdf:about="https://w3id.org/mep#Compressor">
        <rdfs:subClassOf rdf:resource="https://w3id.org/mep#FlowMovingDevice"/>
        <rdfs:comment xml:lang="en">A compressor is a device that compresses a fluid typically used in a refrigeration circuit.</rdfs:comment>
        <rdfs:comment xml:lang="es">Un compresor es un dispositivo que comprime un fluido utilizado normalmente en un circuito de refrigeración.</rdfs:comment>
        <rdfs:label xml:lang="es">Compresor</rdfs:label>
        <rdfs:label xml:lang="en">Compressor</rdfs:label>
    </owl:Class>
    


    <!-- https://w3id.org/mep#Computer -->


    <owl:Class rdf:about="https://w3id.org/mep#Computer">
        <rdfs:subClassOf rdf:resource="https://w3id.org/mep#CommunicationsAppliance"/>
        <rdfs:comment xml:lang="en">A desktop, laptop, tablet, or other type of computer that can be moved from one place to another and connected to an electrical supply via a plugged outlet.</rdfs:comment>
        <rdfs:comment xml:lang="es">Ordenador de sobremesa, portátil, tableta u otro tipo de ordenador que puede trasladarse de un lugar a otro y conectarse a una fuente de alimentación eléctrica mediante un enchufe.</rdfs:comment>
        <rdfs:label xml:lang="es">Computadora</rdfs:label>
        <rdfs:label xml:lang="en">Computer</rdfs:label>
    </owl:Class>
    


    <!-- https://w3id.org/mep#Condenser -->


    <owl:Class rdf:about="https://w3id.org/mep#Condenser">
        <rdfs:subClassOf rdf:resource="https://w3id.org/mep#EnergyConversionDevice"/>
        <rdfs:comment xml:lang="en">A condenser is a device that is used to dissipate heat, typically by condensing a substance such as a refrigerant from its gaseous to its liquid state.</rdfs:comment>
        <rdfs:comment xml:lang="es">Un condensador es un dispositivo que se utiliza para disipar calor, normalmente condensando una sustancia, como un refrigerante, de su estado gaseoso a su estado líquido.</rdfs:comment>
        <rdfs:label xml:lang="en">Condenser</rdfs:label>
        <rdfs:label xml:lang="es">Conensador</rdfs:label>
    </owl:Class>
    


    <!-- https://w3id.org/mep#ConductanceSensor -->


    <owl:Class rdf:about="https://w3id.org/mep#ConductanceSensor">
        <rdfs:subClassOf rdf:resource="https://w3id.org/mep#Sensor"/>
        <rdfs:comment xml:lang="en">A device that senses or detects electrical conductance.</rdfs:comment>
        <rdfs:comment xml:lang="es">Dispositivo que detecta la conductancia eléctrica.</rdfs:comment>
        <rdfs:label xml:lang="en">Conductance Sensor</rdfs:label>
        <rdfs:label xml:lang="es">Sensor de Conductancia</rdfs:label>
    </owl:Class>
    


    <!-- https://w3id.org/mep#ConductorSegment -->


    <owl:Class rdf:about="https://w3id.org/mep#ConductorSegment">
        <rdfs:subClassOf rdf:resource="https://w3id.org/mep#CableSegment"/>
        <rdfs:comment xml:lang="en">A single linear element within a cable or an exposed wire (such as for grounding) with the specific purpose to lead electric current, data, or a telecommunications signal.</rdfs:comment>
        <rdfs:comment xml:lang="es">Un único elemento lineal dentro de un cable o alambre expuesto (como para conexión a tierra) con el propósito específico de conducir corriente eléctrica, datos o una señal de telecomunicaciones.</rdfs:comment>
        <rdfs:label xml:lang="en">Conductor Segment</rdfs:label>
        <rdfs:label xml:lang="es">Segmento de Conductor</rdfs:label>
    </owl:Class>
    


    <!-- https://w3id.org/mep#ConduitSegment -->


    <owl:Class rdf:about="https://w3id.org/mep#ConduitSegment">
        <rdfs:subClassOf rdf:resource="https://w3id.org/mep#CableCarrierSegment"/>
        <rdfs:comment xml:lang="en">An enclosed tubular carrier segment through which cables are pulled.</rdfs:comment>
        <rdfs:comment xml:lang="es">Un segmento tubular cerrado a través del cual se pasan los cables.</rdfs:comment>
        <rdfs:label xml:lang="en">Conduit Segment</rdfs:label>
        <rdfs:label xml:lang="es">Segmento de Conducto</rdfs:label>
    </owl:Class>
    


    <!-- https://w3id.org/mep#ConstantFlowTerminalBox -->


    <owl:Class rdf:about="https://w3id.org/mep#ConstantFlowTerminalBox">
        <rdfs:subClassOf rdf:resource="https://w3id.org/mep#AirTerminalBox"/>
        <rdfs:comment xml:lang="es">La caja de terminales que no incluye un medio para restablecer el volumen automáticamente a una señal externa como un termostato.</rdfs:comment>
        <rdfs:comment xml:lang="en">Terminal box that does not include a means to reset the volume automatically to an outside signal such as thermostat.</rdfs:comment>
        <rdfs:label xml:lang="es">Caja Terminal de Flujo Constante</rdfs:label>
        <rdfs:label xml:lang="en">Constant Flow Terminal Box</rdfs:label>
    </owl:Class>
    


    <!-- https://w3id.org/mep#ConsumerUnit -->


    <owl:Class rdf:about="https://w3id.org/mep#ConsumerUnit">
        <rdfs:subClassOf rdf:resource="https://w3id.org/mep#DistributionBoard"/>
        <rdfs:comment xml:lang="en">A distribution point on the incoming electrical supply, typically in domestic premises, at which protective devices are located.</rdfs:comment>
        <rdfs:comment xml:lang="es">Punto de distribución del suministro eléctrico entrante, normalmente en instalaciones domésticas, en el que se encuentran los dispositivos de protección.</rdfs:comment>
        <rdfs:label xml:lang="en">Consumer Unit</rdfs:label>
        <rdfs:label xml:lang="es">Unidad de Consumo</rdfs:label>
    </owl:Class>
    


    <!-- https://w3id.org/mep#ContactSensor -->


    <owl:Class rdf:about="https://w3id.org/mep#ContactSensor">
        <rdfs:subClassOf rdf:resource="https://w3id.org/mep#Sensor"/>
        <rdfs:comment xml:lang="en">A device that senses or detects contact, such as for detecting if a door is closed.</rdfs:comment>
        <rdfs:comment xml:lang="es">Dispositivo que percibe o detecta el contacto, por ejemplo, para detectar si una puerta está cerrada.</rdfs:comment>
        <rdfs:label xml:lang="en">Contact Sensor</rdfs:label>
        <rdfs:label xml:lang="es">Sensor de Contacto</rdfs:label>
    </owl:Class>
    


    <!-- https://w3id.org/mep#ContactWireSegment -->


    <owl:Class rdf:about="https://w3id.org/mep#ContactWireSegment">
        <rdfs:subClassOf rdf:resource="https://w3id.org/mep#CableSegment"/>
        <rdfs:comment xml:lang="en">An electric conductor of an overhead contact line with which the current collectors make contact. Note: definition from IEC60050 811-33-15.</rdfs:comment>
        <rdfs:comment xml:lang="es">Conductor eléctrico de una línea aérea de contacto con el que hacen contacto los colectores de corriente. Nota: definición de IEC60050 811-33-15.</rdfs:comment>
        <rdfs:label xml:lang="en">Contact Wire Segment</rdfs:label>
        <rdfs:label xml:lang="es">Segmento de cable de Contacto</rdfs:label>
    </owl:Class>
    


    <!-- https://w3id.org/mep#Contactor -->


    <owl:Class rdf:about="https://w3id.org/mep#Contactor">
        <rdfs:subClassOf rdf:resource="https://w3id.org/mep#SwitchingDevice"/>
        <rdfs:comment xml:lang="en">An electrical device used to control the flow of power in a circuit on or off.</rdfs:comment>
        <rdfs:comment xml:lang="es">Dispositivo eléctrico utilizado para controlar el encendido o apagado del flujo de energía en un circuito.</rdfs:comment>
        <rdfs:label xml:lang="en">Contactor</rdfs:label>
        <rdfs:label xml:lang="es">Contactor</rdfs:label>
    </owl:Class>
    


    <!-- https://w3id.org/mep#ControlDamper -->


    <owl:Class rdf:about="https://w3id.org/mep#ControlDamper">
        <rdfs:subClassOf rdf:resource="https://w3id.org/mep#Damper"/>
        <rdfs:comment xml:lang="es">Compuerta de regulación utilizada para modular el caudal de aire ajustando la posición de las lamas. Suele accionarse mediante un actuador de un sistema de automatización de edificios.</rdfs:comment>
        <rdfs:comment xml:lang="en">Control damper used to modulate the flow of air by adjusting the position of the blades. Commonly operated by an actuator of a building automation system.</rdfs:comment>
        <rdfs:label xml:lang="es">Compuerta de Regulacion</rdfs:label>
        <rdfs:label xml:lang="en">Control Damper</rdfs:label>
    </owl:Class>
    


    <!-- https://w3id.org/mep#ControlPanel -->


    <owl:Class rdf:about="https://w3id.org/mep#ControlPanel">
        <rdfs:subClassOf rdf:resource="https://w3id.org/mep#UnitaryControlElement"/>
        <rdfs:comment xml:lang="en">A control element at which devices that control or monitor the operation of a site, building or part of a building are located</rdfs:comment>
        <rdfs:comment xml:lang="es">Un elemento de control en el que se ubican los dispositivos que controlan o monitorean el funcionamiento de un sitio, edificio o parte de un edificio.</rdfs:comment>
        <rdfs:label xml:lang="en">Control Panel</rdfs:label>
        <rdfs:label xml:lang="es">Panel de Control</rdfs:label>
    </owl:Class>
    


    <!-- https://w3id.org/mep#Controller -->


    <owl:Class rdf:about="https://w3id.org/mep#Controller">
        <rdfs:subClassOf rdf:resource="https://w3id.org/mep#DistributionControlElement"/>
        <rdfs:comment xml:lang="en">A controller is a device that monitors inputs and controls outputs within a building automation system. A controller may be physical (having placement within a spatial structure) or logical (a software interface or aggregated within a programmable physical controller).</rdfs:comment>
        <rdfs:comment xml:lang="es">Un controlador es un dispositivo que supervisa las entradas y controla las salidas dentro de un sistema de automatización de edificios. Un controlador puede ser físico (ubicado dentro de una estructura espacial) o lógico (una interfaz de software o agregado dentro de un controlador físico programable).</rdfs:comment>
        <rdfs:label xml:lang="es">Controlador</rdfs:label>
        <rdfs:label xml:lang="en">Controller</rdfs:label>
    </owl:Class>
    


    <!-- https://w3id.org/mep#Convector -->


    <owl:Class rdf:about="https://w3id.org/mep#Convector">
        <rdfs:subClassOf rdf:resource="https://w3id.org/mep#SpaceHeater"/>
        <rdfs:comment xml:lang="en">A heat-distributing unit that operates with gravity-circulated air.</rdfs:comment>
        <rdfs:comment xml:lang="es">Unidad de distribución de calor que funciona con aire circulado por gravedad.</rdfs:comment>
        <rdfs:label xml:lang="en">Convector</rdfs:label>
        <rdfs:label xml:lang="es">Convector</rdfs:label>
    </owl:Class>
    


    <!-- https://w3id.org/mep#ConveyorSegment -->


    <owl:Class rdf:about="https://w3id.org/mep#ConveyorSegment">
        <rdfs:subClassOf rdf:resource="https://w3id.org/mep#FlowSegment"/>
        <rdfs:comment xml:lang="en">A conveyor segment defines an occurrence of a flow segment/ continuous run within a conveyor system that joins two sections of the system. these can utilise different carrying methods such as belt, rope, chain, screw etc.</rdfs:comment>
        <rdfs:comment xml:lang="es">Un segmento transportador define un segmento de flujo o recorrido continuo dentro de un sistema transportador que une dos secciones del sistema. Pueden utilizar diferentes métodos de transporte, como cintas, cables, cadenas, tornillos, etc.</rdfs:comment>
        <rdfs:label xml:lang="en">Conveyor Segment</rdfs:label>
        <rdfs:label xml:lang="es">Segmento Transportador</rdfs:label>
    </owl:Class>
    


    <!-- https://w3id.org/mep#CooledBeam -->


    <owl:Class rdf:about="https://w3id.org/mep#CooledBeam">
        <rdfs:subClassOf rdf:resource="https://w3id.org/mep#EnergyConversionDevice"/>
        <rdfs:comment xml:lang="en">A cooled beam (or chilled beam) is a device typically used to cool air by circulating a fluid such as chilled water through exposed finned tubes above a space. Typically mounted overhead near or within a ceiling, the cooled beam uses convection to cool the space below it by acting as a heat sink for the naturally rising warm air of the space. Once cooled, the air naturally drops back to the floor where the cycle begins again.</rdfs:comment>
        <rdfs:comment xml:lang="es">Una viga fría (o viga refrigerante) es un dispositivo que suele utilizarse para enfriar el aire haciendo circular un fluido, como agua fría, a través de tubos con aletas expuestos por encima de un espacio. La viga fría, que suele montarse en el techo o cerca de él, utiliza la convección para enfriar el espacio que tiene debajo actuando como sumidero de calor para el aire caliente que se eleva de forma natural. Una vez enfriado, el aire desciende de forma natural hasta el suelo, donde el ciclo comienza de nuevo.</rdfs:comment>
        <rdfs:label xml:lang="en">CooledBeam</rdfs:label>
        <rdfs:label xml:lang="es">Viga Refrigerante</rdfs:label>
    </owl:Class>
    


    <!-- https://w3id.org/mep#CoolingTower -->


    <owl:Class rdf:about="https://w3id.org/mep#CoolingTower">
        <rdfs:subClassOf rdf:resource="https://w3id.org/mep#EnergyConversionDevice"/>
        <rdfs:comment xml:lang="en">A cooling tower is a device which rejects heat to ambient air by circulating a fluid such as water through it to reduce its temperature by partial evaporation.</rdfs:comment>
        <rdfs:comment xml:lang="es">Una torre de refrigeración es un dispositivo que expulsa el calor al aire ambiente haciendo circular un fluido, como el agua, para reducir su temperatura por evaporación parcial.</rdfs:comment>
        <rdfs:label xml:lang="en">CoolingTower</rdfs:label>
        <rdfs:label xml:lang="es">Torre de Refrigeración</rdfs:label>
    </owl:Class>
    


    <!-- https://w3id.org/mep#CoreSegment -->


    <owl:Class rdf:about="https://w3id.org/mep#CoreSegment">
        <rdfs:subClassOf rdf:resource="https://w3id.org/mep#CableSegment"/>
        <rdfs:comment xml:lang="en">A self contained element of a cable that comprises one or more conductors and sheathing.The core of one lead is normally single wired or multiwired which are intertwined.</rdfs:comment>
        <rdfs:comment xml:lang="es">Elemento autónomo de un cable que comprende uno o más conductores y revestimiento. El núcleo de un cable normalmente es de un solo cable o de varios cables entrelazados.</rdfs:comment>
        <rdfs:label xml:lang="en">Core Segment</rdfs:label>
        <rdfs:label xml:lang="es">Segmento de Nucleo</rdfs:label>
    </owl:Class>
    


    <!-- https://w3id.org/mep#Coupling -->


    <owl:Class rdf:about="https://w3id.org/mep#Coupling">
        <rdfs:subClassOf rdf:resource="https://w3id.org/mep#MotorConnection"/>
        <rdfs:comment xml:lang="en">An indirect connection made through the medium of the viscosity of a fluid.</rdfs:comment>
        <rdfs:comment xml:lang="es">Conexión indirecta realizada a través de la viscosidad de un fluido.</rdfs:comment>
        <rdfs:label xml:lang="es">Acoplamiento</rdfs:label>
        <rdfs:label xml:lang="en">Coupling</rdfs:label>
    </owl:Class>
    


    <!-- https://w3id.org/mep#Cowl -->


    <owl:Class rdf:about="https://w3id.org/mep#Cowl">
        <rdfs:subClassOf rdf:resource="https://w3id.org/mep#StackTerminal"/>
        <rdfs:comment xml:lang="en">A cowling placed at the top of a stack to eliminate downdraft.</rdfs:comment>
        <rdfs:comment xml:lang="es">El sombrerete Antirrevoco se coloca el la parte superior de la chimenea para elminar la correitne descendiente</rdfs:comment>
        <rdfs:label xml:lang="en">Cowl</rdfs:label>
        <rdfs:label xml:lang="es">Sombrerete Antirrevoco</rdfs:label>
    </owl:Class>
    


    <!-- https://w3id.org/mep#Culvert -->


    <owl:Class rdf:about="https://w3id.org/mep#Culvert">
        <rdfs:subClassOf rdf:resource="https://w3id.org/mep#PipeSegment"/>
        <rdfs:comment xml:lang="en">A covered channel or large pipe that forms a watercourse below ground level, usually under a road or railway.</rdfs:comment>
        <rdfs:comment xml:lang="es">Canal cubierto o tubería grande que forma un curso de agua bajo el nivel del suelo, normalmente bajo una carretera o vía férrea.</rdfs:comment>
        <rdfs:label xml:lang="es">Alcantarilla</rdfs:label>
        <rdfs:label xml:lang="en">Culvert</rdfs:label>
    </owl:Class>
    


    <!-- https://w3id.org/mep#CurrentTransformer -->


    <owl:Class rdf:about="https://w3id.org/mep#CurrentTransformer">
        <rdfs:subClassOf rdf:resource="https://w3id.org/mep#Transformer"/>
        <rdfs:comment xml:lang="en">A transformer that changes the current between circuits.</rdfs:comment>
        <rdfs:comment xml:lang="es">Un conversor que cambia la corriente entre circuitos.</rdfs:comment>
        <rdfs:label xml:lang="es">Conversor de Corriente</rdfs:label>
        <rdfs:label xml:lang="en">Current Transformer</rdfs:label>
    </owl:Class>
    


    <!-- https://w3id.org/mep#CyclonicInterceptor -->


    <owl:Class rdf:about="https://w3id.org/mep#CyclonicInterceptor">
        <rdfs:subClassOf rdf:resource="https://w3id.org/mep#Interceptor"/>
        <rdfs:comment xml:lang="es">Elimina gotas de líquido más grandes o partículas sólidas más grandes.</rdfs:comment>
        <rdfs:comment xml:lang="en">Removes larger liquid drops or larger solid particles.</rdfs:comment>
        <rdfs:label xml:lang="en">Cyclonic Interceptor</rdfs:label>
        <rdfs:label xml:lang="es">Interceptor CYCLONIC</rdfs:label>
    </owl:Class>
    


    <!-- https://w3id.org/mep#DCMotor -->


    <owl:Class rdf:about="https://w3id.org/mep#DCMotor">
        <rdfs:subClassOf rdf:resource="https://w3id.org/mep#ElectricMotor"/>
        <rdfs:comment xml:lang="en">A motor using either generated or rectified Direct Current (DC) power.</rdfs:comment>
        <rdfs:comment xml:lang="es">Un motor que utiliza energía de corriente continua (CC) generada o rectificada.</rdfs:comment>
        <rdfs:label xml:lang="en">DC Motor</rdfs:label>
        <rdfs:label xml:lang="es">Motor CC</rdfs:label>
    </owl:Class>
    


    <!-- https://w3id.org/mep#DXCoolingCoil -->


    <owl:Class rdf:about="https://w3id.org/mep#DXCoolingCoil">
        <rdfs:subClassOf rdf:resource="https://w3id.org/mep#Coil"/>
        <rdfs:comment xml:lang="en">Cooling coil using a refrigerant to cool the air stream directly.</rdfs:comment>
        <rdfs:comment xml:lang="es">Serpentín de enfriamiento que utiliza un refrigerante para enfriar la corriente de aire directamente.</rdfs:comment>
        <rdfs:label xml:lang="en">DX Cooling Coil</rdfs:label>
        <rdfs:label xml:lang="es">Serpentin DX Evaporador</rdfs:label>
    </owl:Class>
    


    <!-- https://w3id.org/mep#Damper -->


    <owl:Class rdf:about="https://w3id.org/mep#Damper">
        <rdfs:subClassOf rdf:resource="https://w3id.org/mep#FlowController"/>
        <rdfs:comment xml:lang="en">A damper typically participates in an HVAC duct distribution system and is used to control or modulate the flow of air.</rdfs:comment>
        <rdfs:comment xml:lang="es">Una compuerta suele participar en un sistema de distribución de conductos de calefacción, ventilación y aire acondicionado y se utiliza para controlar o modular el flujo de aire.</rdfs:comment>
        <rdfs:label xml:lang="es">Compuerta</rdfs:label>
        <rdfs:label xml:lang="en">Damper</rdfs:label>
    </owl:Class>
    


    <!-- https://w3id.org/mep#DataJuntionBox -->


    <owl:Class rdf:about="https://w3id.org/mep#DataJuntionBox">
        <rdfs:subClassOf rdf:resource="https://w3id.org/mep#JunctionBox"/>
        <rdfs:comment xml:lang="en">Contains cables, outlets, and/or switches for communications use.</rdfs:comment>
        <rdfs:comment xml:lang="es">Contiene cables, tomacorrientes y/o interruptores para uso de comunicaciones.</rdfs:comment>
        <rdfs:label xml:lang="es">Caja de conexiones de Datos</rdfs:label>
        <rdfs:label xml:lang="en">Data Juntion Box</rdfs:label>
    </owl:Class>
    


    <!-- https://w3id.org/mep#DataOutlet -->


    <owl:Class rdf:about="https://w3id.org/mep#DataOutlet">
        <rdfs:subClassOf rdf:resource="https://w3id.org/mep#Outlet"/>
        <rdfs:comment xml:lang="en">An outlet used for connecting electrical devices requiring power.</rdfs:comment>
        <rdfs:comment xml:lang="es">Salida utilizada para conectar aparatos eléctricos que necesitan corriente.</rdfs:comment>
        <rdfs:label xml:lang="en">Data Outlet</rdfs:label>
        <rdfs:label xml:lang="es">Salida de Datos</rdfs:label>
    </owl:Class>
    


    <!-- https://w3id.org/mep#Dehumidifier -->


    <owl:Class rdf:about="https://w3id.org/mep#Dehumidifier">
        <rdfs:subClassOf rdf:resource="https://w3id.org/mep#UnitaryEquipment"/>
        <rdfs:comment xml:lang="en">A unitary packaged dehumidification unit. Note: units supporting multiple modes (dehumidification, cooling, and/or heating) should use Air Conditioning Unit.</rdfs:comment>
        <rdfs:comment xml:lang="es">Una unidad de deshumidificación unitaria y empaquetada. Nota: las unidades que admiten múltiples modos (deshumidificación, enfriamiento y/o calefacción) deben usar Unidad de Aire Acondicionado.</rdfs:comment>
        <rdfs:label xml:lang="en">Dehumidifier</rdfs:label>
        <rdfs:label xml:lang="es">Deshumidificador</rdfs:label>
    </owl:Class>
    


    <!-- https://w3id.org/mep#Diffuser -->


    <owl:Class rdf:about="https://w3id.org/mep#Diffuser">
        <rdfs:subClassOf rdf:resource="https://w3id.org/mep#AirTerminal"/>
        <rdfs:comment xml:lang="en">An outlet discharging supply air in various directions and planes.</rdfs:comment>
        <rdfs:comment xml:lang="es">Una salida que descarga el aire suministrado en varias direcciones y planos.</rdfs:comment>
        <rdfs:label xml:lang="en">Diffuser</rdfs:label>
        <rdfs:label xml:lang="es">Difusor</rdfs:label>
    </owl:Class>
    


    <!-- https://w3id.org/mep#DimmerSwitch -->


    <owl:Class rdf:about="https://w3id.org/mep#DimmerSwitch">
        <rdfs:subClassOf rdf:resource="https://w3id.org/mep#SwitchingDevice"/>
        <rdfs:comment xml:lang="en">A dimmer switch has variable positions, and may adjust electrical power or other setting (according to the switched port type).</rdfs:comment>
        <rdfs:comment xml:lang="es">Un regulador de intensidad tiene posiciones variables y puede ajustar la potencia eléctrica u otro ajuste (según el tipo de puerto conmutado).</rdfs:comment>
        <rdfs:label xml:lang="en">Dimmer Switch</rdfs:label>
        <rdfs:label xml:lang="es">Regulador de Intesidad</rdfs:label>
    </owl:Class>
    


    <!-- https://w3id.org/mep#DirectDrive -->


    <owl:Class rdf:about="https://w3id.org/mep#DirectDrive">
        <rdfs:subClassOf rdf:resource="https://w3id.org/mep#MotorConnection"/>
        <rdfs:comment xml:lang="en">A direct, physical connection made between the motor and the driven device.</rdfs:comment>
        <rdfs:comment xml:lang="es">Conexión física directa entre el motor y el dispositivo accionado.</rdfs:comment>
        <rdfs:label xml:lang="en">Direct Drive</rdfs:label>
        <rdfs:label xml:lang="es">Transmision directa</rdfs:label>
    </owl:Class>
    


    <!-- https://w3id.org/mep#DirectEvaporativePackagedRotaryAirCooler -->


    <owl:Class rdf:about="https://w3id.org/mep#DirectEvaporativePackagedRotaryAirCooler">
        <rdfs:subClassOf rdf:resource="https://w3id.org/mep#EvaporativeCooler"/>
        <rdfs:comment xml:lang="en">Direct evaporative packaged rotary air cooler: Cools the air stream by evaporating water dircectly into the air stream using coolers that wet and wash the evaporative pad by rotating it through a water bath.</rdfs:comment>
        <rdfs:comment xml:lang="es">Enfriador de aire rotativo empaquetado por evaporación directa: Enfría la corriente de aire evaporando el agua directamente en la corriente de aire usando enfriadores que humedecen y lavan la almohadilla evaporativa girándola a través de un baño de agua.</rdfs:comment>
        <rdfs:label xml:lang="en">Direct Evaporative Packaged Rotary Air Cooler</rdfs:label>
        <rdfs:label xml:lang="es">Enfriador de Aire Rotativo Empaquetado por Evaporación Directa</rdfs:label>
    </owl:Class>
    


    <!-- https://w3id.org/mep#DirectEvaporativeRandomMediaAirCooler -->


    <owl:Class rdf:about="https://w3id.org/mep#DirectEvaporativeRandomMediaAirCooler">
        <rdfs:subClassOf rdf:resource="https://w3id.org/mep#EvaporativeCooler"/>
        <rdfs:comment xml:lang="en">Direct evaporative random media air cooler: Cools the air stream by evaporating water dircectly into the air stream using coolers with evaporative pads, usually of aspen wood or plastic fiber/foam.</rdfs:comment>
        <rdfs:comment xml:lang="es">Enfriador de aire de medios aleatorios por evaporación directa: enfría la corriente de aire evaporando el agua directamente en la corriente de aire utilizando enfriadores con almohadillas evaporativas, generalmente de madera de álamo temblón o fibra/espuma plástica.</rdfs:comment>
        <rdfs:label xml:lang="en">Direct Evaporative Random Media Air Cooler</rdfs:label>
        <rdfs:label xml:lang="es">Enfriador de Aire de Medios Aleatorios por Evaporación Directa</rdfs:label>
    </owl:Class>
    


    <!-- https://w3id.org/mep#DirectEvaporativeRigidMediaAirCooler -->


    <owl:Class rdf:about="https://w3id.org/mep#DirectEvaporativeRigidMediaAirCooler">
        <rdfs:subClassOf rdf:resource="https://w3id.org/mep#EvaporativeCooler"/>
        <rdfs:comment xml:lang="en">Direct evaporative rigid media air cooler: Cools the air stream by evaporating water dircectly into the air stream using coolers with sheets of rigid, corrugated material as the wetted surface.</rdfs:comment>
        <rdfs:comment xml:lang="es">Enfriador de aire de medio rígido por evaporación directa: enfría la corriente de aire evaporando el agua directamente en la corriente de aire utilizando enfriadores con láminas de material rígido corrugado como superficie humedecida.</rdfs:comment>
        <rdfs:label xml:lang="en">Direct Evaporative Rigid Media Air Cooler</rdfs:label>
        <rdfs:label xml:lang="es">Enfriador de Aire de Medio Rígido por Evaporación Directa</rdfs:label>
    </owl:Class>
    


    <!-- https://w3id.org/mep#DirectEvaporativeSlingersPackagedAirCooler -->


    <owl:Class rdf:about="https://w3id.org/mep#DirectEvaporativeSlingersPackagedAirCooler">
        <rdfs:subClassOf rdf:resource="https://w3id.org/mep#EvaporativeCooler"/>
        <rdfs:comment xml:lang="en">Direct evaporative slingers packaged air cooler: Cools the air stream by evaporating water dircectly into the air stream using coolers with a water slinger in an evaporative cooling section and a fan section.</rdfs:comment>
        <rdfs:comment xml:lang="es">Enfriador de aire compacto con deflectores evaporativos directos: enfría la corriente de aire evaporando el agua directamente en la corriente de aire utilizando enfriadores con un deflector de agua en una sección de enfriamiento por evaporación y una sección de ventilador.</rdfs:comment>
        <rdfs:label xml:lang="en">Direct Evaporative Slingers Packaged Air Cooler</rdfs:label>
        <rdfs:label xml:lang="es">Enfriador de Aire Compacto con Deflectores Evaporativos Directos</rdfs:label>
    </owl:Class>
    


    <!-- https://w3id.org/mep#DirectExpansionBrazedPlateEvaporator -->


    <owl:Class rdf:about="https://w3id.org/mep#DirectExpansionBrazedPlateEvaporator">
        <rdfs:subClassOf rdf:resource="https://w3id.org/mep#Evaporator"/>
        <rdfs:comment xml:lang="en">Direct-expansion evaporator where a refrigerant evaporates inside plates brazed or welded together to make up an assembly of separate channels.</rdfs:comment>
        <rdfs:comment xml:lang="es">Evaporador de expansión directa donde un refrigerante se evapora dentro de placas soldadas entre sí para formar un conjunto de canales separados.</rdfs:comment>
        <rdfs:label xml:lang="en">Direct Expansion Brazed Plate Evaporator</rdfs:label>
        <rdfs:label xml:lang="es">Evaporador de Placas Soldadas de Expansión Directa</rdfs:label>
    </owl:Class>
    


    <!-- https://w3id.org/mep#DirectExpansionEvaporator -->


    <owl:Class rdf:about="https://w3id.org/mep#DirectExpansionEvaporator">
        <rdfs:subClassOf rdf:resource="https://w3id.org/mep#Evaporator"/>
        <rdfs:comment xml:lang="en"></rdfs:comment>
        <rdfs:comment xml:lang="es"></rdfs:comment>
        <rdfs:label xml:lang="en">Direct Expansion Evaporator</rdfs:label>
        <rdfs:label xml:lang="es">Evaporador de Expansion Directa</rdfs:label>
    </owl:Class>
    


    <!-- https://w3id.org/mep#DirectExpansionShell-and-TubeEvaporator -->


    <owl:Class rdf:about="https://w3id.org/mep#DirectExpansionShell-and-TubeEvaporator">
        <rdfs:subClassOf rdf:resource="https://w3id.org/mep#Evaporator"/>
        <rdfs:comment xml:lang="en">Direct-expansion evaporator where a refrigerant evaporates inside a series of baffles that channel the fluid throughout the shell side.</rdfs:comment>
        <rdfs:comment xml:lang="es">Evaporador de expansión directa donde un refrigerante se evapora dentro de una serie de deflectores que canalizan el fluido por todo el lado de la carcasa.</rdfs:comment>
        <rdfs:label xml:lang="en">Direct Expansion Shell-and-Tube Evaporator</rdfs:label>
        <rdfs:label xml:lang="es">Evaporador de Tubo y Carcasa de Expansion Directa</rdfs:label>
    </owl:Class>
    


    <!-- https://w3id.org/mep#DirectExpansionTube-in-TubeEvaporator -->


    <owl:Class rdf:about="https://w3id.org/mep#DirectExpansionTube-in-TubeEvaporator">
        <rdfs:subClassOf rdf:resource="https://w3id.org/mep#Evaporator"/>
        <rdfs:comment xml:lang="en">Direct-expansion evaporator where a refrigerant evaporates inside one or more pairs of coaxial tubes.</rdfs:comment>
        <rdfs:comment xml:lang="es">Evaporador de expansión directa donde un refrigerante se evapora dentro de uno o más pares de tubos coaxiales.</rdfs:comment>
        <rdfs:label xml:lang="en">Direct Expansion Tube-in-Tube Evaporator</rdfs:label>
        <rdfs:label xml:lang="es">Evaporador de Tubo en Tubo de Expansion Directa</rdfs:label>
    </owl:Class>
    


    <!-- https://w3id.org/mep#DirectVaporativeWasher -->


    <owl:Class rdf:about="https://w3id.org/mep#DirectVaporativeWasher">
        <rdfs:subClassOf rdf:resource="https://w3id.org/mep#EvaporativeCooler"/>
        <rdfs:comment xml:lang="en">Direct evaporative air washer: Cools the air stream by evaporating water dircectly into the air stream using coolers with spray-type air washer consist of a chamber or casing containing spray nozzles, and tank for collecting spray water, and an eliminator section for removing entrained drops of water from the air.</rdfs:comment>
        <rdfs:comment xml:lang="es">Lavador de aire por evaporación directa: enfría la corriente de aire evaporando el agua directamente en la corriente de aire usando enfriadores con lavador de aire tipo rociador que consisten en una cámara o carcasa que contiene boquillas rociadoras, un tanque para recolectar el agua rociada y una sección eliminadora para eliminar las gotas arrastradas. de agua del aire.</rdfs:comment>
        <rdfs:label xml:lang="en">Direct Vaporative Washer</rdfs:label>
        <rdfs:label xml:lang="es">Lavador de Aire por Evaporacion Directa</rdfs:label>
    </owl:Class>
    


    <!-- https://w3id.org/mep#DirectionSourceLightFixture -->


    <owl:Class rdf:about="https://w3id.org/mep#DirectionSourceLightFixture">
        <rdfs:subClassOf rdf:resource="https://w3id.org/mep#LightFixture"/>
        <rdfs:comment xml:lang="en">A light fixture that is considered to have a length or surface area from which it emits light in a direction. A light fixture containing one or more fluorescent lamps is an example of a direction source.</rdfs:comment>
        <rdfs:comment xml:lang="es">Un artefacto de iluminación que se considera que tiene una longitud o superficie desde la cual emite luz en una dirección. Un dispositivo de iluminación que contiene una o más lámparas fluorescentes es un ejemplo de fuente direccional.</rdfs:comment>
        <rdfs:label xml:lang="es">Artefacto de Iluminación de fuente de dirección</rdfs:label>
        <rdfs:label xml:lang="en">Direction Source Light Fixture</rdfs:label>
    </owl:Class>
    


    <!-- https://w3id.org/mep#Dishwasher -->


    <owl:Class rdf:about="https://w3id.org/mep#Dishwasher">
        <rdfs:subClassOf rdf:resource="https://w3id.org/mep#ElectricAppliance"/>
        <rdfs:comment xml:lang="en">An appliance that has the primary function of washing dishes.</rdfs:comment>
        <rdfs:comment xml:lang="es">Aparato cuya función principal es lavar la vajilla.</rdfs:comment>
        <rdfs:label xml:lang="en">Dishwasher</rdfs:label>
        <rdfs:label xml:lang="es">Lavavajillas</rdfs:label>
    </owl:Class>
    


    <!-- https://w3id.org/mep#DispatchingBoard -->


    <owl:Class rdf:about="https://w3id.org/mep#DispatchingBoard">
        <rdfs:subClassOf rdf:resource="https://w3id.org/mep#DistributionBoard"/>
        <rdfs:comment xml:lang="en">A distribution point at which voice and data communication signals are managed between communication devices.</rdfs:comment>
        <rdfs:comment xml:lang="es">Punto de distribución en el que se gestionan las señales de comunicación de voz y datos entre los dispositivos de comunicación.</rdfs:comment>
        <rdfs:label xml:lang="es">Centralita</rdfs:label>
        <rdfs:label xml:lang="en">Dispatching Board</rdfs:label>
    </owl:Class>
    


    <!-- https://w3id.org/mep#Display -->


    <owl:Class rdf:about="https://w3id.org/mep#Display">
        <rdfs:subClassOf rdf:resource="https://w3id.org/mep#AudioVisualAppliance"/>
        <rdfs:comment xml:lang="en">An electronic device that represents information in visual form such as a flat-panel display or television.</rdfs:comment>
        <rdfs:comment xml:lang="es">Dispositivo electrónico que representa información en forma visual, como una pantalla plana o un televisor.</rdfs:comment>
        <rdfs:label xml:lang="en">Display</rdfs:label>
        <rdfs:label xml:lang="es">Display</rdfs:label>
    </owl:Class>
    


    <!-- https://w3id.org/mep#DistributionBoard -->


    <owl:Class rdf:about="https://w3id.org/mep#DistributionBoard">
        <rdfs:subClassOf rdf:resource="https://w3id.org/mep#FlowController"/>
        <rdfs:comment xml:lang="en">A distribution board is a flow controller in which instances of electrical or communication devices are brought together at a single place for a particular purpose. A distribution provides a housing for connected distribution elements so that they can be viewed, operated or acted upon from a single place. Each connected item may have its own geometric representation and location.</rdfs:comment>
        <rdfs:comment xml:lang="es">Un cuadro de distribución es un controlador de flujo en el que se reúnen instancias de dispositivos eléctricos o de comunicación en un único lugar para un fin determinado. Una distribución proporciona un alojamiento para los elementos de distribución conectados, de modo que se puedan ver, manejar o actuar sobre ellos desde un único lugar. Cada elemento conectado puede tener su propia representación geométrica y ubicación.</rdfs:comment>
        <rdfs:label xml:lang="es">Cuadro de Distribucion</rdfs:label>
        <rdfs:label xml:lang="en">Distribution Board</rdfs:label>
    </owl:Class>
    


    <!-- https://w3id.org/mep#DistributionChamberElement -->


    <owl:Class rdf:about="https://w3id.org/mep#DistributionChamberElement">
        <rdfs:subClassOf rdf:resource="https://w3id.org/mep#DistributionFlowElement"/>
        <rdfs:comment xml:lang="en">A distribution chamber element defines a place at which distribution systems and their constituent elements may be inspected or through which they may travel.</rdfs:comment>
        <rdfs:comment xml:lang="es">Un elemento de la cámara de distribución define un lugar en el que los sistemas de distribución y sus elementos constitutivos pueden ser inspeccionados o por el que pueden transitar.</rdfs:comment>
        <rdfs:label xml:lang="en">DistributionChamberElement</rdfs:label>
        <rdfs:label xml:lang="es">Elemento de Camara de Distribucion</rdfs:label>
    </owl:Class>
    


    <!-- https://w3id.org/mep#DistributionControlElement -->


    <owl:Class rdf:about="https://w3id.org/mep#DistributionControlElement">
        <rdfs:subClassOf rdf:resource="https://w3id.org/mep#DistributionElement"/>
        <rdfs:comment xml:lang="es">Define los elementos de un sistema de control de automatización de edificios. Se suelen utilizar para controlar elementos del sistema de distribución con el fin de mantener variables como la temperatura, la humedad, la presión, el caudal, la potencia o los niveles de iluminación, mediante la modulación, la puesta en escena o la secuenciación de dispositivos mecánicos o eléctricos</rdfs:comment>
        <rdfs:comment xml:lang="en">Defines elements of a building automation control system. These are typically used to control distribution system elements to maintain variables such as temperature, humidity, pressure, flow, power, or lighting levels, through the modulation, staging or sequencing of mechanical or electrical devices</rdfs:comment>
        <rdfs:label xml:lang="en">DistributionControlElement</rdfs:label>
        <rdfs:label xml:lang="es">Elemento de Control de Distribucion</rdfs:label>
    </owl:Class>
    


    <!-- https://w3id.org/mep#DistributionElement -->


    <owl:Class rdf:about="https://w3id.org/mep#DistributionElement">
        <rdfs:subClassOf rdf:resource="https://schema.org/Product"/>
        <rdfs:comment xml:lang="es">Generalización de todos los elementos que participan en un sistema de distribución.</rdfs:comment>
        <rdfs:comment xml:lang="en">Generalization of all elements that participate in a distribution system.</rdfs:comment>
        <rdfs:label xml:lang="en">Distribution Element</rdfs:label>
        <rdfs:label xml:lang="es">Elemento de Distribución</rdfs:label>
    </owl:Class>
    


    <!-- https://w3id.org/mep#DistributionFlowElement -->


    <owl:Class rdf:about="https://w3id.org/mep#DistributionFlowElement">
        <rdfs:subClassOf rdf:resource="https://w3id.org/mep#DistributionElement"/>
        <rdfs:comment xml:lang="es">Define los elementos de un sistema de distribución que facilitan la distribución de energía o materia, como el aire, el agua o la electricidad.</rdfs:comment>
        <rdfs:comment xml:lang="en">Defines occurrence elements of a distribution system that facilitate the distribution of energy or matter, such as air, water or power.</rdfs:comment>
        <rdfs:label xml:lang="en">DistributionFlowElement</rdfs:label>
        <rdfs:label xml:lang="es">Elemento de Flujo de Distribución</rdfs:label>
    </owl:Class>
    


    <!-- https://w3id.org/mep#DistributionFrame -->


    <owl:Class rdf:about="https://w3id.org/mep#DistributionFrame">
        <rdfs:subClassOf rdf:resource="https://w3id.org/mep#DistributionBoard"/>
        <rdfs:comment xml:lang="en">A distribution frame is used to interconnect and manage wiring between active equipment and subscriber. It might be composed of multiple distribution boards and other components.</rdfs:comment>
        <rdfs:comment xml:lang="es">Un cuadro de distribución se utiliza para interconectar y gestionar el cableado entre los equipos activos y el abonado. Puede estar compuesto por varios cuadros de distribución y otros componentes.</rdfs:comment>
        <rdfs:label xml:lang="es">Centro de Distribucion</rdfs:label>
        <rdfs:label xml:lang="en">Distribution Frame</rdfs:label>
    </owl:Class>
    


    <!-- https://w3id.org/mep#DivertingValve -->


    <owl:Class rdf:about="https://w3id.org/mep#DivertingValve">
        <rdfs:subClassOf rdf:resource="https://w3id.org/mep#Valve"/>
        <rdfs:comment xml:lang="en">Valve that enables flow to be diverted from one branch of a pipeline to another (3 port).</rdfs:comment>
        <rdfs:comment xml:lang="es">Válvula que permite desviar el flujo de un ramal de una tubería a otro (3 puertos).</rdfs:comment>
        <rdfs:label xml:lang="en">Diverting Valve</rdfs:label>
        <rdfs:label xml:lang="es">Válvula Desviadora</rdfs:label>
    </owl:Class>
    


    <!-- https://w3id.org/mep#DoubleCheckValve -->


    <owl:Class rdf:about="https://w3id.org/mep#DoubleCheckValve">
        <rdfs:subClassOf rdf:resource="https://w3id.org/mep#Valve"/>
        <rdfs:comment xml:lang="en">An assembly that incorporates two valves used to prevent backflow.</rdfs:comment>
        <rdfs:comment xml:lang="es">Un conjunto que incorpora dos válvulas utilizadas para evitar el reflujo.</rdfs:comment>
        <rdfs:label xml:lang="en">Double Check Valve</rdfs:label>
        <rdfs:label xml:lang="es">Válvula de Doble Retención</rdfs:label>
    </owl:Class>
    


    <!-- https://w3id.org/mep#DoubleRegulatingValve -->


    <owl:Class rdf:about="https://w3id.org/mep#DoubleRegulatingValve">
        <rdfs:subClassOf rdf:resource="https://w3id.org/mep#Valve"/>
        <rdfs:comment xml:lang="en">Valve used to facilitate regulation of fluid flow in a system.</rdfs:comment>
        <rdfs:comment xml:lang="es">Válvula utilizada para facilitar la regulación del flujo de fluido en un sistema.</rdfs:comment>
        <rdfs:label xml:lang="en">Double Regulating Valve</rdfs:label>
        <rdfs:label xml:lang="es">Válvula reguladora doble</rdfs:label>
    </owl:Class>
    


    <!-- https://w3id.org/mep#Draw-OffCock -->


    <owl:Class rdf:about="https://w3id.org/mep#Draw-OffCock">
        <rdfs:subClassOf rdf:resource="https://w3id.org/mep#Valve"/>
        <rdfs:comment xml:lang="en">A valve used to remove fluid from a piping system.</rdfs:comment>
        <rdfs:comment xml:lang="es">Válvula utilizada para eliminar fluido de un sistema de tuberías.</rdfs:comment>
        <rdfs:label xml:lang="en">Draw-Off Cock</rdfs:label>
        <rdfs:label xml:lang="es">Valvula de Extraccion</rdfs:label>
    </owl:Class>
    


    <!-- https://w3id.org/mep#Dropper -->


    <owl:Class rdf:about="https://w3id.org/mep#Dropper">
        <rdfs:subClassOf rdf:resource="https://w3id.org/mep#CableCarrierSegment"/>
        <rdfs:comment xml:lang="en">A dropper is a cable carrier used to suspend cable from another cable. It could also conduct electricity.</rdfs:comment>
        <rdfs:comment xml:lang="es">Un dropper es un transportador de cables que se utiliza para suspender un cable de otro cable. También podría conducir electricidad.</rdfs:comment>
        <rdfs:label xml:lang="en">Dropper</rdfs:label>
        <rdfs:label xml:lang="es">Dropper</rdfs:label>
    </owl:Class>
    


    <!-- https://w3id.org/mep#DuctBend -->


    <owl:Class rdf:about="https://w3id.org/mep#DuctBend">
        <rdfs:subClassOf rdf:resource="https://w3id.org/mep#DuctFitting"/>
        <rdfs:comment xml:lang="en">A fitting with typically two ports used to change the direction of flow between connected elements.</rdfs:comment>
        <rdfs:comment xml:lang="es">Accesorio con dos puertos que sirve para cambiar la dirección del flujo entre elementos conectados.</rdfs:comment>
        <rdfs:label xml:lang="es">Codo para Conducto</rdfs:label>
        <rdfs:label xml:lang="en">Duct Bend</rdfs:label>
    </owl:Class>
    


    <!-- https://w3id.org/mep#DuctConnector -->


    <owl:Class rdf:about="https://w3id.org/mep#DuctConnector">
        <rdfs:subClassOf rdf:resource="https://w3id.org/mep#DuctFitting"/>
        <rdfs:comment xml:lang="es">Accesorio de conexión, utilizado normalmente para unir dos puertos dentro de un sistema de distribución de flujo (por ejemplo, un acoplamiento utilizado para unir dos segmentos de conducto).</rdfs:comment>
        <rdfs:comment xml:lang="en">Connector fitting, typically used to join two ports together within a flow distribution system (e.g., a coupling used to join two duct segments).</rdfs:comment>
        <rdfs:label xml:lang="es">Conector para Conductos</rdfs:label>
        <rdfs:label xml:lang="en">Duct Connector</rdfs:label>
    </owl:Class>
    


    <!-- https://w3id.org/mep#DuctEntry -->


    <owl:Class rdf:about="https://w3id.org/mep#DuctEntry">
        <rdfs:subClassOf rdf:resource="https://w3id.org/mep#DuctFitting"/>
        <rdfs:comment xml:lang="es">Accesorio de entrada, normalmente desconectado en un puerto y conectado a un sistema de distribución de flujo en el otro (por ejemplo, una abertura de entrada del sistema de conductos de aire exterior).</rdfs:comment>
        <rdfs:comment xml:lang="en">Entry fitting, typically unconnected at one port and connected to a flow distribution system at the other (e.g., an outside air duct system intake opening).</rdfs:comment>
        <rdfs:label xml:lang="en">Duct Entry</rdfs:label>
        <rdfs:label xml:lang="es">Entrada para Conductos</rdfs:label>
    </owl:Class>
    


    <!-- https://w3id.org/mep#DuctExit -->


    <owl:Class rdf:about="https://w3id.org/mep#DuctExit">
        <rdfs:subClassOf rdf:resource="https://w3id.org/mep#DuctFitting"/>
        <rdfs:comment xml:lang="es">Accesorio de salida, normalmente desconectado en un puerto y conectado a un sistema de distribución de flujo en el otro (por ejemplo, una abertura de descarga de aire de escape).</rdfs:comment>
        <rdfs:comment xml:lang="en">Exit fitting, typically unconnected at one port and connected to a flow distribution system at the other (e.g., an exhaust air discharge opening).</rdfs:comment>
        <rdfs:label xml:lang="en">Duct Exit</rdfs:label>
        <rdfs:label xml:lang="es">Salida para Conductos</rdfs:label>
    </owl:Class>
    


    <!-- https://w3id.org/mep#DuctFitting -->


    <owl:Class rdf:about="https://w3id.org/mep#DuctFitting">
        <rdfs:subClassOf rdf:resource="https://w3id.org/mep#FlowFitting"/>
        <rdfs:comment xml:lang="en">A duct fitting is a junction or transition in a ducted flow distribution system or used to connect duct segments, resulting in changes in flow characteristics to the fluid such as direction and flow rate.</rdfs:comment>
        <rdfs:comment xml:lang="es">Un accesorio para conductos es una unión o transición en un sistema de distribución de flujo por conductos o que se utiliza para conectar segmentos de conductos, lo que provoca cambios en las características del flujo al fluido, como la dirección y el caudal.</rdfs:comment>
        <rdfs:label xml:lang="es">Accesorio para Conductos</rdfs:label>
        <rdfs:label xml:lang="en">Duct Fitting</rdfs:label>
    </owl:Class>
    


    <!-- https://w3id.org/mep#DuctJuntion -->


    <owl:Class rdf:about="https://w3id.org/mep#DuctJuntion">
        <rdfs:subClassOf rdf:resource="https://w3id.org/mep#DuctFitting"/>
        <rdfs:comment xml:lang="en">A fitting with typically more than two ports used to redistribute flow among the ports and/or to change the direction of flow between connected elements (e.g, tee, cross, wye, etc.).</rdfs:comment>
        <rdfs:comment xml:lang="es">Accesorio con más de dos puertos utilizado para redistribuir el caudal entre los puertos y/o cambiar la dirección del caudal entre los elementos conectados (por ejemplo, te, cruz, estrella, etc.).</rdfs:comment>
        <rdfs:label xml:lang="en">Duct Juntion</rdfs:label>
        <rdfs:label xml:lang="es">Union para Conductos</rdfs:label>
    </owl:Class>
    


    <!-- https://w3id.org/mep#DuctObstruction -->


    <owl:Class rdf:about="https://w3id.org/mep#DuctObstruction">
        <rdfs:subClassOf rdf:resource="https://w3id.org/mep#DuctFitting"/>
        <rdfs:comment xml:lang="en">A fitting with typically two ports used to obstruct or restrict flow between the connected elements (e.g., screen, perforated plate, etc.).</rdfs:comment>
        <rdfs:comment xml:lang="es">Accesorio con dos orificios típicos utilizado para obstruir o restringir el flujo entre los elementos conectados (por ejemplo, pantalla, placa perforada, etc.).</rdfs:comment>
        <rdfs:label xml:lang="en">Duct Obstruction</rdfs:label>
        <rdfs:label xml:lang="es">Obstruccion para Conductos</rdfs:label>
    </owl:Class>
    


    <!-- https://w3id.org/mep#DuctSegment -->


    <owl:Class rdf:about="https://w3id.org/mep#DuctSegment">
        <rdfs:subClassOf rdf:resource="https://w3id.org/mep#FlowSegment"/>
        <rdfs:comment xml:lang="en">A duct segment is used to typically join two sections of duct network.</rdfs:comment>
        <rdfs:comment xml:lang="es">Un segmento de conducto se utiliza normalmente para unir dos tramos de red de conductos.</rdfs:comment>
        <rdfs:label xml:lang="en">Duct Segment</rdfs:label>
        <rdfs:label xml:lang="es">Segmento de Conducto</rdfs:label>
    </owl:Class>
    


    <!-- https://w3id.org/mep#DuctSilencer -->


    <owl:Class rdf:about="https://w3id.org/mep#DuctSilencer">
        <rdfs:subClassOf rdf:resource="https://w3id.org/mep#FlowTreatmentDevice"/>
        <rdfs:comment xml:lang="en">A duct silencer is a device that is typically installed inside a duct distribution system for the purpose of reducing the noise levels from air movement, fan noise, etc. in the adjacent space or downstream of the duct silencer device.</rdfs:comment>
        <rdfs:comment xml:lang="es">Un silenciador de conductos es un dispositivo que se instala normalmente dentro de un sistema de distribución de conductos con el fin de reducir los niveles de ruido del movimiento del aire, ruido de ventiladores, etc. en el espacio adyacente o aguas abajo del dispositivo silenciador de conductos.</rdfs:comment>
        <rdfs:label xml:lang="en">DuctSilencer</rdfs:label>
        <rdfs:label xml:lang="es">Silenciador de Conductos</rdfs:label>
    </owl:Class>
    


    <!-- https://w3id.org/mep#DuctTransition -->


    <owl:Class rdf:about="https://w3id.org/mep#DuctTransition">
        <rdfs:subClassOf rdf:resource="https://w3id.org/mep#DuctFitting"/>
        <rdfs:comment xml:lang="en">A fitting with typically two ports having different shapes or sizes. Can also be used to change the direction of flow between connected elements.</rdfs:comment>
        <rdfs:comment xml:lang="es">Racor que suele tener dos puertos de formas o tamaños diferentes. También puede utilizarse para cambiar la dirección del flujo entre elementos conectados.</rdfs:comment>
        <rdfs:label xml:lang="en">Duct Transition</rdfs:label>
        <rdfs:label xml:lang="es">Transicion para Conductos</rdfs:label>
    </owl:Class>
    


    <!-- https://w3id.org/mep#DynamicCompressor -->


    <owl:Class rdf:about="https://w3id.org/mep#DynamicCompressor">
        <rdfs:subClassOf rdf:resource="https://w3id.org/mep#Compressor"/>
        <rdfs:comment xml:lang="es">La presión del vapor refrigerante se incrementa mediante una transferencia continua de momento angular desde un miembro giratorio al vapor, seguida de la conversión de este momento en presión estática.</rdfs:comment>
        <rdfs:comment xml:lang="en">The pressure of refrigerant vapor is increased by a continuous transfer of angular momentum from a rotating member to the vapor followed by conversion of this momentum into static pressure.</rdfs:comment>
        <rdfs:label xml:lang="es">Compresor Dinamico</rdfs:label>
        <rdfs:label xml:lang="en">Dynamic Compressor</rdfs:label>
    </owl:Class>
    


    <!-- https://w3id.org/mep#E-UtranNodeB -->


    <owl:Class rdf:about="https://w3id.org/mep#E-UtranNodeB">
        <rdfs:subClassOf rdf:resource="https://w3id.org/mep#MobileTelecommunicationsAppliance"/>
        <rdfs:comment xml:lang="en">An E-utran nodel B is a logical network component which serves one or more E-utran cells. It is the hardware connected to the evolved packet core (EPC), more specifically to the mobility management entity (MME) , which communicates directly with user equipment in wireless way.</rdfs:comment>
        <rdfs:comment xml:lang="es">Un nodo B E-utran es un componente lógico de red que da servicio a una o más células E-utran. Es el hardware conectado al núcleo de paquetes evolucionado (EPC), más concretamente a la entidad de gestión de la movilidad (MME) , que se comunica directamente con los equipos de usuario de forma inalámbrica.</rdfs:comment>
        <rdfs:label xml:lang="en">E-Utran Node B</rdfs:label>
        <rdfs:label xml:lang="es">Node B E-Utran</rdfs:label>
    </owl:Class>
    


    <!-- https://w3id.org/mep#EarthLeakerCircuitBreaker -->


    <owl:Class rdf:about="https://w3id.org/mep#EarthLeakerCircuitBreaker">
        <rdfs:subClassOf rdf:resource="https://w3id.org/mep#ProtectiveDevice"/>
        <rdfs:comment xml:lang="en">A device that opens, closes, or isolates a circuit and has short circuit protection but no overload protection. It attempts to break the circuit when there is a leakage of current from phase to earth, by measuring voltage on the earth conductor.</rdfs:comment>
        <rdfs:comment xml:lang="es">Dispositivo que abre, cierra o aísla un circuito y tiene protección contra cortocircuitos pero no contra sobrecargas. Intenta interrumpir el circuito cuando hay una fuga de corriente de fase a tierra, midiendo la tensión en el conductor de tierra.</rdfs:comment>
        <rdfs:label xml:lang="en">Earth Leaker Circuit Breaker</rdfs:label>
        <rdfs:label xml:lang="es">Interruptor Diferencial</rdfs:label>
    </owl:Class>
    


    <!-- https://w3id.org/mep#EarthingSwitch -->


    <owl:Class rdf:about="https://w3id.org/mep#EarthingSwitch">
        <rdfs:subClassOf rdf:resource="https://w3id.org/mep#ProtectiveDevice"/>
        <rdfs:comment xml:lang="en">A safety device used to open or close a circuit when there is no current. Used to isolate a part of a circuit, a machine, a part of an overhead line or an underground line so that maintenance can be safely conducted.</rdfs:comment>
        <rdfs:comment xml:lang="es">Dispositivo de seguridad utilizado para abrir o cerrar un circuito cuando no hay corriente. Se utiliza para aislar una parte de un circuito, una máquina, una parte de una línea aérea o una línea subterránea para poder realizar el mantenimiento de forma segura.</rdfs:comment>
        <rdfs:label xml:lang="en">Earthing Switch</rdfs:label>
        <rdfs:label xml:lang="es">Interruptor de Tierra</rdfs:label>
    </owl:Class>
    


    <!-- https://w3id.org/mep#EarthquakeSensor -->


    <owl:Class rdf:about="https://w3id.org/mep#EarthquakeSensor">
        <rdfs:subClassOf rdf:resource="https://w3id.org/mep#Sensor"/>
        <rdfs:comment xml:lang="en">A device that senses or detects the seismic wave and measures the seismic intensity in case of earthquake.</rdfs:comment>
        <rdfs:comment xml:lang="es">Dispositivo que percibe o detecta la onda sísmica y mide la intensidad sísmica en caso de terremoto.</rdfs:comment>
        <rdfs:label xml:lang="en">Earthquake Sensor</rdfs:label>
        <rdfs:label xml:lang="es">Sensor Sismico</rdfs:label>
    </owl:Class>
    


    <!-- https://w3id.org/mep#ElectricActuator -->


    <owl:Class rdf:about="https://w3id.org/mep#ElectricActuator">
        <rdfs:subClassOf rdf:resource="https://w3id.org/mep#Actuator"/>
        <rdfs:comment xml:lang="en">A device that electrically actuates a control element.</rdfs:comment>
        <rdfs:comment xml:lang="es">Dispositivo que acciona eléctricamente un elemento de control.</rdfs:comment>
        <rdfs:label xml:lang="es">Actuador Electrico</rdfs:label>
        <rdfs:label xml:lang="en">Electric Actuator</rdfs:label>
    </owl:Class>
    


    <!-- https://w3id.org/mep#ElectricAppliance -->


    <owl:Class rdf:about="https://w3id.org/mep#ElectricAppliance">
        <rdfs:subClassOf rdf:resource="https://w3id.org/mep#FlowTerminal"/>
        <rdfs:comment xml:lang="en">An electric appliance is a device intended for consumer usage that is powered by electricity.</rdfs:comment>
        <rdfs:comment xml:lang="es">Un electrodoméstico es un aparato destinado al consumo que funciona con electricidad.</rdfs:comment>
        <rdfs:label xml:lang="en">ElectricAppliance</rdfs:label>
        <rdfs:label xml:lang="es">Electrodomestico</rdfs:label>
    </owl:Class>
    


    <!-- https://w3id.org/mep#ElectricCooker -->


    <owl:Class rdf:about="https://w3id.org/mep#ElectricCooker">
        <rdfs:subClassOf rdf:resource="https://w3id.org/mep#ElectricAppliance"/>
        <rdfs:comment xml:lang="en">An electrical appliance that has the primary function of cooking food (including oven, hob, grill).</rdfs:comment>
        <rdfs:comment xml:lang="es">Aparato eléctrico cuya función principal es cocinar alimentos (incluidos horno, placa de cocción, grill).</rdfs:comment>
        <rdfs:label xml:lang="es">Aparato de Cocina Electrico</rdfs:label>
        <rdfs:label xml:lang="en">Electric Cooker</rdfs:label>
    </owl:Class>
    


    <!-- https://w3id.org/mep#ElectricFlowStorageDevice -->


    <owl:Class rdf:about="https://w3id.org/mep#ElectricFlowStorageDevice">
        <rdfs:subClassOf rdf:resource="https://w3id.org/mep#FlowStorageDevice"/>
        <rdfs:comment xml:lang="en">An electric flow storage device is a device in which electrical energy is stored and from which energy may be progressively released.</rdfs:comment>
        <rdfs:comment xml:lang="es">Un dispositivo de almacenamiento de flujo eléctrico es un dispositivo en el que se almacena energía eléctrica y del que se puede liberar energía progresivamente.</rdfs:comment>
        <rdfs:label xml:lang="es">Dispositivo de Almacenamiento de Flujo Electrico</rdfs:label>
        <rdfs:label xml:lang="en">Electric Flow Storage Device</rdfs:label>
    </owl:Class>
    


    <!-- https://w3id.org/mep#ElectricFlowTreatmentDevice -->


    <owl:Class rdf:about="https://w3id.org/mep#ElectricFlowTreatmentDevice">
        <rdfs:subClassOf rdf:resource="https://w3id.org/mep#FlowTreatmentDevice"/>
        <rdfs:comment xml:lang="en">An electric flow treatment device is used to remove unwanted matter from an electric or electronic signal in a flow distribution system.</rdfs:comment>
        <rdfs:comment xml:lang="es">Un dispositivo de tratamiento de flujo eléctrico se utiliza para eliminar la materia no deseada de una señal eléctrica o electrónica en un sistema de distribución de flujo.</rdfs:comment>
        <rdfs:label xml:lang="es">Dsipositivo de Tratamiento de Flujo Electrico</rdfs:label>
        <rdfs:label xml:lang="en">Electric Flow Treatment Device</rdfs:label>
    </owl:Class>
    


    <!-- https://w3id.org/mep#ElectricGenerator -->


    <owl:Class rdf:about="https://w3id.org/mep#ElectricGenerator">
        <rdfs:subClassOf rdf:resource="https://w3id.org/mep#EnergyConversionDevice"/>
        <rdfs:comment xml:lang="en">An electric generator is an engine that is a machine for converting mechanical energy into electrical energy.</rdfs:comment>
        <rdfs:comment xml:lang="es">Un generador eléctrico es un motor que es una máquina para convertir energía mecánica en energía eléctrica.</rdfs:comment>
        <rdfs:label xml:lang="en">Electric Generator</rdfs:label>
        <rdfs:label xml:lang="es">Generador Electrico</rdfs:label>
    </owl:Class>
    


    <!-- https://w3id.org/mep#ElectricHeatingCoil -->


    <owl:Class rdf:about="https://w3id.org/mep#ElectricHeatingCoil">
        <rdfs:subClassOf rdf:resource="https://w3id.org/mep#Coil"/>
        <rdfs:comment xml:lang="en">Heating coil using electricity as a heating source.</rdfs:comment>
        <rdfs:comment xml:lang="es">Serpentín calefactor que utiliza electricidad como fuente de calor.</rdfs:comment>
        <rdfs:label xml:lang="en">Electric Heating Coil</rdfs:label>
        <rdfs:label xml:lang="es">Serpentin Calefactor Electrico</rdfs:label>
    </owl:Class>
    


    <!-- https://w3id.org/mep#ElectricMotor -->


    <owl:Class rdf:about="https://w3id.org/mep#ElectricMotor">
        <rdfs:subClassOf rdf:resource="https://w3id.org/mep#EnergyConversionDevice"/>
        <rdfs:comment xml:lang="en">An electric motor is an engine that is a machine for converting electrical energy into mechanical energy.</rdfs:comment>
        <rdfs:comment xml:lang="es">Un motor eléctrico es un motor que es una máquina para convertir energía eléctrica en energía mecánica.</rdfs:comment>
        <rdfs:label xml:lang="en">Electric Motor</rdfs:label>
        <rdfs:label xml:lang="es">Motor Electrico</rdfs:label>
    </owl:Class>
    


    <!-- https://w3id.org/mep#ElectricTimeControl -->


    <owl:Class rdf:about="https://w3id.org/mep#ElectricTimeControl">
        <rdfs:subClassOf rdf:resource="https://w3id.org/mep#FlowController"/>
        <rdfs:comment xml:lang="en">An electric time control is a device that applies control to the provision or flow of electrical energy over time.</rdfs:comment>
        <rdfs:comment xml:lang="es">Un contador de tiempo eléctrico es un dispositivo que aplica control al suministro o flujo de energía eléctrica a lo largo del tiempo.</rdfs:comment>
        <rdfs:label xml:lang="es">Contador de Tiempo Electrico</rdfs:label>
        <rdfs:label xml:lang="en">Electric Time Control</rdfs:label>
    </owl:Class>
    


    <!-- https://w3id.org/mep#ElectromagneticTrippingUnit -->


    <owl:Class rdf:about="https://w3id.org/mep#ElectromagneticTrippingUnit">
        <rdfs:subClassOf rdf:resource="https://w3id.org/mep#ProtectiveDeviceTrippingUnit"/>
        <rdfs:comment xml:lang="en">A tripping unit activated by electromagnetic action.</rdfs:comment>
        <rdfs:comment xml:lang="es">Una unidad de disparo activada por acción electromagnética.</rdfs:comment>
        <rdfs:label xml:lang="en">Electromagnetic Tripping Unit</rdfs:label>
        <rdfs:label xml:lang="es">Unidad de Disparo Electromagnetica</rdfs:label>
    </owl:Class>
    


    <!-- https://w3id.org/mep#ElectronicFilter -->


    <owl:Class rdf:about="https://w3id.org/mep#ElectronicFilter">
        <rdfs:subClassOf rdf:resource="https://w3id.org/mep#ElectricFlowTreatmentDevice"/>
        <rdfs:comment xml:lang="es">Dispositivo lineal de dos puertos diseñado para transmitir componentes espectrales de la cantidad de entrada de acuerdo con una ley especificada, generalmente con el fin de pasar los componentes en ciertas bandas de frecuencia y atenuar los de otras bandas.</rdfs:comment>
        <rdfs:comment xml:lang="en">Linear two-port device designed to transmit spectral components of the input quantity according to a specified law, generally in order to pass the components in certain frequency bands and to attenuate those in other bands</rdfs:comment>
        <rdfs:label xml:lang="en">Electronic Filter</rdfs:label>
        <rdfs:label xml:lang="es">Filtro Electronico</rdfs:label>
    </owl:Class>
    


    <!-- https://w3id.org/mep#ElectronicTrippingUnit -->


    <owl:Class rdf:about="https://w3id.org/mep#ElectronicTrippingUnit">
        <rdfs:subClassOf rdf:resource="https://w3id.org/mep#ProtectiveDeviceTrippingUnit"/>
        <rdfs:comment xml:lang="en">A tripping unit activated by electronic action.</rdfs:comment>
        <rdfs:comment xml:lang="es">Una unidad de disparo activada por acción electrónica.</rdfs:comment>
        <rdfs:label xml:lang="en">Electronic Tripping Unit</rdfs:label>
        <rdfs:label xml:lang="es">Unidad de Disparo Electronica</rdfs:label>
    </owl:Class>
    


    <!-- https://w3id.org/mep#EmergencyStop -->


    <owl:Class rdf:about="https://w3id.org/mep#EmergencyStop">
        <rdfs:subClassOf rdf:resource="https://w3id.org/mep#SwitchingDevice"/>
        <rdfs:comment xml:lang="en">An emergency stop device acts to remove as quickly as possible any danger that may have arisen unexpectedly.</rdfs:comment>
        <rdfs:comment xml:lang="es">Un dispositivo de parada de emergencia actúa para eliminar lo antes posible cualquier peligro que pueda haber surgido de forma inesperada.</rdfs:comment>
        <rdfs:label xml:lang="en">Emergency Stop</rdfs:label>
        <rdfs:label xml:lang="es">Parada de Emergencia</rdfs:label>
    </owl:Class>
    


    <!-- https://w3id.org/mep#EndSuctionPump -->


    <owl:Class rdf:about="https://w3id.org/mep#EndSuctionPump">
        <rdfs:subClassOf rdf:resource="https://w3id.org/mep#Pump"/>
        <rdfs:comment xml:lang="en">An End Suction pump, when mounted horizontally, has a single horizontal inlet on the impeller suction side and a vertical discharge. It may have a direct or close-coupled motor.</rdfs:comment>
        <rdfs:comment xml:lang="es">Una bomba de aspiración axial, cuando está montada horizontalmente, tiene una sola entrada horizontal en el lado de aspiración del impulsor y una descarga vertical. Puede tener un motor directo o acoplado.</rdfs:comment>
        <rdfs:label xml:lang="es">Bomba de Aspiracion Axial</rdfs:label>
        <rdfs:label xml:lang="en">End Suction Pump</rdfs:label>
    </owl:Class>
    


    <!-- https://w3id.org/mep#EnergyConversionDevice -->


    <owl:Class rdf:about="https://w3id.org/mep#EnergyConversionDevice">
        <rdfs:subClassOf rdf:resource="https://w3id.org/mep#DistributionFlowElement"/>
        <rdfs:comment xml:lang="es">Define la aparición de un dispositivo utilizado para realizar la conversión de energía o la transferencia de calor y normalmente participa en un sistema de distribución de flujo.</rdfs:comment>
        <rdfs:comment xml:lang="en">Defines the occurrence of a device used to perform energy conversion or heat transfer and typically participates in a flow distribution system.</rdfs:comment>
        <rdfs:label xml:lang="es">Dispositivo de Conversion de Energia</rdfs:label>
        <rdfs:label xml:lang="en">EnergyConversionDevice</rdfs:label>
    </owl:Class>
    


    <!-- https://w3id.org/mep#EnergyMeter -->


    <owl:Class rdf:about="https://w3id.org/mep#EnergyMeter">
        <rdfs:subClassOf rdf:resource="https://w3id.org/mep#FlowMeter"/>
        <rdfs:comment xml:lang="en">An electric meter or energy meter is a device that measures the amount of electrical energy supplied to or produced by a residence, business or machine.</rdfs:comment>
        <rdfs:comment xml:lang="es">Un medidor eléctrico o medidor de energía es un dispositivo que mide la cantidad de energía eléctrica suministrada o producida por una residencia, negocio o máquina.</rdfs:comment>
        <rdfs:label xml:lang="en">Energy Meter</rdfs:label>
        <rdfs:label xml:lang="es">Medidor de Energia</rdfs:label>
    </owl:Class>
    


    <!-- https://w3id.org/mep#Engine -->


    <owl:Class rdf:about="https://w3id.org/mep#Engine">
        <rdfs:subClassOf rdf:resource="https://w3id.org/mep#EnergyConversionDevice"/>
        <rdfs:comment xml:lang="en">An engine is a device that converts fuel into mechanical energy through combustion.</rdfs:comment>
        <rdfs:comment xml:lang="es">Un motor es un dispositivo que convierte el combustible en energía mecánica mediante la combustión.</rdfs:comment>
        <rdfs:label xml:lang="en">Engine</rdfs:label>
        <rdfs:label xml:lang="es">Motor</rdfs:label>
    </owl:Class>
    


    <!-- https://w3id.org/mep#EngineGenerator -->


    <owl:Class rdf:about="https://w3id.org/mep#EngineGenerator">
        <rdfs:subClassOf rdf:resource="https://w3id.org/mep#ElectricGenerator"/>
        <rdfs:comment xml:lang="en">Electrical generator with a fuel-driven engine, for example a diesel-driven emergency power supply.</rdfs:comment>
        <rdfs:comment xml:lang="es">Generador eléctrico con motor de combustible, por ejemplo un suministro de energía de emergencia diésel.</rdfs:comment>
        <rdfs:label xml:lang="en">Engine Generator</rdfs:label>
        <rdfs:label xml:lang="es">Generador a Motor</rdfs:label>
    </owl:Class>
    


    <!-- https://w3id.org/mep#EvaporativeCooledCondenser -->


    <owl:Class rdf:about="https://w3id.org/mep#EvaporativeCooledCondenser">
        <rdfs:subClassOf rdf:resource="https://w3id.org/mep#Condenser"/>
        <rdfs:comment xml:lang="en">A condenser that is cooled evaporatively.</rdfs:comment>
        <rdfs:comment xml:lang="es">Un condensador que se enfría por evaporación.</rdfs:comment>
        <rdfs:label xml:lang="es">Condensador Refrigerado por Evaporacion</rdfs:label>
        <rdfs:label xml:lang="en">Evaporative Cooled Condenser</rdfs:label>
    </owl:Class>
    


    <!-- https://w3id.org/mep#EvaporativeCooler -->


    <owl:Class rdf:about="https://w3id.org/mep#EvaporativeCooler">
        <rdfs:subClassOf rdf:resource="https://w3id.org/mep#EnergyConversionDevice"/>
        <rdfs:comment xml:lang="en">An evaporative cooler is a device that cools air by saturating it with water vapor.</rdfs:comment>
        <rdfs:comment xml:lang="es">Un enfriador evaporativo es un dispositivo que enfría el aire saturándolo con vapor de agua.</rdfs:comment>
        <rdfs:label xml:lang="es">Enfriador Evaporativo</rdfs:label>
        <rdfs:label xml:lang="en">Evaporative Cooler</rdfs:label>
    </owl:Class>
    


    <!-- https://w3id.org/mep#Evaporator -->


    <owl:Class rdf:about="https://w3id.org/mep#Evaporator">
        <rdfs:subClassOf rdf:resource="https://w3id.org/mep#EnergyConversionDevice"/>
        <rdfs:comment xml:lang="en">An evaporator is a device in which a liquid refrigerent is vaporized and absorbs heat from the surrounding fluid.</rdfs:comment>
        <rdfs:comment xml:lang="es">Un evaporador es un dispositivo en el que un refrigerante líquido se vaporiza y absorbe calor del fluido circundante.</rdfs:comment>
        <rdfs:label xml:lang="es">Evaporador</rdfs:label>
        <rdfs:label xml:lang="en">Evaporator</rdfs:label>
    </owl:Class>
    


    <!-- https://w3id.org/mep#ExpansionTank -->


    <owl:Class rdf:about="https://w3id.org/mep#ExpansionTank">
        <rdfs:subClassOf rdf:resource="https://w3id.org/mep#Tank"/>
        <rdfs:comment xml:lang="en">A closed container used in a closed fluid distribution system to mitigate the effects of thermal expansion or water hammer. The tank is typically constructed with a diaphragm dividing the tank into two sections, with fluid on one side of the diaphragm and air on the other. One example application is when connected to the primary circuit of a hot water system to accommodate the increase in volume of the water when it is heated.</rdfs:comment>
        <rdfs:comment xml:lang="es">Recipiente cerrado utilizado en un sistema cerrado de distribución de fluidos para mitigar los efectos de la dilatación térmica o el golpe de ariete. El depósito se construye normalmente con un diafragma que divide el depósito en dos secciones, con el fluido a un lado del diafragma y el aire al otro. Un ejemplo de aplicación es cuando se conecta al circuito primario de un sistema de agua caliente para acomodar el aumento de volumen del agua cuando se calienta.</rdfs:comment>
        <rdfs:label xml:lang="es">Deposito de Expansion</rdfs:label>
        <rdfs:label xml:lang="en">Expansion Tank</rdfs:label>
    </owl:Class>
    


    <!-- https://w3id.org/mep#ExternalCombustionMotor -->


    <owl:Class rdf:about="https://w3id.org/mep#ExternalCombustionMotor">
        <rdfs:subClassOf rdf:resource="https://w3id.org/mep#Engine"/>
        <rdfs:comment xml:lang="en">Combustion is external.</rdfs:comment>
        <rdfs:comment xml:lang="es">La combustión es externa.</rdfs:comment>
        <rdfs:label xml:lang="en">External Combustion Motor</rdfs:label>
        <rdfs:label xml:lang="es">Motor de Combustion Externa</rdfs:label>
    </owl:Class>
    


    <!-- https://w3id.org/mep#Fan -->


    <owl:Class rdf:about="https://w3id.org/mep#Fan">
        <rdfs:subClassOf rdf:resource="https://w3id.org/mep#FlowMovingDevice"/>
        <rdfs:comment xml:lang="en">A fan is a device which imparts mechanical work on a gas. A typical usage of a fan is to induce airflow in a building services air distribution system.</rdfs:comment>
        <rdfs:comment xml:lang="es">Un ventilador es un dispositivo que imparte trabajo mecánico a un gas. Un uso típico de un ventilador es inducir el flujo de aire en un sistema de distribución de aire de servicios de un edificio.</rdfs:comment>
        <rdfs:label xml:lang="en">Fan</rdfs:label>
        <rdfs:label xml:lang="es">Ventilador</rdfs:label>
    </owl:Class>
    


    <!-- https://w3id.org/mep#Faucet -->


    <owl:Class rdf:about="https://w3id.org/mep#Faucet">
        <rdfs:subClassOf rdf:resource="https://w3id.org/mep#Valve"/>
        <rdfs:comment xml:lang="en">Faucet valve typically used as a flow discharge.</rdfs:comment>
        <rdfs:comment xml:lang="es">Válvula que normalmente se utiliza como descarga de flujo.</rdfs:comment>
        <rdfs:label xml:lang="en">Faucet</rdfs:label>
        <rdfs:label xml:lang="es">Grifo</rdfs:label>
    </owl:Class>
    


    <!-- https://w3id.org/mep#Fax -->


    <owl:Class rdf:about="https://w3id.org/mep#Fax">
        <rdfs:subClassOf rdf:resource="https://w3id.org/mep#CommunicationsAppliance"/>
        <rdfs:comment xml:lang="en">A machine that has the primary function of transmitting a facsimile copy of printed matter using a telephone line.</rdfs:comment>
        <rdfs:comment xml:lang="es">Máquina cuya función principal es transmitir una copia facsímil de material impreso utilizando una línea telefónica.</rdfs:comment>
        <rdfs:label xml:lang="en">Fax</rdfs:label>
        <rdfs:label xml:lang="es">Fax</rdfs:label>
    </owl:Class>
    


    <!-- https://w3id.org/mep#Feed-AirUnit -->


    <owl:Class rdf:about="https://w3id.org/mep#Feed-AirUnit">
        <rdfs:subClassOf rdf:resource="https://w3id.org/mep#MedicalDevice"/>
        <rdfs:comment xml:lang="en">Device that feeds air to an oxygen generator, composed of an air compressor, air treatment line, and an air receiver.</rdfs:comment>
        <rdfs:comment xml:lang="es">Dispositivo que alimenta de aire a un generador de oxígeno, compuesto por un compresor de aire, una línea de tratamiento de aire y un receptor de aire.</rdfs:comment>
        <rdfs:label xml:lang="en">Feed-Air Unit</rdfs:label>
        <rdfs:label xml:lang="es">Unidad de Alimentacion de Aire</rdfs:label>
    </owl:Class>
    


    <!-- https://w3id.org/mep#FeedandExpansionTank -->


    <owl:Class rdf:about="https://w3id.org/mep#FeedandExpansionTank">
        <rdfs:subClassOf rdf:resource="https://w3id.org/mep#Tank"/>
        <rdfs:comment xml:lang="en">An open tank that is used for both storage and thermal expansion. A typical example is a tank used to store make-up water at ambient pressure for supply to a hot water system, simultaneously accommodating increases in volume of the water when heated.</rdfs:comment>
        <rdfs:comment xml:lang="es">Depósito abierto que se utiliza tanto para almacenamiento como para expansión térmica. Un ejemplo típico es un depósito utilizado para almacenar agua de reposición a presión ambiente para el suministro a un sistema de agua caliente, acomodando simultáneamente aumentos en el volumen del agua cuando se calienta.</rdfs:comment>
        <rdfs:label xml:lang="es">Deposito de Alimentacion y Expansion</rdfs:label>
        <rdfs:label xml:lang="en">Feed and Expansion Tank</rdfs:label>
    </owl:Class>
    


    <!-- https://w3id.org/mep#FiberSegment -->


    <owl:Class rdf:about="https://w3id.org/mep#FiberSegment">
        <rdfs:subClassOf rdf:resource="https://w3id.org/mep#CableSegment"/>
        <rdfs:comment xml:lang="en">A fiber segment is an individual optical fiber used in telecommunication systems to transmit data by means of optical signals.</rdfs:comment>
        <rdfs:comment xml:lang="es">Un segmento de fibra es una fibra óptica individual utilizada en sistemas de telecomunicaciones para transmitir datos mediante señales ópticas.</rdfs:comment>
        <rdfs:label xml:lang="en">Fiber Segment</rdfs:label>
        <rdfs:label xml:lang="es">Segmento de Fibra</rdfs:label>
    </owl:Class>
    


    <!-- https://w3id.org/mep#FiberTube -->


    <owl:Class rdf:about="https://w3id.org/mep#FiberTube">
        <rdfs:subClassOf rdf:resource="https://w3id.org/mep#CableSegment"/>
        <rdfs:comment xml:lang="en">A fiber tube is semi-rigid hollow plastic tube with a very small radius that houses and protects a certain number of optical fiber segments. An optical cable segment may contain many fiber tubes.</rdfs:comment>
        <rdfs:comment xml:lang="es">Un tubo de fibra es un tubo de plástico hueco semirrígido de radio muy pequeño que aloja y protege un número determinado de segmentos de fibra óptica. Un segmento de cable óptico puede contener muchos tubos de fibra.</rdfs:comment>
        <rdfs:label xml:lang="en">Fiber Tube</rdfs:label>
        <rdfs:label xml:lang="es">Tubo de Fibra</rdfs:label>
    </owl:Class>
    


    <!-- https://w3id.org/mep#Filter -->


    <owl:Class rdf:about="https://w3id.org/mep#Filter">
        <rdfs:subClassOf rdf:resource="https://w3id.org/mep#FlowTreatmentDevice"/>
        <rdfs:comment xml:lang="en">A filter is an apparatus used to remove particulate or gaseous matter from fluids and gases.</rdfs:comment>
        <rdfs:comment xml:lang="es">Un filtro es un aparato que se utiliza para eliminar partículas o materia gaseosa de fluidos y gases.</rdfs:comment>
        <rdfs:label xml:lang="en">Filter</rdfs:label>
        <rdfs:label xml:lang="es">Filtro</rdfs:label>
    </owl:Class>
    


    <!-- https://w3id.org/mep#FinnedTubeBundle -->


    <owl:Class rdf:about="https://w3id.org/mep#FinnedTubeBundle">
        <rdfs:subClassOf rdf:resource="https://w3id.org/mep#TubeBundle"/>
        <rdfs:comment xml:lang="en">Finned tube bundle type.</rdfs:comment>
        <rdfs:comment xml:lang="es">Tipo de haz de tubos con aletas.</rdfs:comment>
        <rdfs:label xml:lang="en">Finned Tube Bundle</rdfs:label>
        <rdfs:label xml:lang="es">Haz de Tubos con Aletas</rdfs:label>
    </owl:Class>
    


    <!-- https://w3id.org/mep#FireDamper -->


    <owl:Class rdf:about="https://w3id.org/mep#FireDamper">
        <rdfs:subClassOf rdf:resource="https://w3id.org/mep#Damper"/>
        <rdfs:comment xml:lang="es">Compuerta cortafuegos que impide la propagación del fuego durante un tiempo determinado. Suele accionarse mediante un fusible que se funde a partir de cierta temperatura.</rdfs:comment>
        <rdfs:comment xml:lang="en">Fire damper used to prevent the spread of fire for a specified duration. Commonly operated by fusable link that melts above a certain temperature.</rdfs:comment>
        <rdfs:label xml:lang="es">Compuerta Cortafuegos</rdfs:label>
        <rdfs:label xml:lang="en">Fire Damper</rdfs:label>
    </owl:Class>
    


    <!-- https://w3id.org/mep#FireHosereel -->


    <owl:Class rdf:about="https://w3id.org/mep#FireHosereel">
        <rdfs:subClassOf rdf:resource="https://w3id.org/mep#FireSuppressionTerminal"/>
        <rdfs:comment xml:lang="en">A supporting framework on which a hose may be wound.</rdfs:comment>
        <rdfs:comment xml:lang="es">Soporte sobre el cual se puede enrollar una manguera.</rdfs:comment>
        <rdfs:label xml:lang="es">Carrete de Manguera</rdfs:label>
        <rdfs:label xml:lang="en">Fire Hosereel</rdfs:label>
    </owl:Class>
    


    <!-- https://w3id.org/mep#FireHydrant -->


    <owl:Class rdf:about="https://w3id.org/mep#FireHydrant">
        <rdfs:subClassOf rdf:resource="https://w3id.org/mep#FireSuppressionTerminal"/>
        <rdfs:comment xml:lang="en">Device, fitted to a pipe, through which a temporary supply of water may be provided. May also be termed a stand pipe.</rdfs:comment>
        <rdfs:comment xml:lang="es">Un hidrante de incendios es un dispositivo que se instala en una tubería y permite suministrar agua temporalmente. También puede denominarse boca de incendios</rdfs:comment>
        <rdfs:label xml:lang="en">Fire Hydrant</rdfs:label>
        <rdfs:label xml:lang="es">Hydrante de Incendios</rdfs:label>
    </owl:Class>
    


    <!-- https://w3id.org/mep#FireMonitor -->


    <owl:Class rdf:about="https://w3id.org/mep#FireMonitor">
        <rdfs:subClassOf rdf:resource="https://w3id.org/mep#FireSuppressionTerminal"/>
        <rdfs:comment xml:lang="en">Fire monitor.</rdfs:comment>
        <rdfs:comment xml:lang="es">Monitor de Incendios</rdfs:comment>
        <rdfs:label xml:lang="en">Fire Monitor</rdfs:label>
        <rdfs:label xml:lang="es">Monitor de Incendios</rdfs:label>
    </owl:Class>
    


    <!-- https://w3id.org/mep#FireSensor -->


    <owl:Class rdf:about="https://w3id.org/mep#FireSensor">
        <rdfs:subClassOf rdf:resource="https://w3id.org/mep#Sensor"/>
        <rdfs:comment xml:lang="en">A device that senses or detects fire</rdfs:comment>
        <rdfs:comment xml:lang="es">Dispositivo de detección de incendios</rdfs:comment>
        <rdfs:label xml:lang="en">Fire Sensor</rdfs:label>
        <rdfs:label xml:lang="es">Sensor de Incendios</rdfs:label>
    </owl:Class>
    


    <!-- https://w3id.org/mep#FireSmokeDamper -->


    <owl:Class rdf:about="https://w3id.org/mep#FireSmokeDamper">
        <rdfs:subClassOf rdf:resource="https://w3id.org/mep#Damper"/>
        <rdfs:comment xml:lang="es">Combinación de compuerta cortafuegos y cortahumos utilizada para evitar la propagación del fuego y el humo. Suele accionarse mediante un fusible y un detector de humo.</rdfs:comment>
        <rdfs:comment xml:lang="en">Combination fire and smoke damper used to prevent the spread of fire and smoke. Commonly operated by a fusable link and a smoke detector.</rdfs:comment>
        <rdfs:label xml:lang="es">Compuerta Cortafuegos-humo</rdfs:label>
        <rdfs:label xml:lang="en">FireSmoke Damper</rdfs:label>
    </owl:Class>
    


    <!-- https://w3id.org/mep#FireSuppressionTerminal -->


    <owl:Class rdf:about="https://w3id.org/mep#FireSuppressionTerminal">
        <rdfs:subClassOf rdf:resource="https://w3id.org/mep#FlowTerminal"/>
        <rdfs:comment xml:lang="en">A fire suppression terminal has the purpose of delivering a fluid (gas or liquid) that will suppress a fire. A fire suppression terminal provides for all forms of sprinkler, spreader and other form of terminal that is connected to a pipework system and intended to act in the role of suppressing a fire.</rdfs:comment>
        <rdfs:comment xml:lang="es">Una terminal de extinción de incendios tiene el propósito de entregar un fluido (gas o líquido) que extinguirá un incendio. Una terminal de extinción de incendios proporciona todas las formas de rociadores, esparcidores y otras formas de terminal que están conectadas a un sistema de tuberías y destinadas a actuar en la función de extinción de un incendio.</rdfs:comment>
        <rdfs:label xml:lang="en">Fire Suppression Terminal</rdfs:label>
        <rdfs:label xml:lang="es">Terminal de Extincion de Incendios</rdfs:label>
    </owl:Class>
    


    <!-- https://w3id.org/mep#FixedPlateCounterFlowExchanger -->


    <owl:Class rdf:about="https://w3id.org/mep#FixedPlateCounterFlowExchanger">
        <rdfs:subClassOf rdf:resource="https://w3id.org/mep#AirToAirHeatRecovery"/>
        <rdfs:comment xml:lang="en">Heat exchanger with moving parts and alternate layers of plates, separated and sealed from the exhaust and supply air stream passages with primary air entering at secondary air outlet location and exiting at secondary air inlet location.</rdfs:comment>
        <rdfs:comment xml:lang="es">Intercambiador de calor con piezas móviles y capas alternas de placas, separadas y selladas de los conductos de la corriente de aire de escape y suministro, con aire primario entrando por la ubicación de salida de aire secundario y saliendo por la ubicación de entrada de aire secundario.</rdfs:comment>
        <rdfs:label xml:lang="en">Fixed Plate Counter Flow Exchanger</rdfs:label>
        <rdfs:label xml:lang="es">Intercambiador de Placas Fijas de Contracorriente</rdfs:label>
    </owl:Class>
    


    <!-- https://w3id.org/mep#FixedPlateCrossFlowExchanger -->


    <owl:Class rdf:about="https://w3id.org/mep#FixedPlateCrossFlowExchanger">
        <rdfs:subClassOf rdf:resource="https://w3id.org/mep#AirToAirHeatRecovery"/>
        <rdfs:comment xml:lang="en">Heat exchanger with moving parts and alternate layers of plates, separated and sealed from the exhaust and supply air stream passages with secondary air flow in the direction perpendicular to primary air flow.</rdfs:comment>
        <rdfs:comment xml:lang="es">Intercambiador de calor con partes móviles y capas alternas de placas, separadas y selladas de los conductos de la corriente de aire de escape y suministro con flujo de aire secundario en dirección perpendicular al flujo de aire primario.</rdfs:comment>
        <rdfs:label xml:lang="en">Fixed Plate Cross Flow Exchanger</rdfs:label>
        <rdfs:label xml:lang="es">Intercambiador de Placas Fijas de Flujo Cruzado</rdfs:label>
    </owl:Class>
    


    <!-- https://w3id.org/mep#FixedPlateParallelFlowExchanger -->


    <owl:Class rdf:about="https://w3id.org/mep#FixedPlateParallelFlowExchanger">
        <rdfs:subClassOf rdf:resource="https://w3id.org/mep#AirToAirHeatRecovery"/>
        <rdfs:comment xml:lang="en">Heat exchanger with moving parts and alternate layers of plates, separated and sealed from the exhaust and supply air stream passages with primary air entering at secondary air inlet location and exiting at secondary air outlet location.</rdfs:comment>
        <rdfs:comment xml:lang="es">Intercambiador de calor con partes móviles y capas alternas de placas, separadas y selladas de los conductos de la corriente de aire de escape y suministro con aire primario que ingresa por la ubicación de entrada de aire secundario y sale por la ubicación de salida de aire secundario.</rdfs:comment>
        <rdfs:label xml:lang="en">Fixed Plate Parallel Flow Exchanger</rdfs:label>
        <rdfs:label xml:lang="es">Intercambiador de Placas Fijas de Flujo Paralelo</rdfs:label>
    </owl:Class>
    


    <!-- https://w3id.org/mep#Flat-ovalSilencer -->


    <owl:Class rdf:about="https://w3id.org/mep#Flat-ovalSilencer">
        <rdfs:subClassOf rdf:resource="https://w3id.org/mep#DuctSilencer"/>
        <rdfs:comment xml:lang="en">Flat-oval shaped duct silencer type.</rdfs:comment>
        <rdfs:comment xml:lang="es">Silenciador de conducto de forma ovalada plana</rdfs:comment>
        <rdfs:label xml:lang="en">Flat-oval Silencer</rdfs:label>
        <rdfs:label xml:lang="es">Silenciador plano-ovalado</rdfs:label>
    </owl:Class>
    


    <!-- https://w3id.org/mep#FlexibleDuctSegment -->


    <owl:Class rdf:about="https://w3id.org/mep#FlexibleDuctSegment">
        <rdfs:subClassOf rdf:resource="https://w3id.org/mep#DuctSegment"/>
        <rdfs:comment xml:lang="en">A flexible segment is a continuous non-linear segment of duct that can be deformed and change the direction of flow.</rdfs:comment>
        <rdfs:comment xml:lang="es">Un segmento flexible es un segmento continuo no lineal de conducto que puede deformarse y cambiar la dirección del flujo.</rdfs:comment>
        <rdfs:label xml:lang="en">Flexible Duct Segment</rdfs:label>
        <rdfs:label xml:lang="es">Segmento de Conducto Flexible</rdfs:label>
    </owl:Class>
    


    <!-- https://w3id.org/mep#FlexiblePipeSegment -->


    <owl:Class rdf:about="https://w3id.org/mep#FlexiblePipeSegment">
        <rdfs:subClassOf rdf:resource="https://w3id.org/mep#PipeSegment"/>
        <rdfs:comment xml:lang="en">A flexible segment is a continuous non-linear segment of pipe that can be deformed and change the direction of flow.</rdfs:comment>
        <rdfs:comment xml:lang="es">Un segmento flexible es un segmento continuo no lineal de tubería que puede deformarse y cambiar la dirección del flujo.</rdfs:comment>
        <rdfs:label xml:lang="en">Flexible Pipe Segment</rdfs:label>
        <rdfs:label xml:lang="es">Segmento de Tuberia Flexible</rdfs:label>
    </owl:Class>
    


    <!-- https://w3id.org/mep#FloatingController -->


    <owl:Class rdf:about="https://w3id.org/mep#FloatingController">
        <rdfs:subClassOf rdf:resource="https://w3id.org/mep#Controller"/>
        <rdfs:comment xml:lang="es">La salida aumenta o disminuye a un ritmo constante o acelerado</rdfs:comment>
        <rdfs:comment xml:lang="en">Output increases or decreases at a constant or accelerating rate.</rdfs:comment>
        <rdfs:label xml:lang="es">Controlador Flotante</rdfs:label>
        <rdfs:label xml:lang="en">Floating Controller</rdfs:label>
    </owl:Class>
    


    <!-- https://w3id.org/mep#FloodedShellandTubeEvaporator -->


    <owl:Class rdf:about="https://w3id.org/mep#FloodedShellandTubeEvaporator">
        <rdfs:subClassOf rdf:resource="https://w3id.org/mep#Evaporator"/>
        <rdfs:comment xml:lang="es">Evaporador en el que el refrigerante se evapora fuera de los tubos.</rdfs:comment>
        <rdfs:comment xml:lang="en">Evaporator in which refrigerant evaporates outside tubes.</rdfs:comment>
        <rdfs:label xml:lang="es">Evaporador deTubo y Carcasa Inundado</rdfs:label>
        <rdfs:label xml:lang="en">Flooded Shell and Tube Evaporator</rdfs:label>
    </owl:Class>
    


    <!-- https://w3id.org/mep#FloorTrap -->


    <owl:Class rdf:about="https://w3id.org/mep#FloorTrap">
        <rdfs:subClassOf rdf:resource="https://w3id.org/mep#WasteTerminal"/>
        <rdfs:comment xml:lang="es">Accesorio de tubería, colocado en el piso, que retiene líquido para evitar el paso de aire viciado.</rdfs:comment>
        <rdfs:comment xml:lang="en">Pipe fitting, set into the floor, that retains liquid to prevent the passage of foul air.</rdfs:comment>
        <rdfs:label xml:lang="en">Floor Trap</rdfs:label>
        <rdfs:label xml:lang="es">Trampa de Piso</rdfs:label>
    </owl:Class>
    


    <!-- https://w3id.org/mep#FloorWaste -->


    <owl:Class rdf:about="https://w3id.org/mep#FloorWaste">
        <rdfs:subClassOf rdf:resource="https://w3id.org/mep#WasteTerminal"/>
        <rdfs:comment xml:lang="es">Accesorio de tubería, colocado en el piso, que recolecta aguas residuales y las descarga en una trampa separada.</rdfs:comment>
        <rdfs:comment xml:lang="en">Pipe fitting, set into the floor, that collects waste water and discharges it to a separate trap.</rdfs:comment>
        <rdfs:label xml:lang="en">Floor Waste</rdfs:label>
        <rdfs:label xml:lang="es">Residuo  de Piso</rdfs:label>
    </owl:Class>
    


    <!-- https://w3id.org/mep#FlowController -->


    <owl:Class rdf:about="https://w3id.org/mep#FlowController">
        <rdfs:subClassOf rdf:resource="https://w3id.org/mep#DistributionFlowElement"/>
        <rdfs:comment xml:lang="en">Defines the occurrence of elements of a distribution system that are used to regulate flow through a distribution system. Examples include dampers, valves, switches, and relays. </rdfs:comment>
        <rdfs:comment xml:lang="es">Se refiere a aquellos componentes de un sistema de distribución que se utilizan para regular el flujo a través del sistema. Algunos ejemplos de estos elementos son amortiguadores, válvulas, interruptores y relés</rdfs:comment>
        <rdfs:label xml:lang="en">FlowController</rdfs:label>
        <rdfs:label xml:lang="es">Regulador de Flujo</rdfs:label>
    </owl:Class>
    


    <!-- https://w3id.org/mep#FlowFitting -->


    <owl:Class rdf:about="https://w3id.org/mep#FlowFitting">
        <rdfs:subClassOf rdf:resource="https://w3id.org/mep#DistributionFlowElement"/>
        <rdfs:comment xml:lang="es">Define la aparición de una unión o transición en un sistema de distribución de flujo, como un codo o una T.</rdfs:comment>
        <rdfs:comment xml:lang="en">Defines the occurrence of a junction or transition in a flow distribution system, such as an elbow or tee. Its type is defined by IfcFlowFittingType or its subtypes.</rdfs:comment>
        <rdfs:label xml:lang="es">Accesorio de Flujo</rdfs:label>
        <rdfs:label xml:lang="en">FlowFitting</rdfs:label>
    </owl:Class>
    


    <!-- https://w3id.org/mep#FlowInstrument -->


    <owl:Class rdf:about="https://w3id.org/mep#FlowInstrument">
        <rdfs:subClassOf rdf:resource="https://w3id.org/mep#DistributionControlElement"/>
        <rdfs:comment xml:lang="en">A flow instrument reads and displays the value of a particular property of a system at a point, or displays the difference in the value of a property between two points. Instrumentation is typically for the purpose of determining the value of the property at a point in time. It is not the purpose of an instrument to record or integrate the values over time (although they may be connected to recording devices that do perform such a function). This entity provides for all forms of mechanical flow instrument (thermometers, pressure gauges etc.) and electrical flow instruments (ammeters, voltmeters etc.)</rdfs:comment>
        <rdfs:comment xml:lang="es">Un instrumento de flujo lee y muestra el valor de una propiedad particular de un sistema en un punto, o muestra la diferencia en el valor de una propiedad entre dos puntos. La instrumentación suele tener como objetivo determinar el valor de la propiedad en un momento dado. No es el propósito de un instrumento registrar o integrar los valores a lo largo del tiempo (aunque pueden estar conectados a dispositivos de registro que sí realizan dicha función). Esta entidad proporciona todas las formas de instrumentos de flujo mecánico (termómetros, manómetros, etc.) e instrumentos de flujo eléctrico (amperímetros, voltímetros, etc.)</rdfs:comment>
        <rdfs:label xml:lang="en">FlowInstrument</rdfs:label>
        <rdfs:label xml:lang="es">Instrumento de Flujo</rdfs:label>
    </owl:Class>
    


    <!-- https://w3id.org/mep#FlowMeter -->


    <owl:Class rdf:about="https://w3id.org/mep#FlowMeter">
        <rdfs:subClassOf rdf:resource="https://w3id.org/mep#FlowController"/>
        <rdfs:comment xml:lang="en">A flow meter is a device that is used to measure the flow rate in a system.</rdfs:comment>
        <rdfs:comment xml:lang="es">Un medidor de flujo es un dispositivo que se utiliza para medir la cantidad  de flujo en un sistema.</rdfs:comment>
        <rdfs:label xml:lang="en">FlowMeter</rdfs:label>
        <rdfs:label xml:lang="es">Meidor de Flujo</rdfs:label>
    </owl:Class>
    


    <!-- https://w3id.org/mep#FlowMovingDevice -->


    <owl:Class rdf:about="https://w3id.org/mep#FlowMovingDevice">
        <rdfs:subClassOf rdf:resource="https://w3id.org/mep#DistributionFlowElement"/>
        <rdfs:comment xml:lang="es">Define la aparición de un aparato utilizado para distribuir, hacer circular o realizar el transporte de fluidos, incluidos líquidos y gases (como una bomba o un ventilador), y normalmente participa en un sistema de distribución de flujo.</rdfs:comment>
        <rdfs:comment xml:lang="en">Defines the occurrence of an apparatus used to distribute, circulate or perform conveyance of fluids, including liquids and gases (such as a pump or fan), and typically participates in a flow distribution system</rdfs:comment>
        <rdfs:label xml:lang="es">Dispositivo de Movimiento de Flujo</rdfs:label>
        <rdfs:label xml:lang="en">Flow Moving Device</rdfs:label>
    </owl:Class>
    


    <!-- https://w3id.org/mep#FlowSegment -->


    <owl:Class rdf:about="https://w3id.org/mep#FlowSegment">
        <rdfs:subClassOf rdf:resource="https://w3id.org/mep#DistributionFlowElement"/>
        <rdfs:comment xml:lang="es">Define la ocurrencia de un segmento de un sistema de distribución de flujo.</rdfs:comment>
        <rdfs:comment xml:lang="en">Defines the occurrence of a segment of a flow distribution system.</rdfs:comment>
        <rdfs:label xml:lang="en">Flow Segment</rdfs:label>
        <rdfs:label xml:lang="es">Segmento de Flujo</rdfs:label>
    </owl:Class>
    


    <!-- https://w3id.org/mep#FlowSensor -->


    <owl:Class rdf:about="https://w3id.org/mep#FlowSensor">
        <rdfs:subClassOf rdf:resource="https://w3id.org/mep#Sensor"/>
        <rdfs:comment xml:lang="en">A device that senses or detects flow in a fluid.</rdfs:comment>
        <rdfs:comment xml:lang="es">Dispositivo que detecta el caudal de un fluido.</rdfs:comment>
        <rdfs:label xml:lang="en">Flow Sensor</rdfs:label>
        <rdfs:label xml:lang="es">Sensor de Flujo</rdfs:label>
    </owl:Class>
    


    <!-- https://w3id.org/mep#FlowStorageDevice -->


    <owl:Class rdf:about="https://w3id.org/mep#FlowStorageDevice">
        <rdfs:subClassOf rdf:resource="https://w3id.org/mep#DistributionFlowElement"/>
        <rdfs:comment xml:lang="es">Define la ocurrencia de un dispositivo que participa en un sistema de distribución y se utiliza para almacenamiento temporal (como un tanque)</rdfs:comment>
        <rdfs:comment xml:lang="en">Defines the occurrence of a device that participates in a distribution system and is used for temporary storage (such as a tank)</rdfs:comment>
        <rdfs:label xml:lang="es">Dispositivo de Almacenamiento de Flujo</rdfs:label>
        <rdfs:label xml:lang="en">Flow Storage Device</rdfs:label>
    </owl:Class>
    


    <!-- https://w3id.org/mep#FlowTerminal -->


    <owl:Class rdf:about="https://w3id.org/mep#FlowTerminal">
        <rdfs:subClassOf rdf:resource="https://w3id.org/mep#DistributionFlowElement"/>
        <rdfs:comment xml:lang="es">Define la aparición de un elemento permanentemente adjunto que actúa como término o comienzo de un sistema de distribución (como una salida de aire, un desagüe, un inodoro o un fregadero). Una terminal suele ser un punto en el que un sistema interactúa con un entorno externo.</rdfs:comment>
        <rdfs:comment xml:lang="en">Defines the occurrence of a permanently attached element that acts as a terminus or beginning of a distribution system (such as an air outlet, drain, water closet, or sink). A terminal is typically a point at which a system interfaces with an external environment.</rdfs:comment>
        <rdfs:label xml:lang="en">Flow Terminal</rdfs:label>
        <rdfs:label xml:lang="es">Terminal de Flujo</rdfs:label>
    </owl:Class>
    


    <!-- https://w3id.org/mep#FlowTreatmentDevice -->


    <owl:Class rdf:about="https://w3id.org/mep#FlowTreatmentDevice">
        <rdfs:subClassOf rdf:resource="https://w3id.org/mep#DistributionFlowElement"/>
        <rdfs:comment xml:lang="es">Define la aparición de un dispositivo utilizado típicamente para eliminar materia no deseada de un fluido, ya sea líquido o gaseoso, y normalmente participa en un sistema de distribución de flujo.</rdfs:comment>
        <rdfs:comment xml:lang="en">Defines the occurrence of a device typically used to remove unwanted matter from a fluid, either liquid or gas, and typically participates in a flow distribution system.</rdfs:comment>
        <rdfs:label xml:lang="es">Dispositivo de Tratamiento de Flujo</rdfs:label>
        <rdfs:label xml:lang="en">Flow Treatment Device</rdfs:label>
    </owl:Class>
    


    <!-- https://w3id.org/mep#FluorescentLamp -->


    <owl:Class rdf:about="https://w3id.org/mep#FluorescentLamp">
        <rdfs:subClassOf rdf:resource="https://w3id.org/mep#Lamp"/>
        <rdfs:comment xml:lang="en">A typically tubular discharge lamp in which most of the light is emitted by one or several layers of phosphors excited by ultraviolet radiation from the discharge.</rdfs:comment>
        <rdfs:comment xml:lang="es">Lámpara de descarga típicamente tubular en la que la mayor parte de la luz es emitida por una o varias capas de fósforo excitadas por la radiación ultravioleta de la descarga.</rdfs:comment>
        <rdfs:label xml:lang="en">Fluorescent Lamp</rdfs:label>
        <rdfs:label xml:lang="es">Lampara Fluorescente</rdfs:label>
    </owl:Class>
    


    <!-- https://w3id.org/mep#FlushingValve -->


    <owl:Class rdf:about="https://w3id.org/mep#FlushingValve">
        <rdfs:subClassOf rdf:resource="https://w3id.org/mep#Valve"/>
        <rdfs:comment xml:lang="en">Valve that flushes a predetermined quantity of water to cleanse a toilet, urinal, etc.</rdfs:comment>
        <rdfs:comment xml:lang="es">Válvula que descarga una cantidad predeterminada de agua para limpiar un inodoro, urinario, etc.</rdfs:comment>
        <rdfs:label xml:lang="en">Flushing Valve</rdfs:label>
        <rdfs:label xml:lang="es">Valvula de Descarga</rdfs:label>
    </owl:Class>
    


    <!-- https://w3id.org/mep#ForeignObjectDetectionSensor -->


    <owl:Class rdf:about="https://w3id.org/mep#ForeignObjectDetectionSensor">
        <rdfs:subClassOf rdf:resource="https://w3id.org/mep#Sensor"/>
        <rdfs:comment xml:lang="en">A device that senses or detects foreign objects that shock or break the power network. It may alarm when such accidents happen.</rdfs:comment>
        <rdfs:comment xml:lang="es">Dispositivo que detecta o detecta objetos extraños que provocan descargas o roturas en la red eléctrica. Puede dar la alarma cuando se producen tales accidentes.</rdfs:comment>
        <rdfs:label xml:lang="en">Foreign Object Detection Sensor</rdfs:label>
        <rdfs:label xml:lang="es">Sensor de Deteccion de Objetos Extraños</rdfs:label>
    </owl:Class>
    


    <!-- https://w3id.org/mep#FormedDuct -->


    <owl:Class rdf:about="https://w3id.org/mep#FormedDuct">
        <rdfs:subClassOf rdf:resource="https://w3id.org/mep#DistributionChamberElement"/>
        <rdfs:comment xml:lang="es">Espacio formado en el suelo para el paso de tuberías, cables, conductos.</rdfs:comment>
        <rdfs:comment xml:lang="en">Space formed in the ground for the passage of pipes, cables, ducts.</rdfs:comment>
        <rdfs:label xml:lang="es">Conducto Formado</rdfs:label>
        <rdfs:label xml:lang="en">Formed Duct</rdfs:label>
    </owl:Class>
    


    <!-- https://w3id.org/mep#FreestandingElectricHeater -->


    <owl:Class rdf:about="https://w3id.org/mep#FreestandingElectricHeater">
        <rdfs:subClassOf rdf:resource="https://w3id.org/mep#ElectricAppliance"/>
        <rdfs:comment xml:lang="en">An electrical appliance that is used occasionally to provide heat. A freestanding electric heater is a &apos;plugged&apos; appliance whose load may be removed from an electric circuit.</rdfs:comment>
        <rdfs:comment xml:lang="es">Aparato eléctrico que se utiliza ocasionalmente para proporcionar calor. Un calefactor eléctrico independiente es un aparato &apos;enchufado&apos; cuya carga puede retirarse de un circuito eléctrico.</rdfs:comment>
        <rdfs:label xml:lang="es">Calefactor Eléctrico Independiente</rdfs:label>
        <rdfs:label xml:lang="en">Freestanding Electric Heater</rdfs:label>
    </owl:Class>
    


    <!-- https://w3id.org/mep#FreestandingFan -->


    <owl:Class rdf:about="https://w3id.org/mep#FreestandingFan">
        <rdfs:subClassOf rdf:resource="https://w3id.org/mep#ElectricAppliance"/>
        <rdfs:comment xml:lang="en">An electrical appliance that is used occasionally to provide ventilation. A freestanding fan is a &apos;plugged&apos; appliance whose load may be removed from an electric circuit.</rdfs:comment>
        <rdfs:comment xml:lang="es">Aparato eléctrico que se utiliza ocasionalmente para proporcionar ventilación. Un ventilador independiente es un aparato &apos;enchufado&apos; cuya carga puede retirarse de un circuito eléctrico.</rdfs:comment>
        <rdfs:label xml:lang="en">Freestanding Fan</rdfs:label>
        <rdfs:label xml:lang="es">Ventilador Independiente</rdfs:label>
    </owl:Class>
    


    <!-- https://w3id.org/mep#FreestandingWaterCooler -->


    <owl:Class rdf:about="https://w3id.org/mep#FreestandingWaterCooler">
        <rdfs:subClassOf rdf:resource="https://w3id.org/mep#ElectricAppliance"/>
        <rdfs:comment xml:lang="en">A small, local electrical appliance for cooling water. A freestanding water cooler is a &apos;plugged&apos; appliance whose load may be removed from an electric circuit.</rdfs:comment>
        <rdfs:comment xml:lang="es">Pequeño aparato eléctrico local para enfriar agua. Un refrigerador de agua independiente es un aparato &apos;enchufado&apos; cuya carga puede retirarse de un circuito eléctrico</rdfs:comment>
        <rdfs:label xml:lang="en">Freestanding Water Cooler </rdfs:label>
        <rdfs:label xml:lang="es">Refrigerador de Agua Independiente</rdfs:label>
    </owl:Class>
    


    <!-- https://w3id.org/mep#FreestandingWaterHeater -->


    <owl:Class rdf:about="https://w3id.org/mep#FreestandingWaterHeater">
        <rdfs:subClassOf rdf:resource="https://w3id.org/mep#ElectricAppliance"/>
        <rdfs:comment xml:lang="en">A small, local electrical appliance for heating water. A freestanding water heater is a &apos;plugged&apos; appliance whose load may be removed from an electric circuit.</rdfs:comment>
        <rdfs:comment xml:lang="es">Pequeño aparato eléctrico local para calentar agua. Un calentador de agua independiente es un aparato &apos;enchufado&apos; cuya carga puede retirarse de un circuito eléctrico.</rdfs:comment>
        <rdfs:label xml:lang="es">Calentador de Agua Independiente</rdfs:label>
        <rdfs:label xml:lang="en">Freestanding Water Heater</rdfs:label>
    </owl:Class>
    


    <!-- https://w3id.org/mep#Freezer -->


    <owl:Class rdf:about="https://w3id.org/mep#Freezer">
        <rdfs:subClassOf rdf:resource="https://w3id.org/mep#ElectricAppliance"/>
        <rdfs:comment xml:lang="en">An electrical appliance that has the primary function of storing food at temperatures below the freezing point of water.</rdfs:comment>
        <rdfs:comment xml:lang="es">Aparato eléctrico cuya función principal es conservar alimentos a temperaturas inferiores al punto de congelación del agua.</rdfs:comment>
        <rdfs:label xml:lang="es">Congelador</rdfs:label>
        <rdfs:label xml:lang="en">Freezer</rdfs:label>
    </owl:Class>
    


    <!-- https://w3id.org/mep#FrequencyMeter -->


    <owl:Class rdf:about="https://w3id.org/mep#FrequencyMeter">
        <rdfs:subClassOf rdf:resource="https://w3id.org/mep#FlowInstrument"/>
        <rdfs:comment xml:lang="en">A device that reads and displays the electrical frequency of an alternating current circuit.</rdfs:comment>
        <rdfs:comment xml:lang="es">Dispositivo que lee y muestra la frecuencia eléctrica de un circuito de corriente alterna.</rdfs:comment>
        <rdfs:label xml:lang="en">Frequency Meter</rdfs:label>
        <rdfs:label xml:lang="es">Medidor de Frecuencia</rdfs:label>
    </owl:Class>
    


    <!-- https://w3id.org/mep#FrequencyTransformer -->


    <owl:Class rdf:about="https://w3id.org/mep#FrequencyTransformer">
        <rdfs:subClassOf rdf:resource="https://w3id.org/mep#Transformer"/>
        <rdfs:comment xml:lang="en">A transformer that changes the frequency between circuits.</rdfs:comment>
        <rdfs:comment xml:lang="es">Un conversor que cambia la frecuencia entre circuitos.</rdfs:comment>
        <rdfs:label xml:lang="es">Conversor de Frecuencia</rdfs:label>
        <rdfs:label xml:lang="en">Frequency Transformer</rdfs:label>
    </owl:Class>
    


    <!-- https://w3id.org/mep#Fridge-Freezer -->


    <owl:Class rdf:about="https://w3id.org/mep#Fridge-Freezer">
        <rdfs:subClassOf rdf:resource="https://w3id.org/mep#ElectricAppliance"/>
        <rdfs:comment xml:lang="en">An electrical appliance that combines the functions of a freezer and a refrigerator through the provision of separate compartments.</rdfs:comment>
        <rdfs:comment xml:lang="es">Electrodoméstico que combina las funciones de un congelador y un frigorífico mediante la disposición de compartimentos separados.</rdfs:comment>
        <rdfs:label xml:lang="en">Fridge-Freezer</rdfs:label>
        <rdfs:label xml:lang="es">Frigorifico-Congelador</rdfs:label>
    </owl:Class>
    


    <!-- https://w3id.org/mep#FrostSensor -->


    <owl:Class rdf:about="https://w3id.org/mep#FrostSensor">
        <rdfs:subClassOf rdf:resource="https://w3id.org/mep#Sensor"/>
        <rdfs:comment xml:lang="en">A device that senses or detects frost on a window.</rdfs:comment>
        <rdfs:comment xml:lang="es">Dispositivo que detecta la escarcha en una ventana.</rdfs:comment>
        <rdfs:label xml:lang="en">Frost Sensor</rdfs:label>
        <rdfs:label xml:lang="es">Sensor de Congelacion</rdfs:label>
    </owl:Class>
    


    <!-- https://w3id.org/mep#FumeHoodExhaustDamper -->


    <owl:Class rdf:about="https://w3id.org/mep#FumeHoodExhaustDamper">
        <rdfs:subClassOf rdf:resource="https://w3id.org/mep#Damper"/>
        <rdfs:comment xml:lang="es">Compuerta de extracción de la campana extractora. Normalmente se acciona mediante un actuador.</rdfs:comment>
        <rdfs:comment xml:lang="en">Fume hood exhaust damper. Commonly operated by actuator.</rdfs:comment>
        <rdfs:label xml:lang="es">Compuerta de Extraccion</rdfs:label>
        <rdfs:label xml:lang="en">Fume Hood Exhaust Damper</rdfs:label>
    </owl:Class>
    


    <!-- https://w3id.org/mep#FuseDisconnector -->


    <owl:Class rdf:about="https://w3id.org/mep#FuseDisconnector">
        <rdfs:subClassOf rdf:resource="https://w3id.org/mep#ProtectiveDevice"/>
        <rdfs:comment xml:lang="en">A device that will electrically open the circuit after a period of prolonged, abnormal current flow.</rdfs:comment>
        <rdfs:comment xml:lang="es">Dispositivo que abre eléctricamente el circuito tras un periodo prolongado de flujo anormal de corriente.</rdfs:comment>
        <rdfs:label xml:lang="es">Descnector Fusible</rdfs:label>
        <rdfs:label xml:lang="en">Fuse Disconnector</rdfs:label>
    </owl:Class>
    


    <!-- https://w3id.org/mep#GasCock -->


    <owl:Class rdf:about="https://w3id.org/mep#GasCock">
        <rdfs:subClassOf rdf:resource="https://w3id.org/mep#Valve"/>
        <rdfs:comment xml:lang="en">Valve that is used for controlling the flow of gas.</rdfs:comment>
        <rdfs:comment xml:lang="es">Válvula que se utiliza para controlar el flujo de gas.</rdfs:comment>
        <rdfs:label xml:lang="en">Gas Cock</rdfs:label>
        <rdfs:label xml:lang="es">Valvula de Regulación de Gas</rdfs:label>
    </owl:Class>
    


    <!-- https://w3id.org/mep#GasDetectionPanel -->


    <owl:Class rdf:about="https://w3id.org/mep#GasDetectionPanel">
        <rdfs:subClassOf rdf:resource="https://w3id.org/mep#UnitaryControlElement"/>
        <rdfs:comment xml:lang="en">A control element that senses and regulates the humidity of a system or space so that the humidity is maintained near a desired setpoint.</rdfs:comment>
        <rdfs:comment xml:lang="es">Un elemento de control en el que se anuncia la detección de gas.</rdfs:comment>
        <rdfs:label xml:lang="en">Gas Detection Panel</rdfs:label>
        <rdfs:label xml:lang="es">Panel de Deteccion de Gas</rdfs:label>
    </owl:Class>
    


    <!-- https://w3id.org/mep#GasHeatCoil -->


    <owl:Class rdf:about="https://w3id.org/mep#GasHeatCoil">
        <rdfs:subClassOf rdf:resource="https://w3id.org/mep#Coil"/>
        <rdfs:comment xml:lang="en">Heating coil using gas as a heating source.</rdfs:comment>
        <rdfs:comment xml:lang="es">Serpentín calefactor que utiliza gas como fuente de calor.</rdfs:comment>
        <rdfs:label xml:lang="en">Gas Heat Coil</rdfs:label>
        <rdfs:label xml:lang="es">Serpentin Calefactor de Gas</rdfs:label>
    </owl:Class>
    


    <!-- https://w3id.org/mep#GasMeter -->


    <owl:Class rdf:about="https://w3id.org/mep#GasMeter">
        <rdfs:subClassOf rdf:resource="https://w3id.org/mep#FlowMeter"/>
        <rdfs:comment xml:lang="en">A device that measures the quantity of a gas or fuel.</rdfs:comment>
        <rdfs:comment xml:lang="es">Dispositivo que mide la cantidad de un gas o combustible.</rdfs:comment>
        <rdfs:label xml:lang="en">Gas Meter</rdfs:label>
        <rdfs:label xml:lang="es">Medidor de Gas</rdfs:label>
    </owl:Class>
    


    <!-- https://w3id.org/mep#GasSensor -->


    <owl:Class rdf:about="https://w3id.org/mep#GasSensor">
        <rdfs:subClassOf rdf:resource="https://w3id.org/mep#Sensor"/>
        <rdfs:comment xml:lang="en">A device that senses or detects gas concentration (other than CO2)</rdfs:comment>
        <rdfs:comment xml:lang="es">Dispositivo que detecta la concentración de gas (distinto del CO2)</rdfs:comment>
        <rdfs:label xml:lang="en">Gas Sensor</rdfs:label>
        <rdfs:label xml:lang="es">Sensor de gas</rdfs:label>
    </owl:Class>
    


    <!-- https://w3id.org/mep#GasTap -->


    <owl:Class rdf:about="https://w3id.org/mep#GasTap">
        <rdfs:subClassOf rdf:resource="https://w3id.org/mep#Valve"/>
        <rdfs:comment xml:lang="en">Gas tap typically used for venting or discharging gas from a system.</rdfs:comment>
        <rdfs:comment xml:lang="es">Grifo de gas que normalmente se utiliza para ventilar o descargar gas de un sistema.</rdfs:comment>
        <rdfs:label xml:lang="en">Gas Tap</rdfs:label>
        <rdfs:label xml:lang="es">Valvula de Descarga de Gas</rdfs:label>
    </owl:Class>
    


    <!-- https://w3id.org/mep#Gateway -->


    <owl:Class rdf:about="https://w3id.org/mep#Gateway">
        <rdfs:subClassOf rdf:resource="https://w3id.org/mep#CommunicationsAppliance"/>
        <rdfs:comment xml:lang="en">A gateway connects multiple network segments with different protocols at all layers (layers 1-7) of the Open Systems Interconnection (OSI) model.</rdfs:comment>
        <rdfs:comment xml:lang="es">Un gateway conecta varios segmentos de red con protocolos diferentes en todas las capas (capas 1-7) del modelo de Interconexión de Sistemas Abiertos (OSI).</rdfs:comment>
        <rdfs:label xml:lang="en">Gateway</rdfs:label>
        <rdfs:label xml:lang="es">Gateway</rdfs:label>
    </owl:Class>
    


    <!-- https://w3id.org/mep#GatewayGPRSNodeSupport -->


    <owl:Class rdf:about="https://w3id.org/mep#GatewayGPRSNodeSupport">
        <rdfs:subClassOf rdf:resource="https://w3id.org/mep#MobileTelecommunicationsAppliance"/>
        <rdfs:comment xml:lang="es">El nodo de soporte GPRS gateway es un componente de la red central GPRS que amplía el GSM para permitir funcionalidades de conmutación de paquetes. Este componente es responsable de la interconexión entre la red GPRS y las redes externas de conmutación de paquetes (por ejemplo, Internet).</rdfs:comment>
        <rdfs:comment xml:lang="en">The gateway GPRS support node is a component of the GPRS core network that extends the GSM to allow packet switching functionalities. This component is responsible for the internetworking between the GPRS network and external packet switched networks (e.g. the internet).</rdfs:comment>
        <rdfs:label xml:lang="en">Gateway GPRS Node Support</rdfs:label>
        <rdfs:label xml:lang="es">Nodo de Soport GPRS Gateway</rdfs:label>
    </owl:Class>
    


    <!-- https://w3id.org/mep#Gravity-reliefDamper -->


    <owl:Class rdf:about="https://w3id.org/mep#Gravity-reliefDamper">
        <rdfs:subClassOf rdf:resource="https://w3id.org/mep#Damper"/>
        <rdfs:comment xml:lang="es">Compuerta de alivio de la gravedad que permite el movimiento del aire cuando se acumula suficiente presión para vencer la fuerza gravitatoria ejercida sobre las lamas de la compuerta. Normalmente se acciona por el peso de la gravedad.</rdfs:comment>
        <rdfs:comment xml:lang="en">Gravity-relief damper used to allow air to move upon a buildup of enough pressure to overcome the gravitational force exerted upon the damper blades. Commonly operated by gravitational weight.</rdfs:comment>
        <rdfs:label xml:lang="es">Compuerta de Alivio de La Gravedad</rdfs:label>
        <rdfs:label xml:lang="en">Gravity-relief Damper</rdfs:label>
    </owl:Class>
    


    <!-- https://w3id.org/mep#GravityDamper -->


    <owl:Class rdf:about="https://w3id.org/mep#GravityDamper">
        <rdfs:subClassOf rdf:resource="https://w3id.org/mep#Damper"/>
        <rdfs:comment xml:lang="en">Gravity damper closes from the force of gravity. Commonly operated by gravitational weight.</rdfs:comment>
        <rdfs:comment xml:lang="es">La compuerta de gravedad se cierra por la fuerza de la gravedad. Normalmente se acciona por el peso de la gravedad.</rdfs:comment>
        <rdfs:label xml:lang="es">Compuerta de Gravedad</rdfs:label>
        <rdfs:label xml:lang="en">Gravity Damper</rdfs:label>
    </owl:Class>
    


    <!-- https://w3id.org/mep#GreaseInterceptor -->


    <owl:Class rdf:about="https://w3id.org/mep#GreaseInterceptor">
        <rdfs:subClassOf rdf:resource="https://w3id.org/mep#Interceptor"/>
        <rdfs:comment xml:lang="en">Chamber, on the line of a drain or discharge pipe, that prevents grease passing into a drainage system.</rdfs:comment>
        <rdfs:comment xml:lang="es">Cámara, en la línea de una tubería de desagüe o descarga, que impide el paso de grasa a un sistema de drenaje.</rdfs:comment>
        <rdfs:label xml:lang="en">Grease Interceptor</rdfs:label>
        <rdfs:label xml:lang="es">Interceptor de Grasa</rdfs:label>
    </owl:Class>
    


    <!-- https://w3id.org/mep#Grille -->


    <owl:Class rdf:about="https://w3id.org/mep#Grille">
        <rdfs:subClassOf rdf:resource="https://w3id.org/mep#AirTerminal"/>
        <rdfs:comment xml:lang="en">A covering for any area through which air passes.</rdfs:comment>
        <rdfs:comment xml:lang="es">Un revestimiento para cualquier zona por la que pase el aire.</rdfs:comment>
        <rdfs:label xml:lang="en">Grille</rdfs:label>
        <rdfs:label xml:lang="es">Rejilla</rdfs:label>
    </owl:Class>
    


    <!-- https://w3id.org/mep#GullySump -->


    <owl:Class rdf:about="https://w3id.org/mep#GullySump">
        <rdfs:subClassOf rdf:resource="https://w3id.org/mep#WasteTerminal"/>
        <rdfs:comment xml:lang="es">Accesorio o conjunto de accesorios para recibir aguas superficiales o residuales, provisto de una rejilla o cubierta sellada.</rdfs:comment>
        <rdfs:comment xml:lang="en">Pipe fitting or assembly of fittings to receive surface water or waste water, fitted with a grating or sealed cover.</rdfs:comment>
        <rdfs:label xml:lang="en">Gully Sump</rdfs:label>
        <rdfs:label xml:lang="es">Sumidero</rdfs:label>
    </owl:Class>
    


    <!-- https://w3id.org/mep#GullyTrap -->


    <owl:Class rdf:about="https://w3id.org/mep#GullyTrap">
        <rdfs:subClassOf rdf:resource="https://w3id.org/mep#WasteTerminal"/>
        <rdfs:comment xml:lang="es">Accesorio de tubería o un conjunto de accesorios que recibe agua superficial o aguas residuales; Equipado con una rejilla o cubierta sellada que descarga el agua a través de una trampa.</rdfs:comment>
        <rdfs:comment xml:lang="en">Pipe fitting or assembly of fittings that receives surface water or waste water; fitted with a grating or sealed cover that discharges water through a trap.</rdfs:comment>
        <rdfs:label xml:lang="en">Gully Trap</rdfs:label>
        <rdfs:label xml:lang="es">Trampa de Barranco</rdfs:label>
    </owl:Class>
    


    <!-- https://w3id.org/mep#Gutter -->


    <owl:Class rdf:about="https://w3id.org/mep#Gutter">
        <rdfs:subClassOf rdf:resource="https://w3id.org/mep#PipeSegment"/>
        <rdfs:comment xml:lang="en">A gutter segment is a continuous open-channel segment of pipe.</rdfs:comment>
        <rdfs:comment xml:lang="es">Un canalon es un segmento continuo de canal abierto de tubería.</rdfs:comment>
        <rdfs:label xml:lang="es">Canalon</rdfs:label>
        <rdfs:label xml:lang="en">Gutter</rdfs:label>
    </owl:Class>
    


    <!-- https://w3id.org/mep#HalogenLamp -->


    <owl:Class rdf:about="https://w3id.org/mep#HalogenLamp">
        <rdfs:subClassOf rdf:resource="https://w3id.org/mep#Lamp"/>
        <rdfs:comment xml:lang="en">An incandescent lamp in which a tungsten filament is sealed into a compact transport envelope filled with an inert gas and a small amount of halogen such as iodine or bromine.</rdfs:comment>
        <rdfs:comment xml:lang="es">Lámpara incandescente en la que un filamento de tungsteno está sellado en una envoltura de transporte compacta llena de un gas inerte y una pequeña cantidad de halógeno como yodo o bromo.</rdfs:comment>
        <rdfs:label xml:lang="en">Halogen Lamp</rdfs:label>
        <rdfs:label xml:lang="es">Lampara Halogena</rdfs:label>
    </owl:Class>
    


    <!-- https://w3id.org/mep#HandDryer -->


    <owl:Class rdf:about="https://w3id.org/mep#HandDryer">
        <rdfs:subClassOf rdf:resource="https://w3id.org/mep#ElectricAppliance"/>
        <rdfs:comment xml:lang="en">An electrical appliance that has the primary function of drying hands.</rdfs:comment>
        <rdfs:comment xml:lang="es">Aparato eléctrico cuya función principal es secar las manos.</rdfs:comment>
        <rdfs:label xml:lang="en">Hand Dryer</rdfs:label>
        <rdfs:label xml:lang="es">Secador de Manos</rdfs:label>
    </owl:Class>
    


    <!-- https://w3id.org/mep#HandOperatedActuator -->


    <owl:Class rdf:about="https://w3id.org/mep#HandOperatedActuator">
        <rdfs:subClassOf rdf:resource="https://w3id.org/mep#Actuator"/>
        <rdfs:comment xml:lang="en">A device that manually actuates a control element.</rdfs:comment>
        <rdfs:comment xml:lang="es">Dispositivo que acciona manualmente un elemento de control.</rdfs:comment>
        <rdfs:label xml:lang="es">Actuador Manual</rdfs:label>
        <rdfs:label xml:lang="en">Hand Operated Actuator</rdfs:label>
    </owl:Class>
    


    <!-- https://w3id.org/mep#HarmonicFilter -->


    <owl:Class rdf:about="https://w3id.org/mep#HarmonicFilter">
        <rdfs:subClassOf rdf:resource="https://w3id.org/mep#ElectricFlowStorageDevice"/>
        <rdfs:comment xml:lang="en">A device that constantly injects currents that precisely correspond to the harmonic components drawn by the load.</rdfs:comment>
        <rdfs:comment xml:lang="es">Dispositivo que inyecta constantemente corrientes que corresponden con precisión a los componentes armónicos extraídos por la carga.</rdfs:comment>
        <rdfs:label xml:lang="es">Filtro de Armonicos</rdfs:label>
        <rdfs:label xml:lang="en">Harmonic Filter</rdfs:label>
    </owl:Class>
    


    <!-- https://w3id.org/mep#HeatExchanger -->


    <owl:Class rdf:about="https://w3id.org/mep#HeatExchanger">
        <rdfs:subClassOf rdf:resource="https://w3id.org/mep#EnergyConversionDevice"/>
        <rdfs:comment xml:lang="en">A heat exchanger is a device used to provide heat transfer between non-mixing media such as plate and shell and tube heat exchangers.</rdfs:comment>
        <rdfs:comment xml:lang="es">Un intercambiador de calor es un dispositivo que se utiliza para proporcionar transferencia de calor entre medios que no se mezclan, como intercambiadores de calor de placas y de carcasa y tubos.</rdfs:comment>
        <rdfs:label xml:lang="en">Heat Exchanger</rdfs:label>
        <rdfs:label xml:lang="es">Intercambiador de Calor</rdfs:label>
    </owl:Class>
    


    <!-- https://w3id.org/mep#HeatPipe -->


    <owl:Class rdf:about="https://w3id.org/mep#HeatPipe">
        <rdfs:subClassOf rdf:resource="https://w3id.org/mep#AirToAirHeatRecovery"/>
        <rdfs:comment xml:lang="en">A passive energy recovery device with a heat pipe divided into evaporator and condenser sections.</rdfs:comment>
        <rdfs:comment xml:lang="es">Un dispositivo pasivo de recuperación de energía con un tubo de calor dividido en secciones de evaporador y condensador.</rdfs:comment>
        <rdfs:label xml:lang="en">Heat Pipe</rdfs:label>
        <rdfs:label xml:lang="es">Tubo de Calor</rdfs:label>
    </owl:Class>
    


    <!-- https://w3id.org/mep#HeatRecoveryChiller -->


    <owl:Class rdf:about="https://w3id.org/mep#HeatRecoveryChiller">
        <rdfs:subClassOf rdf:resource="https://w3id.org/mep#Chiller"/>
        <rdfs:comment xml:lang="es">Enfirador con Recuperacion de Calor</rdfs:comment>
        <rdfs:comment xml:lang="en">Heat Recovery Chiller</rdfs:comment>
        <rdfs:label xml:lang="es">Enfirador con Recuperacion de Calor</rdfs:label>
        <rdfs:label xml:lang="en">Heat Recovery Chiller</rdfs:label>
    </owl:Class>
    


    <!-- https://w3id.org/mep#HeatSensor -->


    <owl:Class rdf:about="https://w3id.org/mep#HeatSensor">
        <rdfs:subClassOf rdf:resource="https://w3id.org/mep#Sensor"/>
        <rdfs:comment xml:lang="en">A device that senses or detects heat.</rdfs:comment>
        <rdfs:comment xml:lang="es">Dispositivo que percibe o detecta el calor.</rdfs:comment>
        <rdfs:label xml:lang="en">Heat Sensor</rdfs:label>
        <rdfs:label xml:lang="es">Sensor de Calor</rdfs:label>
    </owl:Class>
    


    <!-- https://w3id.org/mep#HermeticCompressor -->


    <owl:Class rdf:about="https://w3id.org/mep#HermeticCompressor">
        <rdfs:subClassOf rdf:resource="https://w3id.org/mep#Compressor"/>
        <rdfs:comment xml:lang="es">Compresor alternativo de desplazamiento positivo en el que el motor y el compresor están contenidos en la misma carcasa, con el eje del motor integrado en el cigüeñal del compresor y el motor en contacto con el refrigerante.</rdfs:comment>
        <rdfs:comment xml:lang="en">Positive-displacement reciprocating compressor where the motor and compressor are contained within the same housing, with the motor shaft integral with the compressor crankshaft and the motor in contact with refrigerant.</rdfs:comment>
        <rdfs:label xml:lang="es">Compresor Hermetico</rdfs:label>
        <rdfs:label xml:lang="en">Hermetic Compressor</rdfs:label>
    </owl:Class>
    


    <!-- https://w3id.org/mep#HighPressureMercuryLamp -->


    <owl:Class rdf:about="https://w3id.org/mep#HighPressureMercuryLamp">
        <rdfs:subClassOf rdf:resource="https://w3id.org/mep#Lamp"/>
        <rdfs:comment xml:lang="en">A discharge lamp in which most of the light is emitted by exciting mercury at high pressure.</rdfs:comment>
        <rdfs:comment xml:lang="es">Lámpara de descarga en la que la mayor parte de la luz se emite excitando mercurio a alta presión.</rdfs:comment>
        <rdfs:label xml:lang="en">High Pressure Mercury Lamp</rdfs:label>
        <rdfs:label xml:lang="es">Lampara de Mercurio a Alta Presion</rdfs:label>
    </owl:Class>
    


    <!-- https://w3id.org/mep#HighPressureSodiumLamp -->


    <owl:Class rdf:about="https://w3id.org/mep#HighPressureSodiumLamp">
        <rdfs:subClassOf rdf:resource="https://w3id.org/mep#Lamp"/>
        <rdfs:comment xml:lang="en">A discharge lamp in which most of the light is emitted by exciting sodium at high pressure.</rdfs:comment>
        <rdfs:comment xml:lang="es">Lámpara de descarga en la que la mayor parte de la luz se emite excitando sodio a alta presión.</rdfs:comment>
        <rdfs:label xml:lang="en">High Pressure Sodium Lamp</rdfs:label>
        <rdfs:label xml:lang="es">Lampara de Sodio a Alta Presion</rdfs:label>
    </owl:Class>
    


    <!-- https://w3id.org/mep#Hosereel -->


    <owl:Class rdf:about="https://w3id.org/mep#Hosereel">
        <rdfs:subClassOf rdf:resource="https://w3id.org/mep#LiquidTerminal"/>
        <rdfs:comment xml:lang="en">A Supporting framework on which a hose may be wound whose primary purpose is to connect and interact with the external environment.</rdfs:comment>
        <rdfs:comment xml:lang="es">Estructura de soporte sobre la que se puede enrollar una manguera cuyo objetivo principal es conectarse e interactuar con el entorno externo.</rdfs:comment>
        <rdfs:label xml:lang="en">Hosereel</rdfs:label>
        <rdfs:label xml:lang="es">Terminal de Manguera</rdfs:label>
    </owl:Class>
    


    <!-- https://w3id.org/mep#Humidifier -->


    <owl:Class rdf:about="https://w3id.org/mep#Humidifier">
        <rdfs:subClassOf rdf:resource="https://w3id.org/mep#EnergyConversionDevice"/>
        <rdfs:comment xml:lang="en">A humidifier is a device that adds moisture into the air.</rdfs:comment>
        <rdfs:comment xml:lang="es">Un humidificador es un dispositivo que agrega humedad al aire.</rdfs:comment>
        <rdfs:label xml:lang="es">Humidificador</rdfs:label>
        <rdfs:label xml:lang="en">Humidifier</rdfs:label>
    </owl:Class>
    


    <!-- https://w3id.org/mep#Humidistat -->


    <owl:Class rdf:about="https://w3id.org/mep#Humidistat">
        <rdfs:subClassOf rdf:resource="https://w3id.org/mep#UnitaryControlElement"/>
        <rdfs:comment xml:lang="en">A control element that senses and regulates the humidity of a system or space so that the humidity is maintained near a desired setpoint.</rdfs:comment>
        <rdfs:comment xml:lang="es">Un elemento de control que detecta y regula la humedad de un sistema o espacio para que la humedad se mantenga cerca de un punto de ajuste deseado.</rdfs:comment>
        <rdfs:label xml:lang="es">Higrostato</rdfs:label>
        <rdfs:label xml:lang="en">Humidistat</rdfs:label>
    </owl:Class>
    


    <!-- https://w3id.org/mep#HumiditySensor -->


    <owl:Class rdf:about="https://w3id.org/mep#HumiditySensor">
        <rdfs:subClassOf rdf:resource="https://w3id.org/mep#Sensor"/>
        <rdfs:comment xml:lang="en">A device that senses or detects humidity.</rdfs:comment>
        <rdfs:comment xml:lang="es">Dispositivo que detecta la humedad.</rdfs:comment>
        <rdfs:label xml:lang="en">Humidity Sensor</rdfs:label>
        <rdfs:label xml:lang="es">Sensor de Humedad</rdfs:label>
    </owl:Class>
    


    <!-- https://w3id.org/mep#HydraulicActuator -->


    <owl:Class rdf:about="https://w3id.org/mep#HydraulicActuator">
        <rdfs:subClassOf rdf:resource="https://w3id.org/mep#Actuator"/>
        <rdfs:comment xml:lang="en">A device that hydraulically actuates a control element.</rdfs:comment>
        <rdfs:comment xml:lang="es">Dispositivo que acciona hidráulicamente un elemento de control.</rdfs:comment>
        <rdfs:label xml:lang="es">Actuador Hidraulico</rdfs:label>
        <rdfs:label xml:lang="en">Hydraulic Actuator</rdfs:label>
    </owl:Class>
    


    <!-- https://w3id.org/mep#HydronicCoil -->


    <owl:Class rdf:about="https://w3id.org/mep#HydronicCoil">
        <rdfs:subClassOf rdf:resource="https://w3id.org/mep#Coil"/>
        <rdfs:comment xml:lang="en">Cooling or Heating coil that uses a hydronic fluid as a cooling or heating source.</rdfs:comment>
        <rdfs:comment xml:lang="es">Serpentín de enfriamiento o calentamiento que utiliza un fluido hidrónico como fuente de enfriamiento o calentamiento.</rdfs:comment>
        <rdfs:label xml:lang="en">Hydronic Coil</rdfs:label>
        <rdfs:label xml:lang="es">Serpentin Hidronico</rdfs:label>
    </owl:Class>
    


    <!-- https://w3id.org/mep#IPNetworkEquipment -->


    <owl:Class rdf:about="https://w3id.org/mep#IPNetworkEquipment">
        <rdfs:subClassOf rdf:resource="https://w3id.org/mep#CommunicationsAppliance"/>
        <rdfs:comment xml:lang="en">An IP network equipment is a device that provides IP data transmission channel for telecom subsystems or other subsystems e.g., routers, network switches or firewalls.</rdfs:comment>
        <rdfs:comment xml:lang="es">Un equipo de red IP es un dispositivo que proporciona un canal de transmisión de datos IP para subsistemas de telecomunicaciones u otros subsistemas, por ejemplo, enrutadores, conmutadores de red o cortafuegos.</rdfs:comment>
        <rdfs:label xml:lang="es">Equipode Red IP</rdfs:label>
        <rdfs:label xml:lang="en">IP Network Equipment</rdfs:label>
    </owl:Class>
    


    <!-- https://w3id.org/mep#IndentifierSensor -->


    <owl:Class rdf:about="https://w3id.org/mep#IndentifierSensor">
        <rdfs:subClassOf rdf:resource="https://w3id.org/mep#Sensor"/>
        <rdfs:comment xml:lang="en">A device that reads a tag, such as for gaining access to a door or elevator</rdfs:comment>
        <rdfs:comment xml:lang="es">Dispositivo que lee una etiqueta, por ejemplo para acceder a una puerta o a un ascensor.</rdfs:comment>
        <rdfs:label xml:lang="en">Indentifier Sensor</rdfs:label>
        <rdfs:label xml:lang="es">Sensor de Identificación</rdfs:label>
    </owl:Class>
    


    <!-- https://w3id.org/mep#IndicatorPanel -->


    <owl:Class rdf:about="https://w3id.org/mep#IndicatorPanel">
        <rdfs:subClassOf rdf:resource="https://w3id.org/mep#UnitaryControlElement"/>
        <rdfs:comment xml:lang="en">A control element at which equipment operational status, condition, safety state or other required parameters are indicated.</rdfs:comment>
        <rdfs:comment xml:lang="es">Un elemento de control en el que se indican el estado operativo, la condición, el estado de seguridad u otros parámetros requeridos del equipo.</rdfs:comment>
        <rdfs:label xml:lang="en">Indicator Panel</rdfs:label>
        <rdfs:label xml:lang="es">Panel Indicador</rdfs:label>
    </owl:Class>
    


    <!-- https://w3id.org/mep#IndirectDirectCombination -->


    <owl:Class rdf:about="https://w3id.org/mep#IndirectDirectCombination">
        <rdfs:subClassOf rdf:resource="https://w3id.org/mep#EvaporativeCooler"/>
        <rdfs:comment xml:lang="es">Combinación indirecta/directa: Enfría la corriente de aire evaporando el agua indirectamente y sin agregar humedad a la corriente de aire usando un enfriador de dos etapas con un enfriador evaporativo indirecto de primera etapa y un enfriador evaporativo directo de segunda etapa.</rdfs:comment>
        <rdfs:comment xml:lang="en">Indirect/Direct combination: Cools the air stream by evaporating water indirectly and without adding moisture into the air stream using a two-stage cooler with a first-stage indirect evaporative cooler and second-stage direct evaporative cooler.</rdfs:comment>
        <rdfs:label xml:lang="es">Combinación Indirecta/Directa</rdfs:label>
        <rdfs:label xml:lang="en">Indirect Direct Combination</rdfs:label>
    </owl:Class>
    


    <!-- https://w3id.org/mep#IndirectEvaporativeCoolingTowerorCoilCooler -->


    <owl:Class rdf:about="https://w3id.org/mep#IndirectEvaporativeCoolingTowerorCoilCooler">
        <rdfs:subClassOf rdf:resource="https://w3id.org/mep#EvaporativeCooler"/>
        <rdfs:comment xml:lang="en">Indirect evaporative cooling tower or coil cooler: Cools the air stream by evaporating water indirectly and without adding moisture into the air stream using a combination of a cooling tower or other evaporative water cooler with a water-to-air heat exchanger coil and water circulating pump.</rdfs:comment>
        <rdfs:comment xml:lang="es">Torre de enfriamiento evaporativo indirecto o enfriador de serpentín: enfría la corriente de aire evaporando el agua indirectamente y sin agregar humedad a la corriente de aire usando una combinación de una torre de enfriamiento u otro enfriador de agua por evaporación con un serpentín intercambiador de calor agua-aire y una bomba de circulación de agua. .</rdfs:comment>
        <rdfs:label xml:lang="en">Indirect Evaporative Cooling Tower or Coil Cooler</rdfs:label>
        <rdfs:label xml:lang="es">Torre de Enfriamiento Evaporativo Indirecto o Enfriador de Serpentín</rdfs:label>
    </owl:Class>
    


    <!-- https://w3id.org/mep#IndirectEvaporativePackageAirCooler -->


    <owl:Class rdf:about="https://w3id.org/mep#IndirectEvaporativePackageAirCooler">
        <rdfs:subClassOf rdf:resource="https://w3id.org/mep#EvaporativeCooler"/>
        <rdfs:comment xml:lang="es">Enfriador de aire por evaporación indirecta: enfría la corriente de aire evaporando el agua indirectamente y sin agregar humedad a la corriente de aire. En un lado del intercambiador de calor, la corriente de aire secundaria se enfría mediante evaporación, mientras que en el otro lado del intercambiador de calor, la corriente de aire primaria (aire acondicionado que se suministrará a la habitación) se enfría sensiblemente mediante las superficies del intercambiador de calor.</rdfs:comment>
        <rdfs:comment xml:lang="en">Indirect evaporative package air cooler: Cools the air stream by evaporating water indirectly and without adding moisture into the air stream. On one side of the heat exchanger, the secondary air stream is cooled by evaporation, while on the other side of heat exchanger, the primary air stream (conditioned air to be supplied to the room) is sensibly cooled by the heat exchanger surfaces.</rdfs:comment>
        <rdfs:label xml:lang="es">Enfriador de Aire por Evaporación Indirecta</rdfs:label>
        <rdfs:label xml:lang="en">Indirect Evaporative Package Air Cooler</rdfs:label>
    </owl:Class>
    


    <!-- https://w3id.org/mep#IndirectEvaporativeWetCoil -->


    <owl:Class rdf:about="https://w3id.org/mep#IndirectEvaporativeWetCoil">
        <rdfs:subClassOf rdf:resource="https://w3id.org/mep#EvaporativeCooler"/>
        <rdfs:comment xml:lang="en">Indirect evaporative wet coil: Cools the air stream by evaporating water indirectly and without adding moisture into the air stream. Water is sprayed directly on the tubes of the heat exchanger where latent cooling takes place and the vaporization of the water on the outside of the heat exchanger tubes allows the simultaneous heat and mass transfer which removes heat from the supply air on the tube side.</rdfs:comment>
        <rdfs:comment xml:lang="es">Serpentín húmedo de evaporación indirecta: enfría la corriente de aire evaporando el agua indirectamente y sin agregar humedad a la corriente de aire. El agua se rocía directamente sobre los tubos del intercambiador de calor donde tiene lugar el enfriamiento latente y la vaporización del agua en el exterior de los tubos del intercambiador de calor permite la transferencia simultánea de calor y masa que elimina el calor del aire de suministro en el lado del tubo.</rdfs:comment>
        <rdfs:label xml:lang="en">Indirect Evaporative Wet Coil</rdfs:label>
        <rdfs:label xml:lang="es">Serpentín Húmedo de Evaporación Indirecta</rdfs:label>
    </owl:Class>
    


    <!-- https://w3id.org/mep#InductionMotor -->


    <owl:Class rdf:about="https://w3id.org/mep#InductionMotor">
        <rdfs:subClassOf rdf:resource="https://w3id.org/mep#ElectricMotor"/>
        <rdfs:comment xml:lang="en">An alternating current motor in which the primary winding on one member (usually the stator) is connected to the power source and a secondary winding or a squirrel-cage secondary winding on the other member (usually the rotor) carries the induced current. There is no physical electrical connection to the secondary winding, its current is induced.</rdfs:comment>
        <rdfs:comment xml:lang="es">Un motor de corriente alterna en el que el devanado primario de un miembro (generalmente el estator) está conectado a la fuente de energía y un devanado secundario o un devanado secundario de jaula de ardilla en el otro miembro (generalmente el rotor) transporta la corriente inducida. No existe una conexión eléctrica física con el devanado secundario, su corriente es inducida.</rdfs:comment>
        <rdfs:label xml:lang="en">Induction Motor</rdfs:label>
        <rdfs:label xml:lang="es">Motor de Induccion</rdfs:label>
    </owl:Class>
    


    <!-- https://w3id.org/mep#Inductor -->


    <owl:Class rdf:about="https://w3id.org/mep#Inductor">
        <rdfs:subClassOf rdf:resource="https://w3id.org/mep#ElectricFlowStorageDevice"/>
        <rdfs:comment xml:lang="en">A device used in circuits or power systems due to their inductance, acting as a component of electric storage device.</rdfs:comment>
        <rdfs:comment xml:lang="es">Dispositivo utilizado en circuitos o sistemas de potencia debido a su inductancia, que actúa como componente de un dispositivo de almacenamiento eléctrico.</rdfs:comment>
        <rdfs:label xml:lang="en">Inductor</rdfs:label>
        <rdfs:label xml:lang="es">Inductor</rdfs:label>
    </owl:Class>
    


    <!-- https://w3id.org/mep#InductorBank -->


    <owl:Class rdf:about="https://w3id.org/mep#InductorBank">
        <rdfs:subClassOf rdf:resource="https://w3id.org/mep#ElectricFlowStorageDevice"/>
        <rdfs:comment xml:lang="en">A device that stores electrical energy in a magnetic field using electrical property of inductance.</rdfs:comment>
        <rdfs:comment xml:lang="es">Dispositivo que almacena energía eléctrica en un campo magnético utilizando la propiedad eléctrica de la inductancia.</rdfs:comment>
        <rdfs:label xml:lang="es">Bateria de Inductores</rdfs:label>
        <rdfs:label xml:lang="en">Inductor Bank</rdfs:label>
    </owl:Class>
    


    <!-- https://w3id.org/mep#InspectionChamber -->


    <owl:Class rdf:about="https://w3id.org/mep#InspectionChamber">
        <rdfs:subClassOf rdf:resource="https://w3id.org/mep#DistributionChamberElement"/>
        <rdfs:comment xml:lang="en">Chamber constructed on a drain, sewer or pipeline with a removable cover that permits visible inspection.</rdfs:comment>
        <rdfs:comment xml:lang="es">Cámara construida en un desagüe, alcantarilla o tubería con una tapa desmontable que permite la inspección visible.</rdfs:comment>
        <rdfs:label xml:lang="es">Camara de Inspeccion</rdfs:label>
        <rdfs:label xml:lang="en">Inspection Chamber</rdfs:label>
    </owl:Class>
    


    <!-- https://w3id.org/mep#InspectionPit -->


    <owl:Class rdf:about="https://w3id.org/mep#InspectionPit">
        <rdfs:subClassOf rdf:resource="https://w3id.org/mep#DistributionChamberElement"/>
        <rdfs:comment xml:lang="es">Rebaje o cámara formada para permitir el acceso para la inspección de la subestructura y los servicios.</rdfs:comment>
        <rdfs:comment xml:lang="en">Recess or chamber formed to permit access for inspection of substructure and services.</rdfs:comment>
        <rdfs:label xml:lang="es">Foso de Inspeccion</rdfs:label>
        <rdfs:label xml:lang="en">Inspection Pit</rdfs:label>
    </owl:Class>
    


    <!-- https://w3id.org/mep#IntelligentPeripheral -->


    <owl:Class rdf:about="https://w3id.org/mep#IntelligentPeripheral">
        <rdfs:subClassOf rdf:resource="https://w3id.org/mep#CommunicationsAppliance"/>
        <rdfs:comment xml:lang="en">An intelligent peripheral is a device that offers a variety of specialized resources according to the corresponding service logical program under the control of SCP. These resources contain the receiver of DTMF (Dual-Tone Multi-Frequency, signal generator, record notice, etc.). An intelligent peripheral provides dedicated resource functions in the intelligent network, allocates, controls and manages various dedicated resources, communicates with other entities in the network, and completes SRF resource functions as well as the maintenance, management and statistics functions of resources.</rdfs:comment>
        <rdfs:comment xml:lang="es">Un periférico inteligente es un dispositivo que ofrece una variedad de recursos especializados según el programa lógico de servicio correspondiente bajo el control de SCP. Estos recursos contienen el receptor de DTMF (multifrecuencia de doble tono, generador de señales, aviso de grabación, etc.). Un periférico inteligente ofrece funciones de recursos especializados en la red inteligente, asigna, controla y gestiona diversos recursos especializados, se comunica con otras entidades de la red y completa las funciones de recursos SRF, así como las funciones de mantenimiento, gestión y estadísticas de los recursos.</rdfs:comment>
        <rdfs:label xml:lang="en">Intelligent Peripheral</rdfs:label>
        <rdfs:label xml:lang="es">Periférico Inteligente</rdfs:label>
    </owl:Class>
    


    <!-- https://w3id.org/mep#Interceptor -->


    <owl:Class rdf:about="https://w3id.org/mep#Interceptor">
        <rdfs:subClassOf rdf:resource="https://w3id.org/mep#FlowTreatmentDevice"/>
        <rdfs:comment xml:lang="en">An interceptor is a device designed and installed in order to separate and retain deleterious, hazardous or undesirable matter while permitting normal sewage or liquids to discharge into a collection system by gravity.</rdfs:comment>
        <rdfs:comment xml:lang="es">Un interceptor es un dispositivo diseñado e instalado para separar y retener materias nocivas, peligrosas o indeseables mientras permite que las aguas residuales o líquidos normales se descarguen en un sistema de recolección por gravedad.</rdfs:comment>
        <rdfs:label xml:lang="en">Interceptor</rdfs:label>
        <rdfs:label xml:lang="es">Interceptor</rdfs:label>
    </owl:Class>
    


    <!-- https://w3id.org/mep#InternalCombustionMotor -->


    <owl:Class rdf:about="https://w3id.org/mep#InternalCombustionMotor">
        <rdfs:subClassOf rdf:resource="https://w3id.org/mep#Engine"/>
        <rdfs:comment xml:lang="en">Combusiton is internal.</rdfs:comment>
        <rdfs:comment xml:lang="es">La combustión es interna</rdfs:comment>
        <rdfs:label xml:lang="en">Internal Combustion Motor</rdfs:label>
        <rdfs:label xml:lang="es">Motor de Combustion Interna</rdfs:label>
    </owl:Class>
    


    <!-- https://w3id.org/mep#Inverter -->


    <owl:Class rdf:about="https://w3id.org/mep#Inverter">
        <rdfs:subClassOf rdf:resource="https://w3id.org/mep#Transformer"/>
        <rdfs:comment xml:lang="en">A transformer that converts from direct current (DC) to alternating current (AC).</rdfs:comment>
        <rdfs:comment xml:lang="es">Un conversor que convierte de corriente continua (DC) a corriente alterna (AC).</rdfs:comment>
        <rdfs:label xml:lang="es">Inversor</rdfs:label>
        <rdfs:label xml:lang="en">Inverter</rdfs:label>
    </owl:Class>
    


    <!-- https://w3id.org/mep#IonConcentrationSensor -->


    <owl:Class rdf:about="https://w3id.org/mep#IonConcentrationSensor">
        <rdfs:subClassOf rdf:resource="https://w3id.org/mep#Sensor"/>
        <rdfs:comment xml:lang="en">A device that senses or detects ion concentration, such as for water hardness.</rdfs:comment>
        <rdfs:comment xml:lang="es">Dispositivo que detecta la concentración de iones, por ejemplo, para determinar la dureza del agua.</rdfs:comment>
        <rdfs:label xml:lang="en">Ion Concentration Sensor</rdfs:label>
        <rdfs:label xml:lang="es">Sensor de Concentracion de Iones</rdfs:label>
    </owl:Class>
    


    <!-- https://w3id.org/mep#IsolatingValve -->


    <owl:Class rdf:about="https://w3id.org/mep#IsolatingValve">
        <rdfs:subClassOf rdf:resource="https://w3id.org/mep#Valve"/>
        <rdfs:comment xml:lang="en">Valve that closes off flow in a pipeline.</rdfs:comment>
        <rdfs:comment xml:lang="es">Válvula que cierra el flujo en una tubería.</rdfs:comment>
        <rdfs:label xml:lang="en">Isolating Valve</rdfs:label>
        <rdfs:label xml:lang="es">Valvula de Aislamiento</rdfs:label>
    </owl:Class>
    


    <!-- https://w3id.org/mep#JunctionBox -->


    <owl:Class rdf:about="https://w3id.org/mep#JunctionBox">
        <rdfs:subClassOf rdf:resource="https://w3id.org/mep#FlowFitting"/>
        <rdfs:comment xml:lang="en">A junction box is an enclosure within which cables are connected. Cables may be members of an electrical circuit (for electrical power systems) or be information carriers (in a telecommunications system). A junction box is typically intended to conceal a cable junction from sight, eliminate tampering or provide a safe place for electrical connection.</rdfs:comment>
        <rdfs:comment xml:lang="es">Una caja de conexiones es un recinto dentro del cual se conectan los cables. Los cables pueden ser miembros de un circuito eléctrico (para sistemas de energía eléctrica) o ser portadores de información (en un sistema de telecomunicaciones). Por lo general, una caja de conexiones está destinada a ocultar la unión de un cable a la vista, eliminar la manipulación o proporcionar un lugar seguro para la conexión eléctrica.</rdfs:comment>
        <rdfs:label xml:lang="es">Caja de Conexiones</rdfs:label>
        <rdfs:label xml:lang="en">Junction Box</rdfs:label>
    </owl:Class>
    


    <!-- https://w3id.org/mep#Keypad -->


    <owl:Class rdf:about="https://w3id.org/mep#Keypad">
        <rdfs:subClassOf rdf:resource="https://w3id.org/mep#SwitchingDevice"/>
        <rdfs:comment xml:lang="en">A set of buttons or switches, each potentially applicable to a different device.</rdfs:comment>
        <rdfs:comment xml:lang="es">Un conjunto de botones o interruptores, cada uno potencialmente aplicable a un dispositivo diferente.</rdfs:comment>
        <rdfs:label xml:lang="en">Keypad</rdfs:label>
        <rdfs:label xml:lang="es">Teclado</rdfs:label>
    </owl:Class>
    


    <!-- https://w3id.org/mep#KitchenMachine -->


    <owl:Class rdf:about="https://w3id.org/mep#KitchenMachine">
        <rdfs:subClassOf rdf:resource="https://w3id.org/mep#ElectricAppliance"/>
        <rdfs:comment xml:lang="en">A specialized appliance used in commercial kitchens such as a mixer.</rdfs:comment>
        <rdfs:comment xml:lang="es">Aparato especializado utilizado en cocinas comerciales, como una batidora.</rdfs:comment>
        <rdfs:label xml:lang="es">Aparato de Cocina</rdfs:label>
        <rdfs:label xml:lang="en">Kitchen Machine</rdfs:label>
    </owl:Class>
    


    <!-- https://w3id.org/mep#LEDLamp -->


    <owl:Class rdf:about="https://w3id.org/mep#LEDLamp">
        <rdfs:subClassOf rdf:resource="https://w3id.org/mep#Lamp"/>
        <rdfs:comment xml:lang="en">A solid state lamp that uses light-emitting diodes as the source of light.</rdfs:comment>
        <rdfs:comment xml:lang="es">Lámpara de estado sólido que utiliza diodos emisores de luz como fuente de luz.</rdfs:comment>
        <rdfs:label xml:lang="en">LED Lamp</rdfs:label>
        <rdfs:label xml:lang="es">Lampara LED</rdfs:label>
    </owl:Class>
    


    <!-- https://w3id.org/mep#Lamp -->


    <owl:Class rdf:about="https://w3id.org/mep#Lamp">
        <rdfs:subClassOf rdf:resource="https://w3id.org/mep#FlowTerminal"/>
        <rdfs:comment xml:lang="en">A lamp that emits light by passing an electrical current through a tungsten wire filament in a near vacuum.</rdfs:comment>
        <rdfs:comment xml:lang="es">Lámpara que emite luz al hacer pasar una corriente eléctrica a través de un filamento de alambre de tungsteno casi en el vacío.</rdfs:comment>
        <rdfs:label xml:lang="en">Lamp</rdfs:label>
        <rdfs:label xml:lang="es">Lampara</rdfs:label>
    </owl:Class>
    


    <!-- https://w3id.org/mep#LevelSensor -->


    <owl:Class rdf:about="https://w3id.org/mep#LevelSensor">
        <rdfs:subClassOf rdf:resource="https://w3id.org/mep#Sensor"/>
        <rdfs:comment xml:lang="en">A device that senses or detects fill level, such as for a tank.</rdfs:comment>
        <rdfs:comment xml:lang="es">Dispositivo que detecta el nivel de llenado de un depósito.</rdfs:comment>
        <rdfs:label xml:lang="en">Level Sensor</rdfs:label>
        <rdfs:label xml:lang="es">Sensor de Llenado</rdfs:label>
    </owl:Class>
    


    <!-- https://w3id.org/mep#Light -->


    <owl:Class rdf:about="https://w3id.org/mep#Light">
        <rdfs:subClassOf rdf:resource="https://w3id.org/mep#Alarm"/>
        <rdfs:comment xml:lang="en">A visual alarm.</rdfs:comment>
        <rdfs:comment xml:lang="es">Una alarma visual.</rdfs:comment>
        <rdfs:label xml:lang="en">Light</rdfs:label>
        <rdfs:label xml:lang="es">Luz</rdfs:label>
    </owl:Class>
    


    <!-- https://w3id.org/mep#LightFixture -->


    <owl:Class rdf:about="https://w3id.org/mep#LightFixture">
        <rdfs:subClassOf rdf:resource="https://w3id.org/mep#FlowTerminal"/>
        <rdfs:comment xml:lang="en">A light fixture is a container that is designed for the purpose of housing one or more lamps and optionally devices that control, restrict or vary their emission.</rdfs:comment>
        <rdfs:comment xml:lang="es">Un artefacto de iluminación es un contenedor que está diseñado con el propósito de albergar una o más lámparas y opcionalmente dispositivos que controlen, restrinjan o varíen su emisión.</rdfs:comment>
        <rdfs:label xml:lang="es">Artefacto de Iluminacion</rdfs:label>
        <rdfs:label xml:lang="en">LightFixture</rdfs:label>
    </owl:Class>
    


    <!-- https://w3id.org/mep#LightSensor -->


    <owl:Class rdf:about="https://w3id.org/mep#LightSensor">
        <rdfs:subClassOf rdf:resource="https://w3id.org/mep#Sensor"/>
        <rdfs:comment xml:lang="en">A device that senses or detects light.</rdfs:comment>
        <rdfs:comment xml:lang="es">Dispositivo que detecta la luz.</rdfs:comment>
        <rdfs:label xml:lang="en">Light Sensor</rdfs:label>
        <rdfs:label xml:lang="es">Sensor Lumínico</rdfs:label>
    </owl:Class>
    


    <!-- https://w3id.org/mep#LinesideElectronicUnit -->


    <owl:Class rdf:about="https://w3id.org/mep#LinesideElectronicUnit">
        <rdfs:subClassOf rdf:resource="https://w3id.org/mep#CommunicationsAppliance"/>
        <rdfs:comment xml:lang="es">La unidad electrónica de tierra (LEU) es la interfaz entre la baliza y el enclavamiento ferroviario. La LEU adquiere la información del enclavamiento y envía la información adecuada a las balizas en concordancia con la señalización en tierra (si existe).</rdfs:comment>
        <rdfs:comment xml:lang="en">The lineside electronic unit (LEU) is the interface between the balise and interlocking in railway. The LEU acquires the information from the interlocking, and sends the appropriate information to the balises in concordance with the lineside signalling (if available).</rdfs:comment>
        <rdfs:label xml:lang="en">Lineside Electronic Unit </rdfs:label>
        <rdfs:label xml:lang="es">Unidad Electronica de Tierra</rdfs:label>
    </owl:Class>
    


    <!-- https://w3id.org/mep#LiquidTerminal -->


    <owl:Class rdf:about="https://w3id.org/mep#LiquidTerminal">
        <rdfs:subClassOf rdf:resource="https://w3id.org/mep#FlowTerminal"/>
        <rdfs:comment xml:lang="en">A liquid terminal is a terminating or origination point for the transfer of liquid between distribution system(s). this is the point where the liquid distribution system interacts with the external environment. An example of this is a loading arm for the transfer of liquid from a docked vessel.</rdfs:comment>
        <rdfs:comment xml:lang="es">Una terminal de líquidos es un punto de terminación o de origen para la transferencia de líquido entre sistemas de distribución. este es el punto donde el sistema de distribución de líquido interactúa con el entorno externo. Un ejemplo de esto es un brazo de carga para la transferencia de líquido desde un buque atracado.</rdfs:comment>
        <rdfs:label xml:lang="en">Liquid Terminal</rdfs:label>
        <rdfs:label xml:lang="es">Terminal de Liquidos</rdfs:label>
    </owl:Class>
    


    <!-- https://w3id.org/mep#LoadingArm -->


    <owl:Class rdf:about="https://w3id.org/mep#LoadingArm">
        <rdfs:subClassOf rdf:resource="https://w3id.org/mep#LiquidTerminal"/>
        <rdfs:comment xml:lang="en">A loading arm permits the transfer of liquid or liquefied gas from one system to another, through the use of an articulated arm that accounts for the movement of docked vessels.</rdfs:comment>
        <rdfs:comment xml:lang="es">Un brazo de carga permite la transferencia de líquido o gas licuado de un sistema a otro, mediante el uso de un brazo articulado que da cuenta del movimiento de las embarcaciones atracadas.</rdfs:comment>
        <rdfs:label xml:lang="en">Loading Arm</rdfs:label>
        <rdfs:label xml:lang="es">brazo de Carga</rdfs:label>
    </owl:Class>
    


    <!-- https://w3id.org/mep#Louvre -->


    <owl:Class rdf:about="https://w3id.org/mep#Louvre">
        <rdfs:subClassOf rdf:resource="https://w3id.org/mep#AirTerminal"/>
        <rdfs:comment xml:lang="en">A rectilinear louvre.</rdfs:comment>
        <rdfs:comment xml:lang="es">Una lumbrera rectilínea.</rdfs:comment>
        <rdfs:label xml:lang="en">Louvre</rdfs:label>
        <rdfs:label xml:lang="es">Lumbrera</rdfs:label>
    </owl:Class>
    


    <!-- https://w3id.org/mep#MSCServer -->


    <owl:Class rdf:about="https://w3id.org/mep#MSCServer">
        <rdfs:subClassOf rdf:resource="https://w3id.org/mep#MobileTelecommunicationsAppliance"/>
        <rdfs:comment xml:lang="es">El servidor MSC comprende principalmente las partes de control de llamadas (CC) y control de movilidad de un centro de conmutación móvil (MSC). Un servidor MSC y una pasarela de medios conforman la funcionalidad completa de un MSC</rdfs:comment>
        <rdfs:comment xml:lang="en">The MSC server mainly comprises the call control (CC) and mobility control parts of a mobile switching center (MSC). An MSC server and a media gateway make up the full functionality of an MSC</rdfs:comment>
        <rdfs:label xml:lang="en">MSC Server</rdfs:label>
        <rdfs:label xml:lang="es">Servidor MSC</rdfs:label>
    </owl:Class>
    


    <!-- https://w3id.org/mep#Manhole -->


    <owl:Class rdf:about="https://w3id.org/mep#Manhole">
        <rdfs:subClassOf rdf:resource="https://w3id.org/mep#DistributionChamberElement"/>
        <rdfs:comment xml:lang="en">Chamber constructed on a drain, sewer or pipeline with a removable cover that permits the entry of a person.</rdfs:comment>
        <rdfs:comment xml:lang="es">Cámara construida en un desagüe, alcantarilla o tubería con una tapa desmontable que permite la entrada de una persona.</rdfs:comment>
        <rdfs:label xml:lang="es">Arqueta</rdfs:label>
        <rdfs:label xml:lang="en">Manhole</rdfs:label>
    </owl:Class>
    


    <!-- https://w3id.org/mep#ManualPullBox -->


    <owl:Class rdf:about="https://w3id.org/mep#ManualPullBox">
        <rdfs:subClassOf rdf:resource="https://w3id.org/mep#Alarm"/>
        <rdfs:comment xml:lang="en">An alarm activation mechanism in which activation is achieved by a pulling action.</rdfs:comment>
        <rdfs:comment xml:lang="es">Un mecanismo de activación de alarma en el que la activación se logra mediante una acción de tracción.</rdfs:comment>
        <rdfs:label xml:lang="es">Caja de Extracción Manual</rdfs:label>
        <rdfs:label xml:lang="en">Manual Pull Box</rdfs:label>
    </owl:Class>
    


    <!-- https://w3id.org/mep#MasterUnit -->


    <owl:Class rdf:about="https://w3id.org/mep#MasterUnit">
        <rdfs:subClassOf rdf:resource="https://w3id.org/mep#MobileTelecommunicationsAppliance"/>
        <rdfs:comment xml:lang="en">A master unit is a component of a repeater for coupling base station signals.</rdfs:comment>
        <rdfs:comment xml:lang="es">Una unidad maestra es un componente de un repetidor para acoplar señales de estación base.</rdfs:comment>
        <rdfs:label xml:lang="en">Master Unit</rdfs:label>
        <rdfs:label xml:lang="es">Unidad Maestra</rdfs:label>
    </owl:Class>
    


    <!-- https://w3id.org/mep#MechanicalForcedDraftCoolingTower -->


    <owl:Class rdf:about="https://w3id.org/mep#MechanicalForcedDraftCoolingTower">
        <rdfs:subClassOf rdf:resource="https://w3id.org/mep#CoolingTower"/>
        <rdfs:comment xml:lang="en">Air flow is produced by a mechanical device, typically one or more fans, located on the inlet air side of the cooling tower.</rdfs:comment>
        <rdfs:comment xml:lang="es">El flujo de aire es producido por un dispositivo mecánico, normalmente uno o más ventiladores, situado en el lado de entrada de aire de la torre de refrigeración.</rdfs:comment>
        <rdfs:label xml:lang="en">Mechanical Forced Draft Cooling Tower</rdfs:label>
        <rdfs:label xml:lang="es">Torre de Enfriamiento Mecanica de Tiro Forzado</rdfs:label>
    </owl:Class>
    


    <!-- https://w3id.org/mep#MechanicalInducedDraftCoolingTower -->


    <owl:Class rdf:about="https://w3id.org/mep#MechanicalInducedDraftCoolingTower">
        <rdfs:subClassOf rdf:resource="https://w3id.org/mep#CoolingTower"/>
        <rdfs:comment xml:lang="en">Air flow is produced by a mechanical device, typically one or more fans, located on the air outlet side of the cooling tower.</rdfs:comment>
        <rdfs:comment xml:lang="es">El flujo de aire es producido por un dispositivo mecánico, normalmente uno o más ventiladores, situado en el lado de salida de aire de la torre de refrigeración.</rdfs:comment>
        <rdfs:label xml:lang="en">Mechanical Induced Draft Cooling Tower</rdfs:label>
        <rdfs:label xml:lang="es">Torre de Enfriamiento Mecanica de Tiro Inducido</rdfs:label>
    </owl:Class>
    


    <!-- https://w3id.org/mep#MedicalDevice -->


    <owl:Class rdf:about="https://w3id.org/mep#MedicalDevice">
        <rdfs:subClassOf rdf:resource="https://w3id.org/mep#FlowTerminal"/>
        <rdfs:comment xml:lang="en">A medical device is attached to a medical piping system and operates upon medical gases to perform a specific function. Medical gases include medical air, medical vacuum, oxygen, carbon dioxide, nitrogen, and nitrous oxide.</rdfs:comment>
        <rdfs:comment xml:lang="es">Un dispositivo médico está conectado a un sistema de tuberías médicas y funciona con gases médicos para realizar una función específica. Los gases medicinales incluyen aire medicinal, vacío medicinal, oxígeno, dióxido de carbono, nitrógeno y óxido nitroso.</rdfs:comment>
        <rdfs:label xml:lang="es">Dispositivo Medico</rdfs:label>
        <rdfs:label xml:lang="en">Medical Device</rdfs:label>
    </owl:Class>
    


    <!-- https://w3id.org/mep#MetalHalideLamp -->


    <owl:Class rdf:about="https://w3id.org/mep#MetalHalideLamp">
        <rdfs:subClassOf rdf:resource="https://w3id.org/mep#Lamp"/>
        <rdfs:comment xml:lang="en">A discharge lamp in which most of the light is emitted by exciting a metal halide.</rdfs:comment>
        <rdfs:comment xml:lang="es">Lámpara de descarga en la que la mayor parte de la luz se emite excitando un haluro metálico.</rdfs:comment>
        <rdfs:label xml:lang="es">Lampara de Halogenuros Metalicos</rdfs:label>
        <rdfs:label xml:lang="en">Metal Halide Lamp</rdfs:label>
    </owl:Class>
    


    <!-- https://w3id.org/mep#MeterChamber -->


    <owl:Class rdf:about="https://w3id.org/mep#MeterChamber">
        <rdfs:subClassOf rdf:resource="https://w3id.org/mep#DistributionChamberElement"/>
        <rdfs:comment xml:lang="en">Chamber that houses a meter(s).</rdfs:comment>
        <rdfs:comment xml:lang="es">Cámara que aloja un contador o contadores.</rdfs:comment>
        <rdfs:label xml:lang="es">Camara de Contadores</rdfs:label>
        <rdfs:label xml:lang="en">Meter Chamber</rdfs:label>
    </owl:Class>
    


    <!-- https://w3id.org/mep#Microphone -->


    <owl:Class rdf:about="https://w3id.org/mep#Microphone">
        <rdfs:subClassOf rdf:resource="https://w3id.org/mep#AudioVisualAppliance"/>
        <rdfs:comment xml:lang="en">An acoustic-to-electric transducer or sensor that converts sound into an electrical signal. Microphones types in use include electromagnetic induction (dynamic microphones), capacitance change (condenser microphones) or piezoelectric generation to produce the signal from mechanical vibration.</rdfs:comment>
        <rdfs:comment xml:lang="es">Un transductor o sensor acústico a eléctrico que convierte el sonido en una señal eléctrica. Los tipos de micrófonos en uso incluyen inducción electromagnética (micrófonos dinámicos), cambio de capacitancia (micrófonos de condensador) o generación piezoeléctrica para producir la señal a partir de vibración mecánica.</rdfs:comment>
        <rdfs:label xml:lang="es">Microfono</rdfs:label>
        <rdfs:label xml:lang="en">Microphone</rdfs:label>
    </owl:Class>
    


    <!-- https://w3id.org/mep#Microwave -->


    <owl:Class rdf:about="https://w3id.org/mep#Microwave">
        <rdfs:subClassOf rdf:resource="https://w3id.org/mep#ElectricAppliance"/>
        <rdfs:comment xml:lang="en">An electrical appliance that has the primary function of cooking food using microwaves.</rdfs:comment>
        <rdfs:comment xml:lang="es">Aparato eléctrico cuya función principal es cocinar alimentos mediante microondas.</rdfs:comment>
        <rdfs:label xml:lang="es">Microondas</rdfs:label>
        <rdfs:label xml:lang="en">Microwave</rdfs:label>
    </owl:Class>
    


    <!-- https://w3id.org/mep#MimicPanel -->


    <owl:Class rdf:about="https://w3id.org/mep#MimicPanel">
        <rdfs:subClassOf rdf:resource="https://w3id.org/mep#UnitaryControlElement"/>
        <rdfs:comment xml:lang="en">A control element at which information that is available elsewhere is repeated or &apos;mimicked&apos;.</rdfs:comment>
        <rdfs:comment xml:lang="es">Un panel mímico es un elemento de control en el que se repite o &apos;imita&apos; información que está disponible en otros lugares.</rdfs:comment>
        <rdfs:label xml:lang="en">Mimic Panel</rdfs:label>
        <rdfs:label xml:lang="es">Panel de Imitación</rdfs:label>
    </owl:Class>
    


    <!-- https://w3id.org/mep#MixedSignalingDevice -->


    <owl:Class rdf:about="https://w3id.org/mep#MixedSignalingDevice">
        <rdfs:subClassOf rdf:resource="https://w3id.org/mep#Signal"/>
        <rdfs:comment xml:lang="en">A signal type formed of an active device conveying information in both a visual and audio manner.</rdfs:comment>
        <rdfs:comment xml:lang="es">Tipo de señal formada por un dispositivo activo que transmite información de forma visual y sonora.</rdfs:comment>
        <rdfs:label xml:lang="es">Dispositivo de señalización mixto</rdfs:label>
        <rdfs:label xml:lang="en">Mixed Signaling Device</rdfs:label>
    </owl:Class>
    


    <!-- https://w3id.org/mep#MixingValve -->


    <owl:Class rdf:about="https://w3id.org/mep#MixingValve">
        <rdfs:subClassOf rdf:resource="https://w3id.org/mep#Valve"/>
        <rdfs:comment xml:lang="en">Valve that enables flow from two branches of a pipeline to be mixed together (3 port).</rdfs:comment>
        <rdfs:comment xml:lang="es">Válvula que permite mezclar el flujo de dos ramales de una tubería (3 puertos).</rdfs:comment>
        <rdfs:label xml:lang="en">Mixing Valve</rdfs:label>
        <rdfs:label xml:lang="es">Valvula Mezcladora</rdfs:label>
    </owl:Class>
    


    <!-- https://w3id.org/mep#MobileSwitchingCenter -->


    <owl:Class rdf:about="https://w3id.org/mep#MobileSwitchingCenter">
        <rdfs:subClassOf rdf:resource="https://w3id.org/mep#MobileTelecommunicationsAppliance"/>
        <rdfs:comment xml:lang="es">El centro de conmutación móvil (MSC) constituye la interfaz entre el sistema radioeléctrico y las redes fijas. Es una central que realiza todas las funciones de conmutación y señalización para las estaciones móviles situadas en una zona geográfica designada como zona MSC. Consta de un servidor MSC y una pasarela de medios.</rdfs:comment>
        <rdfs:comment xml:lang="en">The mobile switching centre (MSC) constitutes the interface between the radio system and the fixed networks. It is an exchange which performs all the switching and signalling functions for mobile station located in a geographical area designated as the MSC area. It consists of a MSC server and a media gateway.</rdfs:comment>
        <rdfs:label xml:lang="es">Centro de Conmutacion Movil</rdfs:label>
        <rdfs:label xml:lang="en">Mobile Switching Center</rdfs:label>
    </owl:Class>
    


    <!-- https://w3id.org/mep#MobileTelecommunicationsAppliance -->


    <owl:Class rdf:about="https://w3id.org/mep#MobileTelecommunicationsAppliance">
        <rdfs:subClassOf rdf:resource="https://w3id.org/mep#FlowTerminal"/>
        <rdfs:comment xml:lang="en">A mobile telecommunications appliance is a device that transmits, converts, amplifies or receives signals used in mobile networks. Note: This entity is used to define specific appliances used in mobile telecommunication networks.</rdfs:comment>
        <rdfs:comment xml:lang="es">Un aparato de telecomunicaciones móviles es un dispositivo que transmite, convierte, amplifica o recibe señales utilizadas en redes móviles. Nota: Esta entidad se utiliza para definir aparatos específicos utilizados en las redes de telecomunicaciones móviles.</rdfs:comment>
        <rdfs:label xml:lang="es">Aparato de Telecomunicaciones Moviles</rdfs:label>
        <rdfs:label xml:lang="en">MobileTelecommunicationsAppliance</rdfs:label>
    </owl:Class>
    


    <!-- https://w3id.org/mep#Modem -->


    <owl:Class rdf:about="https://w3id.org/mep#Modem">
        <rdfs:subClassOf rdf:resource="https://w3id.org/mep#CommunicationsAppliance"/>
        <rdfs:comment xml:lang="en">A modem (from modulator-demodulator) is a device that modulates an analog carrier signal to encode digital information, and also demodulates such a carrier signal to decode the transmitted information.</rdfs:comment>
        <rdfs:comment xml:lang="es">Un módem (de modulador-demodulador) es un dispositivo que modula una señal portadora analógica para codificar información digital, y también demodula dicha señal portadora para descodificar la información transmitida.</rdfs:comment>
        <rdfs:label xml:lang="en">Modem</rdfs:label>
        <rdfs:label xml:lang="es">Modem</rdfs:label>
    </owl:Class>
    


    <!-- https://w3id.org/mep#MomentarySwitch -->


    <owl:Class rdf:about="https://w3id.org/mep#MomentarySwitch">
        <rdfs:subClassOf rdf:resource="https://w3id.org/mep#SwitchingDevice"/>
        <rdfs:comment xml:lang="en">A momentary switch has no position, and may trigger some action to occur.</rdfs:comment>
        <rdfs:comment xml:lang="es">Un interruptor momentáneo no tiene posición y puede desencadenar alguna acción.</rdfs:comment>
        <rdfs:label xml:lang="es">Interruptor Momentaneo</rdfs:label>
        <rdfs:label xml:lang="en">Momentary Switch</rdfs:label>
    </owl:Class>
    


    <!-- https://w3id.org/mep#MotorConnection -->


    <owl:Class rdf:about="https://w3id.org/mep#MotorConnection">
        <rdfs:subClassOf rdf:resource="https://w3id.org/mep#EnergyConversionDevice"/>
        <rdfs:comment xml:lang="en">A motor connection provides the means for connecting a motor as the driving device to the driven device.</rdfs:comment>
        <rdfs:comment xml:lang="es">Una conexión de motor proporciona los medios para conectar un motor como dispositivo de accionamiento al dispositivo accionado.</rdfs:comment>
        <rdfs:label xml:lang="es">Conexion de Motor</rdfs:label>
        <rdfs:label xml:lang="en">Motor Connection</rdfs:label>
    </owl:Class>
    


    <!-- https://w3id.org/mep#MotorControlCentre -->


    <owl:Class rdf:about="https://w3id.org/mep#MotorControlCentre">
        <rdfs:subClassOf rdf:resource="https://w3id.org/mep#DistributionBoard"/>
        <rdfs:comment xml:lang="en">A distribution point at which starting and control devices for major plant items are located.</rdfs:comment>
        <rdfs:comment xml:lang="es">Un punto de distribución en el que se encuentran los dispositivos de arranque y control de los principales elementos de la planta.</rdfs:comment>
        <rdfs:label xml:lang="es">Centro de Control de Motores</rdfs:label>
        <rdfs:label xml:lang="en">Motor Control Centre</rdfs:label>
    </owl:Class>
    


    <!-- https://w3id.org/mep#MovementSensor -->


    <owl:Class rdf:about="https://w3id.org/mep#MovementSensor">
        <rdfs:subClassOf rdf:resource="https://w3id.org/mep#Sensor"/>
        <rdfs:comment xml:lang="en">A device that senses or detects movement.</rdfs:comment>
        <rdfs:comment xml:lang="es">Dispositivo que detecta el movimiento.</rdfs:comment>
        <rdfs:label xml:lang="en">Movement Sensor</rdfs:label>
        <rdfs:label xml:lang="es">Sensor de Movimiento</rdfs:label>
    </owl:Class>
    


    <!-- https://w3id.org/mep#MultipositionController -->


    <owl:Class rdf:about="https://w3id.org/mep#MultipositionController">
        <rdfs:subClassOf rdf:resource="https://w3id.org/mep#Controller"/>
        <rdfs:comment xml:lang="es">La salida es un valor discreto, puede ser uno de tres o más valores.</rdfs:comment>
        <rdfs:comment xml:lang="en">Output is discrete value, can be one of three or more values.</rdfs:comment>
        <rdfs:label xml:lang="es">Controlador Multiposicion</rdfs:label>
        <rdfs:label xml:lang="en">Multiposition Controller</rdfs:label>
    </owl:Class>
    


    <!-- https://w3id.org/mep#NaturalDraftCoolingTower -->


    <owl:Class rdf:about="https://w3id.org/mep#NaturalDraftCoolingTower">
        <rdfs:subClassOf rdf:resource="https://w3id.org/mep#CoolingTower"/>
        <rdfs:comment xml:lang="en">Air flow is produced naturally.</rdfs:comment>
        <rdfs:comment xml:lang="es">El flujo de aire se produce de forma natural.</rdfs:comment>
        <rdfs:label xml:lang="en">Natural Draft Cooling Tower</rdfs:label>
        <rdfs:label xml:lang="es">Torre de Enfriamiento de Tiro Natural</rdfs:label>
    </owl:Class>
    


    <!-- https://w3id.org/mep#NetworkAppliance -->


    <owl:Class rdf:about="https://w3id.org/mep#NetworkAppliance">
        <rdfs:subClassOf rdf:resource="https://w3id.org/mep#CommunicationsAppliance"/>
        <rdfs:comment xml:lang="en">A network appliance performs a dedicated function such as firewall protection, content filtering, load balancing, or equipment management.</rdfs:comment>
        <rdfs:comment xml:lang="es">Un dispositivo de red realiza una función específica, como la protección mediante cortafuegos, el filtrado de contenidos, el equilibrio de carga o la gestión de equipos.</rdfs:comment>
        <rdfs:label xml:lang="es">Dispositivo de Red</rdfs:label>
        <rdfs:label xml:lang="en">Network Appliance</rdfs:label>
    </owl:Class>
    


    <!-- https://w3id.org/mep#NetworkBridge -->


    <owl:Class rdf:about="https://w3id.org/mep#NetworkBridge">
        <rdfs:subClassOf rdf:resource="https://w3id.org/mep#CommunicationsAppliance"/>
        <rdfs:comment xml:lang="en">A network bridge connects multiple network segments at the data link layer (layer 2) of the OSI model, and the term layer 2 switch is very often used interchangeably with bridge.</rdfs:comment>
        <rdfs:comment xml:lang="es">Un puente de red conecta varios segmentos de red en la capa de enlace de datos (capa 2) del modelo OSI, y el término conmutador de capa 2 se utiliza muy a menudo indistintamente con puente.</rdfs:comment>
        <rdfs:label xml:lang="en">Network Bridge</rdfs:label>
        <rdfs:label xml:lang="es">Puente de Red</rdfs:label>
    </owl:Class>
    


    <!-- https://w3id.org/mep#NetworkHub -->


    <owl:Class rdf:about="https://w3id.org/mep#NetworkHub">
        <rdfs:subClassOf rdf:resource="https://w3id.org/mep#CommunicationsAppliance"/>
        <rdfs:comment xml:lang="en">A network hub connects multiple network segments at the physical layer (layer 1) of the OSI model.</rdfs:comment>
        <rdfs:comment xml:lang="es">Un hub de red conecta varios segmentos de red en la capa física (capa 1) del modelo OSI.</rdfs:comment>
        <rdfs:label xml:lang="es">Hub de Red</rdfs:label>
        <rdfs:label xml:lang="en">Network Hub</rdfs:label>
    </owl:Class>
    


    <!-- https://w3id.org/mep#OLEDLamp -->


    <owl:Class rdf:about="https://w3id.org/mep#OLEDLamp">
        <rdfs:subClassOf rdf:resource="https://w3id.org/mep#Lamp"/>
        <rdfs:comment xml:lang="en">A solid state lamp that uses light-emitting diodes as the source of light whose emissive electroluminescent layer is composed of a film of organic compounds.</rdfs:comment>
        <rdfs:comment xml:lang="es">Lámpara de estado sólido que utiliza diodos emisores de luz como fuente de luz cuya capa electroluminiscente emisiva está compuesta por una película de compuestos orgánicos.</rdfs:comment>
        <rdfs:label xml:lang="es">Lampara OLED</rdfs:label>
        <rdfs:label xml:lang="en">OLED Lamp</rdfs:label>
    </owl:Class>
    


    <!-- https://w3id.org/mep#ObstacleSensor -->


    <owl:Class rdf:about="https://w3id.org/mep#ObstacleSensor">
        <rdfs:subClassOf rdf:resource="https://w3id.org/mep#Sensor"/>
        <rdfs:comment xml:lang="en">A device that senses or detects any obstacles. Examples are: detectors sensing objects falling from a bridge, rock-fall detectors, etc.</rdfs:comment>
        <rdfs:comment xml:lang="es">Dispositivo que percibe o detecta cualquier obstáculo. Ejemplos: detectores de objetos que caen de un puente, detectores de caída de rocas, etc.</rdfs:comment>
        <rdfs:label xml:lang="en">Obstacle Sensor</rdfs:label>
        <rdfs:label xml:lang="es">Sensor de Obstaculos</rdfs:label>
    </owl:Class>
    


    <!-- https://w3id.org/mep#OdorFilter -->


    <owl:Class rdf:about="https://w3id.org/mep#OdorFilter">
        <rdfs:subClassOf rdf:resource="https://w3id.org/mep#Filter"/>
        <rdfs:comment xml:lang="en">A filter used to remove odors from air.</rdfs:comment>
        <rdfs:comment xml:lang="es">Un filtro utilizado para eliminar los olores del aire.</rdfs:comment>
        <rdfs:label xml:lang="es">Filtro de Olores</rdfs:label>
        <rdfs:label xml:lang="en">Odor Filter</rdfs:label>
    </owl:Class>
    


    <!-- https://w3id.org/mep#OilFilter -->


    <owl:Class rdf:about="https://w3id.org/mep#OilFilter">
        <rdfs:subClassOf rdf:resource="https://w3id.org/mep#Filter"/>
        <rdfs:comment xml:lang="en">A filter used to remove particulates from oil.</rdfs:comment>
        <rdfs:comment xml:lang="es">Un filtro utilizado para eliminar partículas del aceite.</rdfs:comment>
        <rdfs:label xml:lang="es">Filtro de Aceite</rdfs:label>
        <rdfs:label xml:lang="en">Oil Filter</rdfs:label>
    </owl:Class>
    


    <!-- https://w3id.org/mep#OilInterceptor -->


    <owl:Class rdf:about="https://w3id.org/mep#OilInterceptor">
        <rdfs:subClassOf rdf:resource="https://w3id.org/mep#Interceptor"/>
        <rdfs:comment xml:lang="en">One or more chambers arranged to prevent the ingress of oil to a drain or sewer that retains the oil for later removal.</rdfs:comment>
        <rdfs:comment xml:lang="es">Una o más cámaras dispuestas para impedir el ingreso de aceite a un desagüe o alcantarillado que retiene el aceite para su posterior eliminación.</rdfs:comment>
        <rdfs:label xml:lang="es">Interceptor de Aceite</rdfs:label>
        <rdfs:label xml:lang="en">Oil Interceptor</rdfs:label>
    </owl:Class>
    


    <!-- https://w3id.org/mep#OilMeter -->


    <owl:Class rdf:about="https://w3id.org/mep#OilMeter">
        <rdfs:subClassOf rdf:resource="https://w3id.org/mep#FlowMeter"/>
        <rdfs:comment xml:lang="en">A device that measures the quantity of oil.</rdfs:comment>
        <rdfs:comment xml:lang="es">Un dispositivo que mide la cantidad de aceite.</rdfs:comment>
        <rdfs:label xml:lang="es">Meididor de Aceie</rdfs:label>
        <rdfs:label xml:lang="en">Oil Meter</rdfs:label>
    </owl:Class>
    


    <!-- https://w3id.org/mep#OilRetentionTray -->


    <owl:Class rdf:about="https://w3id.org/mep#OilRetentionTray">
        <rdfs:subClassOf rdf:resource="https://w3id.org/mep#Tank"/>
        <rdfs:comment xml:lang="en">An open container for environmental protection and storage of chemical products.</rdfs:comment>
        <rdfs:comment xml:lang="es">Un contenedor abierto para la protección del medio ambiente y el almacenamiento de productos químicos.</rdfs:comment>
        <rdfs:label xml:lang="es">Bandeja de Retencion de Aceite</rdfs:label>
        <rdfs:label xml:lang="en">Oil Retention Tray</rdfs:label>
    </owl:Class>
    


    <!-- https://w3id.org/mep#OpenTypeCompressor -->


    <owl:Class rdf:about="https://w3id.org/mep#OpenTypeCompressor">
        <rdfs:subClassOf rdf:resource="https://w3id.org/mep#Compressor"/>
        <rdfs:comment xml:lang="es">Compresor alternativo de desplazamiento positivo en el que el eje se extiende a través de una junta en el cárter para un accionamiento externo.</rdfs:comment>
        <rdfs:comment xml:lang="en">Positive-displacement reciprocating compressor where the shaft extends through a seal in the crankcase for an external drive.</rdfs:comment>
        <rdfs:label xml:lang="es">Compresor de Tipo Abierto</rdfs:label>
        <rdfs:label xml:lang="en">Open Type Compressor</rdfs:label>
    </owl:Class>
    


    <!-- https://w3id.org/mep#OpticalCableSegment -->


    <owl:Class rdf:about="https://w3id.org/mep#OpticalCableSegment">
        <rdfs:subClassOf rdf:resource="https://w3id.org/mep#CableSegment"/>
        <rdfs:comment xml:lang="en">An optical cable segment is a cable segment that contains a variable number of optical fiber segments.</rdfs:comment>
        <rdfs:comment xml:lang="es">Un segmento de fibra es una fibra óptica individual utilizada en sistemas de telecomunicaciones para transmitir datos mediante señales ópticas.</rdfs:comment>
        <rdfs:label xml:lang="en">Optical Cable Segment</rdfs:label>
        <rdfs:label xml:lang="es">Segmento de Cable Optico</rdfs:label>
    </owl:Class>
    


    <!-- https://w3id.org/mep#OpticalLineTerminal -->


    <owl:Class rdf:about="https://w3id.org/mep#OpticalLineTerminal">
        <rdfs:subClassOf rdf:resource="https://w3id.org/mep#CommunicationsAppliance"/>
        <rdfs:comment xml:lang="en">An optical line terminal is a service provider endpoint of a passive or active optical network. It is the terminal equipment for connecting fiber optic trunks.</rdfs:comment>
        <rdfs:comment xml:lang="es">Un terminal de línea óptica es un punto final del proveedor de servicios de una red óptica pasiva o activa. Es el equipo terminal para conectar troncales de fibra óptica.</rdfs:comment>
        <rdfs:label xml:lang="en">Optical Line Terminal</rdfs:label>
        <rdfs:label xml:lang="es">terminal de línea óptica</rdfs:label>
    </owl:Class>
    


    <!-- https://w3id.org/mep#OpticalNetworkUnit -->


    <owl:Class rdf:about="https://w3id.org/mep#OpticalNetworkUnit">
        <rdfs:subClassOf rdf:resource="https://w3id.org/mep#CommunicationsAppliance"/>
        <rdfs:comment xml:lang="en">An optical network unit is a kind of optical transmission network connection equipment which is installed at user side.</rdfs:comment>
        <rdfs:comment xml:lang="es">Una unidad de red óptica es un tipo de equipo de conexión de red de transmisión óptica que se instala en el lado del usuario.</rdfs:comment>
        <rdfs:label xml:lang="en">Optical Network Unit</rdfs:label>
        <rdfs:label xml:lang="es">Unidad de Red Optica</rdfs:label>
    </owl:Class>
    


    <!-- https://w3id.org/mep#Outlet -->


    <owl:Class rdf:about="https://w3id.org/mep#Outlet">
        <rdfs:subClassOf rdf:resource="https://w3id.org/mep#FlowTerminal"/>
        <rdfs:comment xml:lang="en">An outlet is a device installed at a point to receive one or more inserted plugs for electrical power or communications. Power outlets are commonly connected within a junction box; data outlets may be directly connected to a wall. For power outlets sharing the same circuit within a junction box, the ports should indicate the logical wiring relationship to the enclosing junction box, even though they may be physically connected to a cable going to another outlet, switch, or fixture.</rdfs:comment>
        <rdfs:comment xml:lang="es">Una salida es un dispositivo instalado en un punto para recibir uno o varios enchufes insertados para alimentación eléctrica o comunicaciones. Las tomas de corriente suelen estar conectadas dentro de una caja de empalmes; las tomas de datos pueden estar conectadas directamente a una pared. En el caso de las tomas de corriente que comparten el mismo circuito dentro de una caja de empalmes, los puertos deben indicar la relación lógica del cableado con la caja de empalmes que las encierra, aunque puedan estar físicamente conectadas a un cable que vaya a otra toma, interruptor o aparato.</rdfs:comment>
        <rdfs:label xml:lang="en">Outlet</rdfs:label>
        <rdfs:label xml:lang="es">Salida</rdfs:label>
    </owl:Class>
    


    <!-- https://w3id.org/mep#OxygenGenerator -->


    <owl:Class rdf:about="https://w3id.org/mep#OxygenGenerator">
        <rdfs:subClassOf rdf:resource="https://w3id.org/mep#MedicalDevice"/>
        <rdfs:comment xml:lang="en">Device that generates oxygen from air.</rdfs:comment>
        <rdfs:comment xml:lang="es">Dispositivo que genera oxígeno a partir del aire.</rdfs:comment>
        <rdfs:label xml:lang="es">Generador de Oxigeno</rdfs:label>
        <rdfs:label xml:lang="en">Oxygen Generator</rdfs:label>
    </owl:Class>
    


    <!-- https://w3id.org/mep#OxygenPlant -->


    <owl:Class rdf:about="https://w3id.org/mep#OxygenPlant">
        <rdfs:subClassOf rdf:resource="https://w3id.org/mep#MedicalDevice"/>
        <rdfs:comment xml:lang="en">Device that combines a feed air unit, oxygen generator, and backup oxygen cylinders.</rdfs:comment>
        <rdfs:comment xml:lang="es">Dispositivo que combina una unidad de aire de alimentación, un generador de oxígeno y botellas de oxígeno de reserva.</rdfs:comment>
        <rdfs:label xml:lang="en">Oxygen Plant</rdfs:label>
        <rdfs:label xml:lang="es">Planta de Oxigeno</rdfs:label>
    </owl:Class>
    


    <!-- https://w3id.org/mep#PHSensor -->


    <owl:Class rdf:about="https://w3id.org/mep#PHSensor">
        <rdfs:subClassOf rdf:resource="https://w3id.org/mep#Sensor"/>
        <rdfs:comment xml:lang="en">A device that senses or detects acidity.</rdfs:comment>
        <rdfs:comment xml:lang="es">Dispositivo que detecta la acidez.</rdfs:comment>
        <rdfs:label xml:lang="en">PH Sensor</rdfs:label>
        <rdfs:label xml:lang="es">Sensor de PH</rdfs:label>
    </owl:Class>
    


    <!-- https://w3id.org/mep#PacketControlUnit -->


    <owl:Class rdf:about="https://w3id.org/mep#PacketControlUnit">
        <rdfs:subClassOf rdf:resource="https://w3id.org/mep#MobileTelecommunicationsAppliance"/>
        <rdfs:comment xml:lang="en">A packet control unit performs some of the processing tasks of the base station controller for packet data. It is responsible for data packet, wireless channel management, error sending detection and automatic retransmission.</rdfs:comment>
        <rdfs:comment xml:lang="es">Una unidad de control de paquetes realiza algunas de las tareas de procesamiento del controlador de la estación base para los paquetes de datos. Es responsable de los paquetes de datos, la gestión de canales inalámbricos, la detección de errores de envío y la retransmisión automática.</rdfs:comment>
        <rdfs:label xml:lang="en">Packet Control Unit</rdfs:label>
        <rdfs:label xml:lang="es">Unidad de Control de Paquetes</rdfs:label>
    </owl:Class>
    


    <!-- https://w3id.org/mep#PassiveCooledBeam -->


    <owl:Class rdf:about="https://w3id.org/mep#PassiveCooledBeam">
        <rdfs:subClassOf rdf:resource="https://w3id.org/mep#CooledBeam"/>
        <rdfs:comment xml:lang="en">A passive or static cooled beam provides cooling (and heating) to a room or zone.</rdfs:comment>
        <rdfs:comment xml:lang="es">Una viga de refrigeración pasiva o estática proporciona refrigeración (y calefacción) a una habitación o zona.</rdfs:comment>
        <rdfs:label xml:lang="en">Passive Cooled Beam</rdfs:label>
        <rdfs:label xml:lang="es">Viga Refrigerante Pasiva</rdfs:label>
    </owl:Class>
    


    <!-- https://w3id.org/mep#PetrolInterceptor -->


    <owl:Class rdf:about="https://w3id.org/mep#PetrolInterceptor">
        <rdfs:subClassOf rdf:resource="https://w3id.org/mep#Interceptor"/>
        <rdfs:comment xml:lang="es">Dos o más cámaras con tubos de entrada y salida dispuestos para permitir que la gasolina recogida en la superficie del agua drenada se evapore a través de tubos de ventilación.</rdfs:comment>
        <rdfs:comment xml:lang="en">Two or more chambers with inlet and outlet pipes arranged to allow petrol/gasoline collected on the surface of water drained into them to evaporate through ventilating pipes.</rdfs:comment>
        <rdfs:label xml:lang="es">Interceptor de Petroleo</rdfs:label>
        <rdfs:label xml:lang="en">Petrol Interceptor</rdfs:label>
    </owl:Class>
    


    <!-- https://w3id.org/mep#PhaseAngleMeter -->


    <owl:Class rdf:about="https://w3id.org/mep#PhaseAngleMeter">
        <rdfs:subClassOf rdf:resource="https://w3id.org/mep#FlowInstrument"/>
        <rdfs:comment xml:lang="en">A device that reads and displays the phase angle of a phase in a polyphase electrical circuit.</rdfs:comment>
        <rdfs:comment xml:lang="es">Dispositivo que lee y muestra el ángulo de fase de una fase en un circuito eléctrico polifásico.</rdfs:comment>
        <rdfs:label xml:lang="es">Medidor de Angulo de Fase</rdfs:label>
        <rdfs:label xml:lang="en">Phase Angle Meter</rdfs:label>
    </owl:Class>
    


    <!-- https://w3id.org/mep#Photocopier -->


    <owl:Class rdf:about="https://w3id.org/mep#Photocopier">
        <rdfs:subClassOf rdf:resource="https://w3id.org/mep#ElectricAppliance"/>
        <rdfs:comment xml:lang="en">A machine that has the primary function of reproduction of printed matter.</rdfs:comment>
        <rdfs:comment xml:lang="es">Máquina cuya función principal es la reproducción de material impreso.</rdfs:comment>
        <rdfs:label xml:lang="es">Fotocopiadora</rdfs:label>
        <rdfs:label xml:lang="en">Photocopier</rdfs:label>
    </owl:Class>
    


    <!-- https://w3id.org/mep#PipeBend -->


    <owl:Class rdf:about="https://w3id.org/mep#PipeBend">
        <rdfs:subClassOf rdf:resource="https://w3id.org/mep#PipeFitting"/>
        <rdfs:comment xml:lang="en">A fitting with typically two ports used to change the direction of flow between connected elements.</rdfs:comment>
        <rdfs:comment xml:lang="es">Accesorio con dos puertos que sirve para cambiar la dirección del flujo entre elementos conectados.</rdfs:comment>
        <rdfs:label xml:lang="es">Codo de Tuberia</rdfs:label>
        <rdfs:label xml:lang="en">Pipe Bend</rdfs:label>
    </owl:Class>
    


    <!-- https://w3id.org/mep#PipeConector -->


    <owl:Class rdf:about="https://w3id.org/mep#PipeConector">
        <rdfs:subClassOf rdf:resource="https://w3id.org/mep#PipeFitting"/>
        <rdfs:comment xml:lang="es">Accesorio de conexión, utilizado normalmente para unir dos puertos dentro de un sistema de distribución de flujo (por ejemplo, un acoplamiento utilizado para unir dos segmentos de tubería).</rdfs:comment>
        <rdfs:comment xml:lang="en">Connector fitting, typically used to join two ports together within a flow distribution system (e.g., a coupling used to join two pipe segments).</rdfs:comment>
        <rdfs:label xml:lang="es">Conector de Tuberia</rdfs:label>
        <rdfs:label xml:lang="en">Pipe Conector</rdfs:label>
    </owl:Class>
    


    <!-- https://w3id.org/mep#PipeEntry -->


    <owl:Class rdf:about="https://w3id.org/mep#PipeEntry">
        <rdfs:subClassOf rdf:resource="https://w3id.org/mep#PipeFitting"/>
        <rdfs:comment xml:lang="es">Accesorio de entrada, normalmente desconectado en un puerto y conectado a un sistema de distribución de flujo en el otro (por ejemplo, una entrada de brecha).</rdfs:comment>
        <rdfs:comment xml:lang="en">Entry fitting, typically unconnected at one port and connected to a flow distribution system at the other (e.g., a breeching inlet).</rdfs:comment>
        <rdfs:label xml:lang="es">Entrada de Tuberia</rdfs:label>
        <rdfs:label xml:lang="en">Pipe Entry</rdfs:label>
    </owl:Class>
    


    <!-- https://w3id.org/mep#PipeExit -->


    <owl:Class rdf:about="https://w3id.org/mep#PipeExit">
        <rdfs:subClassOf rdf:resource="https://w3id.org/mep#PipeFitting"/>
        <rdfs:comment xml:lang="es">Accesorio de salida, normalmente desconectado en un puerto y conectado a un sistema de distribución de caudal en el otro (por ejemplo, un grifo de manguera).</rdfs:comment>
        <rdfs:comment xml:lang="en">Exit fitting, typically unconnected at one port and connected to a flow distribution system at the other (e.g., a hose bibb).</rdfs:comment>
        <rdfs:label xml:lang="en">Pipe Exit</rdfs:label>
        <rdfs:label xml:lang="es">Salida de Tuberia</rdfs:label>
    </owl:Class>
    


    <!-- https://w3id.org/mep#PipeFitting -->


    <owl:Class rdf:about="https://w3id.org/mep#PipeFitting">
        <rdfs:subClassOf rdf:resource="https://w3id.org/mep#FlowFitting"/>
        <rdfs:comment xml:lang="en">A pipe fitting is a junction or transition in a piping flow distribution system used to connect pipe segments, resulting in changes in flow characteristics to the fluid such as direction or flow rate. Pipe fittings include elbows, junctions, manifolds, and plumbing boxes.</rdfs:comment>
        <rdfs:comment xml:lang="es">Un accesorio de tubería es una unión o transición en un sistema de distribución de flujo de tuberías que se utiliza para conectar segmentos de tuberías, lo que provoca cambios en las características de flujo al fluido, como la dirección o el caudal. Los accesorios de tubería incluyen codos, uniones, colectores y cajas de fontanería.</rdfs:comment>
        <rdfs:label xml:lang="es">Accesorio de Tuberia</rdfs:label>
        <rdfs:label xml:lang="en">Pipe Fitting</rdfs:label>
    </owl:Class>
    


    <!-- https://w3id.org/mep#PipeJunction -->


    <owl:Class rdf:about="https://w3id.org/mep#PipeJunction">
        <rdfs:subClassOf rdf:resource="https://w3id.org/mep#PipeFitting"/>
        <rdfs:comment xml:lang="en">A fitting with typically more than two ports used to redistribute flow among the ports and/or to change the direction of flow between connected elements (e.g, tee, cross, wye, etc.).</rdfs:comment>
        <rdfs:comment xml:lang="es">Accesorio con más de dos puertos utilizado para redistribuir el caudal entre los puertos y/o cambiar la dirección del caudal entre los elementos conectados (por ejemplo, te, cruz, estrella, etc.).</rdfs:comment>
        <rdfs:label xml:lang="es">Junta de Tuberia</rdfs:label>
        <rdfs:label xml:lang="en">Pipe Junction</rdfs:label>
    </owl:Class>
    


    <!-- https://w3id.org/mep#PipeObstruction -->


    <owl:Class rdf:about="https://w3id.org/mep#PipeObstruction">
        <rdfs:subClassOf rdf:resource="https://w3id.org/mep#PipeFitting"/>
        <rdfs:comment xml:lang="en">A fitting with typically two ports used to obstruct or restrict flow between the connected elements (e.g., screen, perforated plate, etc.).</rdfs:comment>
        <rdfs:comment xml:lang="es">Accesorio con dos orificios típicos utilizado para obstruir o restringir el flujo entre los elementos conectados (por ejemplo, pantalla, placa perforada, etc.).</rdfs:comment>
        <rdfs:label xml:lang="es">Obstruccion de Tuberia</rdfs:label>
        <rdfs:label xml:lang="en">Pipe Obstruction</rdfs:label>
    </owl:Class>
    


    <!-- https://w3id.org/mep#PipeSegment -->


    <owl:Class rdf:about="https://w3id.org/mep#PipeSegment">
        <rdfs:subClassOf rdf:resource="https://w3id.org/mep#FlowSegment"/>
        <rdfs:comment xml:lang="en">A pipe segment is used to typically join two sections of a piping network.</rdfs:comment>
        <rdfs:comment xml:lang="es">Un segmento de tubería se utiliza normalmente para unir dos tramos de una red de tuberías.</rdfs:comment>
        <rdfs:label xml:lang="en">Pipe Segment</rdfs:label>
        <rdfs:label xml:lang="es">Segmento de Tuberia</rdfs:label>
    </owl:Class>
    


    <!-- https://w3id.org/mep#PipeTransition -->


    <owl:Class rdf:about="https://w3id.org/mep#PipeTransition">
        <rdfs:subClassOf rdf:resource="https://w3id.org/mep#PipeFitting"/>
        <rdfs:comment xml:lang="en">A fitting with typically two ports having different shapes or sizes. Can also be used to change the direction of flow between connected elements.</rdfs:comment>
        <rdfs:comment xml:lang="es">Accesorio que suele tener dos puertos de formas o tamaños diferentes. También puede utilizarse para cambiar la dirección del flujo entre elementos conectados.</rdfs:comment>
        <rdfs:label xml:lang="en">Pipe Transition</rdfs:label>
        <rdfs:label xml:lang="es">Trasicion de Tuberia</rdfs:label>
    </owl:Class>
    


    <!-- https://w3id.org/mep#PlateHeatExchanger -->


    <owl:Class rdf:about="https://w3id.org/mep#PlateHeatExchanger">
        <rdfs:subClassOf rdf:resource="https://w3id.org/mep#HeatExchanger"/>
        <rdfs:comment xml:lang="es">Intercambiador de calor de placas</rdfs:comment>
        <rdfs:comment xml:lang="en">Plate heat exchanger.</rdfs:comment>
        <rdfs:label xml:lang="es">Intercambiador  de Calor de Placas</rdfs:label>
        <rdfs:label xml:lang="en">Plate Heat Exchanger</rdfs:label>
    </owl:Class>
    


    <!-- https://w3id.org/mep#Player -->


    <owl:Class rdf:about="https://w3id.org/mep#Player">
        <rdfs:subClassOf rdf:resource="https://w3id.org/mep#AudioVisualAppliance"/>
        <rdfs:comment xml:lang="en">A device that plays audio and/or video content directly or to another device, having fixed or removable storage media.</rdfs:comment>
        <rdfs:comment xml:lang="es">Un dispositivo que reproduce contenido de audio y/o video directamente o a otro dispositivo, que tiene medios de almacenamiento fijos o extraíbles.</rdfs:comment>
        <rdfs:label xml:lang="en">Player</rdfs:label>
        <rdfs:label xml:lang="es">Reproductor</rdfs:label>
    </owl:Class>
    


    <!-- https://w3id.org/mep#PneumaticActuator -->


    <owl:Class rdf:about="https://w3id.org/mep#PneumaticActuator">
        <rdfs:subClassOf rdf:resource="https://w3id.org/mep#Actuator"/>
        <rdfs:comment xml:lang="en">A device that pneumatically actuates a control element.</rdfs:comment>
        <rdfs:comment xml:lang="es">Dispositivo que acciona neumáticamente un elemento de control.</rdfs:comment>
        <rdfs:label xml:lang="es">Actuador Pneumático</rdfs:label>
        <rdfs:label xml:lang="en">Pneumatic Actuator</rdfs:label>
    </owl:Class>
    


    <!-- https://w3id.org/mep#PointSourceLightFixture -->


    <owl:Class rdf:about="https://w3id.org/mep#PointSourceLightFixture">
        <rdfs:subClassOf rdf:resource="https://w3id.org/mep#LightFixture"/>
        <rdfs:comment xml:lang="en">A light fixture that is considered to have negligible area and that emit light with approximately equal intensity in all directions. A light fixture containing a tungsten, halogen or similar bulb is an example of a point source.</rdfs:comment>
        <rdfs:comment xml:lang="es">Un artefacto de iluminación que se considera que tiene un área insignificante y que emite luz con aproximadamente la misma intensidad en todas las direcciones. Un artefacto de iluminación que contiene una bombilla de tungsteno, halógena o similar es un ejemplo de fuente puntual.</rdfs:comment>
        <rdfs:label xml:lang="es">Luminaria de fuente puntual</rdfs:label>
        <rdfs:label xml:lang="en">Point Source Light Fixture</rdfs:label>
    </owl:Class>
    


    <!-- https://w3id.org/mep#PolyphaseMotor -->


    <owl:Class rdf:about="https://w3id.org/mep#PolyphaseMotor">
        <rdfs:subClassOf rdf:resource="https://w3id.org/mep#ElectricMotor"/>
        <rdfs:comment xml:lang="en">A two or three-phase induction motor in which the windings, one for each phase, are evenly divided by the same number of electrical degrees.</rdfs:comment>
        <rdfs:comment xml:lang="es">Motor de inducción bifásico o trifásico en el que los devanados, uno para cada fase, están divididos uniformemente por el mismo número de grados eléctricos.</rdfs:comment>
        <rdfs:label xml:lang="es">Motor Polifasico</rdfs:label>
        <rdfs:label xml:lang="en">Polyphase Motor</rdfs:label>
    </owl:Class>
    


    <!-- https://w3id.org/mep#PowerFactorMeter -->


    <owl:Class rdf:about="https://w3id.org/mep#PowerFactorMeter">
        <rdfs:subClassOf rdf:resource="https://w3id.org/mep#FlowInstrument"/>
        <rdfs:comment xml:lang="en">A device that reads and displays the power factor of an electrical circuit.</rdfs:comment>
        <rdfs:comment xml:lang="es">Dispositivo que lee y muestra el factor de potencia de un circuito eléctrico.</rdfs:comment>
        <rdfs:label xml:lang="es">Medidor de Factor de Potencia</rdfs:label>
        <rdfs:label xml:lang="en">Power Factor Meter</rdfs:label>
    </owl:Class>
    


    <!-- https://w3id.org/mep#PowerJuntionBox -->


    <owl:Class rdf:about="https://w3id.org/mep#PowerJuntionBox">
        <rdfs:subClassOf rdf:resource="https://w3id.org/mep#JunctionBox"/>
        <rdfs:comment xml:lang="en">Contains cables, outlets, and/or switches for electrical power.</rdfs:comment>
        <rdfs:comment xml:lang="es">Contiene cables, tomacorrientes y/o interruptores para energía eléctrica.</rdfs:comment>
        <rdfs:label xml:lang="es">Caja de Conexiones Electricas</rdfs:label>
        <rdfs:label xml:lang="en">Power Juntion Box</rdfs:label>
    </owl:Class>
    


    <!-- https://w3id.org/mep#PowerOutlet -->


    <owl:Class rdf:about="https://w3id.org/mep#PowerOutlet">
        <rdfs:subClassOf rdf:resource="https://w3id.org/mep#Outlet"/>
        <rdfs:comment xml:lang="en">An outlet used for connecting electrical devices requiring power.</rdfs:comment>
        <rdfs:comment xml:lang="es">Salida utilizada para conectar aparatos eléctricos que necesitan corriente.</rdfs:comment>
        <rdfs:label xml:lang="en">Power Outlet</rdfs:label>
        <rdfs:label xml:lang="es">Toma de Corriente</rdfs:label>
    </owl:Class>
    


    <!-- https://w3id.org/mep#PressureGauge -->


    <owl:Class rdf:about="https://w3id.org/mep#PressureGauge">
        <rdfs:subClassOf rdf:resource="https://w3id.org/mep#FlowInstrument"/>
        <rdfs:comment xml:lang="en">A device that reads and displays a pressure value at a point or the pressure difference between two points.</rdfs:comment>
        <rdfs:comment xml:lang="es">Dispositivo que lee y muestra un valor de presión en un punto o la diferencia de presión entre dos puntos.</rdfs:comment>
        <rdfs:label xml:lang="es">Manometro</rdfs:label>
        <rdfs:label xml:lang="en">Pressure Gauge</rdfs:label>
    </owl:Class>
    


    <!-- https://w3id.org/mep#PressureReducingValve -->


    <owl:Class rdf:about="https://w3id.org/mep#PressureReducingValve">
        <rdfs:subClassOf rdf:resource="https://w3id.org/mep#Valve"/>
        <rdfs:comment xml:lang="en">Valve that reduces the pressure of a fluid immediately downstream of its position in a pipeline to a preselected value or by a predetermined ratio.</rdfs:comment>
        <rdfs:comment xml:lang="es">Válvula que reduce la presión de un fluido inmediatamente aguas abajo de su posición en una tubería a un valor preseleccionado o en una proporción predeterminada.</rdfs:comment>
        <rdfs:label xml:lang="en">Pressure Reducing Valve</rdfs:label>
        <rdfs:label xml:lang="es">Valvula de Reducción de Presion</rdfs:label>
    </owl:Class>
    


    <!-- https://w3id.org/mep#PressureReliefValve -->


    <owl:Class rdf:about="https://w3id.org/mep#PressureReliefValve">
        <rdfs:subClassOf rdf:resource="https://w3id.org/mep#Valve"/>
        <rdfs:comment xml:lang="en">Spring or weight loaded valve that automatically discharges to a safe place fluid that has built up to excessive pressure in pipes or fittings.</rdfs:comment>
        <rdfs:comment xml:lang="es">Válvula cargada por un resorte o peso que descarga automáticamente a un lugar seguro el fluido que se ha acumulado a una presión excesiva en tuberías o accesorios.</rdfs:comment>
        <rdfs:label xml:lang="en">Pressure Relief Valve</rdfs:label>
        <rdfs:label xml:lang="es">Valvula de Descarga de Presion</rdfs:label>
    </owl:Class>
    


    <!-- https://w3id.org/mep#PressureSensor -->


    <owl:Class rdf:about="https://w3id.org/mep#PressureSensor">
        <rdfs:subClassOf rdf:resource="https://w3id.org/mep#Sensor"/>
        <rdfs:comment xml:lang="en">A device that senses or detects pressure.</rdfs:comment>
        <rdfs:comment xml:lang="es">Dispositivo que detecta la presión.</rdfs:comment>
        <rdfs:label xml:lang="en">Pressure Sensor</rdfs:label>
        <rdfs:label xml:lang="es">Sensor de Presion</rdfs:label>
    </owl:Class>
    


    <!-- https://w3id.org/mep#PressureVessel -->


    <owl:Class rdf:about="https://w3id.org/mep#PressureVessel">
        <rdfs:subClassOf rdf:resource="https://w3id.org/mep#Tank"/>
        <rdfs:comment xml:lang="en">A closed container used for storing fluids or gases at a pressure different from the ambient pressure. A pressure vessel is typically rated by an authority having jurisdiction for the operational pressure.</rdfs:comment>
        <rdfs:comment xml:lang="es">Recipiente cerrado utilizado para almacenar fluidos o gases a una presión diferente de la presión ambiente. Un recipiente a presión suele estar clasificado por una autoridad competente para la presión operativa.</rdfs:comment>
        <rdfs:label xml:lang="en">Pressure Vessel</rdfs:label>
        <rdfs:label xml:lang="es">Recipiente a Presion</rdfs:label>
    </owl:Class>
    


    <!-- https://w3id.org/mep#Printer -->


    <owl:Class rdf:about="https://w3id.org/mep#Printer">
        <rdfs:subClassOf rdf:resource="https://w3id.org/mep#CommunicationsAppliance"/>
        <rdfs:comment xml:lang="en">A machine that has the primary function of printing text and/or graphics onto paper or other media.</rdfs:comment>
        <rdfs:comment xml:lang="es">Máquina cuya función principal es imprimir texto y/o gráficos en papel u otros soportes.</rdfs:comment>
        <rdfs:label xml:lang="es">Impresora</rdfs:label>
        <rdfs:label xml:lang="en">Printer</rdfs:label>
    </owl:Class>
    


    <!-- https://w3id.org/mep#ProgrammableController -->


    <owl:Class rdf:about="https://w3id.org/mep#ProgrammableController">
        <rdfs:subClassOf rdf:resource="https://w3id.org/mep#Controller"/>
        <rdfs:comment xml:lang="es">La salida es programable como Control Digital Discreto (DDC).</rdfs:comment>
        <rdfs:comment xml:lang="en">Output is programmable such as Discrete Digital Control (DDC).</rdfs:comment>
        <rdfs:label xml:lang="es">Controlador Programable</rdfs:label>
        <rdfs:label xml:lang="en">Programmable Controller</rdfs:label>
    </owl:Class>
    


    <!-- https://w3id.org/mep#Projector -->


    <owl:Class rdf:about="https://w3id.org/mep#Projector">
        <rdfs:subClassOf rdf:resource="https://w3id.org/mep#AudioVisualAppliance"/>
        <rdfs:comment xml:lang="en">An apparatus for projecting a picture on a screen. Whether the device is an overhead, slide projector, or a film projector, it is usually referred to as simply a projector.</rdfs:comment>
        <rdfs:comment xml:lang="es">Un aparato para proyectar una imagen en una pantalla. Ya sea que el dispositivo sea un proyector de transparencias, de diapositivas o de películas, generalmente se lo denomina simplemente proyector.</rdfs:comment>
        <rdfs:label xml:lang="en">Projector</rdfs:label>
        <rdfs:label xml:lang="es">proyector</rdfs:label>
    </owl:Class>
    


    <!-- https://w3id.org/mep#PropellorAxialFan -->


    <owl:Class rdf:about="https://w3id.org/mep#PropellorAxialFan">
        <rdfs:subClassOf rdf:resource="https://w3id.org/mep#Fan"/>
        <rdfs:comment xml:lang="es"> (??) El aire fluye axialmente  a través del impulsor y el impulsor con una pequeña relación de cubo a punta está montado en una placa de orificio o anillo de entrada.</rdfs:comment>
        <rdfs:comment xml:lang="en">(??) Air flows through the impeller axially and small hub-to-tip ratio impeller mounted in an orifice plate or inlet ring.</rdfs:comment>
        <rdfs:label xml:lang="en">Propellor Axial Fan</rdfs:label>
        <rdfs:label xml:lang="es">Ventilador Axial de Propulsor</rdfs:label>
    </owl:Class>
    


    <!-- https://w3id.org/mep#ProportionalController -->


    <owl:Class rdf:about="https://w3id.org/mep#ProportionalController">
        <rdfs:subClassOf rdf:resource="https://w3id.org/mep#Controller"/>
        <rdfs:comment xml:lang="es">La salida es proporcional al error de control y opcionalmente integral de tiempo y derivada.</rdfs:comment>
        <rdfs:comment xml:lang="en">Output is proportional to the control error and optionally time integral and derivative.</rdfs:comment>
        <rdfs:label xml:lang="es">Controlador Proporcional</rdfs:label>
        <rdfs:label xml:lang="en">Proportional Controller</rdfs:label>
    </owl:Class>
    


    <!-- https://w3id.org/mep#ProtectiveDevice -->


    <owl:Class rdf:about="https://w3id.org/mep#ProtectiveDevice">
        <rdfs:subClassOf rdf:resource="https://w3id.org/mep#FlowController"/>
        <rdfs:comment xml:lang="en">A protective device breaks an electrical circuit when a stated electric current that passes through it is exceeded. A protective device provides protection against electrical current only (not as a general protective device). It may be used to represent the complete set of elements including both the tripping unit and the breaking unit that provide the protection. This may be particularly useful at earlier stages of design where the approach to breaking the electrical supply may be determined but the method of tripping may not. Alternatively, this entity may be used to specifically represent the breaking unit alone (in which case the tripping unit will also be specifically identified). This entity is specific to dedicated protective devices and excludes electrical outlets that may have circuit protection.</rdfs:comment>
        <rdfs:comment xml:lang="es">Un dispositivo de protección interrumpe un circuito eléctrico cuando se supera la corriente eléctrica establecida que pasa a través de él. Un dispositivo de protección sólo proporciona protección contra la corriente eléctrica (no como dispositivo de protección general). Puede utilizarse para representar el conjunto completo de elementos que incluyen tanto la unidad de disparo como la unidad de corte que proporcionan la protección. Esto puede resultar especialmente útil en las primeras fases del diseño, en las que puede determinarse el método de corte del suministro eléctrico, pero no el método de disparo. Alternativamente, esta entidad puede utilizarse para representar específicamente la unidad de corte sola (en cuyo caso la unidad de disparo también se identificará específicamente). Esta entidad es específica de los dispositivos de protección dedicados y excluye las tomas de corriente que puedan tener protección de circuito.</rdfs:comment>
        <rdfs:label xml:lang="es">Dispositivo de Proteccion</rdfs:label>
        <rdfs:label xml:lang="en">Protective Device</rdfs:label>
    </owl:Class>
    


    <!-- https://w3id.org/mep#ProtectiveDeviceTrippingUnit -->


    <owl:Class rdf:about="https://w3id.org/mep#ProtectiveDeviceTrippingUnit">
        <rdfs:subClassOf rdf:resource="https://w3id.org/mep#DistributionControlElement"/>
        <rdfs:comment xml:lang="en">A protective device tripping unit breaks an electrical circuit at a separate breaking unit when a stated electric current that passes through the unit is exceeded.</rdfs:comment>
        <rdfs:comment xml:lang="es">Una unidad de disparo de un dispositivo de protección interrumpe un circuito eléctrico en una unidad de corte independiente cuando se supera una corriente eléctrica establecida que pasa por la unidad.</rdfs:comment>
        <rdfs:label xml:lang="en">Protective Device Tripping Unit</rdfs:label>
        <rdfs:label xml:lang="es">Unidad de Disparo de Dispositivo de Proteccion</rdfs:label>
    </owl:Class>
    


    <!-- https://w3id.org/mep#Pump -->


    <owl:Class rdf:about="https://w3id.org/mep#Pump">
        <rdfs:subClassOf rdf:resource="https://w3id.org/mep#FlowMovingDevice"/>
        <rdfs:comment xml:lang="en">A pump is a device which imparts mechanical work on fluids or slurries to move them through a channel or pipeline. A typical use of a pump is to circulate chilled water or heating hot water in a building services distribution system.</rdfs:comment>
        <rdfs:comment xml:lang="es">Una bomba es un dispositivo que imparte trabajo mecánico a fluidos o lodos para moverlos a través de un canal o tubería. El uso típico de una bomba es hacer circular agua refrigerada o agua caliente para calefacción en un sistema de distribución de servicios de un edificio.</rdfs:comment>
        <rdfs:label xml:lang="es">Bomba</rdfs:label>
        <rdfs:label xml:lang="en">Pump</rdfs:label>
    </owl:Class>
    


    <!-- https://w3id.org/mep#RadiactivitySensor -->


    <owl:Class rdf:about="https://w3id.org/mep#RadiactivitySensor">
        <rdfs:subClassOf rdf:resource="https://w3id.org/mep#Sensor"/>
        <rdfs:comment xml:lang="en">A device that senses or detects atomic decay.</rdfs:comment>
        <rdfs:comment xml:lang="es">Dispositivo que detecta la desintegración atómica.</rdfs:comment>
        <rdfs:label xml:lang="en">Radiactivity Sensor</rdfs:label>
        <rdfs:label xml:lang="es">Sensor de Radiactividad</rdfs:label>
    </owl:Class>
    


    <!-- https://w3id.org/mep#RadiationSensor -->


    <owl:Class rdf:about="https://w3id.org/mep#RadiationSensor">
        <rdfs:subClassOf rdf:resource="https://w3id.org/mep#Sensor"/>
        <rdfs:comment xml:lang="en">A device that senses or detects radiation.</rdfs:comment>
        <rdfs:comment xml:lang="es">Dispositivo que detecta radiación.</rdfs:comment>
        <rdfs:label xml:lang="en">Radiation Sensor</rdfs:label>
        <rdfs:label xml:lang="es">Sensor de Radiacion</rdfs:label>
    </owl:Class>
    


    <!-- https://w3id.org/mep#Radiator -->


    <owl:Class rdf:about="https://w3id.org/mep#Radiator">
        <rdfs:subClassOf rdf:resource="https://w3id.org/mep#SpaceHeater"/>
        <rdfs:comment xml:lang="en">A heat-distributing unit that operates with thermal radiation.</rdfs:comment>
        <rdfs:comment xml:lang="es">Unidad de distribución de calor que funciona por radiación térmica.</rdfs:comment>
        <rdfs:label xml:lang="es">Radiador</rdfs:label>
        <rdfs:label xml:lang="en">Radiator</rdfs:label>
    </owl:Class>
    


    <!-- https://w3id.org/mep#RadioBlockCenter -->


    <owl:Class rdf:about="https://w3id.org/mep#RadioBlockCenter">
        <rdfs:subClassOf rdf:resource="https://w3id.org/mep#CommunicationsAppliance"/>
        <rdfs:comment xml:lang="en">A radio block center is a specialised computing device in railway with specification for generating Movement Authorities (MA) and transmitting it to trains. It gets information from signalling control and from the trains in its section.</rdfs:comment>
        <rdfs:comment xml:lang="es">Un centro de bloque radioeléctrico es un dispositivo informático especializado en el ferrocarril con la especificación de generar Autoridades de Movimiento (AM) y transmitirlas a los trenes. Recibe información del control de señalización y de los trenes de su sección.</rdfs:comment>
        <rdfs:label xml:lang="es">Centro de Bloque Radioelectrico</rdfs:label>
        <rdfs:label xml:lang="en">Radio Block Center</rdfs:label>
    </owl:Class>
    


    <!-- https://w3id.org/mep#RailwayCrocodile -->


    <owl:Class rdf:about="https://w3id.org/mep#RailwayCrocodile">
        <rdfs:subClassOf rdf:resource="https://w3id.org/mep#Alarm"/>
        <rdfs:comment xml:lang="en">An electrical contact placed between the rails (in the four-foot way) to provide warnings in the locomotive cab.</rdfs:comment>
        <rdfs:comment xml:lang="es">Un contacto eléctrico colocado entre los rieles (a cuatro pies) para proporcionar advertencias en la cabina de la locomotora.</rdfs:comment>
        <rdfs:label xml:lang="es">Cocodrilo Ferroviario</rdfs:label>
        <rdfs:label xml:lang="en">Railway Crocodile</rdfs:label>
    </owl:Class>
    


    <!-- https://w3id.org/mep#RailwayDetonator -->


    <owl:Class rdf:about="https://w3id.org/mep#RailwayDetonator">
        <rdfs:subClassOf rdf:resource="https://w3id.org/mep#Alarm"/>
        <rdfs:comment xml:lang="en">A coin-sized device that is used as a loud warning signal to train drivers. It is usually placed on the top of the rail, usually secured with two lead straps, one on each side.</rdfs:comment>
        <rdfs:comment xml:lang="es">Un dispositivo del tamaño de una moneda que se utiliza como señal de advertencia sonora para los conductores de trenes. Suele colocarse en la parte superior del riel, normalmente asegurado con dos correas de plomo, una a cada lado.</rdfs:comment>
        <rdfs:label xml:lang="es">Detonador Ferroviario</rdfs:label>
        <rdfs:label xml:lang="en">Railway Detonator</rdfs:label>
    </owl:Class>
    


    <!-- https://w3id.org/mep#RainSensor -->


    <owl:Class rdf:about="https://w3id.org/mep#RainSensor">
        <rdfs:subClassOf rdf:resource="https://w3id.org/mep#Sensor"/>
        <rdfs:comment xml:lang="en">A device that senses or collects rainfall related information.</rdfs:comment>
        <rdfs:comment xml:lang="es">Dispositivo que detecta o recoge información relacionada con la lluvia.</rdfs:comment>
        <rdfs:label xml:lang="en">Rain Sensor</rdfs:label>
        <rdfs:label xml:lang="es">Sensor de Lluvia</rdfs:label>
    </owl:Class>
    


    <!-- https://w3id.org/mep#RainwaterHopper -->


    <owl:Class rdf:about="https://w3id.org/mep#RainwaterHopper">
        <rdfs:subClassOf rdf:resource="https://w3id.org/mep#StackTerminal"/>
        <rdfs:comment xml:lang="en">A box placed at the top of a rainwater downpipe to catch rainwater from guttering.</rdfs:comment>
        <rdfs:comment xml:lang="es">Caja colocada en la parte superior de una bajante de aguas pluviales para recoger el agua de lluvia de los canalones.</rdfs:comment>
        <rdfs:label xml:lang="en">Rainwater Hopper</rdfs:label>
        <rdfs:label xml:lang="es">Recolector de Aguas Pluviales</rdfs:label>
    </owl:Class>
    


    <!-- https://w3id.org/mep#Recharger -->


    <owl:Class rdf:about="https://w3id.org/mep#Recharger">
        <rdfs:subClassOf rdf:resource="https://w3id.org/mep#ElectricFlowStorageDevice"/>
        <rdfs:comment xml:lang="en">A recharger or battery charger is a device used to put energy into a secondary cell or rechargeable battery by forcing an electric current through it.</rdfs:comment>
        <rdfs:comment xml:lang="es">Un cargador de baterías es un dispositivo utilizado para suministrar energía a una pila secundaria o batería recargable forzando una corriente eléctrica a través de ella.</rdfs:comment>
        <rdfs:label xml:lang="es">Cargador</rdfs:label>
        <rdfs:label xml:lang="en">Recharger</rdfs:label>
    </owl:Class>
    


    <!-- https://w3id.org/mep#Reciever -->


    <owl:Class rdf:about="https://w3id.org/mep#Reciever">
        <rdfs:subClassOf rdf:resource="https://w3id.org/mep#AudioVisualAppliance"/>
        <rdfs:comment xml:lang="en">A device that receives audio and/or video signals, switches sources, and amplifies signals to play through speakers.</rdfs:comment>
        <rdfs:comment xml:lang="es">Un dispositivo que recibe señales de audio y/o video, cambia fuentes y amplifica señales para reproducirlas a través de parlantes.</rdfs:comment>
        <rdfs:label xml:lang="es">Receptor</rdfs:label>
        <rdfs:label xml:lang="en">Reciever</rdfs:label>
    </owl:Class>
    


    <!-- https://w3id.org/mep#ReciprocatingCompressor -->


    <owl:Class rdf:about="https://w3id.org/mep#ReciprocatingCompressor">
        <rdfs:subClassOf rdf:resource="https://w3id.org/mep#Compressor"/>
        <rdfs:comment xml:lang="es">Compresor de desplazamiento positivo que utiliza un pistón accionado por una biela desde un cigüeñal.</rdfs:comment>
        <rdfs:comment xml:lang="en">Positive-displacement compressor using a piston driven by a connecting rod from a crankshaft.</rdfs:comment>
        <rdfs:label xml:lang="es">Compresor Alternativo</rdfs:label>
        <rdfs:label xml:lang="en">Reciprocating Compressor</rdfs:label>
    </owl:Class>
    


    <!-- https://w3id.org/mep#RecordingEquipment -->


    <owl:Class rdf:about="https://w3id.org/mep#RecordingEquipment">
        <rdfs:subClassOf rdf:resource="https://w3id.org/mep#AudioVisualAppliance"/>
        <rdfs:comment xml:lang="en">A recording equipment is a device that records telephone calls or other types of audio data. It also provides the function of archiving and immediate replay.</rdfs:comment>
        <rdfs:comment xml:lang="es">Un equipo de grabación es un dispositivo que graba llamadas telefónicas u otros tipos de datos de audio. También proporciona la función de archivo y reproducción inmediata.</rdfs:comment>
        <rdfs:label xml:lang="es">Equipo de Grabacion</rdfs:label>
        <rdfs:label xml:lang="en">Recording Equipment</rdfs:label>
    </owl:Class>
    


    <!-- https://w3id.org/mep#RectangularSilencer -->


    <owl:Class rdf:about="https://w3id.org/mep#RectangularSilencer">
        <rdfs:subClassOf rdf:resource="https://w3id.org/mep#DuctSilencer"/>
        <rdfs:comment xml:lang="en">Rectangular shaped duct silencer type.</rdfs:comment>
        <rdfs:comment xml:lang="es">Tipo de silenciador de conducto de forma rectangular.</rdfs:comment>
        <rdfs:label xml:lang="en">Rectangular Silencer</rdfs:label>
        <rdfs:label xml:lang="es">Silenciador Rectangular</rdfs:label>
    </owl:Class>
    


    <!-- https://w3id.org/mep#Rectifier -->


    <owl:Class rdf:about="https://w3id.org/mep#Rectifier">
        <rdfs:subClassOf rdf:resource="https://w3id.org/mep#Transformer"/>
        <rdfs:comment xml:lang="en">A transformer that converts from alternating current (AC) to direct current (DC).</rdfs:comment>
        <rdfs:comment xml:lang="es">Un conversor que convierte de corriente alterna (CA) a corriente continua (CC).</rdfs:comment>
        <rdfs:label xml:lang="es">Rectificador</rdfs:label>
        <rdfs:label xml:lang="en">Rectifier</rdfs:label>
    </owl:Class>
    


    <!-- https://w3id.org/mep#Refrigerator -->


    <owl:Class rdf:about="https://w3id.org/mep#Refrigerator">
        <rdfs:subClassOf rdf:resource="https://w3id.org/mep#ElectricAppliance"/>
        <rdfs:comment xml:lang="en">An electrical appliance that has the primary function of storing food at low temperature but above the freezing point of water.</rdfs:comment>
        <rdfs:comment xml:lang="es">Aparato eléctrico cuya función principal es conservar alimentos a baja temperatura pero por encima del punto de congelación del agua.</rdfs:comment>
        <rdfs:label xml:lang="es">Refrigerador</rdfs:label>
        <rdfs:label xml:lang="en">Refrigerator</rdfs:label>
    </owl:Class>
    


    <!-- https://w3id.org/mep#Register -->


    <owl:Class rdf:about="https://w3id.org/mep#Register">
        <rdfs:subClassOf rdf:resource="https://w3id.org/mep#AirTerminal"/>
        <rdfs:comment xml:lang="en">A grille typically equipped with a damper or control valve.</rdfs:comment>
        <rdfs:comment xml:lang="es">Una rejilla típicamente equipada con una compuerta o válvula de control.</rdfs:comment>
        <rdfs:label xml:lang="en">Register</rdfs:label>
        <rdfs:label xml:lang="es">Registro</rdfs:label>
    </owl:Class>
    


    <!-- https://w3id.org/mep#RegulatingValve -->


    <owl:Class rdf:about="https://w3id.org/mep#RegulatingValve">
        <rdfs:subClassOf rdf:resource="https://w3id.org/mep#Valve"/>
        <rdfs:comment xml:lang="en">Valve used to facilitate regulation of fluid flow in a system.</rdfs:comment>
        <rdfs:comment xml:lang="es">Válvula utilizada para facilitar la regulación del flujo de fluido en un sistema.</rdfs:comment>
        <rdfs:label xml:lang="en">Regulating Valve</rdfs:label>
        <rdfs:label xml:lang="es">Valvula Reguladora</rdfs:label>
    </owl:Class>
    


    <!-- https://w3id.org/mep#Relay -->


    <owl:Class rdf:about="https://w3id.org/mep#Relay">
        <rdfs:subClassOf rdf:resource="https://w3id.org/mep#SwitchingDevice"/>
        <rdfs:comment xml:lang="en">A device designed to produce sudden predetermined changes in one or more electric output circuits, when certain conditions are fulfilled in the electric input circuits controlling the device. Note: definition from IEC 60050 151-13-31.</rdfs:comment>
        <rdfs:comment xml:lang="es">Dispositivo diseñado para producir cambios repentinos predeterminados en uno o más circuitos eléctricos de salida, cuando se cumplen ciertas condiciones en los circuitos eléctricos de entrada que controlan el dispositivo. Nota: definición de la norma IEC 60050 151-13-31.</rdfs:comment>
        <rdfs:label xml:lang="en">Relay</rdfs:label>
        <rdfs:label xml:lang="es">Rele</rdfs:label>
    </owl:Class>
    


    <!-- https://w3id.org/mep#ReliefDamper -->


    <owl:Class rdf:about="https://w3id.org/mep#ReliefDamper">
        <rdfs:subClassOf rdf:resource="https://w3id.org/mep#Damper"/>
        <rdfs:comment xml:lang="es">Compuerta de alivio utilizada para permitir el movimiento del aire al acumularse un diferencial de presión especificado. Suele accionarse mediante un muelle mecánico.</rdfs:comment>
        <rdfs:comment xml:lang="en">Relief damper used to allow air to move upon a buildup of a specified pressure differential. Commonly operated by mechanical spring.</rdfs:comment>
        <rdfs:label xml:lang="es">Compuerta de Alivio</rdfs:label>
        <rdfs:label xml:lang="en">Relief Damper</rdfs:label>
    </owl:Class>
    


    <!-- https://w3id.org/mep#ReluctanceSynchronousMotor -->


    <owl:Class rdf:about="https://w3id.org/mep#ReluctanceSynchronousMotor">
        <rdfs:subClassOf rdf:resource="https://w3id.org/mep#ElectricMotor"/>
        <rdfs:comment xml:lang="en">A synchronous motor with a special rotor design which directly lines the rotor up with the rotating magnetic field of the stator, allowing for no slip under load.</rdfs:comment>
        <rdfs:comment xml:lang="es">Un motor síncrono con un diseño de rotor especial que alinea directamente el rotor con el campo magnético giratorio del estator, lo que permite que no se deslice bajo carga.</rdfs:comment>
        <rdfs:label xml:lang="es">Motor de Reluctancia Sincrona</rdfs:label>
        <rdfs:label xml:lang="en">Reluctance Synchronous Motor</rdfs:label>
    </owl:Class>
    


    <!-- https://w3id.org/mep#RemoteRadioUnit -->


    <owl:Class rdf:about="https://w3id.org/mep#RemoteRadioUnit">
        <rdfs:subClassOf rdf:resource="https://w3id.org/mep#MobileTelecommunicationsAppliance"/>
        <rdfs:comment xml:lang="en">A remote radio unit is a component of a distributed base transceiver station that converts digital baseband signals into high-frequency (rf) signals and sends high-frequency (rf) signals to the antenna for radiation.</rdfs:comment>
        <rdfs:comment xml:lang="es">Una unidad de control de paquetes realiza algunas de las tareas de procesamiento del controlador de la estación base para los paquetes de datos. Es responsable de los paquetes de datos, la gestión de canales inalámbricos, la detección de errores de envío y la retransmisión automática.</rdfs:comment>
        <rdfs:label xml:lang="en">Remote Radio Unit</rdfs:label>
        <rdfs:label xml:lang="es">Unidad de Radio Remota</rdfs:label>
    </owl:Class>
    


    <!-- https://w3id.org/mep#RemoteUnit -->


    <owl:Class rdf:about="https://w3id.org/mep#RemoteUnit">
        <rdfs:subClassOf rdf:resource="https://w3id.org/mep#MobileTelecommunicationsAppliance"/>
        <rdfs:comment xml:lang="en">A remote unit is a device used to amplify a base station signal.</rdfs:comment>
        <rdfs:comment xml:lang="es">Una unidad remota es un dispositivo utilizado para amplificar la señal de una estación base.</rdfs:comment>
        <rdfs:label xml:lang="en">Remote Unit</rdfs:label>
        <rdfs:label xml:lang="es">Unidad Remota</rdfs:label>
    </owl:Class>
    


    <!-- https://w3id.org/mep#Repeater -->


    <owl:Class rdf:about="https://w3id.org/mep#Repeater">
        <rdfs:subClassOf rdf:resource="https://w3id.org/mep#CommunicationsAppliance"/>
        <rdfs:comment xml:lang="en">A repeater is an electronic device that receives a signal and retransmits it at a higher level and/or higher power, or onto the other side of an obstruction, so that the signal can cover longer distances without degradation.</rdfs:comment>
        <rdfs:comment xml:lang="es">Un repetidor es un dispositivo electrónico que recibe una señal y la retransmite a un nivel y/o potencia más altos, o al otro lado de un obstáculo, para que la señal pueda cubrir distancias más largas sin degradarse.</rdfs:comment>
        <rdfs:label xml:lang="en">Repeater</rdfs:label>
        <rdfs:label xml:lang="es">Repetidor</rdfs:label>
    </owl:Class>
    


    <!-- https://w3id.org/mep#ResidualCurrentCircuitBreaker -->


    <owl:Class rdf:about="https://w3id.org/mep#ResidualCurrentCircuitBreaker">
        <rdfs:subClassOf rdf:resource="https://w3id.org/mep#ProtectiveDevice"/>
        <rdfs:comment xml:lang="en">A device that opens, closes, or isolates a circuit and has short circuit and overload protection. It attempts to break the circuit when there is a difference in current between any two phases. May also be referred to as &apos;Ground Fault Interupter (GFI)&apos; or &apos;Ground Fault Circuit Interuptor (GFCI)&apos;</rdfs:comment>
        <rdfs:comment xml:lang="es">Dispositivo que abre, cierra o aísla un circuito y dispone de protección contra cortocircuitos y sobrecargas. Intenta interrumpir el circuito cuando hay una diferencia de corriente entre dos fases cualesquiera. También puede denominarse &apos;Interruptor de fallo de tierra (GFI)&apos; o &apos;Interruptor de circuito de fallo de tierra (GFCI)&apos;.</rdfs:comment>
        <rdfs:label xml:lang="es">Disyuntor de Corriente</rdfs:label>
        <rdfs:label xml:lang="en">Residual Current Circuit Breaker</rdfs:label>
    </owl:Class>
    


    <!-- https://w3id.org/mep#ResidualCurrentSwitch -->


    <owl:Class rdf:about="https://w3id.org/mep#ResidualCurrentSwitch">
        <rdfs:subClassOf rdf:resource="https://w3id.org/mep#ProtectiveDevice"/>
        <rdfs:comment xml:lang="en">A device that opens, closes or isolates a circuit and has no short circuit or overload protection. May also be identified as a &apos;ground fault switch&apos;.</rdfs:comment>
        <rdfs:comment xml:lang="es">Dispositivo que abre, cierra o aísla un circuito y no tiene protección contra cortocircuitos o sobrecargas. También puede identificarse como &apos;interruptor de fallo a tierra&apos;.</rdfs:comment>
        <rdfs:label xml:lang="es">Interruptor de Corriente Residual</rdfs:label>
        <rdfs:label xml:lang="en">Residual Current Switch</rdfs:label>
    </owl:Class>
    


    <!-- https://w3id.org/mep#ResidualCurrentTrippingUnit -->


    <owl:Class rdf:about="https://w3id.org/mep#ResidualCurrentTrippingUnit">
        <rdfs:subClassOf rdf:resource="https://w3id.org/mep#ProtectiveDeviceTrippingUnit"/>
        <rdfs:comment xml:lang="en">A tripping unit activated by residual current detection.</rdfs:comment>
        <rdfs:comment xml:lang="es">Una unidad de disparo activada por detección de corriente residual.</rdfs:comment>
        <rdfs:label xml:lang="en">Residual Current Tripping Unit</rdfs:label>
        <rdfs:label xml:lang="es">Unidad de Disparo de Corriente Residual</rdfs:label>
    </owl:Class>
    


    <!-- https://w3id.org/mep#RigidDuctSegment -->


    <owl:Class rdf:about="https://w3id.org/mep#RigidDuctSegment">
        <rdfs:subClassOf rdf:resource="https://w3id.org/mep#DuctSegment"/>
        <rdfs:comment xml:lang="en">A rigid segment is a continuous linear segment of duct that cannot be deformed.</rdfs:comment>
        <rdfs:comment xml:lang="es">Un segmento rígido es un segmento lineal continuo de conducto que no puede deformarse.</rdfs:comment>
        <rdfs:label xml:lang="en">Rigid Duct Segment</rdfs:label>
        <rdfs:label xml:lang="es">Segmento de Conducto Rigido</rdfs:label>
    </owl:Class>
    


    <!-- https://w3id.org/mep#RigidPipeSegment -->


    <owl:Class rdf:about="https://w3id.org/mep#RigidPipeSegment">
        <rdfs:subClassOf rdf:resource="https://w3id.org/mep#PipeSegment"/>
        <rdfs:comment xml:lang="en">A rigid segment is continuous linear segment of pipe that cannot be deformed.</rdfs:comment>
        <rdfs:comment xml:lang="es">Un segmento rígido es un segmento lineal continuo de tubería que no puede deformarse.</rdfs:comment>
        <rdfs:label xml:lang="en">Rigid Pipe Segment</rdfs:label>
        <rdfs:label xml:lang="es">Segmento de Tuberia Rigido</rdfs:label>
    </owl:Class>
    


    <!-- https://w3id.org/mep#RollingPiston -->


    <owl:Class rdf:about="https://w3id.org/mep#RollingPiston">
        <rdfs:subClassOf rdf:resource="https://w3id.org/mep#Compressor"/>
        <rdfs:comment xml:lang="es">Compresor rotativo de desplazamiento positivo que utiliza un rodillo montado en la excéntrica de un eje con una sola paleta en la carcasa cilíndrica no giratoria.</rdfs:comment>
        <rdfs:comment xml:lang="en">Positive-displacement rotary compressor using a roller mounted on the eccentric of a shaft with a single vane in the nonrotating cylindrical housing.</rdfs:comment>
        <rdfs:label xml:lang="es">Piston Rodante</rdfs:label>
        <rdfs:label xml:lang="en">Rolling Piston</rdfs:label>
    </owl:Class>
    


    <!-- https://w3id.org/mep#RoofDrain -->


    <owl:Class rdf:about="https://w3id.org/mep#RoofDrain">
        <rdfs:subClassOf rdf:resource="https://w3id.org/mep#WasteTerminal"/>
        <rdfs:comment xml:lang="es">Accesorio de tubería, instalado en el techo, que recoge el agua de lluvia para descargarla al sistema de aguas pluviales.</rdfs:comment>
        <rdfs:comment xml:lang="en">Pipe fitting, set into the roof, that collects rainwater for discharge into the rainwater system.</rdfs:comment>
        <rdfs:label xml:lang="es">Desagüe de Techo</rdfs:label>
        <rdfs:label xml:lang="en">Roof Drain</rdfs:label>
    </owl:Class>
    


    <!-- https://w3id.org/mep#RooftopUnit -->


    <owl:Class rdf:about="https://w3id.org/mep#RooftopUnit">
        <rdfs:subClassOf rdf:resource="https://w3id.org/mep#UnitaryEquipment"/>
        <rdfs:comment xml:lang="en">A packaged assembly that is either field-erected or manufactured atop the roof of a large residential or commercial building and acts as a unitary component.</rdfs:comment>
        <rdfs:comment xml:lang="es">Un conjunto empaquetado que se construye in-situ o fabricado sobre el techo de un gran edificio residencial o comercial y actúa como un componente unitario.</rdfs:comment>
        <rdfs:label xml:lang="en">Rooftop Unit</rdfs:label>
        <rdfs:label xml:lang="es">Unidad de Azotea</rdfs:label>
    </owl:Class>
    


    <!-- https://w3id.org/mep#RotaryCompressor -->


    <owl:Class rdf:about="https://w3id.org/mep#RotaryCompressor">
        <rdfs:subClassOf rdf:resource="https://w3id.org/mep#Compressor"/>
        <rdfs:comment xml:lang="es">Compresor de desplazamiento positivo que utiliza un dispositivo de rodillo o rotor.</rdfs:comment>
        <rdfs:comment xml:lang="en">Positive-displacement compressor using a roller or rotor device.</rdfs:comment>
        <rdfs:label xml:lang="es">Compresor Rotativo</rdfs:label>
        <rdfs:label xml:lang="en">Rotary Compressor</rdfs:label>
    </owl:Class>
    


    <!-- https://w3id.org/mep#RotaryVaneCompressor -->


    <owl:Class rdf:about="https://w3id.org/mep#RotaryVaneCompressor">
        <rdfs:subClassOf rdf:resource="https://w3id.org/mep#Compressor"/>
        <rdfs:comment xml:lang="es">Compresor rotativo de desplazamiento positivo que utiliza un rodillo montado en la excéntrica de un eje con múltiples paletas en la carcasa cilíndrica no basculante.</rdfs:comment>
        <rdfs:comment xml:lang="en">Positive-displacement rotary compressor using a roller mounted on the eccentric of a shaft with multiple vanes in the nontotating cylindrical housing.</rdfs:comment>
        <rdfs:label xml:lang="es">Compresor Rotativo de Paletas</rdfs:label>
        <rdfs:label xml:lang="en">Rotary Vane Compressor</rdfs:label>
    </owl:Class>
    


    <!-- https://w3id.org/mep#RotaryWheel -->


    <owl:Class rdf:about="https://w3id.org/mep#RotaryWheel">
        <rdfs:subClassOf rdf:resource="https://w3id.org/mep#AirToAirHeatRecovery"/>
        <rdfs:comment xml:lang="en">A heat wheel with a revolving cylinder filled with an air-permeable medium having a large internal surface area.</rdfs:comment>
        <rdfs:comment xml:lang="es">Rueda térmica con un cilindro giratorio lleno de un medio permeable al aire que tiene una gran superficie interna.</rdfs:comment>
        <rdfs:label xml:lang="en">Rotary Wheel</rdfs:label>
        <rdfs:label xml:lang="es">Rueda Rotatoria</rdfs:label>
    </owl:Class>
    


    <!-- https://w3id.org/mep#RoundSilencer -->


    <owl:Class rdf:about="https://w3id.org/mep#RoundSilencer">
        <rdfs:subClassOf rdf:resource="https://w3id.org/mep#DuctSilencer"/>
        <rdfs:comment xml:lang="en">Round duct silencer type.</rdfs:comment>
        <rdfs:comment xml:lang="es">Tipo de silenciador de conducto redondo.</rdfs:comment>
        <rdfs:label xml:lang="en">Round Silencer</rdfs:label>
        <rdfs:label xml:lang="es">Silenciador Redondo</rdfs:label>
    </owl:Class>
    


    <!-- https://w3id.org/mep#Router -->


    <owl:Class rdf:about="https://w3id.org/mep#Router">
        <rdfs:subClassOf rdf:resource="https://w3id.org/mep#CommunicationsAppliance"/>
        <rdfs:comment xml:lang="en">A router is a networking device whose software and hardware are usually tailored to the tasks of routing and forwarding information. For example, on the Internet, information is directed to various paths by routers.</rdfs:comment>
        <rdfs:comment xml:lang="es">Un router es un dispositivo de red cuyo software y hardware suelen estar adaptados a las tareas de encaminamiento y reenvío de información.  Por ejemplo, en Internet, los routers dirigen la información a varias rutas.</rdfs:comment>
        <rdfs:label xml:lang="en">Router</rdfs:label>
        <rdfs:label xml:lang="es">Router</rdfs:label>
    </owl:Class>
    


    <!-- https://w3id.org/mep#Run-aroundCoilLoop -->


    <owl:Class rdf:about="https://w3id.org/mep#Run-aroundCoilLoop">
        <rdfs:subClassOf rdf:resource="https://w3id.org/mep#AirToAirHeatRecovery"/>
        <rdfs:comment xml:lang="en">A typical coil energy recovery loop places extended surface, finned tube water coils in the supply and exhaust airstreams of a building.</rdfs:comment>
        <rdfs:comment xml:lang="es">Un circuito de recuperación de energía de serpentín típico coloca serpentines de agua de tubos con aletas de superficie extendida en las corrientes de aire de suministro y escape de un edificio.</rdfs:comment>
        <rdfs:label xml:lang="es">Bucle de Bobina de Intercambio</rdfs:label>
        <rdfs:label xml:lang="en">Run-around Coil Loop</rdfs:label>
    </owl:Class>
    


    <!-- https://w3id.org/mep#SanitaryTerminal -->


    <owl:Class rdf:about="https://w3id.org/mep#SanitaryTerminal">
        <rdfs:subClassOf rdf:resource="https://w3id.org/mep#FlowTerminal"/>
        <rdfs:comment xml:lang="en">A sanitary terminal is a fixed appliance or terminal usually supplied with water and used for drinking, cleaning or foul water disposal or that is an item of equipment directly used with such an appliance or terminal.</rdfs:comment>
        <rdfs:comment xml:lang="es">Un terminal sanitario es un aparato o terminal fijo alimentado habitualmente con agua y utilizado para beber, limpiar o evacuar aguas sucias o que es un elemento del equipo utilizado directamente con dicho aparato o terminal.</rdfs:comment>
        <rdfs:label xml:lang="en">Sanitary Terminal</rdfs:label>
        <rdfs:label xml:lang="es">Terminal Sanitario</rdfs:label>
    </owl:Class>
    


    <!-- https://w3id.org/mep#SantirayFountain -->


    <owl:Class rdf:about="https://w3id.org/mep#SantirayFountain">
        <rdfs:subClassOf rdf:resource="https://w3id.org/mep#SanitaryTerminal"/>
        <rdfs:comment xml:lang="en">A sanitary terminal that provides a low pressure jet of water for a specific purpose.</rdfs:comment>
        <rdfs:comment xml:lang="es">Terminal sanitario que proporciona un chorro de agua a baja presión para un fin específico.</rdfs:comment>
        <rdfs:label xml:lang="es">Fuente Sanitaria</rdfs:label>
        <rdfs:label xml:lang="en">Santiray Fountain</rdfs:label>
    </owl:Class>
    


    <!-- https://w3id.org/mep#Scanner -->


    <owl:Class rdf:about="https://w3id.org/mep#Scanner">
        <rdfs:subClassOf rdf:resource="https://w3id.org/mep#CommunicationsAppliance"/>
        <rdfs:comment xml:lang="en">A machine that has the primary function of scanning the content of printed matter and converting it to digital format that can be stored in a computer.</rdfs:comment>
        <rdfs:comment xml:lang="es">Máquina cuya función principal es escanear el contenido de un documento impreso y convertirlo en formato digital que pueda almacenarse en un ordenador.</rdfs:comment>
        <rdfs:label xml:lang="es">Scaner</rdfs:label>
        <rdfs:label xml:lang="en">Scanner</rdfs:label>
    </owl:Class>
    


    <!-- https://w3id.org/mep#ScrewConveyor -->


    <owl:Class rdf:about="https://w3id.org/mep#ScrewConveyor">
        <rdfs:subClassOf rdf:resource="https://w3id.org/mep#ConveyorSegment"/>
        <rdfs:comment xml:lang="en">composed of a longitudinal screw in a trough or pipe that rotates to force media through the segment</rdfs:comment>
        <rdfs:comment xml:lang="es">compuesto por un tornillo longitudinal en un canal o tubo que gira para forzar los medios a través del segmento</rdfs:comment>
        <rdfs:label xml:lang="en">Screw Conveyor</rdfs:label>
        <rdfs:label xml:lang="es">Transportador de Tornillo</rdfs:label>
    </owl:Class>
    


    <!-- https://w3id.org/mep#ScrollCompressor -->


    <owl:Class rdf:about="https://w3id.org/mep#ScrollCompressor">
        <rdfs:subClassOf rdf:resource="https://w3id.org/mep#Compressor"/>
        <rdfs:comment xml:lang="es">Compresor de desplazamiento positivo que utiliza dos elementos en espiral que se acoplan entre sí.</rdfs:comment>
        <rdfs:comment xml:lang="en">Positive-displacement compressor using two inter-fitting, spiral-shaped scroll members.</rdfs:comment>
        <rdfs:label xml:lang="es">Compresor Scroll</rdfs:label>
        <rdfs:label xml:lang="en">Scroll Compressor</rdfs:label>
    </owl:Class>
    


    <!-- https://w3id.org/mep#SecurityCut-offValve -->


    <owl:Class rdf:about="https://w3id.org/mep#SecurityCut-offValve">
        <rdfs:subClassOf rdf:resource="https://w3id.org/mep#Valve"/>
        <rdfs:comment xml:lang="en">Valve that closes under the action of a safety mechanism such as a drop weight, solenoid etc.</rdfs:comment>
        <rdfs:comment xml:lang="es">Válvula que se cierra bajo la acción de un mecanismo de seguridad como un peso, solenoide, etc.</rdfs:comment>
        <rdfs:label xml:lang="en">Security Cut-off Valve</rdfs:label>
        <rdfs:label xml:lang="es">Valvula de Seguridad</rdfs:label>
    </owl:Class>
    


    <!-- https://w3id.org/mep#SecurityLightning -->


    <owl:Class rdf:about="https://w3id.org/mep#SecurityLightning">
        <rdfs:subClassOf rdf:resource="https://w3id.org/mep#LightFixture"/>
        <rdfs:comment xml:lang="en">A light fixture having specific purpose of directing occupants in an emergency, such as an illuminated exit sign or emergency flood light.</rdfs:comment>
        <rdfs:comment xml:lang="es">Un artefacto de iluminación que tiene el propósito específico de dirigir a los ocupantes en una emergencia, como una señal de salida iluminada o un reflector de emergencia.</rdfs:comment>
        <rdfs:label xml:lang="es">Iluminación de seguridad</rdfs:label>
        <rdfs:label xml:lang="en">Security Lightning</rdfs:label>
    </owl:Class>
    


    <!-- https://w3id.org/mep#SelectorSwitch -->


    <owl:Class rdf:about="https://w3id.org/mep#SelectorSwitch">
        <rdfs:subClassOf rdf:resource="https://w3id.org/mep#SwitchingDevice"/>
        <rdfs:comment xml:lang="en">A selector switch has multiple positions, and may change the source or level of power or other setting (according to the switched port type).</rdfs:comment>
        <rdfs:comment xml:lang="es">Un conmutador selector tiene varias posiciones y puede cambiar la fuente o el nivel de potencia u otro ajuste (según el tipo de puerto conmutado).</rdfs:comment>
        <rdfs:label xml:lang="es">Conmutador Selector</rdfs:label>
        <rdfs:label xml:lang="en">Selector Switch</rdfs:label>
    </owl:Class>
    


    <!-- https://w3id.org/mep#Semi-hermeticCompressor -->


    <owl:Class rdf:about="https://w3id.org/mep#Semi-hermeticCompressor">
        <rdfs:subClassOf rdf:resource="https://w3id.org/mep#Compressor"/>
        <rdfs:comment xml:lang="es">Compresor alternativo de desplazamiento positivo en el que los compresores herméticos utilizan una construcción atornillada susceptible de reparación in situ.</rdfs:comment>
        <rdfs:comment xml:lang="en">Positive-displacement reciprocating compressor where the hermetic compressors use bolted construction amenable to field repair.</rdfs:comment>
        <rdfs:label xml:lang="es">Compresor Semi-hermetico</rdfs:label>
        <rdfs:label xml:lang="en">Semi-hermetic Compressor</rdfs:label>
    </owl:Class>
    


    <!-- https://w3id.org/mep#Sensor -->


    <owl:Class rdf:about="https://w3id.org/mep#Sensor">
        <rdfs:subClassOf rdf:resource="https://w3id.org/mep#DistributionControlElement"/>
        <rdfs:comment xml:lang="en">A sensor is a device that measures a physical quantity and converts it into a signal which can be read by an observer or by an instrument.</rdfs:comment>
        <rdfs:comment xml:lang="es">Un sensor es un dispositivo que mide una magnitud física y la convierte en una señal que puede ser leída por un observador o por un instrumento.</rdfs:comment>
        <rdfs:label xml:lang="en">Sensor</rdfs:label>
        <rdfs:label xml:lang="es">Sensor</rdfs:label>
    </owl:Class>
    


    <!-- https://w3id.org/mep#ServiceGPRSSupportNode -->


    <owl:Class rdf:about="https://w3id.org/mep#ServiceGPRSSupportNode">
        <rdfs:subClassOf rdf:resource="https://w3id.org/mep#MobileTelecommunicationsAppliance"/>
        <rdfs:comment xml:lang="es">El nodo de soporte GPRS de servicio (SGSN) es un componente de la red central GPRS. Es el nodo de soporte GPRS del servicio de estación móvil, y puede realizar la gestión de la movilidad y el enrutamiento y transferencia de paquetes.</rdfs:comment>
        <rdfs:comment xml:lang="en">The service GPRS support node (SGSN) is a component of the GPRS core network. It is the GPRS support node of mobile station service, and it can achieve mobility management and packet routing and transfer.</rdfs:comment>
        <rdfs:label xml:lang="es">Nodeo de Soporte GPRS de Servicio</rdfs:label>
        <rdfs:label xml:lang="en">Service GPRS Support Node</rdfs:label>
    </owl:Class>
    


    <!-- https://w3id.org/mep#ShellandCoilEvaporator -->


    <owl:Class rdf:about="https://w3id.org/mep#ShellandCoilEvaporator">
        <rdfs:subClassOf rdf:resource="https://w3id.org/mep#Evaporator"/>
        <rdfs:comment xml:lang="es">Evaporador en el que el refrigerante se evapora dentro de un simple tubo enrollado sumergido en el fluido a enfriar.</rdfs:comment>
        <rdfs:comment xml:lang="en">Evaporator in which refrigerant evaporates inside a simple coiled tube immersed in the fluid to be cooled.</rdfs:comment>
        <rdfs:label xml:lang="es">Evaporadorde Carcasa y Serpentin</rdfs:label>
        <rdfs:label xml:lang="en">Shell and Coil Evaporator</rdfs:label>
    </owl:Class>
    


    <!-- https://w3id.org/mep#ShellandTubeExchanger -->


    <owl:Class rdf:about="https://w3id.org/mep#ShellandTubeExchanger">
        <rdfs:subClassOf rdf:resource="https://w3id.org/mep#HeatExchanger"/>
        <rdfs:comment xml:lang="es">Intercambiador de tubo y carcasa.</rdfs:comment>
        <rdfs:comment xml:lang="en">Shell and Tube heat exchanger.</rdfs:comment>
        <rdfs:label xml:lang="es">Intercambiador de Tubo y Carcasa</rdfs:label>
        <rdfs:label xml:lang="en">Shell and Tube Exchanger</rdfs:label>
    </owl:Class>
    


    <!-- https://w3id.org/mep#Shower -->


    <owl:Class rdf:about="https://w3id.org/mep#Shower">
        <rdfs:subClassOf rdf:resource="https://w3id.org/mep#SanitaryTerminal"/>
        <rdfs:comment xml:lang="es">Instalación o aparato de aguas residuales que emite un chorro de agua para lavar el cuerpo humano.</rdfs:comment>
        <rdfs:comment xml:lang="en">Installation or waste water appliance that emits a spray of water to wash the human body.</rdfs:comment>
        <rdfs:label xml:lang="es">Ducha</rdfs:label>
        <rdfs:label xml:lang="en">Shower</rdfs:label>
    </owl:Class>
    


    <!-- https://w3id.org/mep#Signal -->


    <owl:Class rdf:about="https://w3id.org/mep#Signal">
        <rdfs:subClassOf rdf:resource="https://w3id.org/mep#FlowTerminal"/>
        <rdfs:comment xml:lang="en">A signal is an active device that conveys information or instructions to users, by means of an audio, visual signal or a combination of both. The primary distinction from an Sign is that a signal is active and therefore a subtype of Flow Terminal usually requiring power and data connections for its operation. An instance of Signal represents a singular signalling device in a larger assembled unit or connected system, such as an individual frame within a railway signal, a single light unit in a traffic light system or an audio signal or light mounted on a navigational buoy. Signals can be physically aggregated together into an assembly which can include multiple signal instances (and also sign instances) and the associated supporting structural elements such as a simple pole or a rigid frame gantry (see Signal Assembly for examples). Signals can be logically (functionally) grouped together into a signalling system (a type of distribution system) to represent a connected group of signals for example a group of traffic lights controlling an road intersection.</rdfs:comment>
        <rdfs:comment xml:lang="es">Una Dispositivo de Señalizacion es un dispositivo activo que transmite información o instrucciones a los usuarios, mediante una señal acústica, visual o una combinación de ambas. La principal distinción con respecto a una Señal es que una señal es activa y, por tanto, un subtipo de Terminal de Flujo que suele requerir conexiones de alimentación y datos para su funcionamiento. Un caso de Señal representa un dispositivo de señalización singular en una unidad ensamblada más grande o un sistema conectado, como un marco individual dentro de una señal ferroviaria, una sola unidad luminosa en un sistema de semáforos o una señal acústica o luminosa montada en una boya de navegación. Las señales pueden agruparse físicamente en un conjunto que puede incluir varias instancias de señales (y también instancias de señales) y los elementos estructurales de soporte asociados, como un poste simple o un pórtico de estructura rígida (véanse ejemplos en Conjunto de señales). Las señales pueden agruparse lógicamente (funcionalmente) en un sistema de señalización (un tipo de sistema de distribución) para representar un grupo conectado de señales, por ejemplo, un grupo de semáforos que controlan una intersección de carreteras.</rdfs:comment>
        <rdfs:label xml:lang="es">Dispositivo de Señalizacion</rdfs:label>
        <rdfs:label xml:lang="en">Signaling Device</rdfs:label>
    </owl:Class>
    


    <!-- https://w3id.org/mep#SingleScrewCompressor -->


    <owl:Class rdf:about="https://w3id.org/mep#SingleScrewCompressor">
        <rdfs:subClassOf rdf:resource="https://w3id.org/mep#Compressor"/>
        <rdfs:comment xml:lang="es">Compresor alternativo de desplazamiento positivo en el que los compresores herméticos utilizan una construcción atornillada susceptible de reparación in situ.</rdfs:comment>
        <rdfs:comment xml:lang="en">Positive-displacement reciprocating compressor where the hermetic compressors use bolted construction amenable to field repair.</rdfs:comment>
        <rdfs:label xml:lang="es">Compresor monotornillo</rdfs:label>
        <rdfs:label xml:lang="en">Single Screw Compressor</rdfs:label>
    </owl:Class>
    


    <!-- https://w3id.org/mep#SingleStageCompressor -->


    <owl:Class rdf:about="https://w3id.org/mep#SingleStageCompressor">
        <rdfs:subClassOf rdf:resource="https://w3id.org/mep#Compressor"/>
        <rdfs:comment xml:lang="es">Compresor alternativo de desplazamiento positivo en el que el vapor se comprime en una sola etapa.</rdfs:comment>
        <rdfs:comment xml:lang="en">Positive-displacement reciprocating compressor where vapor is compressed in a single stage.</rdfs:comment>
        <rdfs:label xml:lang="es">Compresor de Una Etapa</rdfs:label>
        <rdfs:label xml:lang="en">Single Stage Compressor</rdfs:label>
    </owl:Class>
    


    <!-- https://w3id.org/mep#Sink -->


    <owl:Class rdf:about="https://w3id.org/mep#Sink">
        <rdfs:subClassOf rdf:resource="https://w3id.org/mep#SanitaryTerminal"/>
        <rdfs:comment xml:lang="es">Aparato de aguas residuales para recibir, retener o evacuar líquidos domésticos, culinarios, de laboratorio o de procesos industriales.</rdfs:comment>
        <rdfs:comment xml:lang="en">Waste water appliance for receiving, retaining or disposing of domestic, culinary, laboratory or industrial process liquids.</rdfs:comment>
        <rdfs:label xml:lang="es">Fregadero</rdfs:label>
        <rdfs:label xml:lang="en">Sink</rdfs:label>
    </owl:Class>
    


    <!-- https://w3id.org/mep#Siren -->


    <owl:Class rdf:about="https://w3id.org/mep#Siren">
        <rdfs:subClassOf rdf:resource="https://w3id.org/mep#Alarm"/>
        <rdfs:comment xml:lang="en">An audible alarm.</rdfs:comment>
        <rdfs:comment xml:lang="es">Una alarma sonora.</rdfs:comment>
        <rdfs:label xml:lang="en">Siren</rdfs:label>
        <rdfs:label xml:lang="es">Sirena</rdfs:label>
    </owl:Class>
    


    <!-- https://w3id.org/mep#SmokeDamper -->


    <owl:Class rdf:about="https://w3id.org/mep#SmokeDamper">
        <rdfs:subClassOf rdf:resource="https://w3id.org/mep#Damper"/>
        <rdfs:comment xml:lang="es">Compuerta cortahumo utilizada para evitar la propagación del humo. Suele accionarse mediante un detector de humo de un sistema de automatización de edificios.</rdfs:comment>
        <rdfs:comment xml:lang="en">Smoke damper used to prevent the spread of smoke. Commonly operated by a smoke detector of a building automation system.</rdfs:comment>
        <rdfs:label xml:lang="es">Compuerta Cortahumo</rdfs:label>
        <rdfs:label xml:lang="en">Smoke Damper</rdfs:label>
    </owl:Class>
    


    <!-- https://w3id.org/mep#SmokeSensor -->


    <owl:Class rdf:about="https://w3id.org/mep#SmokeSensor">
        <rdfs:subClassOf rdf:resource="https://w3id.org/mep#Sensor"/>
        <rdfs:comment xml:lang="en">A device that senses or detects smoke.</rdfs:comment>
        <rdfs:comment xml:lang="es">Dispositivo que detecta el humo.</rdfs:comment>
        <rdfs:label xml:lang="es">Sensor de Humo</rdfs:label>
        <rdfs:label xml:lang="en">Smoke Sensor</rdfs:label>
    </owl:Class>
    


    <!-- https://w3id.org/mep#SnowDepthSensor -->


    <owl:Class rdf:about="https://w3id.org/mep#SnowDepthSensor">
        <rdfs:subClassOf rdf:resource="https://w3id.org/mep#Sensor"/>
        <rdfs:comment xml:lang="en">A device that senses or measures the depth of snowfall.</rdfs:comment>
        <rdfs:comment xml:lang="es">Dispositivo que detecta o mide la profundidad de las nevadas.</rdfs:comment>
        <rdfs:label xml:lang="es">Sensor de Profundidad de Nieve</rdfs:label>
        <rdfs:label xml:lang="en">Snow Depth Sensor</rdfs:label>
    </owl:Class>
    


    <!-- https://w3id.org/mep#SolarCollector -->


    <owl:Class rdf:about="https://w3id.org/mep#SolarCollector">
        <rdfs:subClassOf rdf:resource="https://w3id.org/mep#SolarDevice"/>
        <rdfs:comment xml:lang="en">A device that converts solar radiation into thermal energy (heating water, etc.).</rdfs:comment>
        <rdfs:comment xml:lang="es">Dispositivo que transforma la radiación solar en energía térmica (calentamiento de agua, etc.).</rdfs:comment>
        <rdfs:label xml:lang="es">Colector Solar</rdfs:label>
        <rdfs:label xml:lang="en">Solar Collector</rdfs:label>
    </owl:Class>
    


    <!-- https://w3id.org/mep#SolarDevice -->


    <owl:Class rdf:about="https://w3id.org/mep#SolarDevice">
        <rdfs:subClassOf rdf:resource="https://w3id.org/mep#EnergyConversionDevice"/>
        <rdfs:comment xml:lang="en">A solar device converts solar radiation into other energy such as electric current or thermal energy.</rdfs:comment>
        <rdfs:comment xml:lang="es">Un dispositivo solar convierte la radiación solar en otro tipo de energía, como corriente eléctrica o energía térmica.</rdfs:comment>
        <rdfs:label xml:lang="es">Dispositivo Solar</rdfs:label>
        <rdfs:label xml:lang="en">Solar Device</rdfs:label>
    </owl:Class>
    


    <!-- https://w3id.org/mep#SolarPanel -->


    <owl:Class rdf:about="https://w3id.org/mep#SolarPanel">
        <rdfs:subClassOf rdf:resource="https://w3id.org/mep#SolarDevice"/>
        <rdfs:comment xml:lang="en">A device that converts solar radiation into electric current.</rdfs:comment>
        <rdfs:comment xml:lang="es">Dispositivo que convierte la radiación solar en corriente eléctrica.</rdfs:comment>
        <rdfs:label xml:lang="es">Panel Solar</rdfs:label>
        <rdfs:label xml:lang="en">Solar Panel</rdfs:label>
    </owl:Class>
    


    <!-- https://w3id.org/mep#SoundSensor -->


    <owl:Class rdf:about="https://w3id.org/mep#SoundSensor">
        <rdfs:subClassOf rdf:resource="https://w3id.org/mep#Sensor"/>
        <rdfs:comment xml:lang="en">A device that senses or detects sound.</rdfs:comment>
        <rdfs:comment xml:lang="es">Dispositivo que percibe o detecta el sonido.</rdfs:comment>
        <rdfs:label xml:lang="es">Sensor de Sonido</rdfs:label>
        <rdfs:label xml:lang="en">Sound Sensor</rdfs:label>
    </owl:Class>
    


    <!-- https://w3id.org/mep#SpaceHeater -->


    <owl:Class rdf:about="https://w3id.org/mep#SpaceHeater">
        <rdfs:subClassOf rdf:resource="https://w3id.org/mep#FlowTerminal"/>
        <rdfs:comment xml:lang="es">Los calefactores utilizan una combinación de radiación y/o convección natural mediante una fuente de calor como la electricidad, el vapor o el agua caliente para calentar un espacio o zona limitados. Algunos ejemplos de calefactores son los radiadores, los convectores, los zócalos y los tubos con aletas.</rdfs:comment>
        <rdfs:comment xml:lang="en">Space heaters utilize a combination of radiation and/or natural convection using a heating source such as electricity, steam or hot water to heat a limited space or area. Examples of space heaters include radiators, convectors, baseboard and finned-tube heaters.</rdfs:comment>
        <rdfs:label xml:lang="es">Calefactores</rdfs:label>
        <rdfs:label xml:lang="en">Space Heater</rdfs:label>
    </owl:Class>
    


    <!-- https://w3id.org/mep#SparkGap -->


    <owl:Class rdf:about="https://w3id.org/mep#SparkGap">
        <rdfs:subClassOf rdf:resource="https://w3id.org/mep#ProtectiveDevice"/>
        <rdfs:comment xml:lang="en">A spark gap is a device used to connect a circuit to earth in the event of a fault in live circuits.</rdfs:comment>
        <rdfs:comment xml:lang="es">Una vía de chispas es un dispositivo utilizado para conectar un circuito a tierra en caso de avería en circuitos con tensión.</rdfs:comment>
        <rdfs:label xml:lang="en">Spark Gap</rdfs:label>
        <rdfs:label xml:lang="es">Via de Chispas</rdfs:label>
    </owl:Class>
    


    <!-- https://w3id.org/mep#Speaker -->


    <owl:Class rdf:about="https://w3id.org/mep#Speaker">
        <rdfs:subClassOf rdf:resource="https://w3id.org/mep#AudioVisualAppliance"/>
        <rdfs:comment xml:lang="en">A loudspeaker, speaker, or speaker system is an electroacoustical transducer that converts an electrical signal to sound.</rdfs:comment>
        <rdfs:comment xml:lang="es">Un altavoz, altavoz o sistema de altavoces es un transductor electroacústico que convierte una señal eléctrica en sonido.</rdfs:comment>
        <rdfs:label xml:lang="es">Altavoz</rdfs:label>
        <rdfs:label xml:lang="en">Speaker</rdfs:label>
    </owl:Class>
    


    <!-- https://w3id.org/mep#SplitCasePump -->


    <owl:Class rdf:about="https://w3id.org/mep#SplitCasePump">
        <rdfs:subClassOf rdf:resource="https://w3id.org/mep#Pump"/>
        <rdfs:comment xml:lang="en">A Split Case pump, when mounted horizontally, has an inlet and outlet on each side of the impeller. The impeller can be easily accessed by removing the front of the impeller casing. It may have a direct or close-coupled motor.</rdfs:comment>
        <rdfs:comment xml:lang="es">Una bomba de cámara partida, cuando se monta horizontalmente, tiene una entrada y una salida a cada lado del impulsor. Se puede acceder fácilmente al impulsor retirando la parte delantera de la carcasa del impulsor. Puede tener un motor directo o acoplado.</rdfs:comment>
        <rdfs:label xml:lang="es">Bomba de Camara Partida</rdfs:label>
        <rdfs:label xml:lang="en">Split Case Pump</rdfs:label>
    </owl:Class>
    


    <!-- https://w3id.org/mep#SplitSystem -->


    <owl:Class rdf:about="https://w3id.org/mep#SplitSystem">
        <rdfs:subClassOf rdf:resource="https://w3id.org/mep#UnitaryEquipment"/>
        <rdfs:comment xml:lang="es"></rdfs:comment>
        <rdfs:comment xml:lang="en">A system which separates the compressor from the evaporator, but acts as a unitary component typically within residential or light commercial applications.</rdfs:comment>
        <rdfs:label xml:lang="es">Sistema Separado</rdfs:label>
        <rdfs:label xml:lang="en">Split System</rdfs:label>
    </owl:Class>
    


    <!-- https://w3id.org/mep#Spool -->


    <owl:Class rdf:about="https://w3id.org/mep#Spool">
        <rdfs:subClassOf rdf:resource="https://w3id.org/mep#PipeSegment"/>
        <rdfs:comment xml:lang="en">A type of rigid segment that is typically shorter and used for providing connectivity within a piping network.</rdfs:comment>
        <rdfs:comment xml:lang="es">Tipo de segmento rígido que suele ser más corto y se utiliza para proporcionar conectividad dentro de una red de tuberías.</rdfs:comment>
        <rdfs:label xml:lang="es">Carrete</rdfs:label>
        <rdfs:label xml:lang="en">Spool</rdfs:label>
    </owl:Class>
    


    <!-- https://w3id.org/mep#Sprinkler -->


    <owl:Class rdf:about="https://w3id.org/mep#Sprinkler">
        <rdfs:subClassOf rdf:resource="https://w3id.org/mep#FireSuppressionTerminal"/>
        <rdfs:comment xml:lang="en">Device for sprinkling water from a pipe under pressure over an area.</rdfs:comment>
        <rdfs:comment xml:lang="es">Dispositivo que dispersa agua desde una tubería bajo presión sobre un área</rdfs:comment>
        <rdfs:label xml:lang="es">Rociador</rdfs:label>
        <rdfs:label xml:lang="en">Sprinkler</rdfs:label>
    </owl:Class>
    


    <!-- https://w3id.org/mep#StackTerminal -->


    <owl:Class rdf:about="https://w3id.org/mep#StackTerminal">
        <rdfs:subClassOf rdf:resource="https://w3id.org/mep#FlowTerminal"/>
        <rdfs:comment xml:lang="en">A stack terminal is placed at the top of a ventilating stack (such as to prevent ingress by birds or rainwater) or rainwater pipe (to act as a collector or hopper for discharge from guttering).</rdfs:comment>
        <rdfs:comment xml:lang="es">El terminal de chimenea se coloca en la parte superior de una chimenea de ventilación (por ejemplo, para evitar la entrada de pájaros o agua de lluvia) o de una tubería de aguas pluviales (para que actúe como colector o tolva de descarga de los canalones).</rdfs:comment>
        <rdfs:label xml:lang="en">Stack Terminal</rdfs:label>
        <rdfs:label xml:lang="es">Terminal de Chimenea</rdfs:label>
    </owl:Class>
    


    <!-- https://w3id.org/mep#StandaloneGenerator -->


    <owl:Class rdf:about="https://w3id.org/mep#StandaloneGenerator">
        <rdfs:subClassOf rdf:resource="https://w3id.org/mep#ElectricGenerator"/>
        <rdfs:comment xml:lang="en">Electrical generator which does not include its source of kinetic energy, that is, a motor, engine, or turbine are all modeled separately.</rdfs:comment>
        <rdfs:comment xml:lang="es">Los generadores eléctricos que no incluyen su fuente de energía cinética, es decir, un motor, un motor o una turbina, se modelan por separado.</rdfs:comment>
        <rdfs:label xml:lang="es">Generador Independiente</rdfs:label>
        <rdfs:label xml:lang="en">Standalone Generator</rdfs:label>
    </owl:Class>
    


    <!-- https://w3id.org/mep#StartandStopSwitch -->


    <owl:Class rdf:about="https://w3id.org/mep#StartandStopSwitch">
        <rdfs:subClassOf rdf:resource="https://w3id.org/mep#SwitchingDevice"/>
        <rdfs:comment xml:lang="en">A switch for alternatively closing and opening one or more electric circuits.</rdfs:comment>
        <rdfs:comment xml:lang="es">Un interruptor para cerrar y abrir alternativamente uno o varios circuitos eléctricos.</rdfs:comment>
        <rdfs:label xml:lang="es">Conmutador de Inicio y Parada</rdfs:label>
        <rdfs:label xml:lang="en">Start and Stop Switch</rdfs:label>
    </owl:Class>
    


    <!-- https://w3id.org/mep#Starter -->


    <owl:Class rdf:about="https://w3id.org/mep#Starter">
        <rdfs:subClassOf rdf:resource="https://w3id.org/mep#SwitchingDevice"/>
        <rdfs:comment xml:lang="en">A starter is a switch which in the closed position controls the application of power to an electrical device.</rdfs:comment>
        <rdfs:comment xml:lang="es">Un arranque es un interruptor que, en posición cerrada, controla la aplicación de energía a un dispositivo eléctrico.</rdfs:comment>
        <rdfs:label xml:lang="es">Arranque</rdfs:label>
        <rdfs:label xml:lang="en">Starter</rdfs:label>
    </owl:Class>
    


    <!-- https://w3id.org/mep#SteamBoiler -->


    <owl:Class rdf:about="https://w3id.org/mep#SteamBoiler">
        <rdfs:subClassOf rdf:resource="https://w3id.org/mep#Boiler"/>
        <rdfs:comment xml:lang="es">Cladera de Vapor</rdfs:comment>
        <rdfs:comment xml:lang="en">Steam boiler.</rdfs:comment>
        <rdfs:label xml:lang="es">Cladera de Vapor</rdfs:label>
        <rdfs:label xml:lang="en">Steam Boiler</rdfs:label>
    </owl:Class>
    


    <!-- https://w3id.org/mep#SteamHeatingCoil -->


    <owl:Class rdf:about="https://w3id.org/mep#SteamHeatingCoil">
        <rdfs:subClassOf rdf:resource="https://w3id.org/mep#Coil"/>
        <rdfs:comment xml:lang="en">Heating coil using steam as heating source.</rdfs:comment>
        <rdfs:comment xml:lang="es">Serpentín calefactor que utiliza vapor como fuente de calor.</rdfs:comment>
        <rdfs:label xml:lang="es">Serpentin Calefactor de Vapor</rdfs:label>
        <rdfs:label xml:lang="en">Steam Heating Coil</rdfs:label>
    </owl:Class>
    


    <!-- https://w3id.org/mep#SteamTrap -->


    <owl:Class rdf:about="https://w3id.org/mep#SteamTrap">
        <rdfs:subClassOf rdf:resource="https://w3id.org/mep#Valve"/>
        <rdfs:comment xml:lang="es"></rdfs:comment>
        <rdfs:comment xml:lang="en">Valve that restricts flow of steam while allowing condensate to pass through.</rdfs:comment>
        <rdfs:label xml:lang="en">Steam Trap</rdfs:label>
        <rdfs:label xml:lang="es">Trampa de Vapor</rdfs:label>
    </owl:Class>
    


    <!-- https://w3id.org/mep#SteaminjectionHumidifier -->


    <owl:Class rdf:about="https://w3id.org/mep#SteaminjectionHumidifier">
        <rdfs:subClassOf rdf:resource="https://w3id.org/mep#Humidifier"/>
        <rdfs:comment xml:lang="es">El vapor de agua se agrega a la corriente de aire mediante inyección directa de vapor.</rdfs:comment>
        <rdfs:comment xml:lang="en">Water vapor is added into the airstream through direct steam injection.</rdfs:comment>
        <rdfs:label xml:lang="es">Humidificador de Injeccion de Vapor</rdfs:label>
        <rdfs:label xml:lang="en">Steam injection Humidifier</rdfs:label>
    </owl:Class>
    


    <!-- https://w3id.org/mep#SticthWire -->


    <owl:Class rdf:about="https://w3id.org/mep#SticthWire">
        <rdfs:subClassOf rdf:resource="https://w3id.org/mep#CableSegment"/>
        <rdfs:comment xml:lang="en">A stitch wire consists of auxiliary wires and different components (clamp) used in stitched suspension.</rdfs:comment>
        <rdfs:comment xml:lang="es">Un alambre de costura consta de alambres auxiliares y diferentes componentes (abrazadera) que se utilizan en la suspensión de costura.</rdfs:comment>
        <rdfs:label xml:lang="es">Alambre de Puntada</rdfs:label>
        <rdfs:label xml:lang="en">Sticth Wire</rdfs:label>
    </owl:Class>
    


    <!-- https://w3id.org/mep#StopCock -->


    <owl:Class rdf:about="https://w3id.org/mep#StopCock">
        <rdfs:subClassOf rdf:resource="https://w3id.org/mep#Valve"/>
        <rdfs:comment xml:lang="en">An isolating valve used on a domestic water service.</rdfs:comment>
        <rdfs:comment xml:lang="es">Una válvula de aislamiento utilizada en un servicio de agua doméstico.</rdfs:comment>
        <rdfs:label xml:lang="es">LLave de Paso</rdfs:label>
        <rdfs:label xml:lang="en">Stop Cock</rdfs:label>
    </owl:Class>
    


    <!-- https://w3id.org/mep#StorageTank -->


    <owl:Class rdf:about="https://w3id.org/mep#StorageTank">
        <rdfs:subClassOf rdf:resource="https://w3id.org/mep#Tank"/>
        <rdfs:comment xml:lang="en">An open or closed container used for storing a fluid at ambient pressure and from which it can be supplied to the fluid distribution system. There are many examples of storage tanks, such as potable water storage tanks, fuel storage tanks, etc.</rdfs:comment>
        <rdfs:comment xml:lang="es">Recipiente abierto o cerrado que sirve para almacenar un fluido a presión ambiente y desde el que se puede suministrar al sistema de distribución de fluidos. Hay muchos ejemplos de tanques de almacenamiento, como los tanques de almacenamiento de agua potable, los tanques de almacenamiento de combustible, etc.</rdfs:comment>
        <rdfs:label xml:lang="es">Depositode Almacenamiento</rdfs:label>
        <rdfs:label xml:lang="en">Storage Tank</rdfs:label>
    </owl:Class>
    


    <!-- https://w3id.org/mep#Strainer -->


    <owl:Class rdf:about="https://w3id.org/mep#Strainer">
        <rdfs:subClassOf rdf:resource="https://w3id.org/mep#Filter"/>
        <rdfs:comment xml:lang="en">A filter used to remove particulates from a fluid.</rdfs:comment>
        <rdfs:comment xml:lang="es">A filter used to remove particulates from a fluid.</rdfs:comment>
        <rdfs:label xml:lang="es">Colador</rdfs:label>
        <rdfs:label xml:lang="en">Strainer</rdfs:label>
    </owl:Class>
    


    <!-- https://w3id.org/mep#SubmersiblePump -->


    <owl:Class rdf:about="https://w3id.org/mep#SubmersiblePump">
        <rdfs:subClassOf rdf:resource="https://w3id.org/mep#Pump"/>
        <rdfs:comment xml:lang="es">A pump designed to be immersed in a fluid, typically a collection tank.</rdfs:comment>
        <rdfs:comment xml:lang="en">Bomba diseñada para sumergirse en un fluido, normalmente un depósito de recogida.</rdfs:comment>
        <rdfs:label xml:lang="es">Bomba Sumergible</rdfs:label>
        <rdfs:label xml:lang="en">Submersible Pump</rdfs:label>
    </owl:Class>
    


    <!-- https://w3id.org/mep#SubscriberServer -->


    <owl:Class rdf:about="https://w3id.org/mep#SubscriberServer">
        <rdfs:subClassOf rdf:resource="https://w3id.org/mep#MobileTelecommunicationsAppliance"/>
        <rdfs:comment xml:lang="es">Es una base de datos encargada de la gestión de los abonados móviles. Puede ser un centro de autenticación (AuC) o un registro de localización de domicilio (HLR).</rdfs:comment>
        <rdfs:comment xml:lang="en">It is a database in charge of the management of mobile subscribers. It can be an authentication center (AuC) or a home location register (HLR).</rdfs:comment>
        <rdfs:label xml:lang="es">Servidor de Abonados</rdfs:label>
        <rdfs:label xml:lang="en">Subscriber Server</rdfs:label>
    </owl:Class>
    


    <!-- https://w3id.org/mep#Sump -->


    <owl:Class rdf:about="https://w3id.org/mep#Sump">
        <rdfs:subClassOf rdf:resource="https://w3id.org/mep#DistributionChamberElement"/>
        <rdfs:comment xml:lang="es">Cámara empotrada o pequeña en la que se drena el líquido para facilitar su recogida para su eliminación.</rdfs:comment>
        <rdfs:comment xml:lang="en">Recessed or small chamber into which liquid is drained to facilitate its collection for removal.</rdfs:comment>
        <rdfs:label xml:lang="es">Sumidero</rdfs:label>
        <rdfs:label xml:lang="en">Sump</rdfs:label>
    </owl:Class>
    


    <!-- https://w3id.org/mep#SumpPump -->


    <owl:Class rdf:about="https://w3id.org/mep#SumpPump">
        <rdfs:subClassOf rdf:resource="https://w3id.org/mep#Pump"/>
        <rdfs:comment xml:lang="en">A pump designed to sit above a collection tank with a suction inlet extending into the tank.</rdfs:comment>
        <rdfs:comment xml:lang="es">Bomba diseñada para situarse encima de un depósito de recogida con una entrada de aspiración que se extiende hasta el depósito.</rdfs:comment>
        <rdfs:label xml:lang="es">Bomba de Sumidero</rdfs:label>
        <rdfs:label xml:lang="en">Sump Pump</rdfs:label>
    </owl:Class>
    


    <!-- https://w3id.org/mep#SwitchBoard -->


    <owl:Class rdf:about="https://w3id.org/mep#SwitchBoard">
        <rdfs:subClassOf rdf:resource="https://w3id.org/mep#DistributionBoard"/>
        <rdfs:comment xml:lang="en">A distribution point at which switching devices are located.</rdfs:comment>
        <rdfs:comment xml:lang="es">Punto de distribución en el que se encuentran los dispositivos de conmutación.</rdfs:comment>
        <rdfs:label xml:lang="es">Cuadro Switch</rdfs:label>
        <rdfs:label xml:lang="en">Switch Board</rdfs:label>
    </owl:Class>
    


    <!-- https://w3id.org/mep#SwitchDisconnector -->


    <owl:Class rdf:about="https://w3id.org/mep#SwitchDisconnector">
        <rdfs:subClassOf rdf:resource="https://w3id.org/mep#SwitchingDevice"/>
        <rdfs:comment xml:lang="en">A switch disconnector is a switch which in the open position satisfies the isolating requirements specified for a disconnector.</rdfs:comment>
        <rdfs:comment xml:lang="es">Un seccionador interruptor es un interruptor que en posición abierta satisface los requisitos de aislamiento especificados para un seccionador.</rdfs:comment>
        <rdfs:label xml:lang="es">Seccionador Interruptor</rdfs:label>
        <rdfs:label xml:lang="en">Switch Disconnector</rdfs:label>
    </owl:Class>
    


    <!-- https://w3id.org/mep#Switcher -->


    <owl:Class rdf:about="https://w3id.org/mep#Switcher">
        <rdfs:subClassOf rdf:resource="https://w3id.org/mep#AudioVisualAppliance"/>
        <rdfs:comment xml:lang="en">A device that receives audio and/or video signals, switches sources, and transmits signals to downstream devices.</rdfs:comment>
        <rdfs:comment xml:lang="es">Un dispositivo que recibe señales de audio y/o video, cambia fuentes y transmite señales a dispositivos posteriores.</rdfs:comment>
        <rdfs:label xml:lang="es">Intercambiador</rdfs:label>
        <rdfs:label xml:lang="en">Switcher</rdfs:label>
    </owl:Class>
    


    <!-- https://w3id.org/mep#SwitchingDevice -->


    <owl:Class rdf:about="https://w3id.org/mep#SwitchingDevice">
        <rdfs:subClassOf rdf:resource="https://w3id.org/mep#FlowController"/>
        <rdfs:comment xml:lang="en">A switch is used in a cable distribution system (electrical circuit) to control or modulate the flow of electricity. Switches include those used for electrical power, communications, audio-visual, or other distribution system types as determined by the available ports.</rdfs:comment>
        <rdfs:comment xml:lang="es">Un conmutador se utiliza en un sistema de distribución por cable (circuito eléctrico) para controlar o modular el flujo de electricidad. Entre los conmutadores se incluyen los utilizados para energía eléctrica, comunicaciones, audiovisuales u otros tipos de sistemas de distribución, según determinen los puertos disponibles.</rdfs:comment>
        <rdfs:label xml:lang="es">Conmutador</rdfs:label>
        <rdfs:label xml:lang="en">Switching Device</rdfs:label>
    </owl:Class>
    


    <!-- https://w3id.org/mep#SynchronousMotor -->


    <owl:Class rdf:about="https://w3id.org/mep#SynchronousMotor">
        <rdfs:subClassOf rdf:resource="https://w3id.org/mep#ElectricMotor"/>
        <rdfs:comment xml:lang="en">A motor that operates at a constant speed up to full load. The rotor speed is equal to the speed of the rotating magnetic field of the stator; there is no slip.</rdfs:comment>
        <rdfs:comment xml:lang="es">Un motor que funciona a velocidad constante hasta carga completa. La velocidad del rotor es igual a la velocidad del campo magnético giratorio del estator; no hay ningún resbalón.</rdfs:comment>
        <rdfs:label xml:lang="es">Motor Sincrono</rdfs:label>
        <rdfs:label xml:lang="en">Synchronous Motor</rdfs:label>
    </owl:Class>
    


    <!-- https://w3id.org/mep#Tank -->


    <owl:Class rdf:about="https://w3id.org/mep#Tank">
        <rdfs:subClassOf rdf:resource="https://w3id.org/mep#FlowStorageDevice"/>
        <rdfs:comment xml:lang="en">A tank is a vessel or container in which a fluid or gas is stored for later use.</rdfs:comment>
        <rdfs:comment xml:lang="es">Un depósito es un recipiente o contenedor en el que se almacena un fluido o gas para su uso posterior.</rdfs:comment>
        <rdfs:label xml:lang="es">Deposito</rdfs:label>
        <rdfs:label xml:lang="en">Tank</rdfs:label>
    </owl:Class>
    


    <!-- https://w3id.org/mep#Telecommand -->


    <owl:Class rdf:about="https://w3id.org/mep#Telecommand">
        <rdfs:subClassOf rdf:resource="https://w3id.org/mep#CommunicationsAppliance"/>
        <rdfs:comment xml:lang="en">A system sending command to control and monitor the switches and circuit breakers or systems directly or not connected (e.g. via wires) within the traction power system remotely.</rdfs:comment>
        <rdfs:comment xml:lang="es">Un sistema que envía órdenes para controlar y supervisar a distancia los interruptores y disyuntores o sistemas conectados directamente o no (por ejemplo, mediante cables) dentro del sistema de alimentación de tracción.</rdfs:comment>
        <rdfs:label xml:lang="es">Telecomando</rdfs:label>
        <rdfs:label xml:lang="en">Telecommand</rdfs:label>
    </owl:Class>
    


    <!-- https://w3id.org/mep#Telephone -->


    <owl:Class rdf:about="https://w3id.org/mep#Telephone">
        <rdfs:subClassOf rdf:resource="https://w3id.org/mep#AudioVisualAppliance"/>
        <rdfs:comment xml:lang="en">A telecommunications device that is used to transmit and receive sound, and optionally video.</rdfs:comment>
        <rdfs:comment xml:lang="es">Dispositivo de telecomunicaciones que se utiliza para transmitir y recibir sonido y, opcionalmente, vídeo.</rdfs:comment>
        <rdfs:label xml:lang="es">Telefono</rdfs:label>
        <rdfs:label xml:lang="en">Telephone</rdfs:label>
    </owl:Class>
    


    <!-- https://w3id.org/mep#TelephoneOutlet -->


    <owl:Class rdf:about="https://w3id.org/mep#TelephoneOutlet">
        <rdfs:subClassOf rdf:resource="https://w3id.org/mep#Outlet"/>
        <rdfs:comment xml:lang="en">An outlet used for connecting telephone communications equipment.</rdfs:comment>
        <rdfs:comment xml:lang="es">Salida utilizada para conectar equipos de comunicaciones.</rdfs:comment>
        <rdfs:label xml:lang="es">Salida de Telefono</rdfs:label>
        <rdfs:label xml:lang="en">Telephone Outlet</rdfs:label>
    </owl:Class>
    


    <!-- https://w3id.org/mep#TelephonyExchange -->


    <owl:Class rdf:about="https://w3id.org/mep#TelephonyExchange">
        <rdfs:subClassOf rdf:resource="https://w3id.org/mep#CommunicationsAppliance"/>
        <rdfs:comment xml:lang="en">A telephony exchange is a device that ensures the routing of telephone calls and communications.</rdfs:comment>
        <rdfs:comment xml:lang="es">Una central telefónica es un dispositivo que garantiza el encaminamiento de las llamadas y comunicaciones telefónicas.</rdfs:comment>
        <rdfs:label xml:lang="es">Central Telefonica</rdfs:label>
        <rdfs:label xml:lang="en">Telephony Exchange</rdfs:label>
    </owl:Class>
    


    <!-- https://w3id.org/mep#TemperatureSensor -->


    <owl:Class rdf:about="https://w3id.org/mep#TemperatureSensor">
        <rdfs:subClassOf rdf:resource="https://w3id.org/mep#Sensor"/>
        <rdfs:comment xml:lang="en">A device that senses or detects temperature.</rdfs:comment>
        <rdfs:comment xml:lang="es">Dispositivo que detecta la temperatura.</rdfs:comment>
        <rdfs:label xml:lang="es">Sensor de Temperatura</rdfs:label>
        <rdfs:label xml:lang="en">Temperature Sensor</rdfs:label>
    </owl:Class>
    


    <!-- https://w3id.org/mep#ThermalTrippingUnit -->


    <owl:Class rdf:about="https://w3id.org/mep#ThermalTrippingUnit">
        <rdfs:subClassOf rdf:resource="https://w3id.org/mep#ProtectiveDeviceTrippingUnit"/>
        <rdfs:comment xml:lang="en">A tripping unit activated by thermal action.</rdfs:comment>
        <rdfs:comment xml:lang="es">Una unidad de disparo activada por acción térmica.</rdfs:comment>
        <rdfs:label xml:lang="en">Thermal Tripping Unit</rdfs:label>
        <rdfs:label xml:lang="es">Unidad de Disparo Termica</rdfs:label>
    </owl:Class>
    


    <!-- https://w3id.org/mep#Thermometer -->


    <owl:Class rdf:about="https://w3id.org/mep#Thermometer">
        <rdfs:subClassOf rdf:resource="https://w3id.org/mep#FlowInstrument"/>
        <rdfs:comment xml:lang="en">A device that reads and displays a temperature value at a point.</rdfs:comment>
        <rdfs:comment xml:lang="es">Dispositivo que lee y muestra un valor de temperatura en un punto.</rdfs:comment>
        <rdfs:label xml:lang="es">Termometro</rdfs:label>
        <rdfs:label xml:lang="en">Thermometer</rdfs:label>
    </owl:Class>
    


    <!-- https://w3id.org/mep#ThermosiphonCoilTypeHeatExchanger -->


    <owl:Class rdf:about="https://w3id.org/mep#ThermosiphonCoilTypeHeatExchanger">
        <rdfs:subClassOf rdf:resource="https://w3id.org/mep#AirToAirHeatRecovery"/>
        <rdfs:comment xml:lang="en">Sealed systems that consist of an evaporator, a condenser, interconnecting piping, and an intermediate working fluid that is present in both liquid and vapor phases where the evaporator and condensor coils are installed independently in the ducts and are interconnected by the working fluid piping.</rdfs:comment>
        <rdfs:comment xml:lang="es">Sistemas sellados que constan de un evaporador, un condensador, tuberías de interconexión y un fluido de trabajo intermedio que está presente tanto en fase líquida como de vapor donde los serpentines del evaporador y del condensador se instalan de forma independiente en los conductos y están interconectados por la tubería del fluido de trabajo.</rdfs:comment>
        <rdfs:label xml:lang="es">Intercambiador de Calor Tipo Bobina de Termosifon</rdfs:label>
        <rdfs:label xml:lang="en">Thermosiphon Coil Type Heat Exchanger</rdfs:label>
    </owl:Class>
    


    <!-- https://w3id.org/mep#ThermosiphonSealedTubeHeatExchanger -->


    <owl:Class rdf:about="https://w3id.org/mep#ThermosiphonSealedTubeHeatExchanger">
        <rdfs:subClassOf rdf:resource="https://w3id.org/mep#AirToAirHeatRecovery"/>
        <rdfs:comment xml:lang="en">Sealed systems that consist of an evaporator, a condenser, interconnecting piping, and an intermediate working fluid that is present in both liquid and vapor phases where the evaporator and the condenser are usually at opposite ends of a bundle of straight, individual thermosiphon tubes and the exhaust and supply ducts are adjacent to each other.</rdfs:comment>
        <rdfs:comment xml:lang="es">Sistemas sellados que constan de un evaporador, un condensador, tuberías de interconexión y un fluido de trabajo intermedio que está presente tanto en la fase líquida como en la de vapor, donde el evaporador y el condensador generalmente están en extremos opuestos de un haz de tubos de termosifón individuales rectos y los conductos de escape y suministro son adyacentes.</rdfs:comment>
        <rdfs:label xml:lang="es">Intercambiadores de Calor de Tubos Sellados por Termosifón</rdfs:label>
        <rdfs:label xml:lang="en">Thermosiphon Sealed Tube Heat Exchanger</rdfs:label>
    </owl:Class>
    


    <!-- https://w3id.org/mep#Thermostat -->


    <owl:Class rdf:about="https://w3id.org/mep#Thermostat">
        <rdfs:subClassOf rdf:resource="https://w3id.org/mep#UnitaryControlElement"/>
        <rdfs:comment xml:lang="en">A control element that senses and regulates the temperature of an element, system or space so that the temperature is maintained near a desired setpoint.</rdfs:comment>
        <rdfs:comment xml:lang="es">Un elemento de control que detecta y regula la temperatura de un elemento, sistema o espacio para que la temperatura se mantenga cerca de un punto de ajuste deseado.</rdfs:comment>
        <rdfs:label xml:lang="es">Termostato</rdfs:label>
        <rdfs:label xml:lang="en">Thermostat</rdfs:label>
    </owl:Class>
    


    <!-- https://w3id.org/mep#ThermostaticActuator -->


    <owl:Class rdf:about="https://w3id.org/mep#ThermostaticActuator">
        <rdfs:subClassOf rdf:resource="https://w3id.org/mep#Actuator"/>
        <rdfs:comment xml:lang="en">A device that thermostatically actuates a control element.</rdfs:comment>
        <rdfs:comment xml:lang="es">Dispositivo que acciona termostáticamente un elemento de control.</rdfs:comment>
        <rdfs:label xml:lang="es">Actuador Termostatico</rdfs:label>
        <rdfs:label xml:lang="en">Thermostatic Actuator</rdfs:label>
    </owl:Class>
    


    <!-- https://w3id.org/mep#ThinScrewCompressor -->


    <owl:Class rdf:about="https://w3id.org/mep#ThinScrewCompressor">
        <rdfs:subClassOf rdf:resource="https://w3id.org/mep#Compressor"/>
        <rdfs:comment xml:lang="es">Compresor rotativo de desplazamiento positivo que utiliza dos rotores acanalados helicoidalmente acoplados, macho (lóbulos) y hembra (flautas) en una carcasa estacionaria con puertos de gas de entrada y salida.</rdfs:comment>
        <rdfs:comment xml:lang="en">Positive-displacement rotary compressor using two mating helically grooved rotors, male (lobes) and female (flutes) in a stationary housing with inlet and outlet gas ports.</rdfs:comment>
        <rdfs:label xml:lang="es">Compresor de Tornillo Delgado</rdfs:label>
        <rdfs:label xml:lang="en">Thin Screw Compressor</rdfs:label>
    </owl:Class>
    


    <!-- https://w3id.org/mep#TimeDelay -->


    <owl:Class rdf:about="https://w3id.org/mep#TimeDelay">
        <rdfs:subClassOf rdf:resource="https://w3id.org/mep#ElectricTimeControl"/>
        <rdfs:comment xml:lang="en">A control that causes action to occur following a set duration.</rdfs:comment>
        <rdfs:comment xml:lang="es">Un control que hace que se produzca una acción después de una duración determinada.</rdfs:comment>
        <rdfs:label xml:lang="es">Delay</rdfs:label>
        <rdfs:label xml:lang="en">Time Delay</rdfs:label>
    </owl:Class>
    


    <!-- https://w3id.org/mep#TimeRelay -->


    <owl:Class rdf:about="https://w3id.org/mep#TimeRelay">
        <rdfs:subClassOf rdf:resource="https://w3id.org/mep#ElectricTimeControl"/>
        <rdfs:comment xml:lang="en">Electromagnetically operated contactor for making or breaking a control circuit.</rdfs:comment>
        <rdfs:comment xml:lang="es">Un relé es un contactor operado electromagnéticamente que se utiliza para abrir o cerrar un circuito de control.</rdfs:comment>
        <rdfs:label xml:lang="es">Rele de Tiempo</rdfs:label>
        <rdfs:label xml:lang="en">Time Relay</rdfs:label>
    </owl:Class>
    


    <!-- https://w3id.org/mep#Timelock -->


    <owl:Class rdf:about="https://w3id.org/mep#Timelock">
        <rdfs:subClassOf rdf:resource="https://w3id.org/mep#ElectricTimeControl"/>
        <rdfs:comment xml:lang="en">A control that causes action to occur at set times.</rdfs:comment>
        <rdfs:comment xml:lang="es">Control que provoca que ocurra una acción en momentos específicos</rdfs:comment>
        <rdfs:label xml:lang="en">Timelock</rdfs:label>
        <rdfs:label xml:lang="es">Timelock</rdfs:label>
    </owl:Class>
    


    <!-- https://w3id.org/mep#ToggleSwitch -->


    <owl:Class rdf:about="https://w3id.org/mep#ToggleSwitch">
        <rdfs:subClassOf rdf:resource="https://w3id.org/mep#SwitchingDevice"/>
        <rdfs:comment xml:lang="en">A toggle switch has two positions, and may enable or isolate electrical power or other setting (according to the switched port type).</rdfs:comment>
        <rdfs:comment xml:lang="es">Un interruptor basculante tiene dos posiciones y puede activar o aislar la alimentación eléctrica u otro ajuste (según el tipo de puerto conmutado).</rdfs:comment>
        <rdfs:label xml:lang="es">Interruptor Basculante</rdfs:label>
        <rdfs:label xml:lang="en">Toggle Switch</rdfs:label>
    </owl:Class>
    


    <!-- https://w3id.org/mep#ToiletPan -->


    <owl:Class rdf:about="https://w3id.org/mep#ToiletPan">
        <rdfs:subClassOf rdf:resource="https://w3id.org/mep#SanitaryTerminal"/>
        <rdfs:comment xml:lang="es">Aparato para la eliminación de excrementos.</rdfs:comment>
        <rdfs:comment xml:lang="en">Soil appliance for the disposal of excrement.</rdfs:comment>
        <rdfs:label xml:lang="es">Inodoro</rdfs:label>
        <rdfs:label xml:lang="en">Toilet Pan</rdfs:label>
    </owl:Class>
    


    <!-- https://w3id.org/mep#TrainSensor -->


    <owl:Class rdf:about="https://w3id.org/mep#TrainSensor">
        <rdfs:subClassOf rdf:resource="https://w3id.org/mep#Sensor"/>
        <rdfs:comment xml:lang="en">A device, usually attached to the rear end of the last vehicle of a train, acting on a fixed equipment to give an indication that the train is complete.</rdfs:comment>
        <rdfs:comment xml:lang="es">Dispositivo, normalmente acoplado al extremo trasero del último vehículo de un tren, que actúa sobre un equipo fijo para dar una indicación de que el tren está completo.</rdfs:comment>
        <rdfs:label xml:lang="es">Sensor de Tren</rdfs:label>
        <rdfs:label xml:lang="en">Train Sensor</rdfs:label>
    </owl:Class>
    


    <!-- https://w3id.org/mep#Transformer -->


    <owl:Class rdf:about="https://w3id.org/mep#Transformer">
        <rdfs:subClassOf rdf:resource="https://w3id.org/mep#EnergyConversionDevice"/>
        <rdfs:comment xml:lang="en">A transformer is an inductive stationary device that transfers electrical energy from one circuit to another.</rdfs:comment>
        <rdfs:comment xml:lang="es">Un Conversor es un dispositivo estacionario inductivo que transfiere energía eléctrica de un circuito a otro.</rdfs:comment>
        <rdfs:label xml:lang="es">Conversor</rdfs:label>
        <rdfs:label xml:lang="en">Transformer</rdfs:label>
    </owl:Class>
    


    <!-- https://w3id.org/mep#TransitionComponent -->


    <owl:Class rdf:about="https://w3id.org/mep#TransitionComponent">
        <rdfs:subClassOf rdf:resource="https://w3id.org/mep#CommunicationsAppliance"/>
        <rdfs:comment xml:lang="en">A transition component is a minor active device that converts electric signals to optical signals at the sender, and converts optical signals to electric signals at the receiver.</rdfs:comment>
        <rdfs:comment xml:lang="es">Un componente de transición es un dispositivo activo menor que convierte señales eléctricas en señales ópticas en el emisor, y convierte señales ópticas en señales eléctricas en el receptor.</rdfs:comment>
        <rdfs:label xml:lang="es">Componente de Transicion</rdfs:label>
        <rdfs:label xml:lang="en">Transition Component</rdfs:label>
    </owl:Class>
    


    <!-- https://w3id.org/mep#Trasnponder -->


    <owl:Class rdf:about="https://w3id.org/mep#Trasnponder">
        <rdfs:subClassOf rdf:resource="https://w3id.org/mep#CommunicationsAppliance"/>
        <rdfs:comment xml:lang="en">A transponder is a communication, monitoring, or control device that, upon receiving a signal, emits a different signal in response. Transponders can be either passive or active (e.g., electronic beacon, balise).</rdfs:comment>
        <rdfs:comment xml:lang="es">Un transpondedor es un dispositivo de comunicación, vigilancia o control que, al recibir una señal, emite una señal diferente como respuesta. Los transpondedores pueden ser pasivos o activos (por ejemplo, baliza electrónica, baliza).</rdfs:comment>
        <rdfs:label xml:lang="en">Trasnponder</rdfs:label>
        <rdfs:label xml:lang="es">Trasnspondedor</rdfs:label>
    </owl:Class>
    


    <!-- https://w3id.org/mep#TrasnportUnit -->


    <owl:Class rdf:about="https://w3id.org/mep#TrasnportUnit">
        <rdfs:subClassOf rdf:resource="https://w3id.org/mep#CommunicationsAppliance"/>
        <rdfs:comment xml:lang="en">A transport equipment is a network element responsible for providing functionality of transport, multiplexing, switching, management and supervision of transmission channels between different hosts. The data transport service uses three specific metrics: the bandwidth, the jitter, and the packet loss rate.</rdfs:comment>
        <rdfs:comment xml:lang="es">Un equipo de transporte es un elemento de red responsable de proporcionar funcionalidades de transporte, multiplexación, conmutación, gestión y supervisión de canales de transmisión entre distintos hosts. El servicio de transporte de datos utiliza tres métricas específicas: el ancho de banda, el jitter y la tasa de pérdida de paquetes.</rdfs:comment>
        <rdfs:label xml:lang="es">Equipo de Transporte</rdfs:label>
        <rdfs:label xml:lang="en">Trasnport Unit</rdfs:label>
    </owl:Class>
    


    <!-- https://w3id.org/mep#Trench -->


    <owl:Class rdf:about="https://w3id.org/mep#Trench">
        <rdfs:subClassOf rdf:resource="https://w3id.org/mep#DistributionChamberElement"/>
        <rdfs:comment xml:lang="es">Cámara excavada cuya longitud suele superar la anchura.</rdfs:comment>
        <rdfs:comment xml:lang="en">Excavated chamber, the length of which typically exceeds the width.</rdfs:comment>
        <rdfs:label xml:lang="en">Trench</rdfs:label>
        <rdfs:label xml:lang="es">Zanja</rdfs:label>
    </owl:Class>
    


    <!-- https://w3id.org/mep#TrochoidalCompressor -->


    <owl:Class rdf:about="https://w3id.org/mep#TrochoidalCompressor">
        <rdfs:subClassOf rdf:resource="https://w3id.org/mep#Compressor"/>
        <rdfs:comment xml:lang="es">Compresor de desplazamiento positivo que utiliza un movimiento de balanceo de un círculo fuera o dentro de la circunferencia de un círculo básico y produce epitrocoides o hipotrocoides.</rdfs:comment>
        <rdfs:comment xml:lang="en">Positive-displacement compressor using a rolling motion of one circle outside or inside the circumference of a basic circle and produce either epitrochoids or hypotrochoids.</rdfs:comment>
        <rdfs:label xml:lang="en">Trochoidal Compressor</rdfs:label>
        <rdfs:label xml:lang="es">Trocoidal Compressor</rdfs:label>
    </owl:Class>
    


    <!-- https://w3id.org/mep#TubeAxialFan -->


    <owl:Class rdf:about="https://w3id.org/mep#TubeAxialFan">
        <rdfs:subClassOf rdf:resource="https://w3id.org/mep#Fan"/>
        <rdfs:comment xml:lang="en">Air flows through the impeller axially with reduced tip clearance and operating at higher tip speeds.</rdfs:comment>
        <rdfs:comment xml:lang="es">El aire fluye a través del impulsor axialmente con un espacio reducido en la punta y operando a velocidades de punta más altas.</rdfs:comment>
        <rdfs:label xml:lang="en">Tube Axial Fan</rdfs:label>
        <rdfs:label xml:lang="es">Ventilador Axial de Tubo</rdfs:label>
    </owl:Class>
    


    <!-- https://w3id.org/mep#TubeBundle -->


    <owl:Class rdf:about="https://w3id.org/mep#TubeBundle">
        <rdfs:subClassOf rdf:resource="https://w3id.org/mep#EnergyConversionDevice"/>
        <rdfs:comment xml:lang="en">A tube bundle is a device consisting of tubes and bundles of tubes used for heat transfer and contained typically within other energy conversion devices, such as a chiller or coil.</rdfs:comment>
        <rdfs:comment xml:lang="es">Un haz de tubos es un dispositivo que consta de tubos y haces de tubos utilizados para la transferencia de calor y contenidos normalmente dentro de otros dispositivos de conversión de energía, como un enfriador o un serpentín.</rdfs:comment>
        <rdfs:label xml:lang="es">Haz de Tubos</rdfs:label>
        <rdfs:label xml:lang="en">TubeBundle</rdfs:label>
    </owl:Class>
    


    <!-- https://w3id.org/mep#TumbleDryer -->


    <owl:Class rdf:about="https://w3id.org/mep#TumbleDryer">
        <rdfs:subClassOf rdf:resource="https://w3id.org/mep#ElectricAppliance"/>
        <rdfs:comment xml:lang="en">An electrical appliance that has the primary function of drying clothes.</rdfs:comment>
        <rdfs:comment xml:lang="es">Aparato eléctrico cuya función principal es secar la ropa.</rdfs:comment>
        <rdfs:label xml:lang="es">Secadora</rdfs:label>
        <rdfs:label xml:lang="en">Tumble Dryer</rdfs:label>
    </owl:Class>
    


    <!-- https://w3id.org/mep#Tuner -->


    <owl:Class rdf:about="https://w3id.org/mep#Tuner">
        <rdfs:subClassOf rdf:resource="https://w3id.org/mep#AudioVisualAppliance"/>
        <rdfs:comment xml:lang="en">An electronic receiver that detects, demodulates, and amplifies transmitted signals.</rdfs:comment>
        <rdfs:comment xml:lang="es">Un receptor electrónico que detecta, demodula y amplifica las señales transmitidas.</rdfs:comment>
        <rdfs:label xml:lang="en">Tuner</rdfs:label>
        <rdfs:label xml:lang="es">Tuner</rdfs:label>
    </owl:Class>
    


    <!-- https://w3id.org/mep#TungstenFilamentLamp -->


    <owl:Class rdf:about="https://w3id.org/mep#TungstenFilamentLamp">
        <rdfs:subClassOf rdf:resource="https://w3id.org/mep#Lamp"/>
        <rdfs:comment xml:lang="en">A discharge lamp in which most of the light is emitted by exciting a metal halide.</rdfs:comment>
        <rdfs:comment xml:lang="es">Lámpara de descarga en la que la mayor parte de la luz se emite excitando un haluro metálico.</rdfs:comment>
        <rdfs:label xml:lang="es">Lampara de Filamento de Tungsteno</rdfs:label>
        <rdfs:label xml:lang="en">Tungsten Filament Lamp</rdfs:label>
    </owl:Class>
    


    <!-- https://w3id.org/mep#TurnoutClosureSensor -->


    <owl:Class rdf:about="https://w3id.org/mep#TurnoutClosureSensor">
        <rdfs:subClassOf rdf:resource="https://w3id.org/mep#Sensor"/>
        <rdfs:comment xml:lang="en">A device that senses or detects the position of a blade of a turnout.</rdfs:comment>
        <rdfs:comment xml:lang="es">Dispositivo que detecta la posición de la hoja de un desvío.</rdfs:comment>
        <rdfs:label xml:lang="es">Sensor de Cierre de Desvíos</rdfs:label>
        <rdfs:label xml:lang="en">Turnout Closure Sensor</rdfs:label>
    </owl:Class>
    


    <!-- https://w3id.org/mep#TurnoutHeating -->


    <owl:Class rdf:about="https://w3id.org/mep#TurnoutHeating">
        <rdfs:subClassOf rdf:resource="https://w3id.org/mep#HeatExchanger"/>
        <rdfs:comment xml:lang="en">A device used to remove snow from railways. E.g. electric heating device, gas heater</rdfs:comment>
        <rdfs:comment xml:lang="es">Dispositivo que se utiliza para quitar la nieve de las vías del ferrocarril. P.ej. dispositivo de calefacción eléctrica, calentador de gas</rdfs:comment>
        <rdfs:label xml:lang="es">Calefaccion de Desvio</rdfs:label>
        <rdfs:label xml:lang="en">Turnout Heating</rdfs:label>
    </owl:Class>
    


    <!-- https://w3id.org/mep#TwinTowerEnthalpyRecoveryLoops -->


    <owl:Class rdf:about="https://w3id.org/mep#TwinTowerEnthalpyRecoveryLoops">
        <rdfs:subClassOf rdf:resource="https://w3id.org/mep#AirToAirHeatRecovery"/>
        <rdfs:comment xml:lang="en">An air-to-liquid, liquid-to-air enthalpy recovery system with a sorbent liquid circulates continuously between supply and exhaust airstreams, alternately contacting both airstreams directly in contactor towers.</rdfs:comment>
        <rdfs:comment xml:lang="es">Sistema de recuperación de entalpía de aire a líquido y de líquido a aire con un líquido absorbente circula continuamente entre las corrientes de aire de suministro y de escape, contactando alternativamente ambas corrientes de aire directamente en las torres de contactores.</rdfs:comment>
        <rdfs:label xml:lang="es">Bucles de Recuperación de Entalpía de Torre Gemela</rdfs:label>
        <rdfs:label xml:lang="en">Twin Tower Enthalpy Recovery Loops</rdfs:label>
    </owl:Class>
    


    <!-- https://w3id.org/mep#Two-positionController -->


    <owl:Class rdf:about="https://w3id.org/mep#Two-positionController">
        <rdfs:subClassOf rdf:resource="https://w3id.org/mep#Controller"/>
        <rdfs:comment xml:lang="es">La salida puede estar activada o desactivada.</rdfs:comment>
        <rdfs:comment xml:lang="en">Output can be either on or off.</rdfs:comment>
        <rdfs:label xml:lang="es">Controlador de Dos Posiciones</rdfs:label>
        <rdfs:label xml:lang="en">Two-position Controller</rdfs:label>
    </owl:Class>
    


    <!-- https://w3id.org/mep#UPS -->


    <owl:Class rdf:about="https://w3id.org/mep#UPS">
        <rdfs:subClassOf rdf:resource="https://w3id.org/mep#ElectricFlowStorageDevice"/>
        <rdfs:comment xml:lang="en">A device that provides a time limited alternative source of power supply in the event of failure of the main supply.</rdfs:comment>
        <rdfs:comment xml:lang="es">Dispositivo que proporciona una fuente de alimentación alternativa limitada en el tiempo en caso de fallo de la alimentación principal.</rdfs:comment>
        <rdfs:label xml:lang="es">SAI</rdfs:label>
        <rdfs:label xml:lang="en">UPS</rdfs:label>
    </owl:Class>
    


    <!-- https://w3id.org/mep#UnitaryControlElement -->


    <owl:Class rdf:about="https://w3id.org/mep#UnitaryControlElement">
        <rdfs:subClassOf rdf:resource="https://w3id.org/mep#DistributionControlElement"/>
        <rdfs:comment xml:lang="en">A unitary control element combines a number of control components into a single product, such as a thermostat or humidistat.</rdfs:comment>
        <rdfs:comment xml:lang="es">Un elemento de control unitario combina varios componentes de control en un solo producto, como un termostato o un higrostato.</rdfs:comment>
        <rdfs:label xml:lang="es">Elemento de Control Unitario</rdfs:label>
        <rdfs:label xml:lang="en">Unitary Control Element</rdfs:label>
    </owl:Class>
    


    <!-- https://w3id.org/mep#UnitaryEquipment -->


    <owl:Class rdf:about="https://w3id.org/mep#UnitaryEquipment">
        <rdfs:subClassOf rdf:resource="https://w3id.org/mep#EnergyConversionDevice"/>
        <rdfs:comment xml:lang="es">Los equipos unitarios suelen combinar varios componentes en un solo producto, como unidades de tratamiento de aire, unidades de aire acondicionado de techo preempaquetadas, bombas de calor y sistemas divididos.</rdfs:comment>
        <rdfs:comment xml:lang="en">Unitary equipment typically combine a number of components into a single product, such as air handlers, pre-packaged rooftop air-conditioning units, heat pumps, and split systems.</rdfs:comment>
        <rdfs:label xml:lang="es">Equipo Unitario</rdfs:label>
        <rdfs:label xml:lang="en">UnitaryEquipment</rdfs:label>
    </owl:Class>
    


    <!-- https://w3id.org/mep#Urinal -->


    <owl:Class rdf:about="https://w3id.org/mep#Urinal">
        <rdfs:subClassOf rdf:resource="https://w3id.org/mep#SanitaryTerminal"/>
        <rdfs:comment xml:lang="es">Aparato de suelo que recibe la orina y la dirige a una salida de residuos.</rdfs:comment>
        <rdfs:comment xml:lang="en">Soil appliance that receives urine and directs it to a waste outlet.</rdfs:comment>
        <rdfs:label xml:lang="es">Orinal</rdfs:label>
        <rdfs:label xml:lang="en">Urinal</rdfs:label>
    </owl:Class>
    


    <!-- https://w3id.org/mep#VacuumStation -->


    <owl:Class rdf:about="https://w3id.org/mep#VacuumStation">
        <rdfs:subClassOf rdf:resource="https://w3id.org/mep#MedicalDevice"/>
        <rdfs:comment xml:lang="en">Device that provides suction, composed of a vacuum pump and bacterial filtration line.</rdfs:comment>
        <rdfs:comment xml:lang="es">Dispositivo que proporciona succión, compuesto por una bomba de vacío y una línea de filtración bacteriana.</rdfs:comment>
        <rdfs:label xml:lang="es">Estacion de Vacio</rdfs:label>
        <rdfs:label xml:lang="en">Vacuum Station</rdfs:label>
    </owl:Class>
    


    <!-- https://w3id.org/mep#Valve -->


    <owl:Class rdf:about="https://w3id.org/mep#Valve">
        <rdfs:subClassOf rdf:resource="https://w3id.org/mep#FlowController"/>
        <rdfs:comment xml:lang="en">A valve is used in a building services piping distribution system to control or modulate the flow of the fluid.</rdfs:comment>
        <rdfs:comment xml:lang="es">Se utiliza una válvula en un sistema de distribución de tuberías de servicios de construcción para controlar o modular el flujo del fluido.</rdfs:comment>
        <rdfs:label xml:lang="en">Valve</rdfs:label>
        <rdfs:label xml:lang="es">Valvula</rdfs:label>
    </owl:Class>
    


    <!-- https://w3id.org/mep#ValveChamber -->


    <owl:Class rdf:about="https://w3id.org/mep#ValveChamber">
        <rdfs:subClassOf rdf:resource="https://w3id.org/mep#DistributionChamberElement"/>
        <rdfs:comment xml:lang="en">Chamber that houses a valve(s).</rdfs:comment>
        <rdfs:comment xml:lang="es">Cámara que aloja una o varias válvulas.</rdfs:comment>
        <rdfs:label xml:lang="es">Cmara de Valvulas</rdfs:label>
        <rdfs:label xml:lang="en">Valve Chamber</rdfs:label>
    </owl:Class>
    


    <!-- https://w3id.org/mep#VaneAxialFan -->


    <owl:Class rdf:about="https://w3id.org/mep#VaneAxialFan">
        <rdfs:subClassOf rdf:resource="https://w3id.org/mep#Fan"/>
        <rdfs:comment xml:lang="en">Air flows through the impeller axially with guide vanes and reduced running blade tip clearance.</rdfs:comment>
        <rdfs:comment xml:lang="es">El aire fluye a través del impulsor axialmente con paletas guía y espacio reducido en la punta de la pala.  </rdfs:comment>
        <rdfs:label xml:lang="en">Vane Axial Fan</rdfs:label>
        <rdfs:label xml:lang="es">Ventilador Axial de Alabes</rdfs:label>
    </owl:Class>
    


    <!-- https://w3id.org/mep#VariableFlowPressureDependantTerminalBOx -->


    <owl:Class rdf:about="https://w3id.org/mep#VariableFlowPressureDependantTerminalBOx">
        <rdfs:subClassOf rdf:resource="https://w3id.org/mep#AirTerminalBox"/>
        <rdfs:comment xml:lang="es">La caja de terminales que incluye un medio para restablecer el volumen automáticamente a un punto de control diferente en respuesta a una señal externa, como un termostato: el caudal de aire depende de la presión del suministro.</rdfs:comment>
        <rdfs:comment xml:lang="en">Terminal box includes a means to reset the volume automatically to a different control point in response to an outside signal such as thermostat: air-flow rate depends on supply pressure.</rdfs:comment>
        <rdfs:label xml:lang="es">Caja Terminal de Flujo Variable y Presion Dependiente</rdfs:label>
        <rdfs:label xml:lang="en">Variable Flow Pressure Dependant Terminal BOx</rdfs:label>
    </owl:Class>
    


    <!-- https://w3id.org/mep#VariableFlowPressureIndependantTerminalBox -->


    <owl:Class rdf:about="https://w3id.org/mep#VariableFlowPressureIndependantTerminalBox">
        <rdfs:subClassOf rdf:resource="https://w3id.org/mep#AirTerminalBox"/>
        <rdfs:comment xml:lang="es">Caja de terminales que incluye un medio para restablecer el volumen automáticamente a un punto de control diferente en respuesta a una señal externa como un termostato: el caudal de aire es independiente de la presión de suministro.</rdfs:comment>
        <rdfs:comment xml:lang="en">Terminal box that includes a means to reset the volume automatically to a different control point in response to an outside signal such as thermostat: air-flow rate is independent of supply pressure.</rdfs:comment>
        <rdfs:label xml:lang="es">Caja Terminal de Flujo Variable y Presion Independiente</rdfs:label>
        <rdfs:label xml:lang="en">Variable Flow Pressure Independant Terminal Box</rdfs:label>
    </owl:Class>
    


    <!-- https://w3id.org/mep#Varistor -->


    <owl:Class rdf:about="https://w3id.org/mep#Varistor">
        <rdfs:subClassOf rdf:resource="https://w3id.org/mep#ProtectiveDevice"/>
        <rdfs:comment xml:lang="en">A high voltage surge protection device.</rdfs:comment>
        <rdfs:comment xml:lang="es">Un dispositivo de protección contra sobretensiones de alta tensión.</rdfs:comment>
        <rdfs:label xml:lang="en">Varistor</rdfs:label>
        <rdfs:label xml:lang="es">Varistor</rdfs:label>
    </owl:Class>
    


    <!-- https://w3id.org/mep#VendingMachine -->


    <owl:Class rdf:about="https://w3id.org/mep#VendingMachine">
        <rdfs:subClassOf rdf:resource="https://w3id.org/mep#ElectricAppliance"/>
        <rdfs:comment xml:lang="en">An appliance that stores and vends goods including food, drink, tickets, and goods of various types.</rdfs:comment>
        <rdfs:comment xml:lang="es">Aparato que almacena y vende productos como alimentos, bebidas, billetes y mercancías de diversos tipos.</rdfs:comment>
        <rdfs:label xml:lang="es">Maquina Expendedora</rdfs:label>
        <rdfs:label xml:lang="en">Vending Machine</rdfs:label>
    </owl:Class>
    


    <!-- https://w3id.org/mep#VerticalInlinePump -->


    <owl:Class rdf:about="https://w3id.org/mep#VerticalInlinePump">
        <rdfs:subClassOf rdf:resource="https://w3id.org/mep#Pump"/>
        <rdfs:comment xml:lang="en">A vertical inline pump has the pump and motor close-coupled on the pump casing. The pump depends on the connected, horizontal piping for support, with the suction and discharge along the piping axis.</rdfs:comment>
        <rdfs:comment xml:lang="es">Una bomba vertical en línea tiene la bomba y el motor acoplados en la carcasa de la bomba. La bomba depende de las tuberías horizontales conectadas para su soporte, con la aspiración y la descarga a lo largo del eje de las tuberías.</rdfs:comment>
        <rdfs:label xml:lang="es">Bomba Vertical en Linea</rdfs:label>
        <rdfs:label xml:lang="en">Vertical Inline Pump</rdfs:label>
    </owl:Class>
    


    <!-- https://w3id.org/mep#VerticalTurbinePump -->


    <owl:Class rdf:about="https://w3id.org/mep#VerticalTurbinePump">
        <rdfs:subClassOf rdf:resource="https://w3id.org/mep#Pump"/>
        <rdfs:comment xml:lang="en">A vertical turbine pump has a motor mounted vertically on the pump casing for either wet-pit sump mounting or dry-well mounting.</rdfs:comment>
        <rdfs:comment xml:lang="es">Una bomba de turbina vertical tiene un motor montado verticalmente en la carcasa de la bomba para montaje en sumidero húmedo o en pozo seco.</rdfs:comment>
        <rdfs:label xml:lang="es">VERTICALTURBINE</rdfs:label>
        <rdfs:label xml:lang="en">Vertical Turbine Pump</rdfs:label>
    </owl:Class>
    


    <!-- https://w3id.org/mep#Vessel -->


    <owl:Class rdf:about="https://w3id.org/mep#Vessel">
        <rdfs:subClassOf rdf:resource="https://w3id.org/mep#Tank"/>
        <rdfs:comment xml:lang="en">An arbitrary closed tank type.</rdfs:comment>
        <rdfs:comment xml:lang="es">Un tipo de depósito cerrado arbitrario.</rdfs:comment>
        <rdfs:label xml:lang="es">Recipiente</rdfs:label>
        <rdfs:label xml:lang="en">Vessel</rdfs:label>
    </owl:Class>
    


    <!-- https://w3id.org/mep#VisualSignalingDevice -->


    <owl:Class rdf:about="https://w3id.org/mep#VisualSignalingDevice">
        <rdfs:subClassOf rdf:resource="https://w3id.org/mep#Signal"/>
        <rdfs:comment xml:lang="en">A signal type formed of an active device conveying information in a visual manner such as a light, cluster of lights, or mechanical moving shapes.</rdfs:comment>
        <rdfs:comment xml:lang="es">Tipo de señal formada por un dispositivo activo que transmite información de forma visual, como una luz, un grupo de luces o formas mecánicas móviles.</rdfs:comment>
        <rdfs:label xml:lang="es">Dispositivo de señalización visual</rdfs:label>
        <rdfs:label xml:lang="en">Visual Signaling Device</rdfs:label>
    </owl:Class>
    


    <!-- https://w3id.org/mep#VoltageLimiter -->


    <owl:Class rdf:about="https://w3id.org/mep#VoltageLimiter">
        <rdfs:subClassOf rdf:resource="https://w3id.org/mep#ProtectiveDevice"/>
        <rdfs:comment xml:lang="en">A voltage limiter is an equipment that prevents the over voltage.</rdfs:comment>
        <rdfs:comment xml:lang="es">Un limitador de tensión es un equipo que evita la sobretensión.</rdfs:comment>
        <rdfs:label xml:lang="es">Limitador de Voltage</rdfs:label>
        <rdfs:label xml:lang="en">Voltage Limiter</rdfs:label>
    </owl:Class>
    


    <!-- https://w3id.org/mep#VoltageTransformer -->


    <owl:Class rdf:about="https://w3id.org/mep#VoltageTransformer">
        <rdfs:subClassOf rdf:resource="https://w3id.org/mep#Transformer"/>
        <rdfs:comment xml:lang="en">A transformer that changes the voltage between circuits.</rdfs:comment>
        <rdfs:comment xml:lang="es">Un transformador que cambia el voltaje entre circuitos.</rdfs:comment>
        <rdfs:label xml:lang="es">Conversor de Voltage</rdfs:label>
        <rdfs:label xml:lang="en">Voltage Transformer</rdfs:label>
    </owl:Class>
    


    <!-- https://w3id.org/mep#Voltmeter -->


    <owl:Class rdf:about="https://w3id.org/mep#Voltmeter">
        <rdfs:subClassOf rdf:resource="https://w3id.org/mep#FlowInstrument"/>
        <rdfs:comment xml:lang="en">A device that measures and displays the voltage in a circuit.</rdfs:comment>
        <rdfs:comment xml:lang="es">Dispositivo que mide y muestra el voltaje en un circuito.</rdfs:comment>
        <rdfs:label xml:lang="es">Voltimetro</rdfs:label>
        <rdfs:label xml:lang="en">Voltmeter</rdfs:label>
    </owl:Class>
    


    <!-- https://w3id.org/mep#VoltmeterPeak -->


    <owl:Class rdf:about="https://w3id.org/mep#VoltmeterPeak">
        <rdfs:subClassOf rdf:resource="https://w3id.org/mep#FlowInstrument"/>
        <rdfs:comment xml:lang="en">A device that reads and displays the peak voltage in an electrical circuit.</rdfs:comment>
        <rdfs:comment xml:lang="es">Un voltímetro de pico es un dispositivo que lee y muestra el voltaje máximo en un circuito eléctrico.</rdfs:comment>
        <rdfs:label xml:lang="es">Voltimetro de Pico</rdfs:label>
        <rdfs:label xml:lang="en">Voltmeter Peak</rdfs:label>
    </owl:Class>
    


    <!-- https://w3id.org/mep#VoltmeterRMS -->


    <owl:Class rdf:about="https://w3id.org/mep#VoltmeterRMS">
        <rdfs:subClassOf rdf:resource="https://w3id.org/mep#FlowInstrument"/>
        <rdfs:comment xml:lang="en">A device that reads and displays the RMS (mean) voltage in an electrical circuit.</rdfs:comment>
        <rdfs:comment xml:lang="es">Dispositivo que mide y muestra el voltaje RMS (valor medio cuadrático) en un circuito eléctrico</rdfs:comment>
        <rdfs:label xml:lang="es">Voltimetro RMS</rdfs:label>
        <rdfs:label xml:lang="en">Voltmeter RMS</rdfs:label>
    </owl:Class>
    


    <!-- https://w3id.org/mep#WashHandBasin -->


    <owl:Class rdf:about="https://w3id.org/mep#WashHandBasin">
        <rdfs:subClassOf rdf:resource="https://w3id.org/mep#SanitaryTerminal"/>
        <rdfs:comment xml:lang="es">Aparato de aguas residuales para el lavado de las partes superiores del cuerpo.</rdfs:comment>
        <rdfs:comment xml:lang="en">Waste water appliance for washing the upper parts of the body.</rdfs:comment>
        <rdfs:label xml:lang="es">Lavabo</rdfs:label>
        <rdfs:label xml:lang="en">Wash Hand Basin</rdfs:label>
    </owl:Class>
    


    <!-- https://w3id.org/mep#WashingMachine -->


    <owl:Class rdf:about="https://w3id.org/mep#WashingMachine">
        <rdfs:subClassOf rdf:resource="https://w3id.org/mep#ElectricAppliance"/>
        <rdfs:comment xml:lang="en">An appliance that has the primary function of washing clothes.</rdfs:comment>
        <rdfs:comment xml:lang="es">Aparato cuya función principal es lavar la ropa.</rdfs:comment>
        <rdfs:label xml:lang="es">Lavadora</rdfs:label>
        <rdfs:label xml:lang="en">Washing Machine</rdfs:label>
    </owl:Class>
    


    <!-- https://w3id.org/mep#WasteDisposalUnit -->


    <owl:Class rdf:about="https://w3id.org/mep#WasteDisposalUnit">
        <rdfs:subClassOf rdf:resource="https://w3id.org/mep#WasteTerminal"/>
        <rdfs:comment xml:lang="es">Dispositivo operado eléctricamente que reduce los desechos de la cocina u otros desechos en fragmentos lo suficientemente pequeños como para ser arrojados a un sistema de drenaje.</rdfs:comment>
        <rdfs:comment xml:lang="en">Electrically operated device that reduces kitchen or other waste into fragments small enough to be flushed into a drainage system.</rdfs:comment>
        <rdfs:label xml:lang="es">Unidad de Eliminación de Residuos </rdfs:label>
        <rdfs:label xml:lang="en">Waste Disposal Unit</rdfs:label>
    </owl:Class>
    


    <!-- https://w3id.org/mep#WasteTerminal -->


    <owl:Class rdf:about="https://w3id.org/mep#WasteTerminal">
        <rdfs:subClassOf rdf:resource="https://w3id.org/mep#FlowTerminal"/>
        <rdfs:comment xml:lang="en">A waste terminal has the purpose of collecting or intercepting waste from one or more sanitary terminals or other fluid waste generating equipment and discharging it into a single waste/drainage system. A waste terminal provides for all forms of trap and waste point that collects discharge from a sanitary terminal and discharges it into a waste/drainage subsystem or that collects waste from several terminals and passes it into a single waste/drainage subsystem. This includes the P and S traps from soil sanitary terminals, sinks, and basins as well as floor wastes and gully traps that provide collection points.</rdfs:comment>
        <rdfs:comment xml:lang="es">Una terminal de residuos tiene el propósito de recoger o interceptar los residuos de una o más terminales sanitarias u otros equipos generadores de residuos de fluidos y descargarlos en un único sistema de desagüe/drenaje. Una terminal de residuos prevé todas las formas de trampas y puntos de recogida de residuos que recogen los vertidos de un terminal sanitario y los vierten en un subsistema de residuos/drenaje o que recogen los residuos de varios terminales y los pasan a un único subsistema de residuos/drenaje. Esto incluye las trampas P y S de las terminales sanitarias del suelo, los fregaderos y las cuencas, así como los desechos del suelo y las trampas de barrancos que proporcionan puntos de recolección.</rdfs:comment>
        <rdfs:label xml:lang="es">Terminal de Residuos</rdfs:label>
        <rdfs:label xml:lang="en">Waste Terminal</rdfs:label>
    </owl:Class>
    


    <!-- https://w3id.org/mep#WasteTrap -->


    <owl:Class rdf:about="https://w3id.org/mep#WasteTrap">
        <rdfs:subClassOf rdf:resource="https://w3id.org/mep#WasteTerminal"/>
        <rdfs:comment xml:lang="es">Accesorio de tubería, colocado adyacente a una terminal sanitaria, que retiene el líquido para evitar el paso del aire viciado.</rdfs:comment>
        <rdfs:comment xml:lang="en">Pipe fitting, set adjacent to a sanitary terminal, that retains liquid to prevent the passage of foul air.</rdfs:comment>
        <rdfs:label xml:lang="es">Trampa de Residuos</rdfs:label>
        <rdfs:label xml:lang="en">Waste Trap</rdfs:label>
    </owl:Class>
    


    <!-- https://w3id.org/mep#Water-cooledBrazed-plateCondenser -->


    <owl:Class rdf:about="https://w3id.org/mep#Water-cooledBrazed-plateCondenser">
        <rdfs:subClassOf rdf:resource="https://w3id.org/mep#Condenser"/>
        <rdfs:comment xml:lang="es">Condensador refrigerado por agua con placas soldadas entre sí para formar un conjunto de canales separados.</rdfs:comment>
        <rdfs:comment xml:lang="en">Water-cooled condenser with plates brazed together to form an assembly of separate channels.</rdfs:comment>
        <rdfs:label xml:lang="es">Condensador de Placas Soldadas Refrigerado por Agua</rdfs:label>
        <rdfs:label xml:lang="en">Water-cooled Brazed-plate Condenser</rdfs:label>
    </owl:Class>
    


    <!-- https://w3id.org/mep#Water-cooledCondenser -->


    <owl:Class rdf:about="https://w3id.org/mep#Water-cooledCondenser">
        <rdfs:subClassOf rdf:resource="https://w3id.org/mep#Condenser"/>
        <rdfs:comment xml:lang="es">Un condensador que se enfría por evaporación.</rdfs:comment>
        <rdfs:comment xml:lang="en">Water-cooled condenser with unspecified operation.</rdfs:comment>
        <rdfs:label xml:lang="es">Condensador Refrigerado por Agua</rdfs:label>
        <rdfs:label xml:lang="en">Water-cooled Condenser</rdfs:label>
    </owl:Class>
    


    <!-- https://w3id.org/mep#Water-cooledShellCoilCondenser -->


    <owl:Class rdf:about="https://w3id.org/mep#Water-cooledShellCoilCondenser">
        <rdfs:subClassOf rdf:resource="https://w3id.org/mep#Condenser"/>
        <rdfs:comment xml:lang="es">Condensador refrigerado por agua con agua de refrigeración que circula a través de uno o más serpentines continuos o ensamblados contenidos dentro de la carcasa.</rdfs:comment>
        <rdfs:comment xml:lang="en">Water-cooled condenser with cooling water circulated through one or more continuous or assembled coils contained within the shell.</rdfs:comment>
        <rdfs:label xml:lang="es">Condensador de Serpentín Refrigerado por Agua</rdfs:label>
        <rdfs:label xml:lang="en">Water-cooled Shell Coil Condenser</rdfs:label>
    </owl:Class>
    


    <!-- https://w3id.org/mep#Water-cooledShellTubeCondenser -->


    <owl:Class rdf:about="https://w3id.org/mep#Water-cooledShellTubeCondenser">
        <rdfs:subClassOf rdf:resource="https://w3id.org/mep#Condenser"/>
        <rdfs:comment xml:lang="es">Condensador refrigerado por agua con agua de refrigeración que circula a través de uno o más tubos contenidos dentro de la carcasa.</rdfs:comment>
        <rdfs:comment xml:lang="en">Water-cooled condenser with cooling water circulated through one or more tubes contained within the shell.</rdfs:comment>
        <rdfs:label xml:lang="es">Condensador de Carcasa Tubular Refrigerado por Agua</rdfs:label>
        <rdfs:label xml:lang="en">Water-cooled Shell Tube Condenser</rdfs:label>
    </owl:Class>
    


    <!-- https://w3id.org/mep#Water-cooledTube-in-TubeCondenser -->


    <owl:Class rdf:about="https://w3id.org/mep#Water-cooledTube-in-TubeCondenser">
        <rdfs:subClassOf rdf:resource="https://w3id.org/mep#Condenser"/>
        <rdfs:comment xml:lang="es">Condensador refrigerado por agua formado por uno o varios conjuntos de dos tubos, uno dentro del otro.</rdfs:comment>
        <rdfs:comment xml:lang="en">Water-cooled condenser consisting of one or more assemblies of two tubes, one within the other.</rdfs:comment>
        <rdfs:label xml:lang="es">Condensador Tubo-en-Tubo Refrigerado por Agua</rdfs:label>
        <rdfs:label xml:lang="en">Water-cooled Tube-in-Tube Condenser</rdfs:label>
    </owl:Class>
    


    <!-- https://w3id.org/mep#WaterBoiler -->


    <owl:Class rdf:about="https://w3id.org/mep#WaterBoiler">
        <rdfs:subClassOf rdf:resource="https://w3id.org/mep#Boiler"/>
        <rdfs:comment xml:lang="es">Caldera de Agua</rdfs:comment>
        <rdfs:comment xml:lang="en">Water Boiler</rdfs:comment>
        <rdfs:label xml:lang="es">Caldera de Agua</rdfs:label>
        <rdfs:label xml:lang="en">Water Boiler</rdfs:label>
    </owl:Class>
    


    <!-- https://w3id.org/mep#WaterCooledChiller -->


    <owl:Class rdf:about="https://w3id.org/mep#WaterCooledChiller">
        <rdfs:subClassOf rdf:resource="https://w3id.org/mep#Chiller"/>
        <rdfs:comment xml:lang="es">Enfirador Refrigerado por Agua</rdfs:comment>
        <rdfs:comment xml:lang="en">Water cooled chiller.</rdfs:comment>
        <rdfs:label xml:lang="es">Enfirador Refrigerado por Agua</rdfs:label>
        <rdfs:label xml:lang="en">Water Cooled Chiller</rdfs:label>
    </owl:Class>
    


    <!-- https://w3id.org/mep#WaterCoolingCoil -->


    <owl:Class rdf:about="https://w3id.org/mep#WaterCoolingCoil">
        <rdfs:subClassOf rdf:resource="https://w3id.org/mep#Coil"/>
        <rdfs:comment xml:lang="en">Cooling coil using chilled water.</rdfs:comment>
        <rdfs:comment xml:lang="es">Serpentín de enfriamiento mediante agua helada.</rdfs:comment>
        <rdfs:label xml:lang="es">Serpentin de Enfriamiento </rdfs:label>
        <rdfs:label xml:lang="en">Water Cooling Coil</rdfs:label>
    </owl:Class>
    


    <!-- https://w3id.org/mep#WaterFilter -->


    <owl:Class rdf:about="https://w3id.org/mep#WaterFilter">
        <rdfs:subClassOf rdf:resource="https://w3id.org/mep#Filter"/>
        <rdfs:comment xml:lang="en">A filter used to remove particulates from water.</rdfs:comment>
        <rdfs:comment xml:lang="es">Un filtro utilizado para eliminar partículas del agua.</rdfs:comment>
        <rdfs:label xml:lang="es">Filtro de Agua</rdfs:label>
        <rdfs:label xml:lang="en">Water Filter</rdfs:label>
    </owl:Class>
    


    <!-- https://w3id.org/mep#WaterHeatingCoil -->


    <owl:Class rdf:about="https://w3id.org/mep#WaterHeatingCoil">
        <rdfs:subClassOf rdf:resource="https://w3id.org/mep#Coil"/>
        <rdfs:comment xml:lang="en">Heating coil using hot water as a heating source.</rdfs:comment>
        <rdfs:comment xml:lang="es">Serpentín de calefacción que utiliza agua caliente como fuente de calor.</rdfs:comment>
        <rdfs:label xml:lang="es">Serpentin Calefactor de Agua</rdfs:label>
        <rdfs:label xml:lang="en">Water Heating Coil</rdfs:label>
    </owl:Class>
    


    <!-- https://w3id.org/mep#WaterMeter -->


    <owl:Class rdf:about="https://w3id.org/mep#WaterMeter">
        <rdfs:subClassOf rdf:resource="https://w3id.org/mep#FlowMeter"/>
        <rdfs:comment xml:lang="en">A device that measures the quantity of water.</rdfs:comment>
        <rdfs:comment xml:lang="es">Un dispositivo que mide la cantidad de agua.</rdfs:comment>
        <rdfs:label xml:lang="es">Caudalimetro</rdfs:label>
        <rdfs:label xml:lang="en">Water Meter</rdfs:label>
    </owl:Class>
    


    <!-- https://w3id.org/mep#WeatherStation -->


    <owl:Class rdf:about="https://w3id.org/mep#WeatherStation">
        <rdfs:subClassOf rdf:resource="https://w3id.org/mep#UnitaryControlElement"/>
        <rdfs:comment xml:lang="en">A control element that senses multiple climate properties such as temperature, humidity, pressure, wind, and rain.</rdfs:comment>
        <rdfs:comment xml:lang="es">Un elemento de control que detecta múltiples propiedades climáticas como temperatura, humedad, presión, viento y lluvia.</rdfs:comment>
        <rdfs:label xml:lang="es">Estacion Meterologica</rdfs:label>
        <rdfs:label xml:lang="en">Weather Station</rdfs:label>
    </owl:Class>
    


    <!-- https://w3id.org/mep#WeldedShellHermeticCompressor -->


    <owl:Class rdf:about="https://w3id.org/mep#WeldedShellHermeticCompressor">
        <rdfs:subClassOf rdf:resource="https://w3id.org/mep#Compressor"/>
        <rdfs:comment xml:lang="es">Compresor alternativo de desplazamiento positivo en el que el motocompresor está montado dentro de una carcasa de acero que, a su vez, está sellada mediante soldadura.</rdfs:comment>
        <rdfs:comment xml:lang="en">Positive-displacement reciprocating compressor where the motor compressor is mounted inside a steel shell, which, in turn is sealed by welding.</rdfs:comment>
        <rdfs:label xml:lang="es">Compresor Hermetico de Cascara Soldada</rdfs:label>
        <rdfs:label xml:lang="en">Welded Shell Hermetic Compressor</rdfs:label>
    </owl:Class>
    


    <!-- https://w3id.org/mep#WheelSensor -->


    <owl:Class rdf:about="https://w3id.org/mep#WheelSensor">
        <rdfs:subClassOf rdf:resource="https://w3id.org/mep#Sensor"/>
        <rdfs:comment xml:lang="en">A device that senses or detects the passage of a wheel.</rdfs:comment>
        <rdfs:comment xml:lang="es">Dispositivo que percibe o detecta el paso de una rueda.</rdfs:comment>
        <rdfs:label xml:lang="es">Sensor de Rueda</rdfs:label>
        <rdfs:label xml:lang="en">Wheel Sensor</rdfs:label>
    </owl:Class>
    


    <!-- https://w3id.org/mep#Whistle -->


    <owl:Class rdf:about="https://w3id.org/mep#Whistle">
        <rdfs:subClassOf rdf:resource="https://w3id.org/mep#Alarm"/>
        <rdfs:comment xml:lang="en">An audible alarm.</rdfs:comment>
        <rdfs:comment xml:lang="es">Una alarma sonora.</rdfs:comment>
        <rdfs:label xml:lang="es">Silbato</rdfs:label>
        <rdfs:label xml:lang="en">Whistle</rdfs:label>
    </owl:Class>
    


    <!-- https://w3id.org/mep#WindSensor -->


    <owl:Class rdf:about="https://w3id.org/mep#WindSensor">
        <rdfs:subClassOf rdf:resource="https://w3id.org/mep#Sensor"/>
        <rdfs:comment xml:lang="en">A device that senses or detects airflow speed and direction.</rdfs:comment>
        <rdfs:comment xml:lang="es">Dispositivo que detecta la velocidad y dirección del flujo de aire.</rdfs:comment>
        <rdfs:label xml:lang="es">Anemomentro</rdfs:label>
        <rdfs:label xml:lang="en">Wind Sensor</rdfs:label>
    </owl:Class>
    


    <!-- https://w3id.org/mep#WirePairSegment -->


    <owl:Class rdf:about="https://w3id.org/mep#WirePairSegment">
        <rdfs:subClassOf rdf:resource="https://w3id.org/mep#CableSegment"/>
        <rdfs:comment xml:lang="en">A pair of conductors contained in a copper cable. The pair is always used together to form a circuit to transmit data by means of electric signals.</rdfs:comment>
        <rdfs:comment xml:lang="es">Un par de conductores contenidos en un cable de cobre. El par siempre se utiliza junto para formar un circuito para transmitir datos mediante señales eléctricas.</rdfs:comment>
        <rdfs:label xml:lang="es">Segmento de Par de Cables </rdfs:label>
        <rdfs:label xml:lang="en">Wire Pair Segment</rdfs:label>
    </owl:Class>
</rdf:RDF>



<!-- Generated by the OWL API (version 5.1.18) https://github.com/owlcs/owlapi/ -->


