@prefix : <https://w3id.org/beo#> .
@prefix owl: <http://www.w3.org/2002/07/owl#> .
@prefix rdf: <http://www.w3.org/1999/02/22-rdf-syntax-ns#> .
@prefix xml: <http://www.w3.org/XML/1998/namespace> .
@prefix xsd: <http://www.w3.org/2001/XMLSchema#> .
@prefix rdfs: <http://www.w3.org/2000/01/rdf-schema#> .
@base <https://w3id.org/beo#> .

<https://w3id.org/beo#> rdf:type owl:Ontology ;
                         owl:versionIRI <https://w3id.org/beo#> ;
                         <http://creativecommons.org/ns#license> "http://creativecommons.org/licenses/by/3.0/" ;
                         <http://purl.org/dc/elements/1.1/abstract> "This Ontology is automatically using the IFCExpress2BEO custom converter developed  by Carlos Ramonell (carlos.ramonell@upc.edu)" ;
                         <http://purl.org/dc/elements/1.1/creator> "Carlos Ramonell Cazador (carlos.ramonell@upc.edu)" ;
                         <http://purl.org/dc/elements/1.1/date> "2024/04/11" ;
                         <http://purl.org/dc/elements/1.1/description> "OWL ontology to describe built elements in the built environment. It is based on the Product ontology descibed in IFC (Insutry Foundation Classes) schema." ;
                         <http://purl.org/dc/elements/1.1/identifier> "Built Element Ontology" ;
                         <http://purl.org/dc/elements/1.1/language> "en" ;
                         <http://purl.org/dc/elements/1.1/title> "Built Element Ontology" ;
                         <http://purl.org/vocab/vann/preferredNamespacePrefix> "beo" ;
                         <http://purl.org/vocab/vann/preferredNamespaceUri> "https://w3id.org/beo#" ;
                         owl:versionInfo "1.0" .

#################################################################
#    Annotation properties
#################################################################

###  http://creativecommons.org/ns#license
<http://creativecommons.org/ns#license> rdf:type owl:AnnotationProperty .


###  http://purl.org/dc/elements/1.1/abstract
<http://purl.org/dc/elements/1.1/abstract> rdf:type owl:AnnotationProperty .


###  http://purl.org/dc/elements/1.1/contributor
<http://purl.org/dc/elements/1.1/contributor> rdf:type owl:AnnotationProperty .


###  http://purl.org/dc/elements/1.1/creator
<http://purl.org/dc/elements/1.1/creator> rdf:type owl:AnnotationProperty .


###  http://purl.org/dc/elements/1.1/date
<http://purl.org/dc/elements/1.1/date> rdf:type owl:AnnotationProperty .


###  http://purl.org/dc/elements/1.1/description
<http://purl.org/dc/elements/1.1/description> rdf:type owl:AnnotationProperty .


###  http://purl.org/dc/elements/1.1/identifier
<http://purl.org/dc/elements/1.1/identifier> rdf:type owl:AnnotationProperty .


###  http://purl.org/dc/elements/1.1/language
<http://purl.org/dc/elements/1.1/language> rdf:type owl:AnnotationProperty .


###  http://purl.org/dc/elements/1.1/title
<http://purl.org/dc/elements/1.1/title> rdf:type owl:AnnotationProperty .


###  http://purl.org/vocab/vann/preferredNamespacePrefix
<http://purl.org/vocab/vann/preferredNamespacePrefix> rdf:type owl:AnnotationProperty .


###  http://purl.org/vocab/vann/preferredNamespaceUri
<http://purl.org/vocab/vann/preferredNamespaceUri> rdf:type owl:AnnotationProperty .


#################################################################
#    Data properties
#################################################################

###  https://w3id.org/beo#anchorageSlip
:anchorageSlip rdf:type owl:DatatypeProperty ,
                        owl:FunctionalProperty ;
               rdfs:domain :Tendon ;
               rdfs:range xsd:float ;
               rdfs:label "AnchorageSlip" .


###  https://w3id.org/beo#barLength
:barLength rdf:type owl:DatatypeProperty ,
                    owl:FunctionalProperty ;
           rdfs:domain :ReinforcingBar ;
           rdfs:range xsd:float ;
           rdfs:label "BarLength" .


###  https://w3id.org/beo#barSurface
:barSurface rdf:type owl:DatatypeProperty ,
                     owl:FunctionalProperty ;
            rdfs:domain :ReinforcingBar ;
            rdfs:range xsd:string ;
            rdfs:label "BarSurface" .


###  https://w3id.org/beo#crossSectionArea
:crossSectionArea rdf:type owl:DatatypeProperty ,
                           owl:FunctionalProperty ;
                  rdfs:domain :ReinforcingBar ,
                              :Tendon ;
                  rdfs:range xsd:float ;
                  rdfs:label "CrossSectionArea" .


###  https://w3id.org/beo#frictionCoefficient
:frictionCoefficient rdf:type owl:DatatypeProperty ,
                              owl:FunctionalProperty ;
                     rdfs:domain :Tendon ;
                     rdfs:range xsd:float ;
                     rdfs:label "FrictionCoefficient" .


###  https://w3id.org/beo#longitudinalBarCrossSectionArea
:longitudinalBarCrossSectionArea rdf:type owl:DatatypeProperty ,
                                          owl:FunctionalProperty ;
                                 rdfs:domain :ReinforcingMesh ;
                                 rdfs:range xsd:float ;
                                 rdfs:label "LongitudinalBarCrossSectionArea" .


###  https://w3id.org/beo#longitudinalBarNominalDiameter
:longitudinalBarNominalDiameter rdf:type owl:DatatypeProperty ,
                                         owl:FunctionalProperty ;
                                rdfs:domain :ReinforcingMesh ;
                                rdfs:range xsd:float ;
                                rdfs:label "LongitudinalBarNominalDiameter" .


###  https://w3id.org/beo#longitudinalBarSpacing
:longitudinalBarSpacing rdf:type owl:DatatypeProperty ,
                                 owl:FunctionalProperty ;
                        rdfs:domain :ReinforcingMesh ;
                        rdfs:range xsd:float ;
                        rdfs:label "LongitudinalBarSpacing" .


###  https://w3id.org/beo#meshLength
:meshLength rdf:type owl:DatatypeProperty ,
                     owl:FunctionalProperty ;
            rdfs:domain :ReinforcingMesh ;
            rdfs:range xsd:float ;
            rdfs:label "MeshLength" .


###  https://w3id.org/beo#meshWidth
:meshWidth rdf:type owl:DatatypeProperty ,
                    owl:FunctionalProperty ;
           rdfs:domain :ReinforcingMesh ;
           rdfs:range xsd:float ;
           rdfs:label "MeshWidth" .


###  https://w3id.org/beo#minCurvatureRadius
:minCurvatureRadius rdf:type owl:DatatypeProperty ,
                             owl:FunctionalProperty ;
                    rdfs:domain :Tendon ;
                    rdfs:range xsd:float ;
                    rdfs:label "MinCurvatureRadius" .


###  https://w3id.org/beo#nominalDiameter
:nominalDiameter rdf:type owl:DatatypeProperty ,
                          owl:FunctionalProperty ;
                 rdfs:domain :MechanicalFastener ,
                             :ReinforcingBar ,
                             :Tendon ;
                 rdfs:range xsd:float ;
                 rdfs:label "NominalDiameter" .


###  https://w3id.org/beo#nominalLength
:nominalLength rdf:type owl:DatatypeProperty ,
                        owl:FunctionalProperty ;
               rdfs:domain :MechanicalFastener ;
               rdfs:range xsd:float ;
               rdfs:label "NominalLength" .


###  https://w3id.org/beo#numberOfRisers
:numberOfRisers rdf:type owl:DatatypeProperty ,
                         owl:FunctionalProperty ;
                rdfs:domain :StairFlight ;
                rdfs:range xsd:integer ;
                rdfs:label "NumberOfRisers" .


###  https://w3id.org/beo#numberOfTreads
:numberOfTreads rdf:type owl:DatatypeProperty ,
                         owl:FunctionalProperty ;
                rdfs:domain :StairFlight ;
                rdfs:range xsd:integer ;
                rdfs:label "NumberOfTreads" .


###  https://w3id.org/beo#overallHeight
:overallHeight rdf:type owl:DatatypeProperty ,
                        owl:FunctionalProperty ;
               rdfs:domain :Door ,
                           :Window ;
               rdfs:range xsd:float ;
               rdfs:label "OverallHeight" .


###  https://w3id.org/beo#overallWidth
:overallWidth rdf:type owl:DatatypeProperty ,
                       owl:FunctionalProperty ;
              rdfs:domain :Door ,
                          :Window ;
              rdfs:range xsd:float ;
              rdfs:label "OverallWidth" .


###  https://w3id.org/beo#preStress
:preStress rdf:type owl:DatatypeProperty ,
                    owl:FunctionalProperty ;
           rdfs:domain :Tendon ;
           rdfs:range xsd:float ;
           rdfs:label "PreStress" .


###  https://w3id.org/beo#riserHeight
:riserHeight rdf:type owl:DatatypeProperty ,
                      owl:FunctionalProperty ;
             rdfs:domain :StairFlight ;
             rdfs:range xsd:float ;
             rdfs:label "RiserHeight" .


###  https://w3id.org/beo#steelGrade
:steelGrade rdf:type owl:DatatypeProperty ,
                     owl:FunctionalProperty ;
            rdfs:domain :ReinforcingElement ;
            rdfs:range xsd:string ;
            rdfs:label "SteelGrade" .


###  https://w3id.org/beo#tensionForce
:tensionForce rdf:type owl:DatatypeProperty ,
                       owl:FunctionalProperty ;
              rdfs:domain :Tendon ;
              rdfs:range xsd:float ;
              rdfs:label "TensionForce" .


###  https://w3id.org/beo#transverseBarCrossSectionArea
:transverseBarCrossSectionArea rdf:type owl:DatatypeProperty ,
                                        owl:FunctionalProperty ;
                               rdfs:domain :ReinforcingMesh ;
                               rdfs:range xsd:float ;
                               rdfs:label "TransverseBarCrossSectionArea" .


###  https://w3id.org/beo#transverseBarNominalDiameter
:transverseBarNominalDiameter rdf:type owl:DatatypeProperty ,
                                       owl:FunctionalProperty ;
                              rdfs:domain :ReinforcingMesh ;
                              rdfs:range xsd:float ;
                              rdfs:label "TransverseBarNominalDiameter" .


###  https://w3id.org/beo#transverseBarSpacing
:transverseBarSpacing rdf:type owl:DatatypeProperty ,
                               owl:FunctionalProperty ;
                      rdfs:domain :ReinforcingMesh ;
                      rdfs:range xsd:float ;
                      rdfs:label "TransverseBarSpacing" .


###  https://w3id.org/beo#treadLength
:treadLength rdf:type owl:DatatypeProperty ,
                      owl:FunctionalProperty ;
             rdfs:domain :StairFlight ;
             rdfs:range xsd:float ;
             rdfs:label "TreadLength" .


#################################################################
#    Classes
#################################################################

###  https://schema.org/Product
<https://schema.org/Product> rdf:type owl:Class .


###  https://w3id.org/beo#AbutmentAssembly
:AbutmentAssembly rdf:type owl:Class ;
                  rdfs:subClassOf :ElementAssembly ;
                  rdfs:comment "A bridge abutment built up of walls, beams, slabs etc."@en ,
                               "Estribo de un puente formado por muros, vigas, losas, etc."@es ;
                  rdfs:label "Abutment Assembly"@en ,
                             "Estribo"@es .


###  https://w3id.org/beo#AchorPlate
:AchorPlate rdf:type owl:Class ;
            rdfs:subClassOf :DiscreteAccessory ;
            rdfs:comment "Accesorio consistente en una placa de acero, conectores de espárragos de cizallamiento o barras de refuerzo soldadas que se empotra en la superficie de un elemento de hormigón para que otros elementos puedan soldarse o atornillarse a él posteriormente."@es ,
                         "An accessory consisting of a steel plate, shear stud connectors or welded-on rebar which is embedded into the surface of a concrete element so that other elements can be welded or bolted onto it later."@en ;
            rdfs:label "Achor Plate"@en ,
                       "Placa de Anclaje"@es .


###  https://w3id.org/beo#AnchorBolt
:AnchorBolt rdf:type owl:Class ;
            rdfs:subClassOf :MechanicalFastener ;
            rdfs:comment "An anchorbolt is a special bolt which is anchored into concrete, stone, or brickwork."@en ,
                         "Un perno de anclaje es unA perno especial que se ancla en hormigón, piedra o mampostería."@es ;
            rdfs:label "Anchor Bolt"@en ,
                       "Perno de Anclaje"@es .


###  https://w3id.org/beo#AnchoringBar
:AnchoringBar rdf:type owl:Class ;
              rdfs:subClassOf :ReinforcingBar ;
              rdfs:comment "Anchoring reinforcement."@en ,
                           "Refuerzo de Anclaje."@es ;
              rdfs:label "Anchoring Bar"@en ,
                         "Barra de Anclaje"@es .


###  https://w3id.org/beo#ApproachSlab
:ApproachSlab rdf:type owl:Class ;
              rdfs:subClassOf :Slab ;
              rdfs:comment "Part of bridge abutment providing transition from embankment to the bridge"@en ,
                           "Parte del estribo del puente que sirve de transición entre el terraplén y el puente"@es ;
              rdfs:label "Approach Slab"@en ,
                         "Losa de Aproximación"@es .


###  https://w3id.org/beo#Apron
:Apron rdf:type owl:Class ;
       rdfs:subClassOf :BuildingElementPart ;
       rdfs:comment "A form of scour protection consisting of timber, concrete, riprap, paving, or other construction placed adjacent to abutments and piers to prevent undermining."@en ,
                    "Una forma de protección contra la socavación que consiste en madera, concreto, escollera, pavimento u otra construcción colocada adyacente a estribos y pilares para evitar el socavamiento."@es ;
       rdfs:label "Apron"@en ,
                  "Apron"@es .


###  https://w3id.org/beo#Arch
:Arch rdf:type owl:Class ;
      rdfs:subClassOf :ElementAssembly ;
      rdfs:comment "A curved structure."@en ,
                   "Una estructura curva."@es ;
      rdfs:label "Arch"@en ,
                 "Arco"@es .


###  https://w3id.org/beo#ArchSegement
:ArchSegement rdf:type owl:Class ;
              rdfs:subClassOf :Member ;
              rdfs:comment "Individual segment of an arch structure."@en ,
                           "Segmento individual de una estructura de arco."@es ;
              rdfs:label "Arch Segement"@en ,
                         "Segmento de Arco"@es .


###  https://w3id.org/beo#Armour
:Armour rdf:type owl:Class ;
        rdfs:subClassOf :Course ;
        rdfs:comment "ISO 21650: capa de protección sobre un rompeolas, un dique u otras estructuras de escollera compuesta por unidades de blindaje."@es ,
                     "ISO 21650: protective layer on a breakwater, seawall or other rubble mound structures composed of armour units"@en ;
        rdfs:label "Armadura"@es ,
                   "Armour"@en .


###  https://w3id.org/beo#ArmourUnit
:ArmourUnit rdf:type owl:Class ;
            rdfs:subClassOf :BuildingElementPart ;
            rdfs:comment "ISO 21650: relatively large quarry stone or concrete shaped unit that is selected to fit specified geometric characteristics and density."@en ,
                         "ISO 21650: unidad relativamente grande de piedra de cantera u hormigón que se selecciona para ajustarse a características geométricas y densidad específicas."@es ;
            rdfs:label "Armour Unit"@en ,
                       "Unidad de Armadura"@es .


###  https://w3id.org/beo#Awning
:Awning rdf:type owl:Class ;
        rdfs:subClassOf :ShadingDevice ;
        rdfs:comment "A rooflike shelter of canvas or other material extending over a doorway, from the top of a window, over a deck, or similar, in order to provide protection, as from the sun."@en ,
                     "Techo de lona u otro material que se extiende sobre una puerta, desde la parte superior de una ventana, sobre una cubierta o similar, con el fin de proteger, por ejemplo, del sol."@es ;
        rdfs:label "Awning"@en ,
                   "Toldo"@es .


###  https://w3id.org/beo#Axial-yieldDamper
:Axial-yieldDamper rdf:type owl:Class ;
                   rdfs:subClassOf :VibrationDamper ;
                   rdfs:comment "A displacement dependent type damper in which the resistance force generated is determined by the plastic strain amount utilizing the plastic deformation of the steel material. The axial yield type is a damper that yields energy by absorbing the steel material against deformation in the axial direction, that is, in the direction of expansion and contraction."@en ,
                                "Un amortiguador dependiente del desplazamiento en el que la fuerza de resistencia generada está determinada por la cantidad de deformación plástica del acero. El amortiguador de rendimiento axial absorbe enrgía deformando el acero en la dirección axial, es decir, en la dirección de expansión y contracción."@es ;
                   rdfs:label "Amortiguador de Rendimiento Axil"@es ,
                              "Axial-yield Damper"@en .


###  https://w3id.org/beo#BRACKET
:BRACKET rdf:type owl:Class ;
         rdfs:subClassOf :DiscreteAccessory ;
         rdfs:comment "Accesorio en forma de L o similar que se fija en una esquina entre elementos para mantenerlos unidos o para transportar un elemento secundario."@es ,
                      "An L-shaped or similarly shaped accessory attached in a corner between elements to hold them together or to carry a secondary element."@en ;
         rdfs:label "BRACKET"@en ,
                    "Escuadra"@es .


###  https://w3id.org/beo#Backfill
:Backfill rdf:type owl:Class ;
          rdfs:subClassOf :EarthworksFill ;
          rdfs:comment "Fill behind retaining walls or other structures such as quays, behind abutments and bridges."@en ,
                       "Relleno detrás de muros de contención u otras estructuras como muelles, detrás de estribos y puentes."@es ;
          rdfs:label "Backfill"@en ,
                     "Backfill"@es .


###  https://w3id.org/beo#BallastedCourse
:BallastedCourse rdf:type owl:Class ;
                 rdfs:subClassOf :Course ;
                 rdfs:comment "Capa compuesta de piedras rotas bajo las traviesas."@es ,
                              "Layer composed of broken stones under the sleepers."@en ;
                 rdfs:label "Ballasted Course"@en ,
                            "Capa de Balasto"@es .


###  https://w3id.org/beo#Balustrade
:Balustrade rdf:type owl:Class ;
            rdfs:subClassOf :Railing ;
            rdfs:comment "Barandilla situada en el borde de un suelo, en lugar de una escalera o rampa. Algunos ejemplos son las balaustradas en azoteas o balcones, o a lo largo de un puente o en la parte superior de un muro de contención."@es ,
                         "Guardrail located at the edge of a floor, rather then a stair or ramp. Examples are balustrades at roof-tops or balconies, or along a bridge or on top of a retaining wall."@en ;
            rdfs:label "Balaustrada"@es ,
                       "Balustrade"@en .


###  https://w3id.org/beo#BarTendon
:BarTendon rdf:type owl:Class ;
           rdfs:subClassOf :Tendon ;
           rdfs:comment "El tendón está configurado como una barra."@es ,
                        "The tendon is configured as a bar."@en ;
           rdfs:label "Bar Tendon"@en ,
                      "Tendon Barra"@es .


###  https://w3id.org/beo#BarrelRoof
:BarrelRoof rdf:type owl:Class ;
            rdfs:subClassOf :Roof ;
            rdfs:comment "A roof or ceiling having a semicylindrical form."@en ,
                         "Techo de forma semicilíndrica."@es ;
            rdfs:label "Barrel Roof"@en ,
                       "Tejado de Cañon"@es .


###  https://w3id.org/beo#BaseIsolator
:BaseIsolator rdf:type owl:Class ;
              rdfs:subClassOf :VibrationIsolator ;
              rdfs:comment "Aislador de base que evita la transferencia de energía del suelo a la estructura."@es ,
                           "Base isolator preventing transfer of energy from the ground to the structure."@en ;
              rdfs:label "Aislador de Base"@es ,
                         "Base Isolator"@en .


###  https://w3id.org/beo#BasePlate
:BasePlate rdf:type owl:Class ;
           rdfs:subClassOf :Plate ;
           rdfs:comment "A plate used to spread load over a surface, such as underneath a bearing or column."@en ,
                        "Placa utilizada para repartir la carga sobre una superficie, como debajo de un cojinete o columna."@es ;
           rdfs:label "Base Plate"@en ,
                      "Placa e Base"@es .


###  https://w3id.org/beo#BaseSlab
:BaseSlab rdf:type owl:Class ;
          rdfs:subClassOf :Slab ;
          rdfs:comment "La losa se utiliza para representar un forjado contra el suelo (y, por tanto, formando parte de la cimentación)."@es ,
                       "The slab is used to represent a floor slab against the ground (and thereby being a part of the foundation). Another name is mat foundation"@en ;
          rdfs:label "Base Slab"@en ,
                     "Losa de Base"@es .


###  https://w3id.org/beo#Beacon
:Beacon rdf:type owl:Class ;
        rdfs:subClassOf :NavigationElement ;
        rdfs:comment "a fixed vertical structure serving as a navigation mark, to show reefs or other hazards, or provide navigational directions."@en ,
                     "una estructura vertical fija que sirve como marca de navegación, para mostrar arrecifes u otros peligros, o proporcionar indicaciones para la navegación."@es ;
        rdfs:label "Baliza"@es ,
                   "Beacon"@en .


###  https://w3id.org/beo#Beam
:Beam rdf:type owl:Class ;
      rdfs:subClassOf :BuiltElement ;
      rdfs:comment "A Beam is typically a horizontal, or nearly horizontal, structural member that is capable of withstanding load primarily by resisting bending. It may also represent such a member from an architectural point of view. It is not required to be load bearing."@en ,
                   "Una viga suele ser un miembro estructural horizontal, o casi horizontal, que es capaz de soportar cargas principalmente resistiendo la flexión. También puede representar a dicho miembro desde un punto de vista arquitectónico. No es necesario que soporte carga."@es ;
      rdfs:label "Beam"@en ,
                 "Viga"@es .


###  https://w3id.org/beo#BeamGrid
:BeamGrid rdf:type owl:Class ;
          rdfs:subClassOf :ElementAssembly ;
          rdfs:comment "Interconnected beams, located in one (typically horizontal) plane."@en ,
                       "Vigas interconectadas, ubicadas en un plano (generalmente horizontal)."@es ;
          rdfs:label "Beam Grid"@en ,
                     "Grid de Vigas"@es .


###  https://w3id.org/beo#Bearing
:Bearing rdf:type owl:Class ;
         rdfs:subClassOf :BuiltElement ;
         rdfs:comment "Tipo de elemento constructivo que suele utilizarse para transmitir cargas de superestructura a subestructura, y que suele permitir movimientos (desplazamiento o rotación) en uno o más grados de libertad. Normalmente es un componente mecánico adquirido en su totalidad e instalado en obra, pero en casos simples puede construirse en obra (compuesto por otros elementos constructivos, componentes de elementos, etc.)."@es ,
                      "Type of building element that is usually used to transmit loads from superstructure to substructure, and usually allowing movement (displacement or rotation) in one or more degrees of freedom. It is typically a mechanical component procured as a whole and installed on site, but in simple cases it may be built on site (composed of other building elements, element components, etc.)."@en ;
         rdfs:label "Bearing"@en ,
                    "Cojinete"@es .


###  https://w3id.org/beo#Bending-yieldDamper
:Bending-yieldDamper rdf:type owl:Class ;
                     rdfs:subClassOf :VibrationDamper ;
                     rdfs:comment "A displacement dependent type damper in which the resistance force generated is determined by the plastic strain amount utilizing the plastic deformation of the steel material. The bending yield type is a damper, which yields steel material by bending."@en ,
                                  "Un amortiguador dependiente del desplazamiento en el que la fuerza de resistencia generada está determinada por la cantidad de deformación plástica del acero. El amortiguador de rendimiento a flexion absorbe enrgía deformando el acero a flexión."@es ;
                     rdfs:label "Amortiguador de Rendimiento a Flexion"@es ,
                                "Bending-yield Damper"@en .


###  https://w3id.org/beo#BirdProtection
:BirdProtection rdf:type owl:Class ;
                rdfs:subClassOf :DiscreteAccessory ;
                rdfs:comment "A device that prevents a sitting down of birds at electrically critical points and thus birds are protected against electrical shocks and disturbances by short circuit are avoided."@en ,
                             "Dispositivo que impide que las aves se posen en puntos eléctricamente críticos, protegiéndolas así contra descargas eléctricas y evitando perturbaciones por cortocircuito."@es ;
                rdfs:label "Bird Protection"@en ,
                           "Proteccion contra Pajaros"@es .


###  https://w3id.org/beo#Blade
:Blade rdf:type owl:Class ;
       rdfs:subClassOf :Rail ;
       rdfs:comment "A blade is a machined rail, often of special section, but fixed and/or joined at the heel end to a rail to provide continuity of wheel support. The two switch rails in a set are the two inside rails. A switch rail is described as right or left hand according to whether it is part of a right hand or left hand half-set of switches. Note: definition from EN 13232-1-2004."@en ,
                    "Una cuchilla es un carril mecanizado, a menudo de sección especial, pero fijo y/o unido en el extremo del talón a un carril para proporcionar continuidad al soporte de la rueda. Los dos carriles de aguja de un juego son los dos carriles interiores. Un carril de aguja se describe como derecho o izquierdo en función de si forma parte de un semijuego de agujas derecho o izquierdo. Nota: definición de la norma EN 13232-1-2004."@es ;
       rdfs:label "Blade"@en ,
                  "Cuchilla"@es .


###  https://w3id.org/beo#BlockingDevice
:BlockingDevice rdf:type owl:Class ;
                rdfs:subClassOf :TrackElement ;
                rdfs:comment "A device composed of pneumatic, mechanic or electric components causing the braking of a train in case of emergency."@en ,
                             "Dispositivo compuesto de componentes neumáticos, mecánicos o eléctricos que provoca el frenado de un tren en caso de emergencia."@es ;
                rdfs:label "Blocking Device"@en ,
                           "Dispositivo de Bloqueo"@es .


###  https://w3id.org/beo#Bollard
:Bollard rdf:type owl:Class ;
         rdfs:subClassOf :MooringDevice ;
         rdfs:comment "A short, thick post on the deck of a ship or a quay side, to which ship's rope may be secured. not to be confused with traffic bollards."@en ,
                      "Poste corto y grueso situado en la cubierta de un barco o en el costado de un muelle, al que se puede amarrar el cabo del barco. no confundir con los bolardos de tráfico."@es ;
         rdfs:label "Bolardo"@es ,
                    "Bollard"@en .


###  https://w3id.org/beo#Bolt
:Bolt rdf:type owl:Class ;
      rdfs:subClassOf :MechanicalFastener ;
      rdfs:comment "A threaded cylindrical rod that engages with a similarly threaded hole in a nut or any other part to form a fastener. The mechanical fastener often also includes one or more washers and one or more nuts."@en ,
                   "Varilla cilíndrica roscada que encaja con un orificio roscado similar en una tuerca o cualquier otra pieza para formar un cierre. El cierre mecánico también suele incluir una o más arandelas y una o más tuercas."@es ;
      rdfs:label "Bolt"@en ,
                 "Perno"@es .


###  https://w3id.org/beo#BoomBarrier
:BoomBarrier rdf:type owl:Class ;
             rdfs:subClassOf :Door ;
             rdfs:comment "A boom barrier (also known as a boom gate) is a bar, or pole pivoted to allow the boom to block vehicular or pedestrian access through a controlled point."@en ,
                          "Una barrera de pluma (también conocida como barrera de pluma) es una barra o poste pivotante que permite bloquear el acceso de vehículos o peatones a través de un punto controlado."@es ;
             rdfs:label "Barrera de Pluma"@es ,
                        "Boom Barrier"@en .


###  https://w3id.org/beo#BorePile
:BorePile rdf:type owl:Class ;
          rdfs:subClassOf :Pile ;
          rdfs:comment "A bore pile."@en ,
                       "Una pilote perforado."@es ;
          rdfs:label "Bore Pile"@en ,
                     "Pilote Perforado"@es .


###  https://w3id.org/beo#Brace
:Brace rdf:type owl:Class ;
       rdfs:subClassOf :Member ;
       rdfs:comment "A linear element (usually sloped) often used for bracing of a girder or truss."@en ,
                    "Elemento lineal (normalmente inclinado) que suele utilizarse para arriostrar una viga o una celosía."@es ;
       rdfs:label "Brace"@en ,
                  "Riostra"@es .


###  https://w3id.org/beo#BracedFrame
:BracedFrame rdf:type owl:Class ;
             rdfs:subClassOf :ElementAssembly ;
             rdfs:comment "A rigid frame with additional bracing members."@en ,
                          "Un portico rígido con miembros de refuerzo adicionales."@es ;
             rdfs:label "Braced Frame"@en ,
                        "Portico Arriostrado"@es .


###  https://w3id.org/beo#BuildingElementPart
:BuildingElementPart rdf:type owl:Class ;
                     rdfs:subClassOf :ElementComponent ;
                     rdfs:comment "A Building Element Part represents major components as subordinate parts of a building element. Typical usage examples include precast concrete sandwich walls, where the layers may have different geometry representations. In this case the layered material representation does not sufficiently describe the element. Each layer is represented by an own instance of the IfcBuildingElementPart with its own geometry description."@en ,
                                  "Una pieza de elemento de construcción representa componentes principales como partes subordinadas de un elemento de construcción. Los ejemplos de uso típicos incluyen muros sándwich de hormigón prefabricado, donde las capas pueden tener diferentes representaciones geométricas. En este caso, la representación del material en capas no describe suficientemente el elemento. Cada capa está representada por una instancia propia de IfcBuildingElementPart con su propia descripción de geometría."@es ;
                     rdfs:label "Building Element Part"@en ,
                                "Pieza de Elemento de Construccion"@es .


###  https://w3id.org/beo#BuildingElementProxy
:BuildingElementProxy rdf:type owl:Class ;
                      rdfs:subClassOf :BuiltElement ;
                      rdfs:comment "El proxy de elemento de construcción es una definición de proxy que proporciona la misma funcionalidad que los subtipos de IfcBuiltElement, pero sin tener un significado predefinido del tipo especial de elemento de construcción que representa."@es ,
                                   "The Building Element Proxy is a proxy definition that provides the same functionality as subtypes of IfcBuiltElement, but without having a predefined meaning of the special type of building element it represents."@en ;
                      rdfs:label "Building Element Proxy"@en ,
                                 "Proxy de Elemento de Construccion"@es .


###  https://w3id.org/beo#BuiltElement
:BuiltElement rdf:type owl:Class ;
              rdfs:subClassOf <https://schema.org/Product> ;
              rdfs:comment "El elemento construido comprende todos los elementos que forman parte principalmente de la construcción de una instalación construida, es decir, su sistema estructural y de separación de espacios. Los elementos construidos son todas cosas físicamente existentes y tangibles."@es ,
                           "The built element comprises all elements that are primarily part of the construction of a built facility, i.e., its structural and space separating system. Built elements are all physically existent and tangible things."@en ;
              rdfs:label "Built Element"@en ,
                         "Elemento Construido"@es .


###  https://w3id.org/beo#Bumper
:Bumper rdf:type owl:Class ;
        rdfs:subClassOf :ImpactProtectionDevice ;
        rdfs:comment "A bumper is a buffer object at end of track that prevents driving over. It can be fixed on rails or the track panel, or can also be a natural element (e.g. rock, sand)."@en ,
                     "Un parachoques es un objeto amortiguador al final de la vía que impide pasar por encima. Puede fijarse a raíles o al panel de vía, o también puede ser un elemento natural (p. ej. roca, arena)."@es ;
        rdfs:label "Bumper"@en ,
                   "Parachoques"@es .


###  https://w3id.org/beo#Buoy
:Buoy rdf:type owl:Class ;
      rdfs:subClassOf :NavigationElement ;
      rdfs:comment "an anchored floating structure serving as a navigation mark, to show reefs or other hazards, or provide navigational directions."@en ,
                   "una estructura vertical fija que sirve como marca de navegación, para mostrar arrecifes u otros peligros, o proporcionar indicaciones para la navegación."@es ;
      rdfs:label "Boya"@es ,
                 "Buoy"@en .


###  https://w3id.org/beo#ButterflyRoof
:ButterflyRoof rdf:type owl:Class ;
               rdfs:subClassOf :Roof ;
               rdfs:comment "A roof having two slopes, each descending inward from the eaves."@en ,
                            "Un tejado con dos vertientes, cada una descendiendo hacia el interior desde el alero."@es ;
               rdfs:label "Butterfly Roof"@en ,
                          "Tejado Mariposa"@es .


###  https://w3id.org/beo#CableArranger
:CableArranger rdf:type owl:Class ;
               rdfs:subClassOf :DiscreteAccessory ;
               rdfs:comment "A cable arranger is a flexible accessory or a part of a component placed around cables to arrange and minimize flexing of them at the point where it is placed."@en ,
                            "Un organizador de cables es un accesorio flexible o una parte de un componente que se coloca alrededor de los cables para organizarlos y minimizar su flexión en el punto donde se coloca."@es ;
               rdfs:label "Cable Arranger"@en ,
                          "Organizador de Cables"@es .


###  https://w3id.org/beo#Caisson
:Caisson rdf:type owl:Class ;
         rdfs:subClassOf :CaissonFoundation ;
         rdfs:comment "Caja cerrada."@es ,
                      "Closed box."@en ;
         rdfs:label "Caisson"@en ,
                    "Caisson"@es .


###  https://w3id.org/beo#CaissonFoundation
:CaissonFoundation rdf:type owl:Class ;
                   rdfs:subClassOf :DeepFoundation ;
                   rdfs:comment "A Caisson Foundation essentially is a hollow box that can be either open or closed."@en ,
                                "Una cimentación tipo cajón es esencialmente una caja hueca que puede estar abierta o cerrada."@es ;
                   rdfs:label "Caisson Foundation"@en ,
                              "Cimentación Caisson"@es .


###  https://w3id.org/beo#Ceiling
:Ceiling rdf:type owl:Class ;
         rdfs:subClassOf :Covering ;
         rdfs:comment "El cubrimiento se utiliza para representar un techo."@es ,
                      "The covering is used to represent a ceiling."@en ;
         rdfs:label "Ceiling"@en ,
                    "Techo"@es .


###  https://w3id.org/beo#Chain
:Chain rdf:type owl:Class ;
       rdfs:subClassOf :MechanicalFastener ;
       rdfs:comment "A series of linked metal rings used for fastening or securing something, or for pulling loads."@en ,
                    "Serie de anillas metálicas unidas entre sí que sirven para sujetar o asegurar algo, o para arrastrar cargas."@es ;
       rdfs:label "Cadena"@es ,
                  "Chain"@en .


###  https://w3id.org/beo#CheckRail
:CheckRail rdf:type owl:Class ;
           rdfs:subClassOf :Rail ;
           rdfs:comment "A check rail is a rail laid close to the gauge face of a running rail which takes part in lateral guidance of the wheel and prevents derailment in small radius curved track and switches and crossings. Note: definition from EN 13481-1."@en ,
                        "Un contracarril es un carril colocado cerca de la cara del ancho de vía de un carril de rodadura que interviene en el guiado lateral de la rueda y evita el descarrilamiento en vías curvas de pequeño radio y en aparatos de vía. Nota: definición de la norma EN 13481-1."@es ;
           rdfs:label "Check Rail"@en ,
                      "Contracarril"@es .


###  https://w3id.org/beo#Chimney
:Chimney rdf:type owl:Class ;
         rdfs:subClassOf :BuiltElement ;
         rdfs:comment "Chimneys are typically vertical, or as near as vertical, parts of the construction of a building and part of the building fabric. Often constructed by pre-cast or insitu concrete, today seldom by bricks. Chimneys are used to evacuate flues from e.g. boilers or fire places."@en ,
                      "Las chimeneas suelen ser partes verticales, o casi verticales, de la construcción de un edificio y parte de la estructura del edificio. A menudo se construyen con hormigón prefabricado o in situ, hoy en día rara vez con ladrillos. Las chimeneas se utilizan para evacuar los humos de, p. calderas o chimeneas."@es ;
         rdfs:label "Chimenea"@es ,
                    "Chimney"@en .


###  https://w3id.org/beo#Chord
:Chord rdf:type owl:Class ;
       rdfs:subClassOf :Member ;
       rdfs:comment "Miembro longitudinal superior o inferior de una cercha, utilizado horizontalmente o inclinado."@es ,
                    "Upper or lower longitudinal member of a truss, used horizontally or sloped."@en ;
       rdfs:label "Chord"@en ,
                  "Cordon"@es .


###  https://w3id.org/beo#Cladding
:Cladding rdf:type owl:Class ;
          rdfs:subClassOf :Covering ;
          rdfs:comment "El cubrimiento se utiliza para representar un revestimiento."@es ,
                       "The covering is used to represent a cladding."@en ;
          rdfs:label "Cladding"@en ,
                     "Revestimiento"@es .


###  https://w3id.org/beo#CoatedTendon
:CoatedTendon rdf:type owl:Class ;
              rdfs:subClassOf :Tendon ;
              rdfs:comment "El tendón está recubierto."@es ,
                           "The tendon is coated."@en ;
              rdfs:label "Coated Tendon"@en ,
                         "Tendon Recubierto"@es .


###  https://w3id.org/beo#CohesionPile
:CohesionPile rdf:type owl:Class ;
              rdfs:subClassOf :Pile ;
              rdfs:comment "A cohesion pile"@en ,
                           "Una pilacohesiva"@es ;
              rdfs:label "Cohesion Pile"@en ,
                         "Pila Cohesiva"@es .


###  https://w3id.org/beo#Collar
:Collar rdf:type owl:Class ;
        rdfs:subClassOf :Member ;
        rdfs:comment "A linear element (usually used horizontally) within a roof structure to connect rafters and posts."@en ,
                     "Elemento lineal (normalmente utilizado horizontalmente) dentro de una estructura de tejado para conectar cabrios y postes."@es ;
        rdfs:label "Collar"@en ,
                   "Collarin"@es .


###  https://w3id.org/beo#Column
:Column rdf:type owl:Class ;
        rdfs:subClassOf :BuiltElement ;
        rdfs:comment "A Column is a vertical structural or architectural member which often is aligned with a structural grid intersection. In most cases it represents a vertical, or nearly vertical, structural member that transmits, through compression, the weight of the structure above to other structural elements below. It may also represent such a member from an architectural point of view in which case it may represent a non load bearing element"@en ,
                     "Una columna es un elemento estructural o arquitectónico vertical que suele estar alineado con una intersección de la retícula estructural. En la mayoría de los casos representa un miembro estructural vertical, o casi vertical, que transmite, mediante compresión, el peso de la estructura superior a otros elementos estructurales inferiores. También puede representar un miembro de este tipo desde el punto de vista arquitectónico, en cuyo caso puede representar un elemento no portante."@es ;
        rdfs:label "Column"@en ,
                   "Columna"@es .


###  https://w3id.org/beo#CompressionIsolator
:CompressionIsolator rdf:type owl:Class ;
                     rdfs:subClassOf :VibrationIsolator ;
                     rdfs:comment "Aislador de vibraciones tipo compresión."@es ,
                                  "Compression type vibration isolator."@en ;
                     rdfs:label "Aislador de Compresion"@es ,
                                "Compression Isolator"@en .


###  https://w3id.org/beo#Coping
:Coping rdf:type owl:Class ;
        rdfs:subClassOf :Covering ;
        rdfs:comment ""@en ,
                     ""@es ;
        rdfs:label "Albardilla"@es ,
                   "Coping"@en .


###  https://w3id.org/beo#CoreCourse
:CoreCourse rdf:type owl:Class ;
            rdfs:subClassOf :Course ;
            rdfs:comment "A core course is the bulk internal structure of aggregate structures."@en ,
                         "Una pista central es la estructura interna a granel de las estructuras agregadas."@es ;
            rdfs:label "Capa Central"@es ,
                       "Core Course"@en .


###  https://w3id.org/beo#Cornice
:Cornice rdf:type owl:Class ;
         rdfs:subClassOf :Beam ;
         rdfs:comment "A non-loadbearing beam on the longitudinal edge of bridge slab, usually encasing installations."@en ,
                      "Viga que no soporta carga en el borde longitudinal de la losa de un puente, que generalmente envuelve instalaciones."@es ;
         rdfs:label "Cornice"@en ,
                    "Cornisa"@es .


###  https://w3id.org/beo#Counterweigth
:Counterweigth rdf:type owl:Class ;
               rdfs:subClassOf :EarthworksFill ;
               rdfs:comment "Embankment built on the side of the main road structure to reduce the settlement of the road."@en ,
                            "Terraplén construido en el lateral de la estructura principal de la carretera para reducir el asentamiento de la carretera."@es ;
               rdfs:label "Contrapeso"@es ,
                          "Counterweigth"@en .


###  https://w3id.org/beo#Coupler
:Coupler rdf:type owl:Class ;
         rdfs:subClassOf :MechanicalFastener ;
         rdfs:comment "A part connecting two rod or bars, such as reinforcement bars."@en ,
                      "Pieza que une dos barras o varillas, como las barras de refuerzo."@es ;
         rdfs:label "Acoplador"@es ,
                    "Coupler"@en .


###  https://w3id.org/beo#Course
:Course rdf:type owl:Class ;
        rdfs:subClassOf :BuiltElement ;
        rdfs:comment "A built element whose length greatly exceeds its thickness and often also its width, usually of a single material laid on site on top of another horizontal or nearly horizontal built element. A course is distinctive from a earthworks element in that a course is a graded granular (which can be bound or unbound) material that is generally processed in some fashion, where as earthworks elements are soil earthen based structure that can be formed by removal and transport of general ground material. Structurally a course does not have capacity to carry loads over open span, or to be removed or replaced as a single unit. examples of courses include: * Graded aggregate layers * Graded sand layers * Cement bounded material (CBM) * Asphalt layers"@en ,
                     "Una pista es un elemento construido cuya longitud supera con creces su grosor y a menudo también su anchura, normalmente de un único material colocado in situ sobre otro elemento construido horizontal o casi horizontal. Una pista se distingue de un elemento de movimiento de tierras en que una pista es un material granular graduado (que puede estar ligado o no) que generalmente se procesa de alguna manera, mientras que los elementos de movimiento de tierras son estructuras basadas en tierra que pueden formarse mediante la retirada y el transporte de material del suelo en general. Estructuralmente, una pista no tiene capacidad para soportar cargas a lo largo de un tramo abierto, o para ser retirada o sustituida como una sola unidad. algunos ejemplos de pistas son: * Capas de áridos graduados * Capas de arena graduada * Material ligado con cemento (CBM) * Capas de asfalto"@es ;
        rdfs:label "Capa"@es ,
                   "Course"@en .


###  https://w3id.org/beo#CoverPlate
:CoverPlate rdf:type owl:Class ;
            rdfs:subClassOf :Plate ;
            rdfs:comment "A plate (underneath or above) a flange to provide additional load capacity."@en ,
                         "Una placa (debajo o encima) de una brida para proporcionar capacidad de carga adicional."@es ;
            rdfs:label "Cover Plate"@en ,
                       "Placa de Cobertura"@es .


###  https://w3id.org/beo#Covering
:Covering rdf:type owl:Class ;
          rdfs:subClassOf :BuiltElement ;
          rdfs:comment "A covering is an element which covers some part of another element and is fully dependent on that other element."@en ,
                       "Un cubrimiento es un elemento que cubre alguna parte de otro elemento y depende totalmente de ese otro elemento."@es ;
          rdfs:label "Covering"@en ,
                     "Cubrimiento"@es .


###  https://w3id.org/beo#CraneWaySystem
:CraneWaySystem rdf:type owl:Class ;
                rdfs:subClassOf :TransportElement ;
                rdfs:comment "A crane way system, normally including the crane rails, fasteners and the crane. It is primarily used to move heavy goods in a factory or other industry buildings."@en ,
                             "Un sistema de grúa que normalmente incluye los rieles de la grúa, los sujetadores y la grúa. Se utiliza principalmente para mover mercancías pesadas en una fábrica u otros edificios industriales."@es ;
                rdfs:label "Crane Way System"@en ,
                           "Puente Grua"@es .


###  https://w3id.org/beo#CrashCushion
:CrashCushion rdf:type owl:Class ;
              rdfs:subClassOf :ImpactProtectionDevice ;
              rdfs:comment "ISO6707-1: dispositivo de absorción de energía instalado delante de un objeto rígido para reducir la gravedad del impacto de un vehículo"@es ,
                           "ISO6707-1: energy-absorbing device installed in front of a rigid object to reduce the severity of impact of a vehicle, (Impact barrier, US)"@en ;
              rdfs:label "Cojin de Choque"@es ,
                         "Crash Cushion"@en .


###  https://w3id.org/beo#CrossBracing
:CrossBracing rdf:type owl:Class ;
              rdfs:subClassOf :ElementAssembly ;
              rdfs:comment "A Structural linear member or assembly of members inside a box girder or between girders, typically on a pier, to resist lateral forces and transfer them to the support."@en ,
                           "Un miembro lineal estructural o un conjunto de miembros dentro de una viga cajón o entre vigas, típicamente en un pilar, para resistir fuerzas laterales y transferirlas al soporte."@es ;
              rdfs:label "Arriostramiento Trasversal"@es ,
                         "Cross Bracing"@en .


###  https://w3id.org/beo#CurtainPanel
:CurtainPanel rdf:type owl:Class ;
              rdfs:subClassOf :Plate ;
              rdfs:comment "A planar element within a curtain wall, often consisting of a frame with fixed glazing."@en ,
                           "Elemento plano de un muro cortina, a menudo constituido por un marco con acristalamiento fijo."@es ;
              rdfs:label "Curtain Panel"@en ,
                         "Panel de Cortina"@es .


###  https://w3id.org/beo#CurtainWall
:CurtainWall rdf:type owl:Class ;
             rdfs:subClassOf :BuiltElement ;
             rdfs:comment "ISO 6707-1: muro no portante situado en el exterior de un edificio y que lo encierra."@es ,
                          "ISO 6707-1: non load bearing wall positioned on the outside of a building and enclosing it."@en ;
             rdfs:label "CurtainWall"@en ,
                        "Muro Cortina"@es .


###  https://w3id.org/beo#CurvedRunStair
:CurvedRunStair rdf:type owl:Class ;
                rdfs:subClassOf :Stair ;
                rdfs:comment "A stair extending from one level to another without turns or winders. The stair is consisting of one curved flight."@en ,
                             "Escalera que se extiende de un nivel a otro sin giros ni devanaderas. La escalera consta de un tramo curvo."@es ;
                rdfs:label "Curved Run Stair"@en ,
                           "Escalera de Tramo Curvo"@es .


###  https://w3id.org/beo#CurvedStairFlight
:CurvedStairFlight rdf:type owl:Class ;
                   rdfs:subClassOf :StairFlight ;
                   rdfs:comment "A stair flight with a curved walking line."@en ,
                                "Un tramo de escalera con una línea de paso curva."@es ;
                   rdfs:label "Curved Stair Flight"@en ,
                              "Tramo de Escalera Curvo"@es .


###  https://w3id.org/beo#CylindricalBearing
:CylindricalBearing rdf:type owl:Class ;
                    rdfs:subClassOf :Bearing ;
                    rdfs:comment "La función de soporte la proporciona un cilindro en un cilindro cóncavo."@es ,
                                 "The bearing functionality is provided by cylinder in a concave cylinder."@en ;
                    rdfs:label "Cojinete Cilindrico"@es ,
                               "Cylindrical Bearing"@en .


###  https://w3id.org/beo#DampingSystem
:DampingSystem rdf:type owl:Class ;
               rdfs:subClassOf :ImpactProtectionDevice ;
               rdfs:comment "An elastic element inserted between the superstructure (track and plate on slab track or ballast bed with ballast inserted in) and the tunnel structure (tunnel floor). Some of the elastic elements have a partial decoupling effect between the superstructure and underground due to vibrations. Both helical springs and elastomer blocks or elastomer strips can be used as suspension systems."@en ,
                            "Elemento elástico insertado entre la superestructura (vía y placa sobre vía en placa o lecho de balasto con balasto insertado) y la estructura del túnel (suelo del túnel). Algunos de los elementos elásticos tienen un efecto de desacoplamiento parcial entre la superestructura y el subsuelo debido a las vibraciones. Como sistemas de suspensión se pueden utilizar tanto muelles helicoidales como bloques o tiras de elastómero."@es ;
               rdfs:label "Damping System"@en ,
                          "Sistema de Amortiguacion"@es .


###  https://w3id.org/beo#DeckAssembly
:DeckAssembly rdf:type owl:Class ;
              rdfs:subClassOf :ElementAssembly ;
              rdfs:comment "A platform (such as floor or bridge deck) built up of beams, slabs."@en ,
                           "Una plataforma (como piso o tablero de puente) construida con vigas y losas."@es ;
              rdfs:label "Deck Assembly"@en ,
                         "Tablero"@es .


###  https://w3id.org/beo#DeepFoundation
:DeepFoundation rdf:type owl:Class ;
                rdfs:subClassOf :BuiltElement ;
                rdfs:comment "Deep foundation is a type of foundation that transfers loads deeper than shallow foundation below the soft soils not capable of bearing the above structure. Depending on the soil strength it might have to reach down to the rock layer."@en ,
                             "La cimentación profunda es un tipo de cimentación que transfiere las cargas a mayor profundidad que la cimentación superficial por debajo de los suelos blandos que no son capaces de soportar la estructura anterior. Dependiendo de la resistencia del suelo, puede llegar hasta la capa rocosa."@es ;
                rdfs:label "Cimentación Profunda"@es ,
                           "DeepFoundation"@en .


###  https://w3id.org/beo#Derailer
:Derailer rdf:type owl:Class ;
          rdfs:subClassOf :TrackElement ;
          rdfs:comment "A fixed device which, when placed on the rail, derails the wheels of a vehicle, and serves to protect a converging line. Note: definition from IEC 60050-821."@en ,
                       "Dispositivo fijo que, colocado sobre el carril, hace descarrilar las ruedas de un vehículo y sirve para proteger una línea convergente. Nota: definición de la norma IEC 60050-821."@es ;
          rdfs:label "Derailer"@en ,
                     "Descarrilador"@es .


###  https://w3id.org/beo#Diabolo
:Diabolo rdf:type owl:Class ;
         rdfs:subClassOf :TendonConduit ;
         rdfs:comment "A part of tendon conduit associated to deviator."@en ,
                      "Parte de delconducto para tendones asociada al desviador"@es ;
         rdfs:label "Diabolo"@en ,
                    "Diabolo"@es .


###  https://w3id.org/beo#Diaphragm
:Diaphragm rdf:type owl:Class ;
           rdfs:subClassOf :Beam ;
           rdfs:comment "End portion of a girder transmitting loads to supports and providing moment resistance to adjoining segment."@en ,
                        "Porción final de una viga que transmite cargas a los soportes y proporciona resistencia al momento al segmento contiguo."@es ;
           rdfs:label "Diafragma"@es ,
                      "Diaphragm"@en .


###  https://w3id.org/beo#DilatationPanel
:DilatationPanel rdf:type owl:Class ;
                 rdfs:subClassOf :ElementAssembly ;
                 rdfs:comment "Device which permits longitudinal relative rail movement of two adjacent rails, while maintaining correct guidance and support."@en ,
                              "Dispositivo que permite el movimiento relativo longitudinal de dos carriles adyacentes, manteniendo un correcto guiado y apoyo."@es ;
                 rdfs:label "Dilatation Panel"@en ,
                            "Panel de Dilatación"@es .


###  https://w3id.org/beo#DiscreteAccessory
:DiscreteAccessory rdf:type owl:Class ;
                   rdfs:subClassOf :ElementComponent ;
                   rdfs:comment "A discrete accessory is a representation of different kinds of accessories included in or added to elements."@en ,
                                "Un accesorio discreto es una representación de diferentes tipos de accesorios incluidos en elementos o añadidos a ellos."@es ;
                   rdfs:label "Accesorio Discreto"@es ,
                              "DiscreteAccessory"@en .


###  https://w3id.org/beo#DiskBearing
:DiskBearing rdf:type owl:Class ;
             rdfs:subClassOf :Bearing ;
             rdfs:comment "A disk bearing consist of an elastomeric disc between two metal plates."@en ,
                          "Un soporte de disco consta de un disco elastomérico entre dos placas metálicas."@es ;
             rdfs:label "Cojinete de Disco"@es ,
                        "Disk Bearing"@en .


###  https://w3id.org/beo#DomeRoof
:DomeRoof rdf:type owl:Class ;
          rdfs:subClassOf :Roof ;
          rdfs:comment "A hemispherical hip roof."@en ,
                       "Un tejado a cuatro aguas semiesférico."@es ;
          rdfs:label "Dome Roof"@en ,
                     "Techo Abovedado"@es .


###  https://w3id.org/beo#Door
:Door rdf:type owl:Class ;
      rdfs:subClassOf :BuiltElement ;
      rdfs:comment "La puerta es un elemento construido que se utiliza predominantemente para proporcionar un acceso controlado a personas, mercancías, animales y vehículos. Incluye construcciones con bisagras, pivotes, correderas y, además, giratorias y plegables."@es ,
                   "The door is a built element that is predominately used to provide controlled access for people, goods, animals and vehicles. It includes constructions with hinged, pivoted, sliding, and additionally revolving and folding operations."@en ;
      rdfs:label "Door"@en ,
                 "Puerta"@es .


###  https://w3id.org/beo#DoubleReturnStair
:DoubleReturnStair rdf:type owl:Class ;
                   rdfs:subClassOf :Stair ;
                   rdfs:comment "A stair having one straight flight to a wide quarterspace landing, and two side flights from that landing into opposite directions. The stair is making a 90° turn. The direction of traffic is determined by the walking line."@en ,
                                "Escalera que tiene un tramo recto hasta un descansillo ancho y dos tramos laterales desde ese descansillo en direcciones opuestas. La escalera realiza un giro de 90°. El sentido de circulación viene determinado por la línea de paso."@es ;
                   rdfs:label "Double Return Stair"@en ,
                              "Escalera de Doble Retorn"@es .


###  https://w3id.org/beo#Dowel
:Dowel rdf:type owl:Class ;
       rdfs:subClassOf :MechanicalFastener ;
       rdfs:comment "A cylindrical rod that is driven into holes of the connected pieces."@en ,
                    "Una varilla cilíndrica que se introduce en los orificios de las piezas conectadas."@es ;
       rdfs:label "Dowel"@en ,
                  "Pasador"@es .


###  https://w3id.org/beo#DrivenPile
:DrivenPile rdf:type owl:Class ;
            rdfs:subClassOf :Pile ;
            rdfs:comment "A rammed, vibrated, or otherwise driven pile."@en ,
                         "Pilote apisonado, vibrado o hincado de otro modo."@es ;
            rdfs:label "Driven Pile"@en ,
                       "Pilote Hincado"@es .


###  https://w3id.org/beo#DynamicallyCompactedSoil
:DynamicallyCompactedSoil rdf:type owl:Class ;
                          rdfs:subClassOf :ReinforcedSoil ;
                          rdfs:comment "El método de utilización de la apisonadora dinámica suele consistir en la caída libre de un pesado martillo desde la altura, compactando el suelo y mejorando rápidamente la capacidad portante de los cimientos."@es ,
                                       "Soil reinforced  method of using dynamic tamping machine usually free falling a heavy hammer from the height, compacting the soil and quickly improving the bearing capacity of the foundation."@en ;
                          rdfs:label "Dynamically Compacted Soil"@en ,
                                     "Suelo Compactado Dinamicamente"@es .


###  https://w3id.org/beo#ESCALATOR
:ESCALATOR rdf:type owl:Class ;
           rdfs:subClassOf :TransportElement ;
           rdfs:comment "Consiste en escalones individuales vinculados que se mueven hacia arriba y hacia abajo sobre rieles manteniendo los hilos horizontales."@es ,
                        "Escalator being a transport device to move people. It consists of individual linked steps that move up and down on tracks while keeping the threads horizontal."@en ;
           rdfs:label "ESCALATOR"@en ,
                      "Escalera Mecanica"@es .


###  https://w3id.org/beo#EarthworksElement
:EarthworksElement rdf:type owl:Class ;
                   rdfs:subClassOf :BuiltElement ;
                   rdfs:comment "A type of built element created by earthwork activities to build subgrade, to raise the level of the ground in general or reinforce or stabilize soil by some mechanical or chemical method."@en ,
                                "Tipo de elemento construido creado por las actividades de movimiento de tierras para construir el subsuelo, elevar el nivel del terreno en general o reforzar o estabilizar el suelo mediante algún método mecánico o químico."@es ;
                   rdfs:label "Earthworks Element"@en ,
                              "Elemento de movimiento de tierras"@es .


###  https://w3id.org/beo#EarthworksFill
:EarthworksFill rdf:type owl:Class ;
                rdfs:subClassOf :EarthworksElement ;
                rdfs:comment "A type of earthworks element created by earthwork activities to build subgrade or to raise the level of the ground in general."@en ,
                             "Tipo de elemento de movimiento de tierras creado por las actividades de movimiento de tierras para construir el subsuelo o para elevar el nivel del terreno en general."@es ;
                rdfs:label "Earthworks Fill"@en ,
                           "Relleno de Movimiento de Tierras"@es .


###  https://w3id.org/beo#EdgeBar
:EdgeBar rdf:type owl:Class ;
         rdfs:subClassOf :ReinforcingBar ;
         rdfs:comment "Edge reinforcement."@en ,
                      "Refuerzo de bordes."@es ;
         rdfs:label "Barra de Borde"@es ,
                    "Edge Bar"@en .


###  https://w3id.org/beo#EdgeBeam
:EdgeBeam rdf:type owl:Class ;
          rdfs:subClassOf :Beam ;
          rdfs:comment "A beam on the longitudinal edge of bridge slab, usually concrete, providing additional stiffening and protection from the elements."@en ,
                       "Una viga en el borde longitudinal de la losa de un puente, generalmente de hormigón, que proporciona rigidez adicional y protección contra los elementos."@es ;
          rdfs:label "Edge Beam"@en ,
                     "Viga de Borde"@es .


###  https://w3id.org/beo#ElasticCushion
:ElasticCushion rdf:type owl:Class ;
                rdfs:subClassOf :DiscreteAccessory ;
                rdfs:comment "A track elastic cushion is a kind of layer set on grooved sides of a concrete base, which is used for mitigating the impact of longitudinal and lateral load on track structures. A track elastic cushion shall only appear in ballastless track structures."@en ,
                             "Un cojín elástico de vía es un tipo de capa colocada en los lados ranurados de una base de hormigón, que se utiliza para mitigar el impacto de la carga longitudinal y lateral en las estructuras de vía. Un cojín elástico de vía sólo aparecerá en estructuras de vía en placa."@es ;
                rdfs:label "Cojin Elastico"@es ,
                           "Elastic Cushion"@en .


###  https://w3id.org/beo#ElastomericBearing
:ElastomericBearing rdf:type owl:Class ;
                    rdfs:subClassOf :Bearing ;
                    rdfs:comment "A pad bearing which carries vertical load by contact stresses between a sheet of sliding material and a mating surface that permits movements by sliding and accommodates rotation by deformation of the elastomer."@en ,
                                 "Un cojinete de almohadillas que soporta carga vertical mediante tensiones de contacto entre una lámina de material deslizante y una superficie de contacto que permite movimientos por deslizamiento y se adapta a la rotación por deformación del elastómero."@es ;
                    rdfs:label "Cojinete Elastomerico"@es ,
                               "Elastomeric Bearing"@en .


###  https://w3id.org/beo#ElementAssembly
:ElementAssembly rdf:type owl:Class ;
                 rdfs:subClassOf <https://schema.org/Product> ;
                 rdfs:comment "Representa conjuntos de elementos complejos agregados a partir de varios elementos, como elementos discretos, elementos de construcción u otros elementos."@es ,
                              "Represents complex element assemblies aggregated from several elements, such as discrete elements, building elements, or other elements."@en ;
                 rdfs:label "Element Assembly"@en ,
                            "Ensamblaje de Elementos"@es .


###  https://w3id.org/beo#ElementComponent
:ElementComponent rdf:type owl:Class ;
                  rdfs:subClassOf <https://schema.org/Product> ;
                  rdfs:comment "An element component is a representation for minor items included in, added to or connecting to or between elements, which usually are not of interest from the overall building structure viewpoint. However, these small parts may have vital and load carrying functions within the construction. These items do not provide any actual space boundaries."@en ,
                               "Un componente de elemento es una representación de elementos menores incluidos, agregados o conectados a o entre elementos, que generalmente no son de interés desde el punto de vista general de la estructura del edificio. Sin embargo, estas piezas pequeñas pueden tener funciones vitales y de transporte de carga dentro de la construcción. Estos elementos no proporcionan límites de espacio reales."@es ;
                  rdfs:label "Componente de Elemento"@es ,
                             "ElementComponent"@en .


###  https://w3id.org/beo#ElementedWall
:ElementedWall rdf:type owl:Class ;
               rdfs:subClassOf :Wall ;
               rdfs:comment "A stud wall framed with studs and faced with sheetings, sidings, wallboard, or plasterwork."@en ,
                            "Una pared de vigas enmarcada con vigas y revestida con láminas, revestimientos, paneles de yeso o yeserías."@es ;
               rdfs:label "Elemented Wall"@en ,
                          "Pared de Elementos"@es .


###  https://w3id.org/beo#Elevator
:Elevator rdf:type owl:Class ;
          rdfs:subClassOf :TransportElement ;
          rdfs:comment "Ascensor o montacargas. Es un dispositivo de transporte para mover personas o mercancías verticalmente."@es ,
                       "Elevator or lift being a transport device to move people or goods vertically."@en ;
          rdfs:label "Ascensor"@es ,
                     "Elevator"@en .


###  https://w3id.org/beo#Embankment
:Embankment rdf:type owl:Class ;
            rdfs:subClassOf :EarthworksFill ;
            rdfs:comment "Elemento de movimiento de tierras de tipo predominantemente longitudinal, sin otro tipo particular asignado en función de su rol en el pavimento o la subrasante. NOTA Definición de ISO6707-1: sección de movimiento de tierras, a menudo formada por corte o relleno, en la que el nivel del terreno acabado está por encima o por debajo del nivel del terreno original y cuya longitud suele superar ampliamente su anchura."@es ,
                         "Predominantly longitudinal type of earthworks element with no other particular assigned type according to its role in Pavement or Subgrade. NOTE Definition from ISO6707-1: section of earthworks, often formed by cut or fill, where the finished ground level is above or below original ground level and whose length usually greatly exceeds its width."@en ;
            rdfs:label "Embankment"@en ,
                       "Terraplen"@es .


###  https://w3id.org/beo#EntranceWorks
:EntranceWorks rdf:type owl:Class ;
               rdfs:subClassOf :ElementAssembly ;
               rdfs:comment "An assembly forming the support structure of a chamber (lock, dock) gate and associated elements, plus the containment of operational equipment."@en ,
                            "Conjunto que forma la estructura de soporte de la puerta de una cámara (esclusa, muelle) y elementos asociados, además de la contención del equipo operativo."@es ;
               rdfs:label "Cabezal"@es ,
                          "Entrance Works"@en .


###  https://w3id.org/beo#ExpansionJointDevice
:ExpansionJointDevice rdf:type owl:Class ;
                      rdfs:subClassOf :DiscreteAccessory ;
                      rdfs:comment "Assembly connection element between construction elements to allow for thermic differential expansions."@en ,
                                   "Ensablaje entre elementos constructivos para permitir dilataciones térmicas diferenciales."@es ;
                      rdfs:label "Expansion Joint Device"@en ,
                                 "Junta de Expansion"@es .


###  https://w3id.org/beo#Fastener
:Fastener rdf:type owl:Class ;
          rdfs:subClassOf :ElementComponent ;
          rdfs:comment "Representaciones de piezas de fijación que se utilizan como elementos de sujeción para conectar o unir elementos con otros elementos. Se excluyen los cierres mecánicos que son modelados por una entidad separada."@es ,
                       "Representations of fixing parts which are used as fasteners to connect or join elements with other elements. Excluded are mechanical fasteners which are modeled by a separate entity"@en ;
          rdfs:label "Cierres"@es ,
                     "Fastener"@en .


###  https://w3id.org/beo#Fence
:Fence rdf:type owl:Class ;
       rdfs:subClassOf :Railing ;
       rdfs:comment "NOTA Definición de ISO6707-1: construcción vertical no portante, normalmente ligera, que delimita o subdivide una zona exterior."@es ,
                    "NOTE Definition from ISO6707-1: non-load bearing vertical construction, usually lightweight, which bounds or subdivides an external area."@en ;
       rdfs:label "Fence"@en ,
                  "Valla"@es .


###  https://w3id.org/beo#Fender
:Fender rdf:type owl:Class ;
        rdfs:subClassOf :ImpactProtectionDevice ;
        rdfs:comment "A passive or active device formed of a damper and impact panel that is mounted on the quayside to protect against vessel impact."@en ,
                     "Dispositivo pasivo o activo formado por un amortiguador y un panel de impacto que se monta en el muelle para proteger contra el impacto del buque."@es ;
        rdfs:label "Defensa"@es ,
                   "Fender"@en .


###  https://w3id.org/beo#Filler
:Filler rdf:type owl:Class ;
        rdfs:subClassOf :DiscreteAccessory ;
        rdfs:comment "Sealant, gap filler rod, packing material or other used to close a gap."@en ,
                     "Sellador, varilla de relleno de huecos, material de empaquetadura u otro utilizado para cerrar un hueco."@es ;
        rdfs:label "Filler"@en ,
                   "Filler"@es .


###  https://w3id.org/beo#FilterCourse
:FilterCourse rdf:type owl:Class ;
              rdfs:subClassOf :Course ;
              rdfs:comment "An Intermediate layer whose primary function is to prevent the washing through of fine materials."@en ,
                           "Capa intermedia cuya función principal es evitar el arrastre de materiales finos."@es ;
              rdfs:label "Capa de filtrado"@es ,
                         "Filter Course"@en .


###  https://w3id.org/beo#FixedEndAnchor
:FixedEndAnchor rdf:type owl:Class ;
                rdfs:subClassOf :TendonAnchor ;
                rdfs:comment "El anclaje fija el extremo de un tendón."@es ,
                             "The anchor fixes the end of a tendon."@en ;
                rdfs:label "Anclaje de Extremo Fijo"@es ,
                           "Fixed End Anchor"@en .


###  https://w3id.org/beo#FlangePlate
:FlangePlate rdf:type owl:Class ;
             rdfs:subClassOf :Plate ;
             rdfs:comment "A flange plate in linear members having box or I-profile (e.g. top or bottom flange plate in box-girder)."@en ,
                          "Una placa de ala en elementos lineales con perfil en caja o en I (por ejemplo, placa de ala superior o inferior en vigas cajón)."@es ;
             rdfs:label "Flange Plate"@en ,
                        "Placa de Ala"@es .


###  https://w3id.org/beo#Flashing
:Flashing rdf:type owl:Class ;
          rdfs:subClassOf :DiscreteAccessory ;
          rdfs:comment "Construction material used to manage the passage of water around objects."@en ,
                       "Material de construcción utilizado para controlar el paso del agua alrededor de los objetos."@es ;
          rdfs:label "Flashing"@en ,
                     "Tapajuntas"@es .


###  https://w3id.org/beo#FlatRoof
:FlatRoof rdf:type owl:Class ;
          rdfs:subClassOf :Roof ;
          rdfs:comment "A roof having no slope, or one with only a slight pitch so as to drain rainwater."@en ,
                       "Cubierta sin pendiente o con una ligera inclinación para evacuar el agua de lluvia."@es ;
          rdfs:label "Flat Roof"@en ,
                     "Techo Plano"@es .


###  https://w3id.org/beo#FlexiblePavement
:FlexiblePavement rdf:type owl:Class ;
                  rdfs:subClassOf :Pavement ;
                  rdfs:comment "Pavement with a bituminous surfacing and with a base layer with or without a hydrocarbon binder."@en ,
                               "Pavimento con un revestimiento bituminoso y con una capa de base con o sin ligante de hidrocarburos."@es ;
                  rdfs:label "Flexible Pavement"@en ,
                             "Pavimento Flexible"@es .


###  https://w3id.org/beo#FloorSlab
:FloorSlab rdf:type owl:Class ;
           rdfs:subClassOf :Slab ;
           rdfs:comment "La losa se utiliza para representar un forjado o el tablero de un puente."@es ,
                        "The slab is used to represent a floor slab or a bridge deck."@en ;
           rdfs:label "Floor Slab"@en ,
                      "Forjado"@es .


###  https://w3id.org/beo#Flooring
:Flooring rdf:type owl:Class ;
          rdfs:subClassOf :Covering ;
          rdfs:comment "El cubrimiento se utiliza para representar un pavimento."@es ,
                       "The covering is used to represent a flooring."@en ;
          rdfs:label "Flooring"@en ,
                     "Pavimento"@es .


###  https://w3id.org/beo#Footing
:Footing rdf:type owl:Class ;
         rdfs:subClassOf :BuiltElement ;
         rdfs:comment "A footing is a part of the foundation of a structure that spreads and transmits the load to the soil. A footing is also characterized as shallow foundation, where the loads are transferred to the ground near the surface."@en ,
                      "Una zapata es parte de los cimientos de una estructura que se extiende y transmite la carga al suelo. Una zapata también se caracteriza por ser una cimentación poco profunda, donde las cargas se transfieren al suelo cerca de la superficie."@es ;
         rdfs:label "Footing"@en ,
                    "Zapata"@es .


###  https://w3id.org/beo#FootingBeam
:FootingBeam rdf:type owl:Class ;
             rdfs:subClassOf :Footing ;
             rdfs:comment "Elementos de zapata que están en flexión y que están apoyados lejos del suelo. Normalmente se extenderán entre pilas, pilotes o encepados. Se distinguen de las vigas de la superestructura del edificio porque normalmente requerirán un grado de acabado inferior."@es ,
                          "Footing elements that are in bending and are supported clear of the ground. They will normally span between piers, piles or pile caps. They are distinguished from beams in the building superstructure since they will normally require a lower grade of finish."@en ;
             rdfs:label "Footing Beam"@en ,
                        "Viga de Cimentación"@es .


###  https://w3id.org/beo#FreeFormRoof
:FreeFormRoof rdf:type owl:Class ;
              rdfs:subClassOf :Roof ;
              rdfs:comment "Free form roof."@en ,
                           "Techo de forma libre."@es ;
              rdfs:label "Free Form Roof"@en ,
                         "Techo de Forma Libre."@es .


###  https://w3id.org/beo#FreeFormStairFlight
:FreeFormStairFlight rdf:type owl:Class ;
                     rdfs:subClassOf :StairFlight ;
                     rdfs:comment "A stair flight with a free form walking line (and outer boundaries)."@en ,
                                  "Un tramo de escalera con una línea de paso de forma libre (y límites exteriores)."@es ;
                     rdfs:label "Free Form Stair Flight"@en ,
                                "Tramo de Escalera de Forma Libre"@es .


###  https://w3id.org/beo#FrictionDamper
:FrictionDamper rdf:type owl:Class ;
                rdfs:subClassOf :VibrationDamper ;
                rdfs:comment "El amortiguador de fricción utiliza la fricción que actúa sobre la superficie de contacto de un material."@es ,
                             "The friction type is a damper utilizing friction acting on the contact surface of a material."@en ;
                rdfs:label "Amortiguador a Friccion"@es ,
                           "Friction Damper"@en .


###  https://w3id.org/beo#FrictionPile
:FrictionPile rdf:type owl:Class ;
              rdfs:subClassOf :Pile ;
              rdfs:comment "A friction pile."@en ,
                           "Una pila de friccion."@es ;
              rdfs:label "Friction Pile"@en ,
                         "Pila de Friccion"@es .


###  https://w3id.org/beo#Frog
:Frog rdf:type owl:Class ;
      rdfs:subClassOf :TrackElement ;
      rdfs:comment "A frog is an arrangement ensuring the intersection of two opposite running edges of turnouts or diamond crossings and having one crossing vee and two wing rails. Note: definition from EN 13232-1-2004."@en ,
                   "Una rana es una disposición que asegura la intersección de dos bordes de rodadura opuestos de desvíos o cruces en rombo y que tiene una uve de cruce y dos carriles de aletas. Nota: definición de la norma EN 13232-1-2004."@es ;
      rdfs:label "FROG"@es ,
                 "Frog"@en .


###  https://w3id.org/beo#GableRoof
:GableRoof rdf:type owl:Class ;
           rdfs:subClassOf :Roof ;
           rdfs:comment "A roof sloping downward in two parts from a central ridge, so as to form a gable at each end."@en ,
                        "Tejado inclinado hacia abajo en dos partes a partir de una cumbrera central, de modo que forma un frontón en cada extremo."@es ;
           rdfs:label "Gable Roof"@en ,
                      "Tejado a Dos Aguas"@es .


###  https://w3id.org/beo#GambrelRoof
:GambrelRoof rdf:type owl:Class ;
             rdfs:subClassOf :Roof ;
             rdfs:comment "A roof sloping downward in two parts from a central ridge, so as to form a gable at each end."@en ,
                          "Tejado inclinado hacia abajo en dos partes a partir de una cumbrera central, de modo que forma un frontón en cada extremo."@es ;
             rdfs:label "Gambrel Roof"@en ,
                        "Techo Gambrel"@es .


###  https://w3id.org/beo#Gate
:Gate rdf:type owl:Class ;
      rdfs:subClassOf :Door ;
      rdfs:comment "A gate is a point of entry into a space usually within an opening in a fence. Or as a 'free standing' gate."@en ,
                   "punto de entrada a un espacio, normalmente dentro de una abertura en una valla. O como puerta de entrada 'independiente'."@es ;
      rdfs:label "Gate"@en ,
                 "Puerta de Entrada"@es .


###  https://w3id.org/beo#Girder
:Girder rdf:type owl:Class ;
        rdfs:subClassOf :ElementAssembly ;
        rdfs:comment "A beam-like superstructure, such as bridge main girder extending between abutments and piers built up of beams, braces (as Members) etc. - may also be an aggregation of girder segments."@en ,
                     "Una superestructura en forma de viga, como la viga principal de un puente que se extiende entre estribos y pilas construidas con vigas, tirantes (como miembros), etc., también puede ser una agregación de segmentos de viga."@es ;
        rdfs:label "Girder"@en ,
                   "Viga Maestra"@es .


###  https://w3id.org/beo#GirderSegment
:GirderSegment rdf:type owl:Class ;
               rdfs:subClassOf :Beam ;
               rdfs:comment "A segment of a girder (e.g. each span of a continuous girder)."@en ,
                            "Un segmento de una viga (por ejemplo, cada tramo de una viga continua)."@es ;
               rdfs:label "Girder Segment"@en ,
                          "Segmento de Viga Principal"@es .


###  https://w3id.org/beo#Glue
:Glue rdf:type owl:Class ;
      rdfs:subClassOf :Fastener ;
      rdfs:comment "A fastening connection where glue is used to join together elements."@en ,
                   "Conexión donde se utiliza cola para unir elementos."@es ;
      rdfs:label "Adhesivo"@es ,
                 "Glue"@en .


###  https://w3id.org/beo#Grid
:Grid rdf:type owl:Class ;
      rdfs:subClassOf :ElementAssembly ;
      rdfs:comment "A framework of spaced cables or bars that are parallel to or cross each other."@en ,
                   "Un marco de cables o barras espaciados que son paralelos o se cruzan entre sí."@es ;
      rdfs:label "Grid"@en ,
                 "Grid"@es .


###  https://w3id.org/beo#GroutedSoil
:GroutedSoil rdf:type owl:Class ;
             rdfs:subClassOf :ReinforcedSoil ;
             rdfs:comment "A method of injecting curable slurry into cracks or pores of a geotechnical foundation to improve its physical and mechanical properties."@en ,
                          "Método de inyección de lechada curable en grietas o poros de una cimentación geotécnica para mejorar sus propiedades físicas y mecánicas."@es ;
             rdfs:label "Grouted Soil"@en ,
                        "Suelo Injectado"@es .


###  https://w3id.org/beo#GroutingDuct
:GroutingDuct rdf:type owl:Class ;
              rdfs:subClassOf :TendonConduit ;
              rdfs:comment "An additional small conduit connected to the main conduit to allow grouting in case of bonded post-tensioning, such as Grout inlet, Grout outlet and Grout vent."@en ,
                           "Un pequeño conducto adicional conectado al conducto principal para permitir la inyección de lechada en caso de postensado adherido, como entrada de lechada, salida de lechada y ventilación de lechada."@es ;
              rdfs:label "Conducto de Lechada"@es ,
                         "Grouting Duct"@en .


###  https://w3id.org/beo#GuardRail
:GuardRail rdf:type owl:Class ;
           rdfs:subClassOf :Rail ;
           rdfs:comment "A guard rail is a rail that limits risk of train derailment, normally not loaded."@en ,
                        "Un guardarraíl es un raíl que limita el riesgo de descarrilamiento de un tren, normalmente sin carga."@es ;
           rdfs:label "Guard Rail"@en ,
                      "Guardarrail"@es .


###  https://w3id.org/beo#Guardrail
:Guardrail rdf:type owl:Class ;
           rdfs:subClassOf :Railing ;
           rdfs:comment "A type of railing designed to guard human or vehicle occupants from falling off a stair, ramp or landing where there is a vertical drop at the edge of such floors/landings, or to provide restraint to an errant road vehicle, installed on the central reserve of or alongside a road."@en ,
                        "Tipo de barandilla diseñada para proteger a los ocupantes de personas o vehículos de la caída de una escalera, rampa o rellano cuando existe un desnivel vertical en el borde de dichos suelos/ rellanos, o para proporcionar retención a un vehículo de carretera errante, instalada en la mediana de una carretera o junto a ella."@es ;
           rdfs:label "Guardrail"@en ,
                      "Quitamiedos"@es .


###  https://w3id.org/beo#GuideBearing
:GuideBearing rdf:type owl:Class ;
              rdfs:subClassOf :Bearing ;
              rdfs:comment "A bearing that ensures that the structure maintains the correct location or expansion/contraction path and takes no vertical load. Includes also restraint bearings."@en ,
                           "Un soporte que garantiza que la estructura mantenga la ubicación correcta o la trayectoria de expansión/contracción y no soporta carga vertical. Incluye también cojinetes de sujeción."@es ;
              rdfs:label "Cojinete de Guia"@es ,
                         "Guide Bearing"@en .


###  https://w3id.org/beo#GussetPlate
:GussetPlate rdf:type owl:Class ;
             rdfs:subClassOf :Plate ;
             rdfs:comment "a plate or bracket for strengthening an angle in framework (as in a building or bridge)."@en ,
                          "una placa o soporte para reforzar un ángulo en un armazón (como en un edificio o puente)."@es ;
             rdfs:label "Gusset Plate"@en ,
                        "Placa Gusset"@es .


###  https://w3id.org/beo#HALFTURNRAMP
:HALFTURNRAMP rdf:type owl:Class ;
              rdfs:subClassOf :Ramp ;
              rdfs:comment "A ramp making a 180° turn, consisting of two straight flights connected by a halfspace landing. The orientation of the turn is determined by the walking line."@en ,
                           "Rampa que realiza un giro de 180°, compuesta por dos tramos rectos conectados por un descansillo a medio espacio. La orientación del giro viene determinada por la línea de marcha."@es ;
              rdfs:label "HALF TURN RAMP"@en ,
                         "Rampa de Media Vuelta"@es .


###  https://w3id.org/beo#HalfSetofBlades
:HalfSetofBlades rdf:type owl:Class ;
                 rdfs:subClassOf :TrackElement ;
                 rdfs:comment "A half set of blades consists of one stock rail and its switch rail complete with small fittings. It is right or left hand as seen by an observer in the centre of the track facing the switch heel from the switch toe. Note: definition from EN 13232-1-2004."@en ,
                              "Un medio juego de agujas consta de una contraaguja y su aguja completa con pequeños herrajes. Se encuentra a la derecha o a la izquierda, según lo vea un observador situado en el centro de la vía, mirando el talón de la aguja desde la punta de la aguja. Nota: definición de la norma EN 13232-1-2004."@es ;
                 rdfs:label "Half Set of Blades"@en ,
                            "Medio Juego de Agujas"@es .


###  https://w3id.org/beo#HalfTurnStair
:HalfTurnStair rdf:type owl:Class ;
               rdfs:subClassOf :Stair ;
               rdfs:comment "A stair making a 180° turn, consisting of two straight flights connected by a halfspace landing. The orientation of the turn is determined by the walking line."@en ,
                            "Escalera que realiza un giro de 180°, formada por dos tramos rectos conectados por un descansillo a medio espacio. La orientación del giro viene determinada por la línea de paso."@es ;
               rdfs:label "Escalera de Medio Giro"@es ,
                          "Half Turn Stair"@en .


###  https://w3id.org/beo#HalfWindingStair
:HalfWindingStair rdf:type owl:Class ;
                  rdfs:subClassOf :Stair ;
                  rdfs:comment "A stair consisting of one flight with one half winder, which makes a 180° turn. The orientation of the turn is determined by the walking line."@en ,
                               "Escalera formada por un tramo con un medio giro, que realiza un giro de 180°. La orientación del giro viene determinada por la línea de paso."@es ;
                  rdfs:label "Escalera de Medio Caracol"@es ,
                             "Half Winding Stair"@en .


###  https://w3id.org/beo#Handrail
:Handrail rdf:type owl:Class ;
          rdfs:subClassOf :Railing ;
          rdfs:comment "A type of railing designed to serve as an optional structural support for loads applied by human occupants (at hand height). Generally located adjacent to ramps and stairs. Generally floor or wall mounted."@en ,
                       "Tipo de barandilla diseñada para servir de soporte estructural opcional de las cargas aplicadas por los ocupantes humanos (a la altura de las manos). Generalmente situada junto a rampas y escaleras. Generalmente montada en el suelo o en la pared."@es ;
          rdfs:label "Handrail "@en ,
                     "Pasamanos"@es .


###  https://w3id.org/beo#HatstoneBeam
:HatstoneBeam rdf:type owl:Class ;
              rdfs:subClassOf :Beam ;
              rdfs:comment "A beam on top of a retaining wall or a wing wall, preventing earth movement."@en ,
                           "Una viga encima de un muro de contención o un muro de ala, evitando el movimiento de tierra."@es ;
              rdfs:label "Hatstone Beam"@en ,
                         "Viga Hatstone"@es .


###  https://w3id.org/beo#HaulingGear
:HaulingGear rdf:type owl:Class ;
             rdfs:subClassOf :TransportElement ;
             rdfs:comment "A device used for hauling goods."@en ,
                          "Dispositivo utilizado para transportar mercancías."@es ;
             rdfs:label "Equipo de Transporte"@es ,
                        "Hauling Gear"@en .


###  https://w3id.org/beo#HipRoof
:HipRoof rdf:type owl:Class ;
         rdfs:subClassOf :Roof ;
         rdfs:comment "A roof having sloping ends and sides meeting at an inclined projecting angle."@en ,
                      "Cubierta con los extremos inclinados y los lados que se unen en un ángulo saliente inclinado."@es ;
         rdfs:label "Hip Roof"@en ,
                    "Tejado a Cuatro Aguas"@es .


###  https://w3id.org/beo#HippedGableRoof
:HippedGableRoof rdf:type owl:Class ;
                 rdfs:subClassOf :Roof ;
                 rdfs:comment "A roof having a hipped end truncating a gable"@en ,
                              "Un tejado con un extremo truncado a cuatro aguas"@es ;
                 rdfs:label "Hipped Gable Roof"@en ,
                            "Techo de Cadera"@es .


###  https://w3id.org/beo#HollowcoreBeam
:HollowcoreBeam rdf:type owl:Class ;
                rdfs:subClassOf :Beam ;
                rdfs:comment "A wide often prestressed beam with a hollow-core profile that usually serves as a slab component."@en ,
                             "Viga ancha, a menudo pretensada, con un perfil de núcleo hueco que suele servir como componente de losa."@es ;
                rdfs:label "Hollowcore Beam"@en ,
                           "Viga Alveolar"@es .


###  https://w3id.org/beo#ImpactProtectionDevice
:ImpactProtectionDevice rdf:type owl:Class ;
                        rdfs:subClassOf :ElementComponent ;
                        rdfs:comment "An impact protection device is a component used to protect other built elements from kinetic damage."@en ,
                                     "Un dispositivo de protección contra impactos es un componente que se utiliza para proteger otros elementos construidos de daños cinéticos."@es ;
                        rdfs:label "Dispositivo de Proteccion contra Impactos"@es ,
                                   "Impact Protection Device"@en .


###  https://w3id.org/beo#Insulation
:Insulation rdf:type owl:Class ;
            rdfs:subClassOf :Covering ;
            rdfs:comment "El cubrimiento sirve para aislar un elemento con fines térmicos o acústicos."@es ,
                         "The covering is used to insulate an element for thermal or acoustic purposes."@en ;
            rdfs:label "Aislamiento"@es ,
                       "Insulation"@en .


###  https://w3id.org/beo#InsulationElement
:InsulationElement rdf:type owl:Class ;
                   rdfs:subClassOf :BuildingElementPart ;
                   rdfs:comment "La pieza proporciona aislamiento térmico, por ejemplo como capa aislante entre paneles de pared en paredes sándwich o como relleno en paredes de entramado."@es ,
                                "The part provides thermal insulation, for example as insulation layer between wall panels in sandwich walls or as infill in stud walls."@en ;
                   rdfs:label "Elemento de Aislamiento"@es ,
                              "Insulation Element"@en .


###  https://w3id.org/beo#Insulator
:Insulator rdf:type owl:Class ;
           rdfs:subClassOf :DiscreteAccessory ;
           rdfs:comment "A device designed to support and insulate a conductive element. Note: definition from IEC 151-15-39."@en ,
                        "Dispositivo destinado a soportar y aislar un elemento conductor. Nota: definición de la norma CEI 151-15-39."@es ;
           rdfs:label "Aislante"@es ,
                      "Insulator"@en .


###  https://w3id.org/beo#Jalouise
:Jalouise rdf:type owl:Class ;
          rdfs:subClassOf :ShadingDevice ;
          rdfs:comment "A blind with adjustable horizontal slats for admitting light and air while excluding direct sun and rain."@en ,
                       "Una Jalouise es una persiana con lamas horizontales ajustables que permiten la entrada de luz y aire, al tiempo que excluyen el sol directo y la lluvia."@es ;
          rdfs:label "Jalouise"@en ,
                     "Jalouise"@es .


###  https://w3id.org/beo#JetGroutingPile
:JetGroutingPile rdf:type owl:Class ;
                 rdfs:subClassOf :Pile ;
                 rdfs:comment "An injected pile-like construction."@en ,
                              "Una construcción inyectada en forma de pilote."@es ;
                 rdfs:label "Jet Grouting Pile"@en ,
                            "Pilote de Jet Grouting"@es .


###  https://w3id.org/beo#JoistBeam
:JoistBeam rdf:type owl:Class ;
           rdfs:subClassOf :Beam ;
           rdfs:comment "A beam used to support a floor or ceiling."@en ,
                        "Viga utilizada para soportar un piso o un techo."@es ;
           rdfs:label "Joist Beam"@en ,
                      "Vigueta"@es .


###  https://w3id.org/beo#Kerb
:Kerb rdf:type owl:Class ;
      rdfs:subClassOf :BuiltElement ;
      rdfs:comment "A border of stone, concrete or other rigid material formed at the edge of the carriageway or footway."@en ,
                   "Borde de piedra, hormigón u otro material rígido formado en el borde de la calzada o acera."@es ;
      rdfs:label "Bordillo"@es ,
                 "Kerb"@en .


###  https://w3id.org/beo#Ladder
:Ladder rdf:type owl:Class ;
        rdfs:subClassOf :Stair ;
        rdfs:comment "A piece of equipment consisting of a series of bars or steps between two upright elements used for climbing up or down something"@en ,
                     "Equipo formado por una serie de barras o peldaños entre dos elementos verticales que sirve para subir o bajar algo"@es ;
        rdfs:label "Escalerilla"@es ,
                   "Ladder"@en .


###  https://w3id.org/beo#LandingSlab
:LandingSlab rdf:type owl:Class ;
             rdfs:subClassOf :Slab ;
             rdfs:comment "La losa se utiliza para representar un rellano dentro de una escalera o rampa."@es ,
                          "The slab is used to represent a landing within a stair or ramp."@en ;
             rdfs:label "Landing Slab"@en ,
                        "Rellano"@es .


###  https://w3id.org/beo#LiftingGear
:LiftingGear rdf:type owl:Class ;
             rdfs:subClassOf :TransportElement ;
             rdfs:comment "A device used for lifting or lowering heavy goods. It may be manually operated or electrically or pneumatically driven."@en ,
                          "Dispositivo utilizado para levantar o bajar mercancías pesadas. Puede ser operado manualmente o eléctrica o neumáticamente."@es ;
             rdfs:label "Lifting Gear"@en ,
                        "Mecanismo de Elevacion"@es .


###  https://w3id.org/beo#Ligature
:Ligature rdf:type owl:Class ;
          rdfs:subClassOf :ReinforcingBar ;
          rdfs:comment "La barra de refuerzo es una ligadura (eslabón, cerco)."@es ,
                       "The reinforcing bar is a ligature (link, stirrup)."@en ;
          rdfs:label "Ligadura"@es ,
                     "Ligature"@en .


###  https://w3id.org/beo#Ligthdome
:Ligthdome rdf:type owl:Class ;
           rdfs:subClassOf :Window ;
           rdfs:comment "A special window that lies horizonally in a roof slab opening."@en ,
                        "Una ventana especial que se encuentra horizontalmente en la abertura de una losa del techo."@es ;
           rdfs:label "Lightdome"@es ,
                      "Ligthdome"@en .


###  https://w3id.org/beo#LineTensioner
:LineTensioner rdf:type owl:Class ;
               rdfs:subClassOf :MooringDevice ;
               rdfs:comment "A mechanical device used to apply a tensioning load to mooring lines to improve vessel stability for port operations."@en ,
                            "Dispositivo mecánico utilizado para aplicar una carga tensora a los cabos de amarre con el fin de mejorar la estabilidad del buque en las operaciones portuarias."@es ;
               rdfs:label "Line Tensioner"@en ,
                          "Tensor de Cabos"@es .


###  https://w3id.org/beo#Lintel
:Lintel rdf:type owl:Class ;
        rdfs:subClassOf :Beam ;
        rdfs:comment "A beam or horizontal piece of material over an opening (e.g. door, window)."@en ,
                     "Viga o pieza horizontal de material sobre una abertura (por ejemplo, puerta, ventana)."@es ;
        rdfs:label "Dintel"@es ,
                   "Lintel"@en .


###  https://w3id.org/beo#Lock
:Lock rdf:type owl:Class ;
      rdfs:subClassOf :DiscreteAccessory ;
      rdfs:comment "A lock is a mechanical or electronic fastening device that is released either by a physical object (e.g., key, fingerprint, RFID card, security token etc.), by supplying secret information (e.g., number permutation, password), or by a combination thereof."@en ,
                   "Una cerradura es un dispositivo de cierre mecánico o electrónico que se desbloquea mediante un objeto físico (por ejemplo, una llave, una huella dactilar, una tarjeta RFID, una ficha de seguridad, etc.), mediante el suministro de información secreta (por ejemplo, una permutación numérica, una contraseña) o mediante una combinación de ambos."@es ;
      rdfs:label "Cerradura"@es ,
                 "Lock"@en .


###  https://w3id.org/beo#MageneticMooringDevice
:MageneticMooringDevice rdf:type owl:Class ;
                        rdfs:subClassOf :MooringDevice ;
                        rdfs:comment "Dispositivo de amarre que utiliza imanes como método principal de sujeción de la embarcación."@es ,
                                     "Mooring device that uses magnets as the primary method of securing the vessel."@en ;
                        rdfs:label "Dispositivo de Amarre Magnetico"@es ,
                                   "Magenetic Mooring Device"@en .


###  https://w3id.org/beo#MainBar
:MainBar rdf:type owl:Class ;
         rdfs:subClassOf :ReinforcingBar ;
         rdfs:comment "La barra de refuerzo es una barra principal."@es ,
                      "The reinforcing bar is a main bar."@en ;
         rdfs:label "Barra de Refuerzo Principal"@es ,
                    "Main Bar"@en .


###  https://w3id.org/beo#MansardRoof
:MansardRoof rdf:type owl:Class ;
             rdfs:subClassOf :Roof ;
             rdfs:comment "A roof having on each side a steeper lower part and a shallower upper part."@en ,
                          "Un tejado que tiene a cada lado una parte inferior más inclinada y una parte superior menos profunda."@es ;
             rdfs:label "Mansard Roof"@en ,
                        "Tejado Mansa"@es .


###  https://w3id.org/beo#Marker
:Marker rdf:type owl:Class ;
        rdfs:subClassOf :Sign ;
        rdfs:comment "A Sign type formed of a vertical post (possibly with some lettering or symbols) usually used to delimitate distance or the location of some equipment."@en ,
                     "Tipo de señal formada por un poste vertical (posiblemente con algunas letras o símbolos) que suele utilizarse para delimitar la distancia o la ubicación de algún equipo."@es ;
        rdfs:label "Marcador"@es ,
                   "Marker"@en .


###  https://w3id.org/beo#Mast
:Mast rdf:type owl:Class ;
      rdfs:subClassOf :ElementAssembly ;
      rdfs:comment "An assembly of plates, members, cables or fasteners that form a vertical structure for the support or mounting of other equipment such as lights, sonar or wireless transmitters."@en ,
                   "Un conjunto de placas, miembros, cables o sujetadores que forman una estructura vertical para el soporte o montaje de otros equipos como luces, sonares o transmisores inalámbricos."@es ;
      rdfs:label "Mast"@en ,
                 "Mastil"@es .


###  https://w3id.org/beo#MechanicalFastener
:MechanicalFastener rdf:type owl:Class ;
                    rdfs:subClassOf :ElementComponent ;
                    rdfs:comment "A mechanical fasteners connecting building elements or parts mechanically. A single instance of this class may represent one or many of actual mechanical fasteners, for example an array of bolts or a row of nails."@en ,
                                 "Elemento de fijación mecánico que conecta mecánicamente elementos o partes de un edificio. Una única instancia de esta clase puede representar una o varias fijaciones mecánicas reales, por ejemplo, una serie de pernos o una fila de clavos."@es ;
                    rdfs:label "Fijacion Mecánica"@es ,
                               "Mechanical Fastener"@en .


###  https://w3id.org/beo#Member
:Member rdf:type owl:Class ;
        rdfs:subClassOf :BuiltElement ;
        rdfs:comment "An Member is a structural member designed to carry loads between or beyond points of support. It is not required to be load bearing. The orientation of the member (being horizontal, vertical or sloped) is not relevant to its definition. I shall be used if it the entity cannot be expressed as a Beam or a Column"@en ,
                     "Un Miembro es un elemento estructural diseñado para soportar cargas entre o más allá de los puntos de apoyo. No es necesario que soporte cargas. La orientación del elemento (horizontal, vertical o inclinado) no es relevante para su definición. Se utilizará I si no puede expresarse como viga o columna."@es ;
        rdfs:label "Member"@en ,
                   "Miembro"@es .


###  https://w3id.org/beo#Membrane
:Membrane rdf:type owl:Class ;
          rdfs:subClassOf :Covering ;
          rdfs:comment "An impervious layer that could be used for e.g. roof covering (below tiling - that may be known as sarking etc.) or as a damp proof course membrane; also, waterproofing material on a bridge structure (typically on top of bridge slab)."@en ,
                       "Capa impermeable que puede utilizarse, por ejemplo, para el cubrimiento de tejados (por debajo de las tejas, que pueden denominarse sarking, etc.) o como membrana impermeabilizante; también, material impermeabilizante en la estructura de un puente (normalmente sobre la losa del puente)."@es ;
          rdfs:label "Membrana"@es ,
                     "Membrane"@en .


###  https://w3id.org/beo#Mirror
:Mirror rdf:type owl:Class ;
        rdfs:subClassOf :Sign ;
        rdfs:comment "A sign type that provides information via a reflective mirror surface."@en ,
                     "Tipo de señal que proporciona información a través de una superficie de espejo reflectante."@es ;
        rdfs:label "Espejo"@es ,
                   "Mirror"@en .


###  https://w3id.org/beo#Molding
:Molding rdf:type owl:Class ;
         rdfs:subClassOf :Covering ;
         rdfs:comment "El cubrimiento se utiliza para representar una moldura que es una tira de material para cubrir la transición de superficies (a menudo entre el revestimiento de la pared y el techo)."@es ,
                      "The covering is used to represent a molding being a strip of material to cover the transition of surfaces (often between wall cladding and ceiling)."@en ;
         rdfs:label "Molding"@en ,
                    "Moldura"@es .


###  https://w3id.org/beo#MooringDevice
:MooringDevice rdf:type owl:Class ;
               rdfs:subClassOf :BuiltElement ;
               rdfs:comment "A mooring device is an active or passive built element who's primary function is to participate in the mooring of a vessel, this could be in the form of a bollard used as an attachment point for lines or active equipment such as quick release hooks."@en ,
                            "Un dispositivo de amarre es un elemento construido activo o pasivo cuya función principal es participar en el amarre de una embarcación, puede ser en forma de bolardo utilizado como punto de enganche para cabos o de equipo activo como ganchos de liberación rápida."@es ;
               rdfs:label "Dispositivo de Amarre"@es ,
                          "Mooring Device"@en .


###  https://w3id.org/beo#MooringHooks
:MooringHooks rdf:type owl:Class ;
              rdfs:subClassOf :MooringDevice ;
              rdfs:comment "Ganchos de amarre de liberación rápida - un dispositivo activo utilizado para asegurar un buque y proporcionar la liberación automática de los buques."@es ,
                           "Quick release mooring hooks - an active device used to secure a vessel and provide automated release of vessels."@en ;
              rdfs:label "Ganchos de Amarre"@es ,
                         "Mooring Hooks"@en .


###  https://w3id.org/beo#Mortar
:Mortar rdf:type owl:Class ;
        rdfs:subClassOf :Fastener ;
        rdfs:comment "A composition of mineralic or other materials used to fill jointing gaps and possibly fulfilling a load carrying role."@en ,
                     "Una composición de materiales minerales u otros utilizados para llenar espacios en las juntas y posiblemente cumplir una función de transporte de carga."@es ;
        rdfs:label "Mortar"@en ,
                   "Mortero"@es .


###  https://w3id.org/beo#MovableWall
:MovableWall rdf:type owl:Class ;
             rdfs:subClassOf :Wall ;
             rdfs:comment "A movable wall that is either movable, such as folding wall or a sliding wall, or can be easily removed as a removable partitioning or mounting wall. Movable walls do normally not define space boundaries and often belong to the furnishing system."@en ,
                          "Una pared móvil que es móvil, como una pared plegable o una pared deslizante, o que se puede quitar fácilmente como una pared divisoria o de montaje removible. Las paredes móviles normalmente no definen límites espaciales y a menudo pertenecen al sistema de decoración."@es ;
             rdfs:label "Movable Wall"@en ,
                        "Pared Móvil"@es .


###  https://w3id.org/beo#MovingWalkway
:MovingWalkway rdf:type owl:Class ;
               rdfs:subClassOf :TransportElement ;
               rdfs:comment "Moving walkway being a transport device to move people horizontally or on an incline. It is a slow conveyor belt that transports people."@en ,
                            "Pasarela móvil que es un dispositivo de transporte para el desplazamiento de personas en sentido horizontal o en pendiente. Es una cinta transportadora lenta que transporta personas."@es ;
               rdfs:label "Moving Walkway"@en ,
                          "Pasarela Movil"@es .


###  https://w3id.org/beo#Mullion
:Mullion rdf:type owl:Class ;
         rdfs:subClassOf :Member ;
         rdfs:comment "A linear element within a curtain wall system to connect two (or more) panels."@en ,
                      "Elemento lineal dentro de un sistema de muro cortina para conectar dos (o más) paneles."@es ;
         rdfs:label "Montante"@es ,
                    "Mullion"@en .


###  https://w3id.org/beo#Nail
:Nail rdf:type owl:Class ;
      rdfs:subClassOf :MechanicalFastener ;
      rdfs:comment "A nail is a thin pointed piece of metal that is hammered into materials as a fastener."@en ,
                   "Un clavo es una pieza metálica fina y puntiaguda que se clava en los materiales para sujetarlos."@es ;
      rdfs:label "Clavo"@es ,
                 "Nail"@en .


###  https://w3id.org/beo#NailPlate
:NailPlate rdf:type owl:Class ;
           rdfs:subClassOf :MechanicalFastener ;
           rdfs:comment "Piece of sheet metal with punched points that overlaps the connected pieces and is pressed into their material."@en ,
                        "Pieza de chapa con punzones que se superpone a las piezas unidas y se introduce a presión en su material."@es ;
           rdfs:label "Nail Plate"@en ,
                      "Placa de Clavos"@es .


###  https://w3id.org/beo#NavigationElement
:NavigationElement rdf:type owl:Class ;
                   rdfs:subClassOf :BuiltElement ;
                   rdfs:comment "A navigation element is an active or passive built element who's primary function is to provide navigational instructions and warnings to vessels, this could be in the form of a floating buoy, a fixed beacon. Navigation elements can aggregate other components and elements to form the entire structure."@en ,
                                "Un elemento de navegación es un elemento construido activo o pasivo cuya función principal es proporcionar instrucciones y avisos de navegación a los buques, puede ser en forma de boya flotante o de baliza fija. Los elementos de navegación pueden agregar otros componentes y elementos para formar la estructura completa."@es ;
                   rdfs:label "Elemento de Navegacion"@es ,
                              "Navigation Element"@en .


###  https://w3id.org/beo#PANELSTRENGTHENING
:PANELSTRENGTHENING rdf:type owl:Class ;
                    rdfs:subClassOf :DiscreteAccessory ;
                    rdfs:comment "A component that minimizes pump effects of the substructure."@en ,
                                 "Un componente que minimiza los efectos de bombeo de la subestructura."@es ;
                    rdfs:label "PANEL STRENGTHENING"@en ,
                               "Refuerzo de Panel"@es .


###  https://w3id.org/beo#PadFooting
:PadFooting rdf:type owl:Class ;
            rdfs:subClassOf :Footing ;
            rdfs:comment ""@es ,
                         "An element that transfers the load of a single column (possibly two) to the ground."@en ;
            rdfs:label "Losa de Cimentacion"@es ,
                       "Pad Footing"@en .


###  https://w3id.org/beo#Parapet
:Parapet rdf:type owl:Class ;
         rdfs:subClassOf :Wall ;
         rdfs:comment "A wall-like barrier to protect human or vehicle from falling, or to prevent the spread of fires. Often designed at the edge of balconies, terraces or roofs, or along edges of bridges."@en ,
                      "Barrera similar a una pared para proteger a personas o vehículos de caídas o para evitar la propagación de incendios. A menudo se diseña en el borde de balcones, terrazas o tejados, o a lo largo de los bordes de puentes."@es ;
         rdfs:label "Parapet"@en ,
                    "Parapeto"@es .


###  https://w3id.org/beo#PartitioningWall
:PartitioningWall rdf:type owl:Class ;
                  rdfs:subClassOf :Wall ;
                  rdfs:comment "A wall designed to partition spaces that often has a light-weight, sandwich-like construction (e.g. using gypsum board). Partitioning walls are normally non load bearing."@en ,
                               "Una pared diseñada para dividir espacios que a menudo tiene una construcción liviana tipo sándwich (por ejemplo, usando paneles de yeso). Las paredes divisorias normalmente no soportan cargas."@es ;
                  rdfs:label "Partitioning Wall"@en ,
                             "Tabique"@es .


###  https://w3id.org/beo#Pavement
:Pavement rdf:type owl:Class ;
          rdfs:subClassOf :BuiltElement ;
          rdfs:comment "Tipo de elemento construido en una carretera u otra zona pavimentada para proporcionar una superficie uniforme que soporte las cargas de vehículos o peatones, normalmente compuesto por varias capas. NOTA Definición de ISO 6707-1: carretera, pista de aterrizaje o construcción similar por encima de la subrasante."@es ,
                       "Type of built element in a road or other paved area to provide an even surface sustaining loads from vehicles or pedestrians, usually comprising several courses. NOTE Definition from ISO 6707-1: road, runway, or similar construction above the subgrade."@en ;
          rdfs:label "Pavement"@en ,
                     "Pavimento"@es .


###  https://w3id.org/beo#PavementCourse
:PavementCourse rdf:type owl:Class ;
                rdfs:subClassOf :Course ;
                rdfs:comment "A layer within a pavement structure that forms a paved area or road."@en ,
                             "Capa dentro de una estructura de pavimento que forma una zona pavimentada o una carretera."@es ;
                rdfs:label "Capa de Pavimento"@es ,
                           "Pavement Course"@en .


###  https://w3id.org/beo#PavilionRoof
:PavilionRoof rdf:type owl:Class ;
              rdfs:subClassOf :Roof ;
              rdfs:comment "A pyramidal hip roof."@en ,
                           "Un tejado piramidal a cuatro aguas."@es ;
              rdfs:label "Pavilion Roof"@en ,
                         "pabellon"@es .


###  https://w3id.org/beo#PavingSlab
:PavingSlab rdf:type owl:Class ;
            rdfs:subClassOf :Slab ;
            rdfs:comment "Capa rígida del pavimento de una carretera u otra zona pavimentada, normalmente de hormigón."@es ,
                         "Rigid pavement course of a road or other paved area, usually concrete."@en ;
            rdfs:label "Losa de Pavimentacion"@es ,
                       "Paving Slab"@en .


###  https://w3id.org/beo#Pictoral
:Pictoral rdf:type owl:Class ;
          rdfs:subClassOf :Sign ;
          rdfs:comment "A sign type formed of a flat plate with some written or symbolic images on it."@en ,
                       "Tipo de signo formado por una placa plana con algunas imágenes escritas o simbólicas sobre ella."@es ;
          rdfs:label "Cartel"@es ,
                     "Pictoral"@en .


###  https://w3id.org/beo#PierAssembly
:PierAssembly rdf:type owl:Class ;
              rdfs:subClassOf :ElementAssembly ;
              rdfs:comment "An intermediate support e.g. in a bridge, built up of walls, columns, beams etc."@en ,
                           "Un soporte intermedio, p.e. en un puente, formado por muros, columnas, vigas, etc."@es ;
              rdfs:label "Pier Assembly"@en ,
                         "Pilar"@es .


###  https://w3id.org/beo#PierCap
:PierCap rdf:type owl:Class ;
         rdfs:subClassOf :Beam ;
         rdfs:comment "A transversal beam on top of a pier (on a single column or extending from one column of a pier to another column of the same pier)."@en ,
                      "Una viga transversal encima de un muelle (sobre una sola columna o que se extiende de una columna de un muelle a otra columna del mismo muelle)."@es ;
         rdfs:label "Cabeza de Pilar"@es ,
                    "Pier Cap"@en .


###  https://w3id.org/beo#PierStem
:PierStem rdf:type owl:Class ;
          rdfs:subClassOf :Column ;
          rdfs:comment "An individual vertical part of a pier, may be a simple column, i.e. no breakdown into segments or separate structural parts such as flanges and web(s), or may be an aggregation of segments and/or parts."@en ,
                       "Una parte vertical individual de un pilar puede ser una columna simple, es decir, sin desglose en segmentos o partes estructurales separadas, como alas y alma(s), o puede ser una agregación de segmentos y/o partes."@es ;
          rdfs:label "Pier Stem"@en ,
                     "Vástago de Pilar"@es .


###  https://w3id.org/beo#PierStemSegment
:PierStemSegment rdf:type owl:Class ;
                 rdfs:subClassOf :Column ;
                 rdfs:comment "A vertical segment of a pier column."@en ,
                              "Un segmento vertical de una columna de pilar."@es ;
                 rdfs:label "Pier Stem Segment"@en ,
                            "Segmento de Vastago de Pilar"@es .


###  https://w3id.org/beo#Pilaster
:Pilaster rdf:type owl:Class ;
          rdfs:subClassOf :Column ;
          rdfs:comment "A column element embedded within a wall that can be required to be load bearing but may also only be used for decorative purposes."@en ,
                       "Un elemento de columna empotrado dentro de una pared que puede requerir que soporte carga pero que también puede usarse solo con fines decorativos."@es ;
          rdfs:label "Pilaster"@en ,
                     "Pilastra"@es .


###  https://w3id.org/beo#Pile
:Pile rdf:type owl:Class ;
      rdfs:subClassOf :DeepFoundation ;
      rdfs:comment "A pile is a slender timber, concrete, or steel structural element, driven, jetted, or otherwise embedded on end in the ground for the purpose of supporting a load. A pile is also characterized as deep foundation, where the loads are transferred to deeper subsurface layers."@en ,
                   "Un pilote es un elemento estructural esbelto de madera, hormigón o acero, hincado, inyectado o incrustado de otro modo en el suelo con el fin de soportar una carga. Un pilote también se caracteriza por ser una cimentación profunda, en la que las cargas se transfieren a capas más profundas del subsuelo."@es ;
      rdfs:label "Pila"@es ,
                 "Pile"@en .


###  https://w3id.org/beo#PileCap
:PileCap rdf:type owl:Class ;
         rdfs:subClassOf :Footing ;
         rdfs:comment "An element that transfers the load from a column or group of columns to a pier or pile or group of piers or piles."@en ,
                      "Elemento que transfiere la carga de una columna o grupo de columnas a un muelle o pilote o grupo de pilares o pilotes."@es ;
         rdfs:label "Encepado"@es ,
                    "Pile Cap"@en .


###  https://w3id.org/beo#Plate
:Plate rdf:type owl:Class ;
       rdfs:subClassOf :BuiltElement ;
       rdfs:comment "An Plate is a planar and often flat part with constant thickness. A plate may carry loads between or beyond points of support, or provide stiffening. The location of the plate (being horizontal, vertical or sloped) is not relevant to its definition."@en ,
                    "Una placa es una pieza plana de espesor constante. Una placa puede soportar cargas entre o más allá de los puntos de apoyo, o proporcionar rigidez. La ubicación de la placa (horizontal, vertical o inclinada) no es relevante para su definición."@es ;
       rdfs:label "Placa"@es ,
                  "Plate"@en .


###  https://w3id.org/beo#PlateMember
:PlateMember rdf:type owl:Class ;
             rdfs:subClassOf :Member ;
             rdfs:comment "A linear continuous horizontal element in wall framing, such as a head piece or a sole plate."@en ,
                          "Elemento horizontal lineal y continuo en el entramado del muro, como una pieza de cabeza o una placa de suela."@es ;
             rdfs:label "Placa"@es ,
                        "Plate Member"@en .


###  https://w3id.org/beo#PlumbingWall
:PlumbingWall rdf:type owl:Class ;
              rdfs:subClassOf :Wall ;
              rdfs:comment "A pier, or enclosure, or encasement, normally used to enclose plumbing in sanitary rooms. Such walls often do not extend to the ceiling."@en ,
                           "Una pila, recinto o revestimiento que normalmente se utiliza para encerrar tuberías en salas sanitarias. Estas paredes a menudo no llegan hasta el techo."@es ;
              rdfs:label "Pared de plomería"@es ,
                         "Plumbing Wall"@en .


###  https://w3id.org/beo#PointMachineLockingDevice
:PointMachineLockingDevice rdf:type owl:Class ;
                           rdfs:subClassOf :DiscreteAccessory ;
                           rdfs:comment "Dispositivo de bloqueo de máquinas de puntos"@es ,
                                        "Point machine locking device."@en ;
                           rdfs:label "Dispositivo de Bloqueo de Maquinas de Puntos"@es ,
                                      "Point Machine Locking Device"@en .


###  https://w3id.org/beo#PointMachineMountingDevice.
<https://w3id.org/beo#PointMachineMountingDevice.> rdf:type owl:Class ;
                                                   rdfs:subClassOf :DiscreteAccessory ;
                                                   rdfs:comment "Dispositivo de montaje de la máquina de puntos"@es ,
                                                                "Point machine mounting device."@en ;
                                                   rdfs:label "Dispositivo de Montaje de la Maquina de Puntos"@es ,
                                                              "Point Machine Mounting Device."@en .


###  https://w3id.org/beo#Post
:Post rdf:type owl:Class ;
      rdfs:subClassOf :Member ;
      rdfs:comment "A linear (usually vertical) member used to support something or to mark a point."@en ,
                   "Elemento lineal (generalmente vertical) utilizado para sostener algo o marcar un punto."@es ;
      rdfs:label "Post"@en ,
                 "Post"@es .


###  https://w3id.org/beo#Pot
:Pot rdf:type owl:Class ;
     rdfs:subClassOf :Bearing ;
     rdfs:comment "A bearing which carries vertical load by compression of an (elastomeric) disc confined in a (steel) cylinder and which accommodates rotations by deformations of the disc."@en ,
                  "Un cojinete que soporta carga vertical por compresión de un disco (elastomérico) confinado en un cilindro (de acero) y que soporta rotaciones por deformaciones del disco."@es ;
     rdfs:label "Pot"@en ,
                "Pot"@es .


###  https://w3id.org/beo#PrecastPanel
:PrecastPanel rdf:type owl:Class ;
              rdfs:subClassOf :BuildingElementPart ;
              rdfs:comment "La pieza es un panel prefabricado, generalmente como capa interna o externa en un panel de pared tipo sándwich."@es ,
                           "The part is a precast panel, usually as an internal or external layer in a sandwich wall panel."@en ;
              rdfs:label "Panel Prefabricado"@es ,
                         "Precast Panel"@en .


###  https://w3id.org/beo#ProtectionCourse
:ProtectionCourse rdf:type owl:Class ;
                  rdfs:subClassOf :Course ;
                  rdfs:comment "Capa cuya función principal es proporcionar protección contra la erosión y la socavación."@es ,
                               "Layer with the primary task to provide protection against erosion and scour."@en ;
                  rdfs:label "Capa de Proteccion"@es ,
                             "Protection Course"@en .


###  https://w3id.org/beo#PunchingBar
:PunchingBar rdf:type owl:Class ;
             rdfs:subClassOf :ReinforcingBar ;
             rdfs:comment "Punching reinforcement."@en ,
                          "Refuerzo de punzonado."@es ;
             rdfs:label "Barra de Punzonamiento"@es ,
                        "Punching Bar"@en .


###  https://w3id.org/beo#Purlin
:Purlin rdf:type owl:Class ;
        rdfs:subClassOf :Member ;
        rdfs:comment "A linear element (usually used horizontally) within a roof structure to support rafters."@en ,
                     "Elemento lineal (generalmente utilizado horizontalmente) dentro de una estructura de cubierta para soportar los cabrios."@es ;
        rdfs:label "Correa"@es ,
                   "Purlin"@en .


###  https://w3id.org/beo#PylonAssembly
:PylonAssembly rdf:type owl:Class ;
               rdfs:subClassOf :ElementAssembly ;
               rdfs:comment ""@en ,
                            ""@es ;
               rdfs:label "Pilon"@es ,
                          "Pylon Assembly"@en .


###  https://w3id.org/beo#QuarterTurnRamp
:QuarterTurnRamp rdf:type owl:Class ;
                 rdfs:subClassOf :Ramp ;
                 rdfs:comment "A ramp making a 90° turn, consisting of two straight flights connected by a quarterspace landing. The direction of the turn is determined by the walking line."@en ,
                              "Rampa que realiza un giro de 90°, compuesta por dos tramos rectos conectados por un aterrizaje a un cuarto de espacio. La dirección del giro viene determinada por la línea de marcha."@es ;
                 rdfs:label "Quarter Turn Ramp"@en ,
                            "Rampa de Cuarto de Vuelta"@es .


###  https://w3id.org/beo#QuarterTurnStair
:QuarterTurnStair rdf:type owl:Class ;
                  rdfs:subClassOf :Stair ;
                  rdfs:comment "A stair making a 90° turn, consisting of two straight flights connected by a quarterspace landing. The direction of the turn is determined by the walking line."@en ,
                               "Escalera que realiza un giro de 90°, compuesta por dos tramos rectos conectados por un descansillo a un cuarto de espacio. La dirección del giro viene determinada por la línea de paso."@es ;
                  rdfs:label "Escalera de cuarto de giro"@es ,
                             "Quarter Turn Stair"@en .


###  https://w3id.org/beo#QuarterWindingStair
:QuarterWindingStair rdf:type owl:Class ;
                     rdfs:subClassOf :Stair ;
                     rdfs:comment "A stair consisting of one flight with a quarter winder, which is making a 90° turn. The direction of the turn is determined by the walking line."@en ,
                                  "Escalera formada por un tramo con un cuarto de giro, que realiza un giro de 90°. La dirección del giro viene determinada por la línea de marcha."@es ;
                     rdfs:label "Escalera de Cuarto de Caracol"@es ,
                                "Quarter Winding Stair"@en .


###  https://w3id.org/beo#RackRail
:RackRail rdf:type owl:Class ;
          rdfs:subClassOf :Rail ;
          rdfs:comment "A rack rail is a building module for enhancing traction and break performance."@en ,
                       "Un raíl de cremallera es un módulo de construcción para mejorar las prestaciones de tracción y rotura."@es ;
          rdfs:label "Rack Rail"@en ,
                     "Rail de Cremallera"@es .


###  https://w3id.org/beo#Rafter
:Rafter rdf:type owl:Class ;
        rdfs:subClassOf :Member ;
        rdfs:comment "A linear elements used to support roof slabs or roof covering, usually used with slope."@en ,
                     "Elemento lineal utilizado para soportar los forjados o la cubierta del tejado, normalmente se utiliza con pendiente."@es ;
        rdfs:label "Cabrio"@es ,
                   "Rafter"@en .


###  https://w3id.org/beo#Rail
:Rail rdf:type owl:Class ;
      rdfs:subClassOf :BuiltElement ;
      rdfs:comment "A rail is a special section bar (usually of steel) ensuring the guidance of the wheel of a rolling stock or other heavy machineries. In railway, two rails are combined to form a track. A rail is a predominately linear built element that has a special section profile. Rail is distinctive from built elements with similar geometric shapes (e.g. beam, member) that its major function is to ensure guidance of moving for vehicles or other kinds of machineries."@en ,
                   "Un raíl es un elemento construido predominantemente lineal que tiene un perfil de sección especial. El raíl se distingue de otros elementos de construcción con formas geométricas similares (por ejemplo, una viga o un travesaño) en que su función principal es garantizar el guiado de vehículos u otros tipos de maquinaria."@es ;
      rdfs:label "Rail"@en ,
                 "Rail"@es .


###  https://w3id.org/beo#RailBrace
:RailBrace rdf:type owl:Class ;
           rdfs:subClassOf :DiscreteAccessory ;
           rdfs:comment "A rail component that prevents rails from tipping and twisting."@en ,
                        "Componente del raíl que impide que los raíles vuelquen y se tuerzan."@es ;
           rdfs:label "Rail Brace"@en ,
                      "Riel de refuerzo"@es .


###  https://w3id.org/beo#RailFastening
:RailFastening rdf:type owl:Class ;
               rdfs:subClassOf :MechanicalFastener ;
               rdfs:comment "An assembly of components which secures a rail to the supporting structure and retains it in the required position whilst permitting any necessary vertical, lateral and longitudinal movement. Note: definition from EN 13481-1."@en ,
                            "Conjunto de componentes que fijan un carril a la estructura de soporte y lo mantienen en la posición requerida, permitiendo al mismo tiempo cualquier movimiento vertical, lateral y longitudinal necesario. Nota: definición de la norma EN 13481-1."@es ;
               rdfs:label "Fijacion de Carril"@es ,
                          "Rail Fastening"@en .


###  https://w3id.org/beo#RailJoint
:RailJoint rdf:type owl:Class ;
           rdfs:subClassOf :MechanicalFastener ;
           rdfs:comment "A mechanical assembly with e.g. fishplates to join two rail ends with optional functions (insulation or expansion capacity)."@en ,
                        "Un conjunto mecánico con, por ejemplo, pletinas para unir dos extremos de carril con funciones opcionales (aislamiento o capacidad de expansión)."@es ;
           rdfs:label "Junta de Carril"@es ,
                      "Rail Joint"@en .


###  https://w3id.org/beo#RailLubrication
:RailLubrication rdf:type owl:Class ;
                 rdfs:subClassOf :DiscreteAccessory ;
                 rdfs:comment "A device that prevents wearing of the rails throughout the flange of wheel to reduce noise emissions. It is often located at inner side of the outer rail in a curve or near turnouts (depends on function wearing or noise reduction)."@en ,
                              "Dispositivo que evita el desgaste de los carriles en toda la pestaña de la rueda para reducir las emisiones de ruido. Suele situarse en el lado interior del carril exterior en una curva o cerca de los desvíos (depende de la función de desgaste o reducción del ruido)."@es ;
                 rdfs:label "Lubricacion de Carriles"@es ,
                            "Rail Lubrication"@en .


###  https://w3id.org/beo#RailMechanicalEquipment
:RailMechanicalEquipment rdf:type owl:Class ;
                         rdfs:subClassOf :DiscreteAccessory ;
                         rdfs:comment "A rail mechanical equipment is a mechnical equipment installed at railside, like blocking device, speed regulator, bias loaded inspector, track scale or controllable retarder."@en ,
                                      "Un equipo mecánico ferroviario es un equipo técnico instalado a pie de vía, como un dispositivo de bloqueo, un regulador de velocidad, un inspector con carga de polarización, una báscula de vía o un ralentizador controlable."@es ;
                         rdfs:label "Equipo Mecanico Ferroviario"@es ,
                                    "Rail Mechanical Equipment"@en .


###  https://w3id.org/beo#RailMechanicalEquipmentAssembly
:RailMechanicalEquipmentAssembly rdf:type owl:Class ;
                                 rdfs:subClassOf :ElementAssembly ;
                                 rdfs:comment "A complex assembly made up of several components like blocking device, speed regulator, bias loaded inspector, track scale or controllable retarder."@en ,
                                              "Un ensamblaje complejo formado por varios componentes como dispositivo de bloqueo, regulador de velocidad, inspector con carga polarizada, báscula de vía o retardador controlable."@es ;
                                 rdfs:label "Ensamblaje de Equipos Mecanicos Ferroviarios"@es ,
                                            "Rail Mechanical Equipment Assembly"@en .


###  https://w3id.org/beo#RailPad
:RailPad rdf:type owl:Class ;
         rdfs:subClassOf :DiscreteAccessory ;
         rdfs:comment "A non-metallic pad placed between rail and baseplate or rail and sleeper, bearer or slab. Note: definition from EN 13481-1."@en ,
                      "Almohadilla no metálica colocada entre el carril y la placa base o el carril y la traviesa, el soporte o la losa. Nota: definición de la norma EN 13481-1."@es ;
         rdfs:label "Almohadilla de Carril"@es ,
                    "Rail Pad"@en .


###  https://w3id.org/beo#Railing
:Railing rdf:type owl:Class ;
         rdfs:subClassOf :BuiltElement ;
         rdfs:comment "La barandilla es un conjunto de armazón adyacente a los espacios de circulación de personas o vehículos y en algunos límites de espacios donde se utiliza en lugar de paredes o como complemento de éstas. Diseñada como soporte físico opcional, o para evitar lesiones o daños, ya sea por caída o colisión."@es ,
                      "The railing is a frame assembly adjacent to human or vehicle circulation spaces and at some space boundaries where it is used in lieu of walls or to complement walls. Designed as an optional physical support, or to prevent injury or damage, either by falling or collision."@en ;
         rdfs:label "Barandilla"@es ,
                    "Railing"@en .


###  https://w3id.org/beo#RainbowRoof
:RainbowRoof rdf:type owl:Class ;
             rdfs:subClassOf :Roof ;
             rdfs:comment "A gable roof in the form of a broad Gothic arch, with gently sloping convex surfaces."@en ,
                          "Un tejado a dos aguas en forma de amplio arco gótico, con superficies convexas suavemente inclinadas."@es ;
             rdfs:label "Rainbow Roof"@en ,
                        "Tejado Arco Iris"@es .


###  https://w3id.org/beo#Ramp
:Ramp rdf:type owl:Class ;
      rdfs:subClassOf :BuiltElement ;
      rdfs:comment "A ramp is a vertical passageway which provides a human or vehicle circulation link between one floor level and another floor level at a different elevation. It may include a landing as an intermediate floor slab. A ramp normally does not include steps.Definition according to ISO 6707-1: Inclined way or floor joining two surfaces at different levels."@en ,
                   "Una rampa es un pasillo vertical que sirve de enlace para la circulación de personas o vehículos entre un nivel de piso y otro nivel de piso situado a diferente altura. Puede incluir un rellano como forjado intermedio. Definición según la norma ISO 6707-1: Camino o suelo inclinado que une dos superficies a distinto nivel."@es ;
      rdfs:label "Ramp"@en ,
                 "Rampa"@es .


###  https://w3id.org/beo#RampFlight
:RampFlight rdf:type owl:Class ;
            rdfs:subClassOf :BuiltElement ;
            rdfs:comment "A ramp comprises a single inclined segment, or several inclined segments that are connected by a horizontal segment, referred to as a landing. A ramp flight is the single inclined segment and part of the ramp construction. In case of single flight ramps, the ramp flight and the ramp are identical."@en ,
                         "Una rampa comprende un único segmento inclinado, o varios segmentos inclinados que están conectados por un segmento horizontal, denominado rellano. Un tramo de rampa es el segmento inclinado único y forma parte de la construcción de la rampa. En el caso de las rampas de un solo tramo, el tramo de rampa y la rampa son idénticos."@es ;
            rdfs:label "RampFlight"@en ,
                       "Tramo de Rampa"@es .


###  https://w3id.org/beo#ReinforcedSoil
:ReinforcedSoil rdf:type owl:Class ;
                rdfs:subClassOf :EarthworksElement ;
                rdfs:comment "Soil reinforced or stabilized by some mechanical or chemical method."@en ,
                             "Suelo reforzado o estabilizado por algún método mecánico o químico."@es ;
                rdfs:label "Reinforced Soil"@en ,
                           "Suelo Reforzado"@es .


###  https://w3id.org/beo#ReinforcementRing
:ReinforcementRing rdf:type owl:Class ;
                   rdfs:subClassOf :ReinforcingBar ;
                   rdfs:comment "Anillo de refuerzo."@es ,
                                "Ring reinforcement."@en ;
                   rdfs:label "Anillo de Refuerzo"@es ,
                              "Reinforcement Ring"@en .


###  https://w3id.org/beo#ReinforcingBar
:ReinforcingBar rdf:type owl:Class ;
                rdfs:subClassOf :ReinforcingElement ;
                rdfs:comment "A reinforcing bar is usually made of steel with manufactured deformations in the surface, and used in concrete and masonry construction to provide additional strength. A single instance of this class may represent one or many of actual rebars, for example a row of rebars."@en ,
                             "Una barra de refuerzo suele ser de acero con deformaciones fabricadas en la superficie, y se utiliza en la construcción de hormigón y mampostería para proporcionar resistencia adicional. Una única instancia de esta clase puede representar una o varias barras de refuerzo reales, por ejemplo, una fila de barras de refuerzo."@es ;
                rdfs:label "Barra de Refuerzo"@es ,
                           "Reinforcing Bar"@en .


###  https://w3id.org/beo#ReinforcingElement
:ReinforcingElement rdf:type owl:Class ;
                    rdfs:subClassOf :ElementComponent ;
                    rdfs:comment "A reinforcing element represents bars, wires, strands, meshes, tendons, and other components embedded in concrete in such a manner that the reinforcement and the concrete act together in resisting forces."@en ,
                                 "Un elemento de refuerzo representa barras, alambres, cordones, mallas, tendones y otros componentes embebidos en el hormigón de tal manera que el refuerzo y el hormigón actúan conjuntamente para resistir las fuerzas."@es ;
                    rdfs:label "Elemento de Refuerzo"@es ,
                               "Reinforcing Element"@en .


###  https://w3id.org/beo#ReinforcingMesh
:ReinforcingMesh rdf:type owl:Class ;
                 rdfs:subClassOf :ReinforcingElement ;
                 rdfs:comment "A reinforcing mesh is a series of longitudinal and transverse wires or bars of various gauges, arranged at right angles to each other and welded at all points of intersection; usually used for concrete slab reinforcement. It is also known as welded wire fabric. In scope are plane meshes as well as bent meshes."@en ,
                              "Una malla de refuerzo es una serie de alambres o barras longitudinales y transversales de diversos calibres, dispuestos en ángulo recto entre sí y soldados en todos los puntos de intersección; suele utilizarse para el refuerzo de losas de hormigón. También se conoce como tejido de alambre soldado. Existen mallas planas y mallas dobladas."@es ;
                 rdfs:label "Malla de Refuerzo"@es ,
                            "Reinforcing Mesh"@en .


###  https://w3id.org/beo#ReinforcmentUnit
:ReinforcmentUnit rdf:type owl:Class ;
                  rdfs:subClassOf :ElementAssembly ;
                  rdfs:comment "Assembled reinforcement elements."@en ,
                               "Elementos de refuerzo ensamblados."@es ;
                  rdfs:label "Reinforcment Unit"@en ,
                             "Unidad de Refuerzo"@es .


###  https://w3id.org/beo#ReplacedSoil
:ReplacedSoil rdf:type owl:Class ;
              rdfs:subClassOf :ReinforcedSoil ;
              rdfs:comment "Dig out the soft soil in a certain range below the foundation ground and then backfill the area with high strength, low compressibility and no corrosive materials."@en ,
                           "Excavar la tierra blanda en un cierto rango por debajo del suelo de cimentación y luego rellenar la zona con materiales de alta resistencia, baja compresibilidad y no corrosivos."@es ;
              rdfs:label "Replaced Soil"@en ,
                         "Suelo Reemplazado"@es .


###  https://w3id.org/beo#RetainingWall
:RetainingWall rdf:type owl:Class ;
               rdfs:subClassOf :Wall ;
               rdfs:comment "A supporting wall used to protect against soil layers behind."@en ,
                            "Un muro de soporte utilizado para proteger contra las capas de suelo detrás."@es ;
               rdfs:label "Muro de Contención"@es ,
                          "Retaining Wall"@en .


###  https://w3id.org/beo#RigidFrame
:RigidFrame rdf:type owl:Class ;
            rdfs:subClassOf :ElementAssembly ;
            rdfs:comment "A structure built up of beams, columns, etc. with moment-resisting joints, such as gantry"@en ,
                         "Una estructura formada por vigas, columnas, etc. con juntas resistentes a momento."@es ;
            rdfs:label "Portico Rigido"@es ,
                       "Rigid Frame"@en .


###  https://w3id.org/beo#RigidPavement
:RigidPavement rdf:type owl:Class ;
               rdfs:subClassOf :Pavement ;
               rdfs:comment "Pavement substantially constructed of cement concrete."@en ,
                            "Pavimento construido sustancialmente de hormigón de cemento."@es ;
               rdfs:label "Pavimento Rigido"@es ,
                          "Rigid Pavement"@en .


###  https://w3id.org/beo#Rivet
:Rivet rdf:type owl:Class ;
       rdfs:subClassOf :MechanicalFastener ;
       rdfs:comment "A fastening part having a head at one end and the other end being hammered flat after being passed through holes in the pieces that are fastened together."@en ,
                    "Pieza de fijación que tiene una cabeza en un extremo y el otro extremo se aplana a martillazos después de pasarlo por los orificios de las piezas que se fijan entre sí."@es ;
       rdfs:label "Remache"@es ,
                  "Rivet"@en .


###  https://w3id.org/beo#Rocker
:Rocker rdf:type owl:Class ;
        rdfs:subClassOf :Bearing ;
        rdfs:comment "La funcionalidad de soporte la proporciona una construccion basculante."@es ,
                     "The bearing functionality is provided by a rocker construction. Includes line rocker and point rocker bearings."@en ;
        rdfs:label "Cojinete Basculante"@es ,
                   "Rocker"@en .


###  https://w3id.org/beo#Roller
:Roller rdf:type owl:Class ;
        rdfs:subClassOf :Bearing ;
        rdfs:comment "La función de soporte la proporcionan uno o más rodillos que se colocan entre dos placas."@es ,
                     "The bearing functionality is provided by one or more rollers that are placed between two plates."@en ;
        rdfs:label "Cojinete de Rodillos"@es ,
                   "Roller"@en .


###  https://w3id.org/beo#RollerCompactedSoil
:RollerCompactedSoil rdf:type owl:Class ;
                     rdfs:subClassOf :ReinforcedSoil ;
                     rdfs:comment "A kind of compacting method that adopts rolling machinery, repeated rolling and vibration compacts the foundation soil, increasing strength and descreasing compressibility."@en ,
                                  "Un tipo de método de compactación que adopta maquinaria de laminación, la laminación repetida y la vibración compactan el suelo de cimentación, aumentando la resistencia y disminuyendo la compresibilidad."@es ;
                     rdfs:label "Roller Compacted Soil"@en ,
                                "Suelo compactado por Laminacion"@es .


###  https://w3id.org/beo#Roof
:Roof rdf:type owl:Class ;
      rdfs:subClassOf :BuiltElement ;
      rdfs:comment "A roof is the covering of the top part of a building, it protects the building against the effects of weather. Definition according to ISO 6707-1: construction enclosing the building from above."@en ,
                   "Un tejado es la cubierta de la parte superior de un edificio, que lo protege de los efectos de la intemperie. Definición según la norma ISO 6707-1: construcción que cierra el edificio por arriba."@es ;
      rdfs:label "Roof"@en ,
                 "Techo"@es .


###  https://w3id.org/beo#RoofSlab
:RoofSlab rdf:type owl:Class ;
          rdfs:subClassOf :Slab ;
          rdfs:comment "La losa se utiliza para representar una losa de cubierta (plana o inclinada)."@es ,
                       "The slab is used to represent a roof slab (either flat or sloped)."@en ;
          rdfs:label "Losa de Techo"@es ,
                     "Roof Slab"@en .


###  https://w3id.org/beo#RoofingCovering
:RoofingCovering rdf:type owl:Class ;
                 rdfs:subClassOf :Covering ;
                 rdfs:comment "El cubrimiento se utiliza para representar el revestimiento de un tejado."@es ,
                              "The covering is used to represent a roof covering."@en ;
                 rdfs:label "Cubrimiento de Tejado"@es ,
                            "Roofing Covering"@en .


###  https://w3id.org/beo#Rope
:Rope rdf:type owl:Class ;
      rdfs:subClassOf :MechanicalFastener ;
      rdfs:comment "Cuerda gruesa y resistente que se fabrica trenzando hebras de cáñamo, sisal, nailon o materiales similares. Se utiliza principalmente para amarrar embarcaciones."@es ,
                   "a length of thick strong cord made by twisting together strands of hemp, sisal, nylon, or similar material. used primarily for mooring vessels"@en ;
      rdfs:label "Cuerda"@es ,
                 "Rope"@en .


###  https://w3id.org/beo#RubberDamper
:RubberDamper rdf:type owl:Class ;
              rdfs:subClassOf :VibrationDamper ;
              rdfs:comment "El amortiguador de caucho es un amortiguador que absorbe energía mediante la deformación del caucho laminado. La diferencia entre el cojinete de aislamiento sísmico y el amortiguador tipo caucho es si soporta o no el peso de las estructuras superiores. El amortiguador de goma no transmite el peso de las estructuras superiores a la subestructura."@es ,
                           "The rubber Damper is a damper that absorbs energy by utilizing deformation of laminated rubber. The difference between the seismic isolation bearing and the rubber type damper is whether or not to support the weight of the upper structures. The rubber damper does not transmit the weight of the upper structures to the sub structure."@en ;
              rdfs:label "Amortiguador de Caucho"@es ,
                         "Rubber Damper"@en .


###  https://w3id.org/beo#STANDCOLUMN
:STANDCOLUMN rdf:type owl:Class ;
             rdfs:subClassOf :Column ;
             rdfs:comment "A column transmitting vertical loads from a superstructure to an arch below it."@en ,
                          "Columna que transmite cargas verticales desde una superestructura a un arco debajo de ella."@es ;
             rdfs:label "Columna de Soporte"@es ,
                        "STANDCOLUMN"@en .


###  https://w3id.org/beo#STRIPFOOTING
:STRIPFOOTING rdf:type owl:Class ;
              rdfs:subClassOf :Footing ;
              rdfs:comment "A linear element that transfers loads into the ground from either a continuous element, such as a wall, or from a series of elements, such as columns."@en ,
                           "Un elemento lineal que transfiere cargas al suelo desde un elemento continuo, como una pared, o desde una serie de elementos, como columnas."@es ;
              rdfs:label "STRIP FOOTING"@en ,
                         "Zapata Corrida"@es .


###  https://w3id.org/beo#SafetyCage
:SafetyCage rdf:type owl:Class ;
            rdfs:subClassOf :BuildingElementPart ;
            rdfs:comment "Las jaulas de seguridad son un conjunto de barras circulares y verticales que se sujetan a los montantes de escaleras fijas y están dispuestas para encerrar el camino de un trabajador al subir la escalera. Las escaleras así cerradas también se conocen como escaleras de jaula o de aros."@es ,
                         "Safety cages are an assembly of circular and vertical bars that are fastened to the stiles of fixed ladders and are arranged to enclose the path of a worker when climbing the ladder. Ladders so enclosed are also known as caged or hooped ladders."@en ;
            rdfs:label "Jaula de Seguridad"@es ,
                       "Safety Cage"@en .


###  https://w3id.org/beo#Screw
:Screw rdf:type owl:Class ;
       rdfs:subClassOf :MechanicalFastener ;
       rdfs:comment "A fastener with a tapered threaded shank and a slotted head."@en ,
                    "Elemento de fijación con un vástago roscado cónico y una cabeza ranurada."@es ;
       rdfs:label "Screw"@en ,
                  "Tornillo"@es .


###  https://w3id.org/beo#ShadingDevice
:ShadingDevice rdf:type owl:Class ;
               rdfs:subClassOf :BuiltElement ;
               rdfs:comment "Los sombreaderos son dispositivos construidos específicamente para proteger de la luz solar, de la luz natural o para ocultarlos de la vista. Los dispositivos de sombreado pueden formar parte de la fachada o montarse en el interior del edificio, y pueden ser fijos o accionables."@es ,
                            "Shading devices are purpose built devices to protect from the sunlight, from natural light, or screening them from view. Shading devices can form part of the facade or can be mounted inside the building, they can be fixed or operable."@en ;
               rdfs:label "Shading Device"@en ,
                          "Sombreaderos"@es .


###  https://w3id.org/beo#Shear-yieldDamper
:Shear-yieldDamper rdf:type owl:Class ;
                   rdfs:subClassOf :VibrationDamper ;
                   rdfs:comment "A displacement dependent type damper in which the resistance force generated is determined by the plastic strain amount utilizing the plastic deformation of the steel material. The shear yield type is a damper, which causes the steel material to yield for deformation in the direction perpendicular to the member."@en ,
                                "Un amortiguador dependiente del desplazamiento en el que la fuerza de resistencia generada está determinada por la cantidad de deformación plástica del acero. El amortiguador de rendimiento a flexion absorbe enrgía deformando el acero en la dirección perpendicular al miembro"@es ;
                   rdfs:label "Amortiguador de Rendimiento a Cortante"@es ,
                              "Shear-yield Damper"@en .


###  https://w3id.org/beo#ShearBar
:ShearBar rdf:type owl:Class ;
          rdfs:subClassOf :ReinforcingBar ;
          rdfs:comment "La barra de refuerzo es una barra de cizallamiento."@es ,
                       "The reinforcing bar is a shear bar."@en ;
          rdfs:label "Barra de Cizallamiento"@es ,
                     "Shear Bar"@en .


###  https://w3id.org/beo#ShearConnector
:ShearConnector rdf:type owl:Class ;
                rdfs:subClassOf :MechanicalFastener ;
                rdfs:comment "A ring connector that is accepted by ring keyways in the connected pieces; or a toothed circular or square connector that is pressed into the connected pieces."@en ,
                             "Un conector anular que se acepta mediante chaveteros anulares en las piezas conectadas; o un conector circular o cuadrado dentado que se introduce a presión en las piezas conectadas."@es ;
                rdfs:label "Conector de Cizallamiento"@es ,
                           "Shear Connector"@en .


###  https://w3id.org/beo#ShearWall
:ShearWall rdf:type owl:Class ;
           rdfs:subClassOf :Wall ;
           rdfs:comment "A wall designed to withstand shear loads. Examples of shear wall are diaphragms inside a box girder, typically on a pier, to resist lateral forces and transfer them to the support."@en ,
                        "Un muro diseñado para soportar cargas de corte. Ejemplos de muro de corte son diafragmas dentro de una viga cajón, típicamente en un muelle, para resistir fuerzas laterales y transferirlas al soporte."@es ;
           rdfs:label "Muro de Cortante"@es ,
                      "Shear Wall"@en .


###  https://w3id.org/beo#ShedRoof
:ShedRoof rdf:type owl:Class ;
          rdfs:subClassOf :Roof ;
          rdfs:comment "A roof having a single slope."@en ,
                       "Un tejado con una sola pendiente."@es ;
          rdfs:label "Cobertizo"@es ,
                     "Shed Roof"@en .


###  https://w3id.org/beo#Sheet
:Sheet rdf:type owl:Class ;
       rdfs:subClassOf :Plate ;
       rdfs:comment "A planar, flat and thin element, comes usually as metal sheet, and is often used as an additional part within an assembly."@en ,
                    "Elemento plano y delgado que suele presentarse en forma de chapa metálica y suele utilizarse como pieza adicional dentro de un conjunto."@es ;
       rdfs:label "Lamina"@es ,
                  "Sheet"@en .


###  https://w3id.org/beo#Shelter
:Shelter rdf:type owl:Class ;
         rdfs:subClassOf :ElementAssembly ;
         rdfs:comment "A structure, fairly quick to setup, move or dismantle, used to give protection, especially from the weather or intrusion."@en ,
                      "Estructura, bastante rápida de montar, mover o desmontar, que se utiliza para ofrecer protección, especialmente contra las inclemencias del tiempo o las intrusiones."@es ;
         rdfs:label "Refugio"@es ,
                    "Shelter"@en .


###  https://w3id.org/beo#Shoe
:Shoe rdf:type owl:Class ;
      rdfs:subClassOf :DiscreteAccessory ;
      rdfs:comment "A column shoe or a beam shoe (beam hanger) used to support or secure an element."@en ,
                   "Una zapata de pilar o una zapata de viga (suspensor de viga) utilizada para soportar o asegurar un elemento."@es ;
      rdfs:label "Shoe"@en ,
                 "Zapata"@es .


###  https://w3id.org/beo#Shutter
:Shutter rdf:type owl:Class ;
         rdfs:subClassOf :ShadingDevice ;
         rdfs:comment "A mechanical device that limits the passage of light. Often used as a a solid or louvered movable cover for a window."@en ,
                      "Dispositivo mecánico que limita el paso de la luz. A menudo se utiliza como una cubierta móvil sólida o de lamas para una ventana."@es ;
         rdfs:label "Persiana"@es ,
                    "Shutter"@en .


###  https://w3id.org/beo#SidewalkSlab
:SidewalkSlab rdf:type owl:Class ;
              rdfs:subClassOf :Slab ;
              rdfs:comment "La losa se utiliza para representar una acera."@es ,
                           "The slab is used to represent a sidewalk."@en ;
              rdfs:label "Losa de Acera"@es ,
                         "Sidewalk Slab"@en .


###  https://w3id.org/beo#Sign
:Sign rdf:type owl:Class ;
      rdfs:subClassOf :ElementComponent ;
      rdfs:comment "A sign is a notice on display that gives information or instructions in a written, symbolic or other form. Signs are passive with the most common form of a pictorial panel. "@en ,
                   "Una señal es un aviso expuesto que da información o instrucciones de forma escrita, simbólica o de otro tipo. Los rótulos son pasivos y su forma más común es un panel pictórico. "@es ;
      rdfs:label "Señal"@es ,
                 "Sign"@en .


###  https://w3id.org/beo#SignalAssembly
:SignalAssembly rdf:type owl:Class ;
                rdfs:subClassOf :ElementAssembly ;
                rdfs:comment "An assembly to physically aggregate together one or more signal instances (and also sign instances) including any supporting structural elements such as a simple pole or a rigid frame gantry."@en ,
                             "Un ensamblaje para agregar físicamente una o más instancias de señales (y también instancias de señales), incluido cualquier elemento estructural de soporte, como un poste simple o un pórtico de marco rígido."@es ;
                rdfs:label "Ensamblaje de Señales"@es ,
                           "Signal Assembly"@en .


###  https://w3id.org/beo#SkirtingBoard
:SkirtingBoard rdf:type owl:Class ;
               rdfs:subClassOf :Covering ;
               rdfs:comment "El cubrimiento se utiliza para representar un rodapié que es una tira de material para cubrir la transición entre el revestimiento de la pared y el suelo."@es ,
                            "The covering is used to represent a skirting board being a strip of material to cover the transition between the wall cladding and the flooring."@en ;
               rdfs:label "Rodapie"@es ,
                          "Skirting Board"@en .


###  https://w3id.org/beo#Skylight
:Skylight rdf:type owl:Class ;
          rdfs:subClassOf :Window ;
          rdfs:comment "A window within a sloped building element, usually a roof slab."@en ,
                       "Una ventana dentro de un elemento de construcción inclinado, generalmente una losa de techo."@es ;
          rdfs:label "Skylight"@en ,
                     "Skylight"@es .


###  https://w3id.org/beo#Slab
:Slab rdf:type owl:Class ;
      rdfs:subClassOf :BuiltElement ;
      rdfs:comment "A slab is a component of the construction that may enclose a space vertically. The slab may provide the lower support (floor) or upper construction (roof slab) in any space in a building. Only the core or constructional part of this construction is considered to be a slab. The upper finish (flooring, roofing) and the lower finish (ceiling, suspended ceiling) are considered to be coverings. A special type of slab is the landing, described as a floor section to which one or more stair flights or ramp flights connect."@en ,
                   "Un forjado es un componente de la construcción que puede cerrar un espacio verticalmente. El forjado puede constituir el soporte inferior (suelo) o superior (forjado de cubierta) de cualquier espacio de un edificio. Sólo se considera losa el núcleo o parte constructiva de esta construcción. El acabado superior (suelo, cubierta) y el acabado inferior (techo, falso techo) se consideran revestimientos. Un tipo especial de forjado es el rellano, descrito como una sección de suelo a la que se conectan uno o varios tramos de escalera o rampa."@es ;
      rdfs:label "Losa"@es ,
                 "Slab"@en .


###  https://w3id.org/beo#SlabField
:SlabField rdf:type owl:Class ;
           rdfs:subClassOf :ElementAssembly ;
           rdfs:comment "Losas dispuestas en un solo plano."@es ,
                        "Slabs, laid out in one plane."@en ;
           rdfs:label "Slab Field"@en ,
                      "Superficie de Losas"@es .


###  https://w3id.org/beo#Sleeper
:Sleeper rdf:type owl:Class ;
         rdfs:subClassOf :TrackElement ;
         rdfs:comment "A sleeper is a track element that supports running rails, guard rails and check rails usually at right angles to its axis."@en ,
                      "Una traviesa es un elemento de la vía que soporta los carriles de rodadura, los guardarraíles y los contracarriles, normalmente en ángulo recto con respecto a su eje."@es ;
         rdfs:label "Sleeper"@en ,
                    "Traviesa"@es .


###  https://w3id.org/beo#Sleeving
:Sleeving rdf:type owl:Class ;
          rdfs:subClassOf :Covering ;
          rdfs:comment "El cubrimiento sirve para aislar un elemento de distribución de un espacio en el que está contenido."@es ,
                       "The covering is used to isolate a distribution element from a space in which it is contained."@en ;
          rdfs:label "Funda"@es ,
                     "Sleeving"@en .


###  https://w3id.org/beo#SlidingChair
:SlidingChair rdf:type owl:Class ;
              rdfs:subClassOf :DiscreteAccessory ;
              rdfs:comment "A component which supports and retains the stock rail and a flat surface upon which the foot of the switch rail slides."@en ,
                           "Componente que soporta y retiene la contraaguja y una superficie plana sobre la que se desliza el pie de la aguja."@es ;
              rdfs:label "Silla Deslizante"@es ,
                         "Sliding Chair"@en .


###  https://w3id.org/beo#SlopeFill
:SlopeFill rdf:type owl:Class ;
           rdfs:subClassOf :EarthworksFill ;
           rdfs:comment "Relleno del talud lateral (bateo) colindante con la estructura de la carretera o relleno del talud posterior."@es ,
                        "Side slope (batter) fill abutting the road structure or back slope fill."@en ;
           rdfs:label "Slope Fill"@en ,
                      "Talud"@es .


###  https://w3id.org/beo#SolidWall
:SolidWall rdf:type owl:Class ;
           rdfs:subClassOf :Wall ;
           rdfs:comment "A massive wall construction for the wall core being the single layer or having multiple layers attached. Such walls are often masonry or concrete walls (both cast in-situ or precast) that are load bearing and fire protecting."@en ,
                        "Una construcción de pared masiva para el núcleo de la pared, ya sea de una sola capa o con múltiples capas unidas. Estos muros suelen ser muros de mampostería u hormigón (tanto moldeados in situ como prefabricados) que soportan cargas y protegen contra incendios."@es ;
           rdfs:label "Muro Solido"@es ,
                      "Solid Wall"@en .


###  https://w3id.org/beo#SoundAbsortion
:SoundAbsortion rdf:type owl:Class ;
                rdfs:subClassOf :DiscreteAccessory ;
                rdfs:comment "A component in the track for sound absorption and may also absorb vibrations. It is often used in combination with slab tracks."@en ,
                             "La absorción acústica es un componente de la vía para la absorción acústica y también puede absorber las vibraciones. Suele utilizarse en combinación con vías de placa."@es ;
                rdfs:label "Absorcion Acustica"@es ,
                           "Sound Absortion"@en .


###  https://w3id.org/beo#SpaceBar
:SpaceBar rdf:type owl:Class ;
          rdfs:subClassOf :ReinforcingBar ;
          rdfs:comment "A stirrup in pre-stressing system to position the Tendon Conduit."@en ,
                       "Un estribo en el sistema de pretensado para colocar el Conducto del Tendon."@es ;
          rdfs:label "Barra Espaciadora"@es ,
                     "Space Bar"@en .


###  https://w3id.org/beo#SpeedRegulator
:SpeedRegulator rdf:type owl:Class ;
                rdfs:subClassOf :TrackElement ;
                rdfs:comment "A device composed of pneumatic, mechanic or electric components causing the breaking of a train in case of emergency."@en ,
                             "Dispositivo compuesto de componentes neumáticos, mecánicos o eléctricos que provoca la rotura de un tren en caso de emergencia."@es ;
                rdfs:label "Regulador de Velocidad"@es ,
                           "Speed Regulator"@en .


###  https://w3id.org/beo#SphericalBearing
:SphericalBearing rdf:type owl:Class ;
                  rdfs:subClassOf :Bearing ;
                  rdfs:comment "La función de soporte la proporciona una cúpula convexa en una cubeta cóncava."@es ,
                               "The bearing functionality is provided by convex dome in a concave basin."@en ;
                  rdfs:label "Cojinete Esferico"@es ,
                             "Spherical Bearing"@en .


###  https://w3id.org/beo#SpiralRamp
:SpiralRamp rdf:type owl:Class ;
            rdfs:subClassOf :Ramp ;
            rdfs:comment "A ramp constructed around a circular or elliptical well without newels and landings."@en ,
                         "Rampa construida alrededor de un pozo circular o elíptico sin newels ni descansillos."@es ;
            rdfs:label "Rampa en Esprial"@es ,
                       "Spiral Ramp"@en .


###  https://w3id.org/beo#SpiralRampFlight
:SpiralRampFlight rdf:type owl:Class ;
                  rdfs:subClassOf :RampFlight ;
                  rdfs:comment "A ramp flight with a circular or elliptic walking line."@en ,
                               "Un vuelo en rampa con una línea de marcha circular o elíptica."@es ;
                  rdfs:label "Spiral Ramp Flight"@en ,
                             "Tramo de Rampa en Espiral"@es .


###  https://w3id.org/beo#SpiralStair
:SpiralStair rdf:type owl:Class ;
             rdfs:subClassOf :Stair ;
             rdfs:comment "A stair constructed with winders around a circular newel often without landings. Depending on outer boundary it can be either a circular, elliptical or rectangular spiral stair. The orientation of the winding stairs is determined by the walking line."@en ,
                          "Escalera construida con devanaderas alrededor de un newel circular, a menudo sin descansillos. Dependiendo del límite exterior, puede ser una escalera de caracol circular, elíptica o rectangular. La orientación de la escalera de caracol viene determinada por la línea de paso."@es ;
             rdfs:label "Escalera de Caracol"@es ,
                        "Spiral Stair"@en .


###  https://w3id.org/beo#SpiralStairFlight
:SpiralStairFlight rdf:type owl:Class ;
                   rdfs:subClassOf :StairFlight ;
                   rdfs:comment "A stair flight with a circular or elliptic walking line."@en ,
                                "Un tramo de escalera con un trazado circular o elíptico."@es ;
                   rdfs:label "Spiral Stair Flight"@en ,
                              "Tramo de Escalera de caracol"@es .


###  https://w3id.org/beo#SplicePlate
:SplicePlate rdf:type owl:Class ;
             rdfs:subClassOf :Plate ;
             rdfs:comment "A plate connecting two members joined at ends."@en ,
                          "Placa que une dos elementos unidos por los extremos."@es ;
             rdfs:label "Placa de Empalme"@es ,
                        "Splice Plate"@en .


###  https://w3id.org/beo#Sprandel
:Sprandel rdf:type owl:Class ;
          rdfs:subClassOf :Beam ;
          rdfs:comment "A tall beam placed on the facade of a building. One tall side is usually finished to provide the exterior of the building. Can be used to support joists or slab elements on its interior side."@en ,
                       "Una viga alta colocada en la fachada de un edificio. Por lo general, se termina un lado alto para proporcionar el exterior del edificio. Puede utilizarse para soportar viguetas o elementos de losa por su cara interior."@es ;
          rdfs:label "Antepecho"@es ,
                     "Sprandel"@en .


###  https://w3id.org/beo#SpringIsolator
:SpringIsolator rdf:type owl:Class ;
                rdfs:subClassOf :VibrationIsolator ;
                rdfs:comment "Aislador de vibraciones tipo resorte."@es ,
                             "Spring type vibration isolator."@en ;
                rdfs:label "Aislador de Resorte"@es ,
                           "Spring Isolator"@en .


###  https://w3id.org/beo#Stair
:Stair rdf:type owl:Class ;
       rdfs:subClassOf :BuiltElement ;
       rdfs:comment "A stair is a vertical passageway allowing occupants to walk (step) from one floor level to another floor level at a different elevation. It may include a landing as an intermediate floor slab.  Definition according to ISO 6707-1: Construction comprising a succession of horizontal stages (steps or landings) that make it possible to pass on foot to other levels."@en ,
                    "Una escalera es un pasillo vertical que permite a los ocupantes caminar (subir) de un nivel de piso a otro nivel de piso a una elevación diferente. Puede incluir un rellano como forjado intermedio.  Definición según la norma ISO 6707-1: Construcción que comprende una sucesión de escalones horizontales (peldaños o rellanos) que permiten pasar a pie a otros niveles."@es ;
       rdfs:label "Escalera"@es ,
                  "Stair"@en .


###  https://w3id.org/beo#StairFlight
:StairFlight rdf:type owl:Class ;
             rdfs:subClassOf :BuiltElement ;
             rdfs:comment "A stair flight is an assembly of building components in a single 'run' of stair steps (not interrupted by a landing). The stair steps and any stringers are included in the stair flight. A winder is also regarded a part of a stair flight."@en ,
                          "Un tramo de escalera es un conjunto de componentes de construcción en un único 'tramo' de peldaños (no interrumpido por un rellano). Los peldaños y los largueros están incluidos en el tramo de escalera. Una devanadera también se considera parte de un tramo de escalera."@es ;
             rdfs:label "StairFlight"@en ,
                        "Tramo de Escalera"@es .


###  https://w3id.org/beo#Staple
:Staple rdf:type owl:Class ;
        rdfs:subClassOf :MechanicalFastener ;
        rdfs:comment "A doubly pointed piece of metal that is hammered into materials as a fastener."@en ,
                     "Pieza de metal con doble punta que se clava en los materiales como cierre."@es ;
        rdfs:label "Grapa"@es ,
                   "Staple"@en .


###  https://w3id.org/beo#StayCable
:StayCable rdf:type owl:Class ;
           rdfs:subClassOf :Member ;
           rdfs:comment "A sloped element suspending a structure (such as bridge deck) from a pylon."@en ,
                        "Elemento inclinado que suspende una estructura (como el tablero de un puente) desde un pilón."@es ;
           rdfs:label "Cable Atirantado"@es ,
                      "Stay Cable"@en .


###  https://w3id.org/beo#StiffenerPlate
:StiffenerPlate rdf:type owl:Class ;
                rdfs:subClassOf :Plate ;
                rdfs:comment "A transversal plate added to a flange or a web plate for local stiffening."@en ,
                             "Placa transversal añadida a un ala o a una placa de alma para rigidizar localmente."@es ;
                rdfs:label "Placa Rigidizadora"@es ,
                           "Stiffener Plate"@en .


###  https://w3id.org/beo#StiffeningRib
:StiffeningRib rdf:type owl:Class ;
               rdfs:subClassOf :Member ;
               rdfs:comment "A linear element added to a flange or a web plate of a girder for local stiffening."@en ,
                            "Elemento lineal que se añade a un ala o a una placa de alma de una viga para rigidizarla localmente."@es ;
               rdfs:label "Nervio de Refuerzo"@es ,
                          "Stiffening Rib"@en .


###  https://w3id.org/beo#StockRail
:StockRail rdf:type owl:Class ;
           rdfs:subClassOf :Rail ;
           rdfs:comment "A stock rail is a fixed machined rail, ensuring the continuity on the main or diverging track with the switch in the open position. The machined part of the stock rail supports its switch rail in the closed position, giving continuity of line through this switch rail. The two stock rails in a set of switches are the two outside rails. A stock rail is described as right or left hand according to whether it is part of a right hand or left hand half-set of switches. Note: definition from EN 13232-1-2004."@en ,
                        "Una contraaguja es un carril mecanizado fijo que garantiza la continuidad en la vía principal o desviada con la aguja en posición abierta. La parte mecanizada de la contraaguja soporta su aguja en la posición cerrada, dando continuidad a la línea a través de esta aguja. Las dos contraagujas de un juego de agujas son las dos vías exteriores. Una contraaguja se describe como derecha o izquierda según forme parte de un medio juego de agujas derecho o izquierdo. Nota: definición de la norma EN 13232-1-2004."@es ;
           rdfs:label "Contraaguja"@es ,
                      "Stock Rail"@en .


###  https://w3id.org/beo#StraightRampFlight
:StraightRampFlight rdf:type owl:Class ;
                    rdfs:subClassOf :RampFlight ;
                    rdfs:comment "A ramp flight with a straight walking line."@en ,
                                 "Un vuelo en rampa con una línea de marcha recta."@es ;
                    rdfs:label "Straight Ramp Flight"@en ,
                               "Tramo de Rampa Recto"@es .


###  https://w3id.org/beo#StraightRunRamp
:StraightRunRamp rdf:type owl:Class ;
                 rdfs:subClassOf :Ramp ;
                 rdfs:comment "A ramp - which is a sloping floor, walk, or roadway - connecting two levels. The straight ramp consists of one straight flight without turns or winders."@en ,
                              "Una rampa -que es un suelo inclinado, un paseo o una calzada- que conecta dos niveles. La rampa recta consiste en un tramo recto sin giros ni devanaderas."@es ;
                 rdfs:label "Rampa Recta"@es ,
                            "Straight Run Ramp"@en .


###  https://w3id.org/beo#StraightRunStair
:StraightRunStair rdf:type owl:Class ;
                  rdfs:subClassOf :Stair ;
                  rdfs:comment "A stair extending from one level to another without turns or winders. The stair consists of one straight flight."@en ,
                               "Escalera que se extiende de un nivel a otro sin giros ni devanaderas. La escalera consta de un tramo recto."@es ;
                  rdfs:label "Escalera de Tramo Recto"@es ,
                             "Straight Run Stair"@en .


###  https://w3id.org/beo#StraightStairFlight
:StraightStairFlight rdf:type owl:Class ;
                     rdfs:subClassOf :StairFlight ;
                     rdfs:comment "A stair flight with a straight walking line."@en ,
                                  "Un tramo de escalera en línea recta."@es ;
                     rdfs:label "Straight Stair Flight"@en ,
                                "Tramo de Escalera Recto"@es .


###  https://w3id.org/beo#Strand
:Strand rdf:type owl:Class ;
        rdfs:subClassOf :Tendon ;
        rdfs:comment "El tendón es un filamento."@es ,
                     "The tendon is a strand."@en ;
        rdfs:label "Filamento"@es ,
                   "Strand"@en .


###  https://w3id.org/beo#Stringer
:Stringer rdf:type owl:Class ;
          rdfs:subClassOf :Member ;
          rdfs:comment "A linear element used to support stair or ramp flights, usually used with slope."@en ,
                       "Elemento lineal utilizado para soportar tramos de escaleras o rampas, generalmente utilizado con pendiente."@es ;
          rdfs:label "Larguero"@es ,
                     "Stringer"@en .


###  https://w3id.org/beo#StructuralCable
:StructuralCable rdf:type owl:Class ;
                 rdfs:subClassOf :Member ;
                 rdfs:comment "A linear cable element used to secure or stabilise a structure by resisting lateral and longitudinal loading through tension only, but cannot resist compression. usually formed of a flexible cable or wire."@en ,
                              "Elemento de cable lineal utilizado para asegurar o estabilizar una estructura resistiendo cargas laterales y longitudinales únicamente por tracción, pero no puede resistir la compresión. suele estar formado por un cable o alambre flexible."@es ;
                 rdfs:label "Cable Estructural"@es ,
                            "Structural Cable"@en .


###  https://w3id.org/beo#Strut
:Strut rdf:type owl:Class ;
       rdfs:subClassOf :Member ;
       rdfs:comment "A linear element often used within a girder or truss."@en ,
                    "Elemento lineal utilizado a menudo en el interior de una viga o celosía."@es ;
       rdfs:label "Puntal"@es ,
                  "Strut"@en .


###  https://w3id.org/beo#Stud
:Stud rdf:type owl:Class ;
      rdfs:subClassOf :ReinforcingBar ;
      rdfs:comment "La barra de refuerzo es un esparrago."@es ,
                   "The reinforcing bar is a stud."@en ;
      rdfs:label "Esparrago"@es ,
                 "Stud"@en .


###  https://w3id.org/beo#StudShearConnector
:StudShearConnector rdf:type owl:Class ;
                    rdfs:subClassOf :MechanicalFastener ;
                    rdfs:comment "Los conectores de cizalladura de espárrago son piezas de fijación cilíndricas con una cabeza en un lado. Por el otro lado se sueldan a elementos de acero para su uso en estructuras mixtas de acero y hormigón."@es ,
                                 "Stud shear connectors are cylindrical fastening parts with a head on one side. On the other side they are welded on steel members for the use in composite steel and concrete structures."@en ;
                    rdfs:label "Esparrago de Cizallameinto"@es ,
                               "Stud Shear Connector"@en .


###  https://w3id.org/beo#Subgrade
:Subgrade rdf:type owl:Class ;
          rdfs:subClassOf :EarthworksFill ;
          rdfs:comment "Tipo de elemento de movimiento de tierras que forma la estructura por debajo del pavimento y por encima del suelo natural. NOTA Definición de ISO 6707-1: Parte superior del suelo, natural o construido, que soporta las cargas transmitidas por la estructura suprayacente de una carretera, pista de aterrizaje o superficie dura similar. NOTA Definición de la AIPCR: Capa superior del suelo natural sobre la que se construye el pavimento."@es ,
                       "Type of earthworks element forming the structure below pavement and above natural soil. NOTE Definition from ISO 6707-1: upper part of the soil, natural or constructed, that supports the loads transmitted by the overlying structure of a road, runway, or similar hard surface. NOTE Definition from PIARC: Upper layer of the natural ground upon which the pavement is constructed."@en ;
          rdfs:label "Subbase"@es ,
                     "Subgrade"@en .


###  https://w3id.org/beo#SubgradeBed
:SubgradeBed rdf:type owl:Class ;
             rdfs:subClassOf :EarthworksFill ;
             rdfs:comment "Parte superior del suelo, natural o construido, que soporta las cargas transmitidas por la estructura suprayacente de una carretera, pista de aterrizaje o superficie dura similar."@es ,
                          "Upper part of the soil, natural or constructed, that supports the loads transmitted by the overlying structure of a road, runway, or similar hard surface."@en ;
             rdfs:label "Lecho de la Subbase"@es ,
                        "Subgrade Bed"@en .


###  https://w3id.org/beo#SumpBuster
:SumpBuster rdf:type owl:Class ;
            rdfs:subClassOf :ElementAssembly ;
            rdfs:comment "An obstacle (with oil catchment basin) installed typically in a bus lane to prevent other traffic with lower ground clearance from using it. Also Sump breaker or Sump trap."@en ,
                         "Un obstáculo (con un depósito de captación de petróleo) instalado típicamente en un carril bus para evitar que otro tráfico con menor distancia al suelo lo utilice. También interruptor de sumidero o trampa de sumidero."@es ;
            rdfs:label "Sump Buster"@en ,
                       "Sump Buster"@es .


###  https://w3id.org/beo#SupportPile
:SupportPile rdf:type owl:Class ;
             rdfs:subClassOf :Pile ;
             rdfs:comment "A support pile."@en ,
                          "Una pila de soporte"@es ;
             rdfs:label "Pila de Soporte"@es ,
                        "Support Pile"@en .


###  https://w3id.org/beo#SupportingGasAssembly
:SupportingGasAssembly rdf:type owl:Class ;
                       rdfs:subClassOf :ElementAssembly ;
                       rdfs:comment "An assembly intends to support Overhead Contact Line System. It includes foundation, supporting elements and suspension assembly."@en ,
                                    "Conjunto diseñado para sostener el sistema de línea aérea de contacto. Esto incluye la base, los elementos de soporte y el conjunto de suspensión"@es ;
                       rdfs:label "Conjunto de Soporte de Gas"@es ,
                                  "Supporting Gas Assembly"@en .


###  https://w3id.org/beo#SurchargePreloadedSoil
:SurchargePreloadedSoil rdf:type owl:Class ;
                        rdfs:subClassOf :ReinforcedSoil ;
                        rdfs:comment "A method that applies load to the foundation to discharge pore water, and the foundation is consolidated to improve the foundation strength. Unloading when the carrying capacity reaches the required level."@en ,
                                     "Método que aplica una carga a los cimientos para descargar el agua de los poros, y los cimientos se consolidan para mejorar la resistencia de los cimientos. Descarga cuando la capacidad de carga alcanza el nivel requerido."@es ;
                        rdfs:label "Suelo Precargado con Sobrecarga"@es ,
                                   "Surcharge Preloaded Soil"@en .


###  https://w3id.org/beo#Suspender
:Suspender rdf:type owl:Class ;
           rdfs:subClassOf :Member ;
           rdfs:comment "A vertical element suspending a structure (such as bridge deck) from a suspension cable or an arch."@en ,
                        "Elemento vertical que suspende una estructura (como el tablero de un puente) de un cable de suspensión o de un arco."@es ;
           rdfs:label "Suspender"@en ,
                      "Tirante"@es .


###  https://w3id.org/beo#SuspensionAssembly
:SuspensionAssembly rdf:type owl:Class ;
                    rdfs:subClassOf :ElementAssembly ;
                    rdfs:comment "A complex assembly of components used to suspend elements or cable segments."@en ,
                                 "Conjunto complejo de componentes utilizados para suspender elementos o segmentos de cable."@es ;
                    rdfs:label "Ensamblaje  de Suspension"@es ,
                               "Suspension Assembly"@en .


###  https://w3id.org/beo#SuspensionCable
:SuspensionCable rdf:type owl:Class ;
                 rdfs:subClassOf :Member ;
                 rdfs:comment "A suspended element, typically comprising steel wire, sheath, etc."@en ,
                              "Un elemento suspendido, normalmente compuesto de alambre de acero, funda, etc."@es ;
                 rdfs:label "Cable de Suspension"@es ,
                            "Suspension Cable"@en .


###  https://w3id.org/beo#TBeam
:TBeam rdf:type owl:Class ;
       rdfs:subClassOf :Beam ;
       rdfs:comment "A beam that forms part of a slab construction and acts together with the slab which it carries. Such beams are often of T-shape (therefore the English name), but may have other shapes as well, e.g. an L-Shape or an Inverted-T-Shape."@en ,
                    "Viga que forma parte de una construcción de losa y actúa junto con la losa que soporta. Estas vigas suelen tener forma de T, pero también pueden tener otras formas, p. ej. una forma de L o una forma de T invertida."@es ;
       rdfs:label "T Beam"@en ,
                  "Viga T"@es .


###  https://w3id.org/beo#Tendon
:Tendon rdf:type owl:Class ;
        rdfs:subClassOf :ReinforcingElement ;
        rdfs:comment "A tendon is a steel element such as a wire, cable, bar, rod, or strand used to impart prestress to concrete when the element is tensioned. Definition according to ISO 6707-1: steel bar(s) or groups of bars, strands or wires given a tensile stress that produces a compressive stress in prestressed concrete or masonry."@en ,
                     "Un tendón es un elemento de acero como un alambre, cable, barra, varilla o cordón utilizado para impartir pretensado al hormigón cuando se tensa el elemento. Definición según la norma ISO 6707-1: barra(s) de acero o grupos de barras, cordones o alambres sometidos a un esfuerzo de tracción que produce un esfuerzo de compresión en el hormigón o la mampostería pretensados."@es ;
        rdfs:label "Tendon"@en ,
                   "Tendon"@es .


###  https://w3id.org/beo#TendonAnchor
:TendonAnchor rdf:type owl:Class ;
              rdfs:subClassOf :ReinforcingElement ;
              rdfs:comment "A tendon anchor is the end connection for tendons in prestressed or posttensioned concrete."@en ,
                           "Un anclaje de tendón es la conexión final para tendones en hormigón pretensado o postensado."@es ;
              rdfs:label "Anclaje de Tendon"@es ,
                         "Tendon Anchor"@en .


###  https://w3id.org/beo#TendonConduit
:TendonConduit rdf:type owl:Class ;
               rdfs:subClassOf :ReinforcingElement ;
               rdfs:comment "A Tendon Conduit represents the components of the conduit system for tendons embedded in concrete structure."@en ,
                            "Un Conducto para Tendones representa los componentes del sistema de conductos para tendones embebidos en estructura de hormigón."@es ;
               rdfs:label "Conducto para Tendones"@es ,
                          "Tendon Conduit"@en .


###  https://w3id.org/beo#TendonConduitCoupler
:TendonConduitCoupler rdf:type owl:Class ;
                      rdfs:subClassOf :TendonConduit ;
                      rdfs:comment "A part to connect the conduits located in two different deck segments and related to the same tendon."@en ,
                                   "Una pieza para conectar los conductos situados en dos segmentos de cubierta diferentes y relacionados con el mismo tendón."@es ;
                      rdfs:label "Acople de Conductos para Tendones"@es ,
                                 "Tendon Conduit Coupler"@en .


###  https://w3id.org/beo#TendonCoupler
:TendonCoupler rdf:type owl:Class ;
               rdfs:subClassOf :TendonAnchor ;
               rdfs:comment "El anclaje es un dispositivo intermedio que conecta dos tendones."@es ,
                            "The anchor is an intermediate device which connects two tendons."@en ;
               rdfs:label "Acoplador de Tendones"@es ,
                          "Tendon Coupler"@en .


###  https://w3id.org/beo#TendonDuct
:TendonDuct rdf:type owl:Class ;
            rdfs:subClassOf :TendonConduit ;
            rdfs:comment "A Sleeve or duct is related to the thickness of the conduit depending on the conduit, either cast into the concrete structure or placed adjacent to it."@en ,
                         "Un manguito o conducto está relacionado con el grosor del conducto dependiendo de éste, ya sea colado en la estructura de hormigón o colocado junto a ella."@es ;
            rdfs:label "Manguito"@es ,
                       "Tendon Duct"@en .


###  https://w3id.org/beo#TensionEquipment
:TensionEquipment rdf:type owl:Class ;
                  rdfs:subClassOf :DiscreteAccessory ;
                  rdfs:comment "An equipment used to maintain the tension of conductors or cables."@en ,
                               "Equipo utilizado para mantener la tensión de conductores o cables."@es ;
                  rdfs:label "Equipo de Tension"@es ,
                             "Tension Equipment"@en .


###  https://w3id.org/beo#TensioningEndAnchor
:TensioningEndAnchor rdf:type owl:Class ;
                     rdfs:subClassOf :TendonAnchor ;
                     rdfs:comment "El anclaje se utiliza o puede utilizarse para pretensar el tendón."@es ,
                                  "The anchor is used or can be used to prestress the tendon."@en ;
                     rdfs:label "Anclaje de Tensionado"@es ,
                                "Tensioning End Anchor"@en .


###  https://w3id.org/beo#ThreeQuarterTurnStair
:ThreeQuarterTurnStair rdf:type owl:Class ;
                       rdfs:subClassOf :Stair ;
                       rdfs:comment "A stair making a 270° turn, consisting of four straight flights connected by three quarterspace landings. The direction of the turns is determined by the walking line."@en ,
                                    "Escalera con un giro de 270°, compuesta por cuatro tramos rectos conectados por tres descansillos a un cuarto de espacio. La dirección de los giros viene determinada por la línea de paso."@es ;
                       rdfs:label "Escalera de Tres Cuartos de Giro"@es ,
                                  "Three Quarter Turn Stair"@en .


###  https://w3id.org/beo#ThreeQuarterWindingStair
:ThreeQuarterWindingStair rdf:type owl:Class ;
                          rdfs:subClassOf :Stair ;
                          rdfs:comment "A stair consisting of one flight with three quarter winders, which make a 90° turn. The stair makes a 270° turn. The direction of the turns is determined by the walking line."@en ,
                                       "Escalera formada por un tramo con tres cuartos de giro que dan una vuelta de 90°. La escalera realiza un giro de 270°. La dirección de los giros viene determinada por la línea de paso."@es ;
                          rdfs:label "Escalera de Tres Cuartos de Caracol"@es ,
                                     "Three Quarter Winding Stair"@en .


###  https://w3id.org/beo#Tiebar
:Tiebar rdf:type owl:Class ;
        rdfs:subClassOf :Member ;
        rdfs:comment "A linear bar element used to secure or stabilise a structure by resisting lateral and longitudinal loading through tension and or compression. usually formed by a solid bar."@en ,
                     "Elemento de barra lineal utilizado para asegurar o estabilizar una estructura resistiendo cargas laterales y longitudinales por tracción y/o compresión. normalmente formado por una barra maciza."@es ;
        rdfs:label "Barra de Anclaje"@es ,
                   "Tiebar"@en .


###  https://w3id.org/beo#Topping
:Topping rdf:type owl:Class ;
         rdfs:subClassOf :Covering ;
         rdfs:comment "El cubrimiento sirve para aislar un elemento de distribución de un espacio en el que está contenido."@es ,
                      "The covering is used to isolate a distribution element from a space in which it is contained."@en ;
         rdfs:label "Topping"@en ,
                    "Topping"@es .


###  https://w3id.org/beo#TrackElement
:TrackElement rdf:type owl:Class ;
              rdfs:subClassOf :BuiltElement ;
              rdfs:comment "A track element is a built element used specifically in the track domain in railway."@en ,
                           "Un elemento de vía es un elemento construido utilizado específicamente en el ámbito de la vía en el ferrocarril."@es ;
              rdfs:label "Elemento de Via"@es ,
                         "Track Element"@en .


###  https://w3id.org/beo#TrackEndofAlignment
:TrackEndofAlignment rdf:type owl:Class ;
                     rdfs:subClassOf :TrackElement ;
                     rdfs:comment "A track end of alignment is a special functional installation such as axle-gauge changeover point or transporter wagon loading point."@en ,
                                  "Un final de alineación de vía es una instalación funcional especial, como un punto de cambio de ancho de vía o un punto de carga de vagones de transporte."@es ;
                     rdfs:label "Final de Alineacion de Via"@es ,
                                "Track End of Alignment"@en .


###  https://w3id.org/beo#TrackPanel
:TrackPanel rdf:type owl:Class ;
            rdfs:subClassOf :ElementAssembly ;
            rdfs:comment "Trackwork ensuring the support and guidance of a vehicle along a route. It consists of assembly of rail, sleepers and fastenings."@en ,
                         "Vía que garantiza el apoyo y guiado de un vehículo a lo largo de una ruta. Consta de montaje de carril, traviesas y fijaciones."@es ;
            rdfs:label "Panel de Vía"@es ,
                       "Track Panel"@en .


###  https://w3id.org/beo#TrackSlab
:TrackSlab rdf:type owl:Class ;
           rdfs:subClassOf :Slab ;
           rdfs:comment "A track slab is a reinforced concrete slab or prestressed reinforced concrete slab, which is a main element of slab track. It can be prefabricated or cast on site and may have sleepers embedded."@en ,
                        "Una losa de vía es una losa de hormigón armado o de hormigón armado pretensado, que constituye un elemento principal de la vía en placa. Puede ser prefabricada o moldeada in situ y puede llevar traviesas empotradas."@es ;
           rdfs:label "Losa de Via"@es ,
                      "Track Slab"@en .


###  https://w3id.org/beo#TrafficCalminfgDevice
:TrafficCalminfgDevice rdf:type owl:Class ;
                       rdfs:subClassOf :ElementAssembly ;
                       rdfs:comment "A structure on the carriageway to control the speed of vehicles."@en ,
                                    "Estructura en la calzada para controlar la velocidad de los vehículos."@es ;
                       rdfs:label "Dispositivo para Calmar el Trafico"@es ,
                                  "Traffic Calminfg Device"@en .


###  https://w3id.org/beo#TransitionSection
:TransitionSection rdf:type owl:Class ;
                   rdfs:subClassOf :EarthworksFill ;
                   rdfs:comment "Sección de la subbase para garantizar la consistencia de la rigidez y evitar asentamientos desiguales. La sección de transición puede aparecer, por ejemplo, entre: terraplén y estribo de puente; terraplén y estructura transversal; desmonte y túnel; terraplén y desmonte."@es ,
                                "Section of subgrade to ensure the consistency of stiffness and prevent uneven settlement. Transition section may appear e.g. between: embankment and bridge abutment; embankment and transverse structure; cutting and tunnel; embankment and cutting."@en ;
                   rdfs:label "Seccion de Transicion"@es ,
                              "Transition Section"@en .


###  https://w3id.org/beo#TransportElement
:TransportElement rdf:type owl:Class ;
                  rdfs:subClassOf <https://schema.org/Product> ;
                  rdfs:comment "A transport element is a generalization of all transport related objects that move people, animals or goods within a Facility. "@en ,
                               "Un elemento de transporte es una generalización de todos los objetos relacionados con el transporte que mueven personas, animales o mercancías dentro de una Instalación."@es ;
                  rdfs:label "Elemento de Transporte"@es ,
                             "Transport Element"@en .


###  https://w3id.org/beo#Trapdoor
:Trapdoor rdf:type owl:Class ;
          rdfs:subClassOf :Door ;
          rdfs:comment "A special door that lies horizonally in a slab opening. Often used for accessing cellar or attic."@en ,
                       "Puerta especial que se sitúa horizontalmente en un hueco de forjado. Suele utilizarse para acceder al sótano o al desván."@es ;
          rdfs:label "Trampilla"@es ,
                     "Trap door"@en .


###  https://w3id.org/beo#Trumpet
:Trumpet rdf:type owl:Class ;
         rdfs:subClassOf :TendonConduit ;
         rdfs:comment "A specific part of conduit which has to be widened when reaching the tendon anchor because the strands are connected individually on the anchor."@en ,
                      "Parte específica del conducto que debe ensancharse al llegar al anclaje del tendón, ya que los torones se conectan individualmente en el anclaje."@es ;
         rdfs:label "Trompeta"@es ,
                    "Trumpet"@en .


###  https://w3id.org/beo#Trunstile
:Trunstile rdf:type owl:Class ;
           rdfs:subClassOf :Door ;
           rdfs:comment "A mechanical gate consisting of revolving arms, allowing only one person at a time to pass through."@es ,
                        "Puerta mecánica formada por brazos giratorios que sólo permiten el paso de una persona a la vez."@en ;
           rdfs:label "Torniquete"@es ,
                      "Trunstile"@en .


###  https://w3id.org/beo#Truss
:Truss rdf:type owl:Class ;
       rdfs:subClassOf :ElementAssembly ;
       rdfs:comment "A structure built up of members with (quasi) pinned joint."@en ,
                    "Una estructura formada por miembros con unión (cuasi) articulada."@es ;
       rdfs:label "Cercha"@es ,
                  "Truss"@en .


###  https://w3id.org/beo#TurnoutPanel
:TurnoutPanel rdf:type owl:Class ;
              rdfs:subClassOf :ElementAssembly ;
              rdfs:comment "Trackwork ensuring the support and guidance of a vehicle along any given route among various diverging or intersecting tracks."@en ,
                           "Vía que garantiza el apoyo y la guía de un vehículo a lo largo de cualquier ruta determinada entre varias vías que divergen o se cruzan."@es ;
              rdfs:label "Panel de Desvio"@es ,
                         "Turnout Panel"@en .


###  https://w3id.org/beo#TwoCurvedRunStair
:TwoCurvedRunStair rdf:type owl:Class ;
                   rdfs:subClassOf :Stair ;
                   rdfs:comment "A curved stair consisting of two curved flights without turns but with one landing."@en ,
                                "Escalera curva formada por dos tramos curvos sin giros pero con un rellano."@es ;
                   rdfs:label "Escalera de Dos Tramos Curvos"@es ,
                              "Two Curved Run Stair"@en .


###  https://w3id.org/beo#TwoQuarterTurnRamp
:TwoQuarterTurnRamp rdf:type owl:Class ;
                    rdfs:subClassOf :Ramp ;
                    rdfs:comment "A ramp making a 180° turn, consisting of three straight flights connected by two quarterspace landings. The direction of the turn is determined by the walking line."@en ,
                                 "Rampa que realiza un giro de 180°, compuesta por tres tramos rectos conectados por dos aterrizajes a un cuarto de espacio. La dirección del giro viene determinada por la línea de marcha."@es ;
                    rdfs:label "Rampa de Dos Cuartos de Vuelta"@es ,
                               "Two Quarter Turn Ramp"@en .


###  https://w3id.org/beo#TwoQuarterTurnStair
:TwoQuarterTurnStair rdf:type owl:Class ;
                     rdfs:subClassOf :Stair ;
                     rdfs:comment "A stair making a 180° turn, consisting of three straight flights connected by two quarterspace landings. The direction of the turns is determined by the walking line."@en ,
                                  "Escalera que realiza un giro de 180°, compuesta por tres tramos rectos conectados por dos descansillos a un cuarto de espacio. La dirección de los giros viene determinada por la línea de paso."@es ;
                     rdfs:label "Escalera de Dos Cuartos de Giro"@es ,
                                "Two Quarter Turn Stair"@en .


###  https://w3id.org/beo#TwoQuarterWindingStair
:TwoQuarterWindingStair rdf:type owl:Class ;
                        rdfs:subClassOf :Stair ;
                        rdfs:comment "A stair consisting of one flight with two quarter winders, which make a 90° turn. The stair makes a 180° turn. The direction of the turns is determined by the walking line."@en ,
                                     "Escalera formada por un tramo con dos cuartos de giro, que dan una vuelta de 90°. La escalera realiza un giro de 180°. La dirección de los giros está determinada por la línea de marcha."@es ;
                        rdfs:label "TEscalera de Dos Cuartos de Caracol"@es ,
                                   "Two Quarter Winding Stair"@en .


###  https://w3id.org/beo#TwoStairRunRamp
:TwoStairRunRamp rdf:type owl:Class ;
                 rdfs:subClassOf :Ramp ;
                 rdfs:comment "A straight ramp consisting of two straight flights without turns but with one landing."@en ,
                              "Rampa recta formada por dos tramos rectos sin giros pero con un aterrizaje."@es ;
                 rdfs:label "Rampa Recta Doble"@es ,
                            "Two Stair Run Ramp"@en .


###  https://w3id.org/beo#TwoStraightRunStair
:TwoStraightRunStair rdf:type owl:Class ;
                     rdfs:subClassOf :Stair ;
                     rdfs:comment "A straight stair consisting of two straight flights without turns but with one landing."@en ,
                                  "Escalera recta formada por dos tramos rectos sin giros pero con un rellano."@es ;
                     rdfs:label "Escalera de dos Tramos Rectos"@es ,
                                "Two Straight Run Stair"@en .


###  https://w3id.org/beo#VacuumMooringDevice
:VacuumMooringDevice rdf:type owl:Class ;
                     rdfs:subClassOf :MooringDevice ;
                     rdfs:comment "Dispositivo de amarre que utiliza la succión por vacío como método principal de sujeción de la embarcación."@es ,
                                  "Mooring device that uses vacuum suction as the primary method of securing the vessel."@en ;
                     rdfs:label "Dispositivo de Amarre de Vacio"@es ,
                                "Vacuum Mooring Device"@en .


###  https://w3id.org/beo#VehicleStop
:VehicleStop rdf:type owl:Class ;
             rdfs:subClassOf :TrackElement ;
             rdfs:comment "A fixed installation at the end of the track which stops any vehicle movement (e.g., buffer stop, sand hump, etc.)."@en ,
                          "Instalación fija al final de la vía que detiene cualquier movimiento del vehículo (por ejemplo, tope, joroba de arena, etc.)."@es ;
             rdfs:label "Parada de Vehiculo"@es ,
                        "Vehicle Stop"@en .


###  https://w3id.org/beo#VerticallyDrainedSoil
:VerticallyDrainedSoil rdf:type owl:Class ;
                       rdfs:subClassOf :ReinforcedSoil ;
                       rdfs:comment "A method to set vertical drainage measures in the foundation, so that pore water in the soil is discharged and the foundation strength is improved."@en ,
                                    "Un método para establecer medidas de drenaje vertical en los cimientos, de forma que se descargue el agua de los poros del suelo y se mejore la resistencia de los cimientos."@es ;
                       rdfs:label "Suelo con Drenaje Vertical"@es ,
                                  "Vertically Drained Soil"@en .


###  https://w3id.org/beo#VibrationDamper
:VibrationDamper rdf:type owl:Class ;
                 rdfs:subClassOf :ElementComponent ;
                 rdfs:comment "A vibration damper is a device used to minimize the effects of vibration in a structure by dissipating kinetic energy. The damper may be passive (elastic, frictional, inertia) or active (in a system using sensors and actuators)."@en ,
                              "Un amortiguador de vibraciones es un dispositivo que se utiliza para minimizar los efectos de las vibraciones en una estructura mediante la disipación de energía cinética. El amortiguador puede ser pasivo (elástico, de fricción, de inercia) o activo (en un sistema que utiliza sensores y actuadores)."@es ;
                 rdfs:label "Amortiguador de Vibraciones"@es ,
                            "Vibration Damper"@en .


###  https://w3id.org/beo#VibrationIsolator
:VibrationIsolator rdf:type owl:Class ;
                   rdfs:subClassOf :ElementComponent ;
                   rdfs:comment "A vibration isolator is a device used to minimize the effects of vibration transmissibility in a structure."@en ,
                                "Un aislador de vibraciones es un dispositivo que se utiliza para minimizar los efectos de la transmisibilidad de vibraciones en una estructura."@es ;
                   rdfs:label "Aislador de Vibraciones"@es ,
                              "Vibration Isolator"@en .


###  https://w3id.org/beo#ViscousDamper
:ViscousDamper rdf:type owl:Class ;
               rdfs:subClassOf :VibrationDamper ;
               rdfs:comment "El tipo viscoso es un amortiguador que absorbe energía utilizando la resistencia de un cuerpo viscoso."@es ,
                            "The viscous type is a damper that absorbs energy by utilizing the resistance of a viscous body."@en ;
               rdfs:label "Amortiguador Viscoso"@es ,
                          "Viscous Damper"@en .


###  https://w3id.org/beo#Wall
:Wall rdf:type owl:Class ;
      rdfs:subClassOf :BuiltElement ;
      rdfs:comment "El muro representa una construcción vertical que puede delimitar o subdividir espacios. Los muros suelen ser elementos planos verticales, o casi verticales, a menudo diseñados para soportar cargas estructurales. Sin embargo, no es necesario que una pared sea portante."@es ,
                   "The wall represents a vertical construction that may bound or subdivide spaces. Wall are usually vertical, or nearly vertical, planar elements, often designed to bear structural loads. A wall is however not required to be load bearing."@en ;
      rdfs:label "Muro"@es ,
                 "Wall"@en .


###  https://w3id.org/beo#WallStud
:WallStud rdf:type owl:Class ;
          rdfs:subClassOf :Member ;
          rdfs:comment "Elemento vertical en el entramado del muro."@es ,
                       "Vertical element in wall framing."@en ;
          rdfs:label "Montante de Muro"@es ,
                     "Wall Stud"@en .


###  https://w3id.org/beo#WaveWall
:WaveWall rdf:type owl:Class ;
          rdfs:subClassOf :Wall ;
          rdfs:comment ""@es ,
                       "Protective wall or screen to block overtopping and impact of waves across a breakwater"@en ;
          rdfs:label "WAVEWALL"@es ,
                     "Wave Wall"@en .


###  https://w3id.org/beo#WearingSlab
:WearingSlab rdf:type owl:Class ;
             rdfs:subClassOf :Slab ;
             rdfs:comment "La losa se utiliza para representar una superficie de desgaste."@es ,
                          "The slab is used to represent a wearing surface."@en ;
             rdfs:label "Losa Portante"@es ,
                        "Wearing Slab"@en .


###  https://w3id.org/beo#WebPlate
:WebPlate rdf:type owl:Class ;
          rdfs:subClassOf :Plate ;
          rdfs:comment "A plate connecting flange plates in linear members having box or I-profile."@en ,
                       "Placa que conecta las placas de Ala en elementos lineales con perfil en caja o en I."@es ;
          rdfs:label "Placa de Alma"@es ,
                     "Web Plate"@en .


###  https://w3id.org/beo#Weld
:Weld rdf:type owl:Class ;
      rdfs:subClassOf :Fastener ;
      rdfs:comment "A weld seam between parts of metallic material or other suitable materials."@en ,
                   "Costura de soldadura entre piezas de material metálico u otros materiales adecuados."@es ;
      rdfs:label "Soldadura"@es ,
                 "Weld"@en .


###  https://w3id.org/beo#Well
:Well rdf:type owl:Class ;
      rdfs:subClassOf :CaissonFoundation ;
      rdfs:comment "Caja abierta"@es ,
                   "Open box."@en ;
      rdfs:label "Well"@en ,
                 "Well"@es .


###  https://w3id.org/beo#WinderStairFlight
:WinderStairFlight rdf:type owl:Class ;
                   rdfs:subClassOf :StairFlight ;
                   rdfs:comment "A stair flight with a walking line including straight and curved sections."@en ,
                                "Un tramo de escalera con una línea de paso que incluye tramos rectos y curvos."@es ;
                   rdfs:label "Tramo de Escalera con Tramos de Caracol"@es ,
                              "Winder Stair Flight"@en .


###  https://w3id.org/beo#Window
:Window rdf:type owl:Class ;
        rdfs:subClassOf :BuiltElement ;
        rdfs:comment "La ventana es un elemento constructivo que se utiliza principalmente para proporcionar luz natural y aire fresco. Incluye apertura vertical pero también apertura horizontal como claraboyas o cúpulas de luz. Incluye construcciones con paneles basculantes, pivotantes, deslizantes o giratorios y paneles fijos. Una ventana consta de un revestimiento y uno o varios paneles."@es ,
                     "The window is a building element that is predominately used to provide natural light and fresh air. It includes vertical opening but also horizontal opening such as skylights or light domes. It includes constructions with swinging, pivoting, sliding, or revolving panels and fixed panels. A window consists of a lining and one or several panels."@en ;
        rdfs:label "Ventana"@es ,
                   "Window"@en .


###  https://w3id.org/beo#Wire
:Wire rdf:type owl:Class ;
      rdfs:subClassOf :Tendon ;
      rdfs:comment "El tendón es un alambre."@es ,
                   "The tendon is a wire."@en ;
      rdfs:label "Wire"@en ,
                 "Wire"@es .


###  https://w3id.org/beo#Wrapping
:Wrapping rdf:type owl:Class ;
          rdfs:subClassOf :Covering ;
          rdfs:comment "El cubrimiento se utiliza para envolver especialmente los elementos de distribución mediante cinta adhesiva."@es ,
                       "The covering is used for wrapping particularly of distribution elements using tape."@en ;
          rdfs:label "Envoltura"@es ,
                     "Wrapping"@en .


###  Generated by the OWL API (version 5.1.18) https://github.com/owlcs/owlapi/
